@prefix at: <http://publications.europa.eu/ontology/authority/> .
@prefix atold: <http://publications.europa.eu/resource/authority/> .
@prefix dc: <http://purl.org/dc/elements/1.1/> .
@prefix owl: <http://www.w3.org/2002/07/owl#> .
@prefix rdfs: <http://www.w3.org/2000/01/rdf-schema#> .
@prefix skos: <http://www.w3.org/2004/02/skos/core#> .

<http://publications.europa.eu/resource/authority/notation-type/AKN4EU> a skos:Concept ;
    at:authority-code "AKN4EU" ;
    at:deprecated "false" ;
    at:op-code "AKN4EU" ;
    at:start.use "2019-03-13" ;
    atold:op-code "AKN4EU" ;
    dc:identifier "AKN4EU" ;
    skos:altLabel "Akoma Ntoso for European Union"@en ;
    skos:definition "This concept identifies the Akoma Ntoso common XML schema. It is developed under the governance of the Interinstitutional Metadata and Formats Committee (IMFC). The specifications are based on the generic Akoma Ntoso standard maintained by OASIS but tailored to the requirements that the EU Institutions define for their legal documents."@en ;
    skos:inScheme atold:notation-type ;
    skos:prefLabel "AKN4EU"@en,
        "AKN4EU"@et ;
    skos:topConceptOf atold:notation-type .

<http://publications.europa.eu/resource/authority/notation-type/ARK> a skos:Concept ;
    at:authority-code "ARK" ;
    at:deprecated "false" ;
    at:op-code "ARK" ;
    at:start.use "2001-12-31" ;
    atold:op-code "ARK" ;
    dc:identifier "ARK" ;
    skos:altLabel "Archival Resource Key"@en ;
    skos:definition "The ARK (Archival Resource Key) identifier is a specially constructed, globally unique actionable URL (Uniform Resource Locator). It provides a naming scheme for persistent access to digital objects."@en ;
    skos:exactMatch <http://purl.org/spar/datacite/ark> ;
    skos:inScheme atold:notation-type ;
    skos:prefLabel "ARK"@en,
        "ARK"@et ;
    skos:topConceptOf atold:notation-type .

<http://publications.europa.eu/resource/authority/notation-type/ARXIV> a skos:Concept ;
    at:authority-code "ARXIV" ;
    at:deprecated "false" ;
    at:op-code "ARXIV" ;
    at:start.use "1991-08-14" ;
    atold:op-code "ARXIV" ;
    dc:identifier "ARXIV" ;
    skos:altLabel "arXiv identifier"@en ;
    skos:definition "The ArXiv identifier is generated by ArXiv, an open access repository and distribution server for electronic preprints featuring, in particular, physics, mathematics, computer science, nonlinear sciences, quantitative biology, quantitative finance, statistics, electrical engineering and systems science and economics."@en ;
    skos:exactMatch <http://purl.org/spar/datacite/arxiv> ;
    skos:inScheme atold:notation-type ;
    skos:prefLabel "arXiv"@en,
        "arXiv"@et ;
    skos:topConceptOf atold:notation-type .

<http://publications.europa.eu/resource/authority/notation-type/BIBCODE> a skos:Concept ;
    at:authority-code "BIBCODE" ;
    at:deprecated "false" ;
    at:op-code "BIBCODE" ;
    at:start.use "1995-12-31" ;
    atold:op-code "BIBCODE" ;
    dc:identifier "BIBCODE" ;
    skos:altLabel "Bibliographic Reference Code"@en ;
    skos:definition "The bibcode is a compact identifier used by several astronomical data systems to uniquely specify literature references. The Bibliographic Reference Code (REFCODE) is used widely, for example, by the NASA Astrophysics Data System who coined and prefer the term \"bibcode\"."@en ;
    skos:exactMatch <http://purl.org/spar/datacite/bibcode> ;
    skos:inScheme atold:notation-type ;
    skos:prefLabel "Bibcode"@en,
        "Bibcode"@et ;
    skos:topConceptOf atold:notation-type .

<http://publications.europa.eu/resource/authority/notation-type/CELEX> a skos:Concept ;
    at:authority-code "CELEX" ;
    at:deprecated "false" ;
    at:op-code "CELEX" ;
    at:op-mapped-code [ a at:MappedCode ;
            at:affected-table "notation-type" ;
            at:legacy-code "celex_id" ;
            dc:source "MDR" ] ;
    at:start.use "1981-01-01" ;
    atold:op-code "CELEX" ;
    dc:identifier "CELEX" ;
    skos:altLabel "CELEX code"@en ;
    skos:definition "The unique identifier of each document in EUR-Lex, regardless of language."@en ;
    skos:inScheme atold:notation-type ;
    skos:prefLabel "CELEX id"@en,
        "CELEX id"@et ;
    skos:topConceptOf atold:notation-type .

<http://publications.europa.eu/resource/authority/notation-type/CELEX_RT> a skos:Concept ;
    at:authority-code "CELEX_RT" ;
    at:deprecated "false" ;
    at:op-code "CELEX_RT" ;
    at:op-mapped-code [ a at:MappedCode ;
            at:affected-table "notation-type" ;
            at:legacy-code "celex_root" ;
            dc:source "MDR" ] ;
    at:start.use "1981-01-01" ;
    atold:op-code "CELEX_RT" ;
    dc:identifier "CELEX_RT" ;
    skos:altLabel "CELEX root code"@en ;
    skos:definition "Code used to identify the root of a CELEX code."@en ;
    skos:inScheme atold:notation-type ;
    skos:prefLabel "CELEX root"@en,
        "CELEX juurelement"@et ;
    skos:topConceptOf atold:notation-type .

<http://publications.europa.eu/resource/authority/notation-type/CELEX_SECT> a skos:Concept ;
    at:authority-code "CELEX_SECT" ;
    at:deprecated "false" ;
    at:op-code "CELEX_SECT" ;
    at:op-mapped-code [ a at:MappedCode ;
            at:affected-table "notation-type" ;
            at:legacy-code "oj.celex.structure.id" ;
            dc:source "MDR" ] ;
    at:start.use "1981-01-01" ;
    atold:op-code "CELEX_SECT" ;
    dc:identifier "CELEX_SECT" ;
    skos:altLabel "CELEX sector code"@en ;
    skos:definition "Code used to identify the sector, the first element (number or letter) of the CELEX code."@en ;
    skos:inScheme atold:notation-type ;
    skos:prefLabel "CELEX sector"@en,
        "CELEX sektor"@et ;
    skos:topConceptOf atold:notation-type .

<http://publications.europa.eu/resource/authority/notation-type/CELLAR_MANIFT> a skos:Concept ;
    at:authority-code "CELLAR_MANIFT" ;
    at:deprecated "false" ;
    at:op-code "CELLAR_MANIFT" ;
    at:op-mapped-code [ a at:MappedCode ;
            at:affected-table "notation-type" ;
            at:legacy-code "manifestation-type-cellar" ;
            dc:source "MDR" ] ;
    at:start.use "2010-09-23" ;
    atold:op-code "CELLAR_MANIFT" ;
    dc:identifier "CELLAR_MANIFT" ;
    skos:altLabel "Media type (Cellar Manifestation) code"@en ;
    skos:definition "Code used in Cellar for manifestations of media types. Cellar is the information system storing all metadata and digital content managed by the Publications Office in a harmonised and standardised format."@en ;
    skos:inScheme atold:notation-type ;
    skos:prefLabel "CELLAR Manif MIME"@en,
        "CELLAR Manif MIME"@et ;
    skos:topConceptOf atold:notation-type .

<http://publications.europa.eu/resource/authority/notation-type/CELLAR_MT> a skos:Concept ;
    at:authority-code "CELLAR_MT" ;
    at:deprecated "false" ;
    at:op-code "CELLAR_MT" ;
    at:op-mapped-code [ a at:MappedCode ;
            at:affected-table "notation-type" ;
            at:legacy-code "mime-type-cellar" ;
            dc:source "MDR" ] ;
    at:start.use "2010-09-23" ;
    atold:op-code "CELLAR_MT" ;
    dc:identifier "CELLAR_MT" ;
    skos:altLabel "Media type (Cellar) code"@en ;
    skos:definition "Code used in Cellar for media types. Cellar is the information system storing all metadata and digital content managed by the Publications Office in a harmonised and standardised format."@en ;
    skos:inScheme atold:notation-type ;
    skos:prefLabel "CELLAR MIME"@en,
        "CELLAR MIME"@et ;
    skos:topConceptOf atold:notation-type .

<http://publications.europa.eu/resource/authority/notation-type/CJ> a skos:Concept ;
    at:authority-code "CJ" ;
    at:deprecated "false" ;
    at:op-code "CJ" ;
    at:start.use "1952-07-24" ;
    atold:op-code "CJ" ;
    dc:identifier "CJ" ;
    skos:altLabel "CJ code"@en ;
    skos:definition "Code used by the Court of Justice."@en ;
    skos:inScheme atold:notation-type ;
    skos:prefLabel "CJ"@en,
        "CJ"@et ;
    skos:topConceptOf atold:notation-type .

<http://publications.europa.eu/resource/authority/notation-type/CODIF_DATA> a skos:Concept ;
    at:authority-code "CODIF_DATA" ;
    at:deprecated "false" ;
    at:op-code "CODIF_DATA" ;
    at:start.use "2022-06-15" ;
    atold:op-code "CODIF_DATA" ;
    dc:identifier "CODIF_DATA" ;
    skos:definition "Code used in several authority tables for codifying concepts in TED portal expert search and used in TED Schema (CODIF_DATA)."@en ;
    skos:inScheme atold:notation-type ;
    skos:prefLabel "Codification data"@en,
        "Codification data"@et ;
    skos:topConceptOf atold:notation-type .

<http://publications.europa.eu/resource/authority/notation-type/COMREF> a skos:Concept ;
    at:authority-code "COMREF" ;
    at:deprecated "false" ;
    at:op-code "COMREF" ;
    at:start.use "1957-03-25" ;
    atold:op-code "COMREF" ;
    dc:identifier "COMREF" ;
    skos:altLabel "COMREF code"@en ;
    skos:definition "Code used by COMREF, the European Commission's Human Resources Database."@en ;
    skos:inScheme atold:notation-type ;
    skos:prefLabel "COMREF"@en,
        "COMREF"@et ;
    skos:topConceptOf atold:notation-type .

<http://publications.europa.eu/resource/authority/notation-type/CONSIL> a skos:Concept ;
    at:authority-code "CONSIL" ;
    at:deprecated "false" ;
    at:op-code "CONSIL" ;
    at:start.use "1993-11-01" ;
    atold:op-code "CONSIL" ;
    dc:identifier "CONSIL" ;
    skos:altLabel "Council code"@en ;
    skos:definition "Code used by the Council of the European Union."@en ;
    skos:inScheme atold:notation-type ;
    skos:prefLabel "Council"@en,
        "Council"@et ;
    skos:topConceptOf atold:notation-type .

<http://publications.europa.eu/resource/authority/notation-type/DEMED> a skos:Concept ;
    at:authority-code "DEMED" ;
    at:deprecated "false" ;
    at:op-code "DEMED" ;
    at:start.use "1969-01-18" ;
    atold:op-code "DEMED" ;
    dc:identifier "DEMED" ;
    skos:altLabel "DEMED code"@en ;
    skos:definition "Code used by the DEMED system."@en ;
    skos:inScheme atold:notation-type ;
    skos:prefLabel "DEMED"@en,
        "DEMED"@et ;
    skos:topConceptOf atold:notation-type .

<http://publications.europa.eu/resource/authority/notation-type/DOI> a skos:Concept ;
    at:authority-code "DOI" ;
    at:deprecated "false" ;
    at:op-code "DOI" ;
    at:start.use "2000-01-01" ;
    atold:op-code "DOI" ;
    dc:identifier "DOI" ;
    skos:altLabel "Digital Object Identifier code"@en ;
    skos:definition "DOI is a permanent identifier given to an electronic document. Similar to a URN, but in contrast to a URL, it is not dependent upon the electronic document's location. A typical use of a DOI is to give a scholarly paper or article a unique identifying number that anyone can use to obtain information about the publication's location on a digital network."@en ;
    skos:exactMatch <http://purl.org/spar/datacite/doi> ;
    skos:inScheme atold:notation-type ;
    skos:prefLabel "DOI"@en,
        "DOI"@et ;
    skos:topConceptOf atold:notation-type .

<http://publications.europa.eu/resource/authority/notation-type/DOI_P> a skos:Concept ;
    at:authority-code "DOI_P" ;
    at:deprecated "false" ;
    at:op-code "DOI_P" ;
    at:op-mapped-code [ a at:MappedCode ;
            at:affected-table "notation-type" ;
            at:legacy-code "id-doi" ;
            dc:source "MDR" ],
        [ a at:MappedCode ;
            at:affected-table "notation-type" ;
            at:legacy-code "id-doi.old" ;
            dc:source "MDR" ] ;
    at:start.use "1970-01-01" ;
    atold:op-code "DOI_P" ;
    dc:identifier "DOI_P" ;
    skos:altLabel "DOI prefix"@en ;
    skos:definition "The DOI prefix is composed of a directory indicator followed by a registrant code. The directory indicator shall be \"10\" and it distinguishes the entire set of character strings (prefix and suffix) as digital object identifiers within the resolution system. The second element of the DOI prefix shall be the registrant code. The registrant code is a unique string assigned to a registrant."@en ;
    skos:inScheme atold:notation-type ;
    skos:prefLabel "DOI pref"@en,
        "DOI pref"@et ;
    skos:topConceptOf atold:notation-type .

<http://publications.europa.eu/resource/authority/notation-type/EAN13> a skos:Concept ;
    at:authority-code "EAN13" ;
    at:deprecated "false" ;
    at:op-code "EAN13" ;
    at:start.use "1978-12-31" ;
    atold:op-code "EAN13" ;
    dc:identifier "EAN13" ;
    skos:altLabel "EAN 13 code"@en ;
    skos:definition "The EAN 13 code is the most widely used commercial distribution code in the world. It is shown on all marketed products. It is managed by GS1, an international agency located in Brussels."@en ;
    skos:exactMatch <http://purl.org/spar/datacite/ean13> ;
    skos:inScheme atold:notation-type ;
    skos:prefLabel "EAN 13"@en,
        "EAN 13"@et ;
    skos:topConceptOf atold:notation-type .

<http://publications.europa.eu/resource/authority/notation-type/ECLI> a skos:Concept ;
    at:authority-code "ECLI" ;
    at:deprecated "false" ;
    at:op-code "ECLI" ;
    at:op-mapped-code [ a at:MappedCode ;
            at:affected-table "notation-type" ;
            at:legacy-code "code-ecli" ;
            dc:source "MDR" ] ;
    at:start.use "2011-04-29" ;
    atold:op-code "ECLI" ;
    dc:identifier "ECLI" ;
    skos:altLabel "European Case Law Identifier code"@en ;
    skos:definition "The European Case Law Identifier (ECLI) has been developed to facilitate the correct and unequivocal citation of judgments from European and national courts. ECLI is a uniform identifier that has the same recognizable format for all Member States and EU courts."@en ;
    skos:historyNote "No time span"@en ;
    skos:inScheme atold:notation-type ;
    skos:prefLabel "ECLI"@en,
        "ECLI"@et ;
    skos:topConceptOf atold:notation-type .

<http://publications.europa.eu/resource/authority/notation-type/EP> a skos:Concept ;
    at:authority-code "EP" ;
    at:deprecated "false" ;
    at:op-code "EP" ;
    at:start.use "1962-03-30" ;
    atold:op-code "EP" ;
    dc:identifier "EP" ;
    skos:altLabel "EP code"@en ;
    skos:definition "Code used by the European Parliament."@en ;
    skos:inScheme atold:notation-type ;
    skos:prefLabel "EP"@en,
        "EP"@et ;
    skos:topConceptOf atold:notation-type .

<http://publications.europa.eu/resource/authority/notation-type/ESPD> a skos:Concept ;
    at:authority-code "ESPD" ;
    at:deprecated "false" ;
    at:op-code "ESPD" ;
    at:start.use "2020-09-23" ;
    atold:op-code "ESPD" ;
    dc:identifier "ESPD" ;
    skos:altLabel "ESPD code"@en ;
    skos:definition "Code used in the European Single Procurement Document (ESPD)."@en ;
    skos:inScheme atold:notation-type ;
    skos:prefLabel "ESPD"@en,
        "ESPD"@et ;
    skos:topConceptOf atold:notation-type .

<http://publications.europa.eu/resource/authority/notation-type/EUBOOKSHOP> a skos:Concept ;
    at:authority-code "EUBOOKSHOP" ;
    at:deprecated "false" ;
    at:op-code "EUBOOKSHOP" ;
    at:start.use "1952-07-24" ;
    atold:op-code "EUBOOKSHOP" ;
    dc:identifier "EUBOOKSHOP" ;
    skos:altLabel "EU Bookshop code"@en ;
    skos:definition "Code used by the EU Bookshop."@en ;
    skos:inScheme atold:notation-type ;
    skos:prefLabel "EU Bookshop"@en,
        "EU Bookshop"@et ;
    skos:topConceptOf atold:notation-type .

<http://publications.europa.eu/resource/authority/notation-type/EUDOR_LNG> a skos:Concept ;
    at:authority-code "EUDOR_LNG" ;
    at:deprecated "false" ;
    at:op-code "EUDOR_LNG" ;
    at:op-mapped-code [ a at:MappedCode ;
            at:affected-table "notation-type" ;
            at:legacy-code "EUDOR" ;
            dc:source "MDR" ] ;
    at:start.use "1998-12-04" ;
    atold:op-code "EUDOR_LNG" ;
    dc:identifier "EUDOR_LNG" ;
    skos:altLabel "Eudor language code"@en ;
    skos:definition "Code used in Eudor system for languages. Eudor supports Idol, a central repository that holds indexed data."@en ;
    skos:inScheme atold:notation-type ;
    skos:prefLabel "Eudor lang"@en,
        "Eudor keel"@et ;
    skos:topConceptOf atold:notation-type .

<http://publications.europa.eu/resource/authority/notation-type/EUDOR_MIME> a skos:Concept ;
    at:authority-code "EUDOR_MIME" ;
    at:deprecated "false" ;
    at:op-code "EUDOR_MIME" ;
    at:op-mapped-code [ a at:MappedCode ;
            at:affected-table "notation-type" ;
            at:legacy-code "eudor-type-cellar" ;
            dc:source "MDR" ] ;
    at:start.use "1998-12-04" ;
    atold:op-code "EUDOR_MIME" ;
    dc:identifier "EUDOR_MIME" ;
    skos:altLabel "Media type (Eudor) code"@en ;
    skos:definition "Code used in Eudor system for media types. Eudor supports Idol, a central repository that holds indexed data."@en ;
    skos:inScheme atold:notation-type ;
    skos:prefLabel "EUDOR MIME"@en,
        "EUDOR MIME"@et ;
    skos:topConceptOf atold:notation-type .

<http://publications.europa.eu/resource/authority/notation-type/EUROVOC> a skos:Concept ;
    at:authority-code "EUROVOC" ;
    at:deprecated "false" ;
    at:op-code "EUROVOC" ;
    at:start.use "1984-01-01" ;
    atold:op-code "EUROVOC" ;
    dc:identifier "EUROVOC" ;
    skos:altLabel "EuroVoc code"@en ;
    skos:definition "Code used in EU's multilingual thesaurus EuroVoc."@en ;
    skos:inScheme atold:notation-type ;
    skos:prefLabel "EuroVoc"@en,
        "EuroVoc"@et ;
    skos:topConceptOf atold:notation-type .

<http://publications.europa.eu/resource/authority/notation-type/E_ISSN> a skos:Concept ;
    at:authority-code "E_ISSN" ;
    at:deprecated "false" ;
    at:op-code "E_ISSN" ;
    at:start.use "2007-12-31" ;
    atold:op-code "E_ISSN" ;
    dc:identifier "E_ISSN" ;
    skos:altLabel "Electronic ISSN"@en ;
    skos:definition "A different ISSN from the print edition, the e-ISSN (Electronic ISSN) is used for the online edition of a journal. This is to enable librarians and other users to distinguish between their print and online holdings."@en ;
    skos:exactMatch <http://purl.org/spar/datacite/eissn> ;
    skos:inScheme atold:notation-type ;
    skos:prefLabel "e-ISSN"@en,
        "e-ISSN"@et ;
    skos:topConceptOf atold:notation-type .

<http://publications.europa.eu/resource/authority/notation-type/FD_010> a skos:Concept ;
    at:authority-code "FD_010" ;
    at:deprecated "false" ;
    at:op-code "FD_010" ;
    at:start.use "2010-03-29" ;
    atold:op-code "FD_010" ;
    dc:identifier "FD_010" ;
    skos:altLabel "FD_Table010 code"@en ;
    skos:definition "Code used by FD_Table010 of Eurlex domain in ATTO."@en ;
    skos:inScheme atold:notation-type ;
    skos:prefLabel "FD_010"@en,
        "FD_010"@et ;
    skos:topConceptOf atold:notation-type .

<http://publications.europa.eu/resource/authority/notation-type/FD_020> a skos:Concept ;
    at:authority-code "FD_020" ;
    at:deprecated "false" ;
    at:op-code "FD_020" ;
    at:start.use "2010-03-29" ;
    atold:op-code "FD_020" ;
    dc:identifier "FD_020" ;
    skos:altLabel "FD_Table020 code"@en ;
    skos:definition "Code used by FD_Table020 of Eurlex domain in ATTO."@en ;
    skos:inScheme atold:notation-type ;
    skos:prefLabel "FD_020"@en,
        "FD_020"@et ;
    skos:topConceptOf atold:notation-type .

<http://publications.europa.eu/resource/authority/notation-type/FD_030> a skos:Concept ;
    at:authority-code "FD_030" ;
    at:deprecated "false" ;
    at:op-code "FD_030" ;
    at:start.use "2010-03-29" ;
    atold:op-code "FD_030" ;
    dc:identifier "FD_030" ;
    skos:altLabel "FD_Table030 code"@en ;
    skos:definition "Code used by FD_Table030 of Eurlex domain in ATTO."@en ;
    skos:inScheme atold:notation-type ;
    skos:prefLabel "FD_030"@en,
        "FD_030"@et ;
    skos:topConceptOf atold:notation-type .

<http://publications.europa.eu/resource/authority/notation-type/FD_040> a skos:Concept ;
    at:authority-code "FD_040" ;
    at:deprecated "false" ;
    at:op-code "FD_040" ;
    at:start.use "2010-03-29" ;
    atold:op-code "FD_040" ;
    dc:identifier "FD_040" ;
    skos:altLabel "FD_Table040 code"@en ;
    skos:definition "Code used by FD_Table040 of Eurlex domain in ATTO."@en ;
    skos:inScheme atold:notation-type ;
    skos:prefLabel "FD_040"@en,
        "FD_040"@et ;
    skos:topConceptOf atold:notation-type .

<http://publications.europa.eu/resource/authority/notation-type/FD_050> a skos:Concept ;
    at:authority-code "FD_050" ;
    at:deprecated "false" ;
    at:op-code "FD_050" ;
    at:start.use "2010-03-29" ;
    atold:op-code "FD_050" ;
    dc:identifier "FD_050" ;
    skos:altLabel "FD_Table050 code"@en ;
    skos:definition "Code used by FD_Table050 of Eurlex domain in ATTO."@en ;
    skos:inScheme atold:notation-type ;
    skos:prefLabel "FD_050"@en,
        "FD_050"@et ;
    skos:topConceptOf atold:notation-type .

<http://publications.europa.eu/resource/authority/notation-type/FD_060> a skos:Concept ;
    at:authority-code "FD_060" ;
    at:deprecated "false" ;
    at:op-code "FD_060" ;
    at:start.use "2010-03-29" ;
    atold:op-code "FD_060" ;
    dc:identifier "FD_060" ;
    skos:altLabel "FD_Table060 code"@en ;
    skos:definition "Code used by FD_Table060 of Eurlex domain in ATTO."@en ;
    skos:inScheme atold:notation-type ;
    skos:prefLabel "FD_060"@en,
        "FD_060"@et ;
    skos:topConceptOf atold:notation-type .

<http://publications.europa.eu/resource/authority/notation-type/FD_070> a skos:Concept ;
    at:authority-code "FD_070" ;
    at:deprecated "false" ;
    at:op-code "FD_070" ;
    at:start.use "2010-03-29" ;
    atold:op-code "FD_070" ;
    dc:identifier "FD_070" ;
    skos:altLabel "FD_Table070 code"@en ;
    skos:definition "Code used by FD_Table070 of Eurlex domain in ATTO."@en ;
    skos:inScheme atold:notation-type ;
    skos:prefLabel "FD_070"@en,
        "FD_070"@et ;
    skos:topConceptOf atold:notation-type .

<http://publications.europa.eu/resource/authority/notation-type/FD_100> a skos:Concept ;
    at:authority-code "FD_100" ;
    at:deprecated "false" ;
    at:op-code "FD_100" ;
    at:start.use "2010-03-29" ;
    atold:op-code "FD_100" ;
    dc:identifier "FD_100" ;
    skos:altLabel "FD_Table100 code"@en ;
    skos:definition "Code used by FD_Table100 of Eurlex domain in ATTO."@en ;
    skos:inScheme atold:notation-type ;
    skos:prefLabel "FD_100"@en,
        "FD_100"@et ;
    skos:topConceptOf atold:notation-type .

<http://publications.europa.eu/resource/authority/notation-type/FD_110> a skos:Concept ;
    at:authority-code "FD_110" ;
    at:deprecated "false" ;
    at:op-code "FD_110" ;
    at:start.use "2010-03-29" ;
    atold:op-code "FD_110" ;
    dc:identifier "FD_110" ;
    skos:altLabel "FD_Table110 code"@en ;
    skos:definition "Code used by FD_Table110 of Eurlex domain in ATTO."@en ;
    skos:inScheme atold:notation-type ;
    skos:prefLabel "FD_110"@en,
        "FD_110"@et ;
    skos:topConceptOf atold:notation-type .

<http://publications.europa.eu/resource/authority/notation-type/FD_140> a skos:Concept ;
    at:authority-code "FD_140" ;
    at:deprecated "false" ;
    at:op-code "FD_140" ;
    at:start.use "2010-03-29" ;
    atold:op-code "FD_140" ;
    dc:identifier "FD_140" ;
    skos:altLabel "FD_Table140 code"@en ;
    skos:definition "Code used by FD_Table140 of Eurlex domain in ATTO."@en ;
    skos:inScheme atold:notation-type ;
    skos:prefLabel "FD_140"@en,
        "FD_140"@et ;
    skos:topConceptOf atold:notation-type .

<http://publications.europa.eu/resource/authority/notation-type/FD_160> a skos:Concept ;
    at:authority-code "FD_160" ;
    at:deprecated "false" ;
    at:op-code "FD_160" ;
    at:start.use "2010-03-29" ;
    atold:op-code "FD_160" ;
    dc:identifier "FD_160" ;
    skos:altLabel "FD_Table160 code"@en ;
    skos:definition "Code used by FD_Table160 of Eurlex domain in ATTO."@en ;
    skos:inScheme atold:notation-type ;
    skos:prefLabel "FD_160"@en,
        "FD_160"@et ;
    skos:topConceptOf atold:notation-type .

<http://publications.europa.eu/resource/authority/notation-type/FD_290> a skos:Concept ;
    at:authority-code "FD_290" ;
    at:deprecated "false" ;
    at:op-code "FD_290" ;
    at:start.use "2010-03-29" ;
    atold:op-code "FD_290" ;
    dc:identifier "FD_290" ;
    skos:altLabel "FD_Table290 code"@en ;
    skos:definition "Code used by FD_Table290 of Eurlex domain in ATTO."@en ;
    skos:inScheme atold:notation-type ;
    skos:prefLabel "FD_290"@en,
        "FD_290"@et ;
    skos:topConceptOf atold:notation-type .

<http://publications.europa.eu/resource/authority/notation-type/FD_325> a skos:Concept ;
    at:authority-code "FD_325" ;
    at:deprecated "false" ;
    at:op-code "FD_325" ;
    at:start.use "2010-03-29" ;
    atold:op-code "FD_325" ;
    dc:identifier "FD_325" ;
    skos:altLabel "FD_Table361 code"@en ;
    skos:definition "Code used by FD_Table361 of Eurlex domain in ATTO."@en ;
    skos:inScheme atold:notation-type ;
    skos:prefLabel "FD_361"@en,
        "FD_361"@et ;
    skos:topConceptOf atold:notation-type .

<http://publications.europa.eu/resource/authority/notation-type/FD_361> a skos:Concept ;
    at:authority-code "FD_361" ;
    at:deprecated "false" ;
    at:op-code "FD_361" ;
    at:start.use "2010-03-29" ;
    atold:op-code "FD_361" ;
    dc:identifier "FD_361" ;
    skos:altLabel "FD_Table325 code"@en ;
    skos:definition "Code used by FD_Table325 of Eurlex domain in ATTO."@en ;
    skos:inScheme atold:notation-type ;
    skos:prefLabel "FD_325"@en,
        "FD_325"@et ;
    skos:topConceptOf atold:notation-type .

<http://publications.europa.eu/resource/authority/notation-type/FD_375> a skos:Concept ;
    at:authority-code "FD_375" ;
    at:deprecated "false" ;
    at:op-code "FD_375" ;
    at:start.use "2010-03-29" ;
    atold:op-code "FD_375" ;
    dc:identifier "FD_375" ;
    skos:altLabel "FD_Table375 code"@en ;
    skos:definition "Code used by FD_Table375 of Eurlex domain in ATTO."@en ;
    skos:inScheme atold:notation-type ;
    skos:prefLabel "FD_375"@en,
        "FD_375"@et ;
    skos:topConceptOf atold:notation-type .

<http://publications.europa.eu/resource/authority/notation-type/FD_380> a skos:Concept ;
    at:authority-code "FD_380" ;
    at:deprecated "false" ;
    at:op-code "FD_380" ;
    at:start.use "2010-03-29" ;
    atold:op-code "FD_380" ;
    dc:identifier "FD_380" ;
    skos:altLabel "FD_Table380 code"@en ;
    skos:definition "Code used by FD_Table380 of Eurlex domain in ATTO."@en ;
    skos:inScheme atold:notation-type ;
    skos:prefLabel "FD_380"@en,
        "FD_380"@et ;
    skos:topConceptOf atold:notation-type .

<http://publications.europa.eu/resource/authority/notation-type/FD_400> a skos:Concept ;
    at:authority-code "FD_400" ;
    at:deprecated "false" ;
    at:op-code "FD_400" ;
    at:start.use "2010-03-29" ;
    atold:op-code "FD_400" ;
    dc:identifier "FD_400" ;
    skos:altLabel "FD_Table400 code"@en ;
    skos:definition "Code used by FD_Table400 of Eurlex domain in ATTO."@en ;
    skos:inScheme atold:notation-type ;
    skos:prefLabel "FD_400"@en,
        "FD_400"@et ;
    skos:topConceptOf atold:notation-type .

<http://publications.europa.eu/resource/authority/notation-type/FD_499> a skos:Concept ;
    at:authority-code "FD_499" ;
    at:deprecated "false" ;
    at:op-code "FD_499" ;
    at:start.use "2010-03-29" ;
    atold:op-code "FD_499" ;
    dc:identifier "FD_499" ;
    skos:altLabel "FD_Table499 code"@en ;
    skos:definition "Code used by FD_Table499 of Eurlex domain in ATTO."@en ;
    skos:inScheme atold:notation-type ;
    skos:prefLabel "FD_499"@en,
        "FD_499"@et ;
    skos:topConceptOf atold:notation-type .

<http://publications.europa.eu/resource/authority/notation-type/FD_557> a skos:Concept ;
    at:authority-code "FD_557" ;
    at:deprecated "false" ;
    at:op-code "FD_557" ;
    at:start.use "2010-03-29" ;
    atold:op-code "FD_557" ;
    dc:identifier "FD_557" ;
    skos:altLabel "FD_Table557 code"@en ;
    skos:definition "Code used by FD_Table557 of Eurlex domain in ATTO."@en ;
    skos:inScheme atold:notation-type ;
    skos:prefLabel "FD_557"@en,
        "FD_557"@et ;
    skos:topConceptOf atold:notation-type .

<http://publications.europa.eu/resource/authority/notation-type/FD_601> a skos:Concept ;
    at:authority-code "FD_601" ;
    at:deprecated "false" ;
    at:op-code "FD_601" ;
    at:start.use "2011-06-09" ;
    atold:op-code "FD_601" ;
    dc:identifier "FD_601" ;
    skos:altLabel "FD_Table601 code"@en ;
    skos:definition "Code used by FD_Table601 of Eurlex domain in ATTO."@en ;
    skos:inScheme atold:notation-type ;
    skos:prefLabel "FD_601"@en,
        "FD_601"@et ;
    skos:topConceptOf atold:notation-type .

<http://publications.europa.eu/resource/authority/notation-type/FD_607> a skos:Concept ;
    at:authority-code "FD_607" ;
    at:deprecated "false" ;
    at:op-code "FD_607" ;
    at:start.use "2010-03-29" ;
    atold:op-code "FD_607" ;
    dc:identifier "FD_607" ;
    skos:altLabel "FD_Table607 code"@en ;
    skos:definition "Code used by FD_Table607 of Eurlex domain in ATTO."@en ;
    skos:inScheme atold:notation-type ;
    skos:prefLabel "FD_607"@en,
        "FD_607"@et ;
    skos:topConceptOf atold:notation-type .

<http://publications.europa.eu/resource/authority/notation-type/FD_608> a skos:Concept ;
    at:authority-code "FD_608" ;
    at:deprecated "false" ;
    at:op-code "FD_608" ;
    at:start.use "2010-03-29" ;
    atold:op-code "FD_608" ;
    dc:identifier "FD_608" ;
    skos:altLabel "FD_Table608 code"@en ;
    skos:definition "Code used by FD_Table608 of Eurlex domain in ATTO."@en ;
    skos:inScheme atold:notation-type ;
    skos:prefLabel "FD_608"@en,
        "FD_608"@et ;
    skos:topConceptOf atold:notation-type .

<http://publications.europa.eu/resource/authority/notation-type/FD_609> a skos:Concept ;
    at:authority-code "FD_609" ;
    at:deprecated "false" ;
    at:op-code "FD_609" ;
    at:start.use "2010-03-29" ;
    atold:op-code "FD_609" ;
    dc:identifier "FD_609" ;
    skos:altLabel "FD_Table609 code"@en ;
    skos:definition "Code used by FD_Table609 of Eurlex domain in ATTO."@en ;
    skos:inScheme atold:notation-type ;
    skos:prefLabel "FD_609"@en,
        "FD_609"@et ;
    skos:topConceptOf atold:notation-type .

<http://publications.europa.eu/resource/authority/notation-type/FD_610> a skos:Concept ;
    at:authority-code "FD_610" ;
    at:deprecated "false" ;
    at:op-code "FD_610" ;
    at:start.use "2011-06-09" ;
    atold:op-code "FD_610" ;
    dc:identifier "FD_610" ;
    skos:altLabel "FD_Table610 code"@en ;
    skos:definition "Code used by FD_Table610 of Eurlex domain in ATTO."@en ;
    skos:inScheme atold:notation-type ;
    skos:prefLabel "FD_610"@en,
        "FD_610"@et ;
    skos:topConceptOf atold:notation-type .

<http://publications.europa.eu/resource/authority/notation-type/FD_612> a skos:Concept ;
    at:authority-code "FD_612" ;
    at:deprecated "false" ;
    at:op-code "FD_612" ;
    at:start.use "2010-03-29" ;
    atold:op-code "FD_612" ;
    dc:identifier "FD_612" ;
    skos:altLabel "FD_Table612 code"@en ;
    skos:definition "Code used by FD_Table612 of Eurlex domain in ATTO."@en ;
    skos:inScheme atold:notation-type ;
    skos:prefLabel "FD_612"@en,
        "FD_612"@et ;
    skos:topConceptOf atold:notation-type .

<http://publications.europa.eu/resource/authority/notation-type/FD_613> a skos:Concept ;
    at:authority-code "FD_613" ;
    at:deprecated "false" ;
    at:op-code "FD_613" ;
    at:start.use "2010-03-29" ;
    atold:op-code "FD_613" ;
    dc:identifier "FD_613" ;
    skos:altLabel "FD_Table613 code"@en ;
    skos:definition "Code used by FD_Table613 of Eurlex domain in ATTO."@en ;
    skos:inScheme atold:notation-type ;
    skos:prefLabel "FD_613"@en,
        "FD_613"@et ;
    skos:topConceptOf atold:notation-type .

<http://publications.europa.eu/resource/authority/notation-type/FILE_EXT> a skos:Concept ;
    at:authority-code "FILE_EXT" ;
    at:deprecated "false" ;
    at:op-code "FILE_EXT" ;
    at:op-mapped-code [ a at:MappedCode ;
            at:affected-table "notation-type" ;
            at:legacy-code "file-extension" ;
            dc:source "MDR" ] ;
    at:start.use "1973-01-01" ;
    atold:op-code "FILE_EXT" ;
    dc:identifier "FILE_EXT" ;
    skos:altLabel "File extensions code"@en ;
    skos:definition "A file extension is an identifier specified as a suffix to the name of a computer file. The extension indicates a characteristic of the file contents or its intended use. A file extension is typically delimited from the filename with a full stop."@en ;
    skos:inScheme atold:notation-type ;
    skos:prefLabel "File ext"@en,
        "File ext"@et ;
    skos:topConceptOf atold:notation-type .

<http://publications.europa.eu/resource/authority/notation-type/FORMEX> a skos:Concept ;
    at:authority-code "FORMEX" ;
    at:deprecated "false" ;
    at:op-code "FORMEX" ;
    at:start.use "2004-05-01" ;
    atold:op-code "FORMEX" ;
    dc:identifier "FORMEX" ;
    skos:altLabel "Formex code"@en ;
    skos:definition "Code used by Formalized Exchange of Electronic Publications."@en ;
    skos:inScheme atold:notation-type ;
    skos:prefLabel "Formex"@en,
        "Formex"@et ;
    skos:topConceptOf atold:notation-type .

<http://publications.europa.eu/resource/authority/notation-type/FUNDREF> a skos:Concept ;
    at:authority-code "FUNDREF" ;
    at:deprecated "false" ;
    at:op-code "FUNDREF" ;
    at:start.use "2012-01-01" ;
    atold:op-code "FUNDREF" ;
    dc:identifier "FUNDREF" ;
    skos:altLabel "FundRef identifier"@en ;
    skos:definition "FundRef is an identifier for an organisation that funds research. It is assigned by Crossref and maintained in its global FundRef registry."@en ;
    skos:exactMatch <http://purl.org/spar/datacite/fundref> ;
    skos:inScheme atold:notation-type ;
    skos:prefLabel "FundRef"@en,
        "FundRef"@et ;
    skos:topConceptOf atold:notation-type .

<http://publications.europa.eu/resource/authority/notation-type/HANDLE> a skos:Concept ;
    at:authority-code "HANDLE" ;
    at:deprecated "false" ;
    at:op-code "HANDLE" ;
    at:start.use "1994-12-31" ;
    atold:op-code "HANDLE" ;
    dc:identifier "HANDLE" ;
    skos:altLabel "Handle identifier"@en ;
    skos:definition "The Handle identifier is generated by the Handle System which allows secured name resolution and administration over the public Internet. A Handle is unique and can be retained over long time periods. The scheme is described in the RFC 1737."@en ;
    skos:exactMatch <http://purl.org/spar/datacite/handle> ;
    skos:inScheme atold:notation-type ;
    skos:prefLabel "Handle"@en,
        "Handle"@et ;
    skos:topConceptOf atold:notation-type .

<http://publications.europa.eu/resource/authority/notation-type/IANA_DOMAIN> a skos:Concept ;
    at:authority-code "IANA_DOMAIN" ;
    at:deprecated "false" ;
    at:op-code "IANA_DOMAIN" ;
    at:op-mapped-code [ a at:MappedCode ;
            at:affected-table "notation-type" ;
            at:legacy-code "code-iana" ;
            dc:source "MDR" ] ;
    at:start.use "1988-01-01" ;
    atold:op-code "IANA_DOMAIN" ;
    dc:identifier "IANA_DOMAIN" ;
    skos:altLabel "Internet Assigned Numbers Authority code"@en ;
    skos:definition "Internet Assigned Numbers Authority codes are two-letter codes for country-coded top-level domains in Internet addresses."@en ;
    skos:inScheme atold:notation-type ;
    skos:prefLabel "IANA"@en,
        "IANA"@et ;
    skos:topConceptOf atold:notation-type .

<http://publications.europa.eu/resource/authority/notation-type/IANA_MT> a skos:Concept ;
    at:authority-code "IANA_MT" ;
    at:deprecated "false" ;
    at:op-code "IANA_MT" ;
    at:op-mapped-code [ a at:MappedCode ;
            at:affected-table "notation-type" ;
            at:legacy-code "internet-media-type" ;
            dc:source "MDR" ] ;
    at:start.use "1988-01-01" ;
    atold:op-code "IANA_MT" ;
    dc:identifier "IANA_MT" ;
    skos:altLabel "Media Type (IANA) code"@en ;
    skos:definition "Code used by the Internet Assigned Numbers Authority (IANA) for media types."@en ;
    skos:inScheme atold:notation-type ;
    skos:prefLabel "IANA MIME"@en,
        "IANA MIME"@et ;
    skos:topConceptOf atold:notation-type .

<http://publications.europa.eu/resource/authority/notation-type/IATE> a skos:Concept ;
    at:authority-code "IATE" ;
    at:deprecated "false" ;
    at:op-code "IATE" ;
    at:op-mapped-code [ a at:MappedCode ;
            at:affected-table "notation-type" ;
            at:legacy-code "IATE.id" ;
            dc:source "MDR" ] ;
    at:start.use "2004-06-01" ;
    atold:op-code "IATE" ;
    dc:identifier "IATE" ;
    skos:altLabel "IATE code"@en ;
    skos:definition "Code used in IATE, Inter-Active Terminology for Europe."@en ;
    skos:inScheme atold:notation-type ;
    skos:prefLabel "IATE"@en,
        "IATE"@et ;
    skos:topConceptOf atold:notation-type .

<http://publications.europa.eu/resource/authority/notation-type/IBAN_COU> a skos:Concept ;
    at:authority-code "IBAN_COU" ;
    at:deprecated "false" ;
    at:op-code "IBAN_COU" ;
    at:start.use "2021-12-08" ;
    atold:op-code "IBAN_COU" ;
    dc:identifier "IBAN_COU" ;
    skos:definition "A two-letter country code (ISO 3166-1 alpha-2) used in the International Bank Account Number (IBAN) system. An IBAN consists of up to 34 alphanumeric characters comprising a country code; two check digits; and a number that includes the domestic bank account number, branch identifier, and potential routing information."@en ;
    skos:inScheme atold:notation-type ;
    skos:prefLabel "IBAN country code"@en ;
    skos:topConceptOf atold:notation-type .

<http://publications.europa.eu/resource/authority/notation-type/IENI> a skos:Concept ;
    at:authority-code "IENI" ;
    at:deprecated "false" ;
    at:op-code "IENI" ;
    at:start.use "2022-04-29" ;
    atold:op-code "IENI" ;
    dc:identifier "IENI" ;
    skos:altLabel "IENI collection"@en ;
    skos:definition "Identifier used in the collection (“IENI collection”) of acts related to the Ireland and Northern Ireland, based on the Protocol annexed to the Agreement on the withdrawal of the United Kingdom of Great Britain and Northern Ireland."@en ;
    skos:inScheme atold:notation-type ;
    skos:prefLabel "IENI"@en,
        "IENI"@et ;
    skos:topConceptOf atold:notation-type .

<http://publications.europa.eu/resource/authority/notation-type/INFOURI> a skos:Concept ;
    at:authority-code "INFOURI" ;
    at:deprecated "false" ;
    at:op-code "INFOURI" ;
    at:start.use "2005-12-30" ;
    atold:op-code "INFOURI" ;
    dc:identifier "INFOURI" ;
    skos:altLabel "Info URI"@en ;
    skos:definition "The Info URI identifier is an URI conforming to the Info URI scheme which enables identifiers from public namespaces to be represented as URIs when they would otherwise have no canonical URL form."@en ;
    skos:exactMatch <http://purl.org/spar/datacite/infouri> ;
    skos:inScheme atold:notation-type ;
    skos:prefLabel "INFO URI"@en,
        "INFO URI"@et ;
    skos:topConceptOf atold:notation-type .

<http://publications.europa.eu/resource/authority/notation-type/ISBN> a skos:Concept ;
    at:authority-code "ISBN" ;
    at:deprecated "false" ;
    at:op-code "ISBN" ;
    at:start.use "1970-01-01" ;
    atold:op-code "ISBN" ;
    dc:identifier "ISBN" ;
    skos:altLabel "International Standard Book Number code"@en ;
    skos:definition "An ISBN is essentially a product identifier used by publishers, booksellers, libraries, internet retailers and other supply chain participants for ordering, listing, sales records and stock control purposes. The ISBN identifies the registrant as well as the specific title, edition and format. ISBNs are calculated using a specific mathematical formula and include a check digit to validate the number. ISBN is an International Standard that is published by ISO."@en ;
    skos:exactMatch <http://purl.org/spar/datacite/isbn> ;
    skos:inScheme atold:notation-type ;
    skos:prefLabel "ISBN"@en,
        "ISBN"@et ;
    skos:topConceptOf atold:notation-type .

<http://publications.europa.eu/resource/authority/notation-type/ISBN_RG> a skos:Concept ;
    at:authority-code "ISBN_RG" ;
    at:deprecated "false" ;
    at:op-code "ISBN_RG" ;
    at:op-mapped-code [ a at:MappedCode ;
            at:affected-table "notation-type" ;
            at:legacy-code "id-isbn.old" ;
            dc:source "MDR" ],
        [ a at:MappedCode ;
            at:affected-table "notation-type" ;
            at:legacy-code "id-isbn" ;
            dc:source "MDR" ] ;
    at:start.use "2000-01-01" ;
    atold:op-code "ISBN_RG" ;
    dc:identifier "ISBN_RG" ;
    skos:altLabel "ISBN registrant element"@en ;
    skos:definition "Each ISBN consists of 5 elements with each section being separated by spaces or hyphens. The ISBN registrant element identifies the particular publisher or imprint."@en ;
    skos:inScheme atold:notation-type ;
    skos:prefLabel "ISBN reg ele"@en,
        "ISBN reg ele"@et ;
    skos:topConceptOf atold:notation-type .

<http://publications.europa.eu/resource/authority/notation-type/ISG_COU> a skos:Concept ;
    at:authority-code "ISG_COU" ;
    at:deprecated "false" ;
    at:op-code "ISG_COU" ;
    at:op-mapped-code [ a at:MappedCode ;
            at:affected-table "notation-type" ;
            at:legacy-code "op-styleguide" ;
            dc:source "MDR" ] ;
    at:start.use "1993-01-01" ;
    atold:op-code "ISG_COU" ;
    dc:identifier "ISG_COU" ;
    skos:altLabel "ISG country code"@en ;
    skos:definition "Country code used in the Interinstitutional style guide."@en ;
    skos:inScheme atold:notation-type ;
    skos:prefLabel "ISG COU"@en,
        "ISG COU"@et ;
    skos:topConceptOf atold:notation-type .

<http://publications.europa.eu/resource/authority/notation-type/ISNI> a skos:Concept ;
    at:authority-code "ISNI" ;
    at:deprecated "false" ;
    at:op-code "ISNI" ;
    at:start.use "2012-03-15" ;
    atold:op-code "ISNI" ;
    dc:identifier "ISNI" ;
    skos:altLabel "International Standard Name Identifier"@en ;
    skos:definition "ISNI is the ISO certified global standard number for identifying the millions of contributors to creative works and those active in their distribution, including researchers, inventors, writers, artists, visual creators, performers, producers, publishers, aggregators, and more."@en ;
    skos:exactMatch <http://purl.org/spar/datacite/isni> ;
    skos:inScheme atold:notation-type ;
    skos:prefLabel "ISNI"@en,
        "ISNI"@et ;
    skos:topConceptOf atold:notation-type .

<http://publications.europa.eu/resource/authority/notation-type/ISO_15924_ALPHA_4> a skos:Concept ;
    at:authority-code "ISO_15924_ALPHA_4" ;
    at:deprecated "false" ;
    at:op-code "ISO_15924_ALPHA_4" ;
    at:op-mapped-code [ a at:MappedCode ;
            at:affected-table "notation-type" ;
            at:legacy-code "iso-15924-alpha-4" ;
            dc:source "MDR" ] ;
    at:start.use "2020-06-24" ;
    atold:op-code "ISO_15924_ALPHA_4" ;
    dc:identifier "ISO_15924_ALPHA_4" ;
    skos:altLabel "ISO 15924 alpha-4 code"@en ;
    skos:definition "ISO 15924 alpha-4 codes are four-letter script codes defined in ISO 15924 standard published by the International Organization for Standardization (ISO), to represent names of scripts. Script is defined as ‘set of graphic characters used for the written form of one or more languages’."@en ;
    skos:inScheme atold:notation-type ;
    skos:prefLabel "ISO 15924 α-4"@en,
        "ISO 15924 α-4"@et ;
    skos:topConceptOf atold:notation-type .

<http://publications.europa.eu/resource/authority/notation-type/ISO_15924_NUM> a skos:Concept ;
    at:authority-code "ISO_15924_NUM" ;
    at:deprecated "false" ;
    at:op-code "ISO_15924_NUM" ;
    at:op-mapped-code [ a at:MappedCode ;
            at:affected-table "notation-type" ;
            at:legacy-code "iso-15924-num" ;
            dc:source "MDR" ] ;
    at:start.use "2020-06-24" ;
    atold:op-code "ISO_15924_NUM" ;
    dc:identifier "ISO_15924_NUM" ;
    skos:altLabel "ISO 15924 numeric code"@en ;
    skos:definition "ISO 15924 numeric codes are three-digit script codes defined in ISO 15924 standard published by the International Organization for Standardization (ISO), to represent names of scripts. Script is defined as ‘set of graphic characters used for the written form of one or more languages’."@en ;
    skos:inScheme atold:notation-type ;
    skos:prefLabel "ISO 15924 num"@en,
        "ISO 15924 num"@et ;
    skos:topConceptOf atold:notation-type .

<http://publications.europa.eu/resource/authority/notation-type/ISO_3166_1_ALPHA_2> a skos:Concept ;
    at:authority-code "ISO_3166_1_ALPHA_2" ;
    at:deprecated "false" ;
    at:op-code "ISO_3166_1_ALPHA_2" ;
    at:op-mapped-code [ a at:MappedCode ;
            at:affected-table "notation-type" ;
            at:legacy-code "code-3166-1-alpha-2" ;
            dc:source "MDR" ] ;
    at:start.use "1997-01-01" ;
    atold:op-code "ISO_3166_1_ALPHA_2" ;
    dc:identifier "ISO_3166_1_ALPHA_2" ;
    skos:altLabel "ISO 3166-1 alpha-2 code"@en ;
    skos:definition "ISO 3166-1 alpha-2 codes are two-letter country codes defined in ISO 3166-1, part of the ISO 3166 standard published by the International Organization for Standardization (ISO), to represent countries, dependent territories, and special areas of geographical interest."@en ;
    skos:inScheme atold:notation-type ;
    skos:prefLabel "ISO 3166-1 α-2"@en,
        "ISO 3166-1 α-2"@et ;
    skos:topConceptOf atold:notation-type .

<http://publications.europa.eu/resource/authority/notation-type/ISO_3166_1_ALPHA_3> a skos:Concept ;
    at:authority-code "ISO_3166_1_ALPHA_3" ;
    at:deprecated "false" ;
    at:op-code "ISO_3166_1_ALPHA_3" ;
    at:op-mapped-code [ a at:MappedCode ;
            at:affected-table "notation-type" ;
            at:legacy-code "code-3166-1-alpha-3" ;
            dc:source "MDR" ] ;
    at:start.use "1997-01-01" ;
    atold:op-code "ISO_3166_1_ALPHA_3" ;
    dc:identifier "ISO_3166_1_ALPHA_3" ;
    skos:altLabel "ISO 3166-1 alpha-3 code"@en ;
    skos:definition "ISO 3166-1 alpha-3 codes are three-letter country codes defined in ISO 3166-1, part of the ISO 3166 standard published by the International Organization for Standardization (ISO), to represent countries, dependent territories, and special areas of geographical interest."@en ;
    skos:inScheme atold:notation-type ;
    skos:prefLabel "ISO 3166-1 α-3"@en,
        "ISO 3166-1 α-3"@et ;
    skos:topConceptOf atold:notation-type .

<http://publications.europa.eu/resource/authority/notation-type/ISO_3166_1_NUM> a skos:Concept ;
    at:authority-code "ISO_3166_1_NUM" ;
    at:deprecated "false" ;
    at:op-code "ISO_3166_1_NUM" ;
    at:op-mapped-code [ a at:MappedCode ;
            at:affected-table "notation-type" ;
            at:legacy-code "code-3166-1-num" ;
            dc:source "MDR" ] ;
    at:start.use "1981-01-01" ;
    atold:op-code "ISO_3166_1_NUM" ;
    dc:identifier "ISO_3166_1_NUM" ;
    skos:altLabel "ISO 3166-1 numeric code"@en ;
    skos:definition "ISO 3166-1 numeric (or numeric-3) codes are three-digit country codes defined in ISO 3166-1, part of the ISO 3166 standard published by the International Organization for Standardization (ISO), to represent countries, dependent territories, and special areas of geographical interest. They are similar to the three-digit country codes developed and maintained by the United Nations Statistics Division, from which they originate in its UN M.49 standard."@en ;
    skos:inScheme atold:notation-type ;
    skos:prefLabel "ISO 3166-1 num"@en,
        "ISO 3166-1 num"@et ;
    skos:topConceptOf atold:notation-type .

<http://publications.europa.eu/resource/authority/notation-type/ISO_3166_2> a skos:Concept ;
    at:authority-code "ISO_3166_2" ;
    at:deprecated "false" ;
    at:op-code "ISO_3166_2" ;
    at:op-mapped-code [ a at:MappedCode ;
            at:affected-table "notation-type" ;
            at:legacy-code "code-3166-2" ;
            dc:source "MDR" ] ;
    at:start.use "1998-01-01" ;
    atold:op-code "ISO_3166_2" ;
    dc:identifier "ISO_3166_2" ;
    skos:altLabel "ISO 3166-2 code"@en ;
    skos:definition "ISO 3166-2 codes identify the principal subdivisions (e.g. provinces or states) of all countries coded in ISO 3166-1."@en ;
    skos:inScheme atold:notation-type ;
    skos:prefLabel "ISO 3166-2"@en,
        "ISO 3166-2"@et ;
    skos:topConceptOf atold:notation-type .

<http://publications.europa.eu/resource/authority/notation-type/ISO_3166_3> a skos:Concept ;
    at:authority-code "ISO_3166_3" ;
    at:deprecated "false" ;
    at:op-code "ISO_3166_3" ;
    at:op-mapped-code [ a at:MappedCode ;
            at:affected-table "notation-type" ;
            at:legacy-code "code-3166-3" ;
            dc:source "MDR" ] ;
    at:start.use "1999-01-01" ;
    atold:op-code "ISO_3166_3" ;
    dc:identifier "ISO_3166_3" ;
    skos:altLabel "ISO 3166-3 code"@en ;
    skos:definition "ISO 3166-3 is part of the ISO 3166 standard published by the International Organization for Standardization (ISO), and defines codes for country names which have been deleted from ISO 3166-1. Each former country name in ISO 3166-3 is assigned a four-letter alphabetic code."@en ;
    skos:inScheme atold:notation-type ;
    skos:prefLabel "ISO 3166-3"@en,
        "ISO 3166-3"@et ;
    skos:topConceptOf atold:notation-type .

<http://publications.europa.eu/resource/authority/notation-type/ISO_4217> a skos:Concept ;
    at:authority-code "ISO_4217" ;
    at:deprecated "false" ;
    at:op-code "ISO_4217" ;
    at:op-mapped-code [ a at:MappedCode ;
            at:affected-table "notation-type" ;
            at:legacy-code "code-4217" ;
            dc:source "MDR" ] ;
    at:start.use "1978-02-01" ;
    atold:op-code "ISO_4217" ;
    dc:identifier "ISO_4217" ;
    skos:altLabel "ISO 4217 code"@en ;
    skos:definition "ISO 4217 codes are used for the identification of currencies and funds organised in the following lists: current currency and funds code, current funds codes, codes for historic denominations of currencies and funds."@en ;
    skos:inScheme atold:notation-type ;
    skos:prefLabel "ISO 4217"@en,
        "ISO 4217"@et ;
    skos:topConceptOf atold:notation-type .

<http://publications.europa.eu/resource/authority/notation-type/ISO_4217_NUM> a skos:Concept ;
    at:authority-code "ISO_4217_NUM" ;
    at:deprecated "false" ;
    at:op-code "ISO_4217_NUM" ;
    at:start.use "1978-02-01" ;
    atold:op-code "ISO_4217_NUM" ;
    dc:identifier "ISO_4217_NUM" ;
    skos:altLabel "ISO 4217 numeric code"@en ;
    skos:definition "ISO 4217 numeric codes are three-digit currency codes defined in ISO 4217 standard published by the International Organization for Standardization (ISO), to represent currencies and funds."@en ;
    skos:inScheme atold:notation-type ;
    skos:prefLabel "ISO 4217 num"@en,
        "ISO 4217 num"@et ;
    skos:topConceptOf atold:notation-type .

<http://publications.europa.eu/resource/authority/notation-type/ISO_5218_2> a skos:Concept ;
    at:authority-code "ISO_5218_2" ;
    at:deprecated "false" ;
    at:op-code "ISO_5218_2" ;
    at:op-mapped-code [ a at:MappedCode ;
            at:affected-table "notation-type" ;
            at:legacy-code "code-5218-2" ;
            dc:source "MDR" ] ;
    at:start.use "1976-11-01" ;
    atold:op-code "ISO_5218_2" ;
    dc:identifier "ISO_5218_2" ;
    skos:altLabel "ISO 5218-2 code"@en ;
    skos:definition "ISO 5218-2 codes define a representation of human sexes through a language-neutral single-digit code."@en ;
    skos:inScheme atold:notation-type ;
    skos:prefLabel "ISO 5218-2"@en,
        "ISO 5218-2"@et ;
    skos:topConceptOf atold:notation-type .

<http://publications.europa.eu/resource/authority/notation-type/ISO_639_1> a skos:Concept ;
    at:authority-code "ISO_639_1" ;
    at:deprecated "false" ;
    at:op-code "ISO_639_1" ;
    at:op-mapped-code [ a at:MappedCode ;
            at:affected-table "notation-type" ;
            at:legacy-code "iso-639-1" ;
            dc:source "MDR" ] ;
    at:start.use "1967-01-01" ;
    atold:op-code "ISO_639_1" ;
    dc:identifier "ISO_639_1" ;
    skos:altLabel "ISO 639-1 code"@en ;
    skos:definition "A two-letter code that has been designed to represent most of the major languages of the world."@en ;
    skos:inScheme atold:notation-type ;
    skos:prefLabel "ISO 639-1"@en,
        "ISO 639-1"@et ;
    skos:topConceptOf atold:notation-type .

<http://publications.europa.eu/resource/authority/notation-type/ISO_639_2B> a skos:Concept ;
    at:authority-code "ISO_639_2B" ;
    at:deprecated "false" ;
    at:op-code "ISO_639_2B" ;
    at:op-mapped-code [ a at:MappedCode ;
            at:affected-table "notation-type" ;
            at:legacy-code "iso-639-2b" ;
            dc:source "MDR" ] ;
    at:start.use "1989-01-01" ;
    atold:op-code "ISO_639_2B" ;
    dc:identifier "ISO_639_2B" ;
    skos:altLabel "ISO 639-2 – bibliographic code"@en ;
    skos:definition "A three-letter code which is derived from the English name for the language and gives more possible combinations, so ISO 639-2:1998 can cover more languages."@en ;
    skos:inScheme atold:notation-type ;
    skos:prefLabel "ISO 639-2 b"@en,
        "ISO 639-2 b"@et ;
    skos:topConceptOf atold:notation-type .

<http://publications.europa.eu/resource/authority/notation-type/ISO_639_2T> a skos:Concept ;
    at:authority-code "ISO_639_2T" ;
    at:deprecated "false" ;
    at:op-code "ISO_639_2T" ;
    at:op-mapped-code [ a at:MappedCode ;
            at:affected-table "notation-type" ;
            at:legacy-code "iso-639-2t" ;
            dc:source "MDR" ] ;
    at:start.use "1989-01-01" ;
    atold:op-code "ISO_639_2T" ;
    dc:identifier "ISO_639_2T" ;
    skos:altLabel "ISO 639-2 – terminological code"@en ;
    skos:definition "A three-letter code which is derived from the native name for the language and resembles the language's two-letter code in ISO 639-1 and which gives more possible combinations, so ISO 639-2:1998 can cover more languages."@en ;
    skos:inScheme atold:notation-type ;
    skos:prefLabel "ISO 639-2 t"@en,
        "ISO 639-2 t"@et ;
    skos:topConceptOf atold:notation-type .

<http://publications.europa.eu/resource/authority/notation-type/ISO_639_3> a skos:Concept ;
    at:authority-code "ISO_639_3" ;
    at:deprecated "false" ;
    at:op-code "ISO_639_3" ;
    at:op-mapped-code [ a at:MappedCode ;
            at:affected-table "notation-type" ;
            at:legacy-code "iso-639-3" ;
            dc:source "MDR" ] ;
    at:start.use "2007-02-01" ;
    atold:op-code "ISO_639_3" ;
    dc:identifier "ISO_639_3" ;
    skos:altLabel "ISO 639-3 code"@en ;
    skos:definition "A three-letter code which aims to give as complete a listing of languages as possible, including living, extinct and ancient languages."@en ;
    skos:inScheme atold:notation-type ;
    skos:prefLabel "ISO 639-3"@en,
        "ISO 639-3"@et ;
    skos:topConceptOf atold:notation-type .

<http://publications.europa.eu/resource/authority/notation-type/ISSN> a skos:Concept ;
    at:authority-code "ISSN" ;
    at:deprecated "false" ;
    at:op-code "ISSN" ;
    at:start.use "1975-01-01" ;
    atold:op-code "ISSN" ;
    dc:identifier "ISSN" ;
    skos:altLabel "International Standard Serial Number"@en ;
    skos:definition "Eight-digit number which identifies all periodical publications as such, including electronic serials. Each ISSN assigned to a serial publication is registered in an international database: the ISSN Register. It is the most comprehensive and authoritative source for the identification of serial publications world-wide."@en ;
    skos:exactMatch <http://purl.org/spar/datacite/issn> ;
    skos:inScheme atold:notation-type ;
    skos:prefLabel "ISSN"@en,
        "ISSN"@et ;
    skos:topConceptOf atold:notation-type .

<http://publications.europa.eu/resource/authority/notation-type/ISSN_L> a skos:Concept ;
    at:authority-code "ISSN_L" ;
    at:deprecated "false" ;
    at:op-code "ISSN_L" ;
    at:start.use "2007-12-31" ;
    atold:op-code "ISSN_L" ;
    dc:identifier "ISSN_L" ;
    skos:altLabel "Linking ISSN"@en ;
    skos:definition "The linking ISSN (ISSN-L) is a specific ISSN that groups the different media of the same serial publication. A single ISSN-L is designated for all media of a serial publication, irrespective of how many there are."@en ;
    skos:exactMatch <http://purl.org/spar/datacite/lissn> ;
    skos:inScheme atold:notation-type ;
    skos:prefLabel "ISSN-L"@en,
        "ISSN-L"@et ;
    skos:topConceptOf atold:notation-type .

<http://publications.europa.eu/resource/authority/notation-type/ISTC> a skos:Concept ;
    at:authority-code "ISTC" ;
    at:deprecated "false" ;
    at:op-code "ISTC" ;
    at:start.use "2009-03-01" ;
    atold:op-code "ISTC" ;
    dc:identifier "ISTC" ;
    skos:altLabel "International Standard Text Code"@en ;
    skos:definition "ISTC is a numbering system for the unique identification of text-based works; the term “work” can refer to any content appearing in conventional printed books, audio-books, static e-books or enhanced digital books, as well as content which might appear in a newspaper or journal."@en ;
    skos:exactMatch <http://purl.org/spar/datacite/istc> ;
    skos:inScheme atold:notation-type ;
    skos:prefLabel "ISTC"@en,
        "ISTC"@et ;
    skos:topConceptOf atold:notation-type .

<http://publications.europa.eu/resource/authority/notation-type/LAC> a skos:Concept ;
    at:authority-code "LAC" ;
    at:deprecated "false" ;
    at:op-code "LAC" ;
    at:start.use "1958-01-01" ;
    atold:op-code "LAC" ;
    dc:identifier "LAC" ;
    skos:altLabel "Legacy authority code"@en ;
    skos:definition "This concept identifies the mnemonic denotation of a concept used in authority tables."@en ;
    skos:inScheme atold:notation-type ;
    skos:prefLabel "Legacy code"@en,
        "Aegunud kood (legacy)"@et ;
    skos:topConceptOf atold:notation-type .

<http://publications.europa.eu/resource/authority/notation-type/LITIGE> a skos:Concept ;
    at:authority-code "LITIGE" ;
    at:deprecated "false" ;
    at:op-code "LITIGE" ;
    at:start.use "1998-11-12" ;
    atold:op-code "LITIGE" ;
    dc:identifier "LITIGE" ;
    skos:altLabel "Litige code"@en ;
    skos:definition "Code used in the system Litige of the Court of Justice."@en ;
    skos:inScheme atold:notation-type ;
    skos:prefLabel "Litige"@en,
        "Litige"@et ;
    skos:topConceptOf atold:notation-type .

<http://publications.europa.eu/resource/authority/notation-type/LRIS> a skos:Concept ;
    at:authority-code "LRIS" ;
    at:deprecated "false" ;
    at:op-code "LRIS" ;
    at:start.use "2012-12-31" ;
    atold:op-code "LRIS" ;
    dc:identifier "LRIS" ;
    skos:altLabel "Local Resource Identifier"@en ;
    skos:definition "The Local Resource Identifier is generated by the resource identifier scheme that provides local resource identifiers that are unique in their local environment and understood by the person submitting the metadata."@en ;
    skos:exactMatch <http://purl.org/spar/datacite/local-resource-identifier-scheme> ;
    skos:inScheme atold:notation-type ;
    skos:prefLabel "LRIS"@en,
        "LRIS"@et ;
    skos:topConceptOf atold:notation-type .

<http://publications.europa.eu/resource/authority/notation-type/LSID> a skos:Concept ;
    at:authority-code "LSID" ;
    at:deprecated "false" ;
    at:op-code "LSID" ;
    at:start.use "2003-09-30" ;
    atold:op-code "LSID" ;
    dc:identifier "LSID" ;
    skos:altLabel "Life Science Identifier"@en ;
    skos:definition "The Life Sciences Identifier (LSID) is a persistent, location-independent, globally unique identifier for biological objects in the life sciences domain specified by OMG Life Sciences Research. LSID is represented as a Uniform Resource Name (URN)."@en ;
    skos:exactMatch <http://purl.org/spar/datacite/lsid> ;
    skos:inScheme atold:notation-type ;
    skos:prefLabel "LSID"@en,
        "LSID"@et ;
    skos:topConceptOf atold:notation-type .

<http://publications.europa.eu/resource/authority/notation-type/MINIDOC> a skos:Concept ;
    at:authority-code "MINIDOC" ;
    at:deprecated "false" ;
    at:op-code "MINIDOC" ;
    at:start.use "1952-07-24" ;
    atold:op-code "MINIDOC" ;
    dc:identifier "MINIDOC" ;
    skos:altLabel "Minidoc code"@en ;
    skos:definition "Code used in the system Minidoc of the Court of Justice."@en ;
    skos:inScheme atold:notation-type ;
    skos:prefLabel "Minidoc"@en,
        "Minidoc"@et ;
    skos:topConceptOf atold:notation-type .

<http://publications.europa.eu/resource/authority/notation-type/MNE> a skos:Concept ;
    at:authority-code "MNE" ;
    at:deprecated "false" ;
    at:op-code "MNE" ;
    at:op-mapped-code [ a at:MappedCode ;
            at:affected-table "notation-type" ;
            at:legacy-code "VOLET_MNE" ;
            dc:source "MDR" ] ;
    at:start.use "1969-01-18" ;
    atold:op-code "MNE" ;
    dc:identifier "MNE" ;
    skos:altLabel "MNE code"@en ;
    skos:definition "Code used by Procat for national transposing measures/mesures nationales de transposition."@en ;
    skos:inScheme atold:notation-type ;
    skos:prefLabel "MNE"@en,
        "MNE"@et ;
    skos:topConceptOf atold:notation-type .

<http://publications.europa.eu/resource/authority/notation-type/NIHMSID> a skos:Concept ;
    at:authority-code "NIHMSID" ;
    at:deprecated "false" ;
    at:op-code "NIHMSID" ;
    at:start.use "2005-12-31" ;
    atold:op-code "NIHMSID" ;
    dc:identifier "NIHMSID" ;
    skos:altLabel "NIH Manuscript Submission Identifier"@en ;
    skos:definition "The NIHMSID is an ID used to identify publications which have been initially submitted into the NIH Manuscript Submission System for eventual deposit in PubMed Central. Once the web version of the publication is approved for inclusion in PMC and the corresponding citation is in PubMed, the article will also be assigned a PMCID."@en ;
    skos:exactMatch <http://purl.org/spar/datacite/nihmsid> ;
    skos:inScheme atold:notation-type ;
    skos:prefLabel "NIHMSID"@en,
        "NIHMSID"@et ;
    skos:topConceptOf atold:notation-type .

<http://publications.europa.eu/resource/authority/notation-type/OCI> a skos:Concept ;
    at:authority-code "OCI" ;
    at:deprecated "false" ;
    at:op-code "OCI" ;
    at:start.use "2015-12-31" ;
    atold:op-code "OCI" ;
    dc:identifier "OCI" ;
    skos:altLabel "Open Citation Identifier"@en ;
    skos:definition "The Open Citation Identifier (OCI) is a globally unique persistent identifier for bibliographic citations. Within the OpenCitations Corpus, these bibliographic resource identifiers are unique, and every citation recorded in OCC has an OCI."@en ;
    skos:exactMatch <http://purl.org/spar/datacite/oci> ;
    skos:inScheme atold:notation-type ;
    skos:prefLabel "OCI"@en,
        "OCI"@et ;
    skos:topConceptOf atold:notation-type .

<http://publications.europa.eu/resource/authority/notation-type/ODP> a skos:Concept ;
    at:authority-code "ODP" ;
    at:deprecated "false" ;
    at:op-code "ODP" ;
    at:start.use "2012-04-19" ;
    atold:op-code "ODP" ;
    dc:identifier "ODP" ;
    skos:altLabel "ODP code"@en ;
    skos:definition "Code used by the EU Open Data Portal which provides access to open public data produced by EU institutions, agencies and bodies."@en ;
    skos:inScheme atold:notation-type ;
    skos:prefLabel "ODP"@en,
        "ODP"@et ;
    skos:topConceptOf atold:notation-type .

<http://publications.europa.eu/resource/authority/notation-type/OJ> a skos:Concept ;
    at:authority-code "OJ" ;
    at:deprecated "false" ;
    at:op-code "OJ" ;
    at:start.use "1952-12-30" ;
    atold:op-code "OJ" ;
    dc:identifier "OJ" ;
    skos:altLabel "OJ code"@en ;
    skos:definition "Code used in the Official Journal."@en ;
    skos:inScheme atold:notation-type ;
    skos:prefLabel "OJ id"@en,
        "OJ id"@et ;
    skos:topConceptOf atold:notation-type .

<http://publications.europa.eu/resource/authority/notation-type/OJ_SECTION> a skos:Concept ;
    at:authority-code "OJ_SECTION" ;
    at:deprecated "false" ;
    at:op-code "OJ_SECTION" ;
    at:op-mapped-code [ a at:MappedCode ;
            at:affected-table "notation-type" ;
            at:legacy-code "oj.section" ;
            dc:source "MDR" ] ;
    at:start.use "1952-12-30" ;
    atold:op-code "OJ_SECTION" ;
    dc:identifier "OJ_SECTION" ;
    skos:altLabel "OJ section code"@en ;
    skos:definition "Code used to identify the section of the OJ."@en ;
    skos:inScheme atold:notation-type ;
    skos:prefLabel "OJ section"@en,
        "OJ osa"@et ;
    skos:topConceptOf atold:notation-type .

<http://publications.europa.eu/resource/authority/notation-type/ONIX> a skos:Concept ;
    at:authority-code "ONIX" ;
    at:deprecated "false" ;
    at:op-code "ONIX" ;
    at:start.use "2000-01-01" ;
    atold:op-code "ONIX" ;
    dc:identifier "ONIX" ;
    skos:altLabel "ONIX code"@en ;
    skos:definition "Code value from ONIX for Books."@en ;
    skos:inScheme atold:notation-type ;
    skos:prefLabel "ONIX"@en,
        "ONIX"@et ;
    skos:topConceptOf atold:notation-type .

<http://publications.europa.eu/resource/authority/notation-type/OP_CAT> a skos:Concept ;
    at:authority-code "OP_CAT" ;
    at:deprecated "false" ;
    at:op-code "OP_CAT" ;
    at:op-mapped-code [ a at:MappedCode ;
            at:affected-table "notation-type" ;
            at:legacy-code "cat.no" ;
            dc:source "MDR" ],
        [ a at:MappedCode ;
            at:affected-table "notation-type" ;
            at:legacy-code "cat.no.old" ;
            dc:source "MDR" ] ;
    at:start.use "1969-01-18" ;
    atold:op-code "OP_CAT" ;
    dc:identifier "OP_CAT" ;
    skos:altLabel "OP catalogue number"@en ;
    skos:definition "An internal identifier assigned to all works created by the Publications Office. It is used to categorise publications in catalogues, amongst other things. It is also used as an identification key in various IT applications, as is the case for EU Bookshop, the European institutions’ online bookshop."@en ;
    skos:inScheme atold:notation-type ;
    skos:prefLabel "OP cat"@en,
        "OP cat"@et ;
    skos:topConceptOf atold:notation-type .

<http://publications.europa.eu/resource/authority/notation-type/OP_DATPRO> a skos:Concept ;
    at:authority-code "OP_DATPRO" ;
    at:deprecated "false" ;
    at:op-code "OP_DATPRO" ;
    at:start.use "1952-07-23" ;
    atold:op-code "OP_DATPRO" ;
    dc:identifier "OP_DATPRO" ;
    skos:inScheme atold:notation-type ;
    skos:prefLabel "НЕОКОНЧАТЕЛНИ ДАННИ"@bg,
        "Předběžné údaje"@cs,
        "Midlertidige data"@da,
        "Vorläufige Daten"@de,
        "Προσωρινά δεδομένα"@el,
        "Provisional data"@en,
        "Datos provisionales"@es,
        "Esialgsed andmed"@et,
        "Alustavat tiedot"@fi,
        "Données provisoires"@fr,
        "Sonraí sealadacha"@ga,
        "Privremeni podaci"@hr,
        "Ideiglenes adatok"@hu,
        "Dati provvisori"@it,
        "Laikinieji duomenys"@lt,
        "Provizoriski dati"@lv,
        "Dejta provviżorja"@mt,
        "Voorlopige gegevens"@nl,
        "Dane tymczasowe"@pl,
        "Dados provisórios"@pt,
        "Date provizorii"@ro,
        "Predbežné údaje"@sk,
        "Začasni podatki"@sl,
        "Tillfälliga uppgifter"@sv ;
    skos:topConceptOf atold:notation-type .

<http://publications.europa.eu/resource/authority/notation-type/ORCID> a skos:Concept ;
    at:authority-code "ORCID" ;
    at:deprecated "false" ;
    at:op-code "ORCID" ;
    at:start.use "2012-10-16" ;
    atold:op-code "ORCID" ;
    dc:identifier "ORCID" ;
    skos:altLabel "ORCID identifier"@en ;
    skos:definition "ORCID is a non-proprietary persistent digital identifier that uniquely identifies researchers."@en ;
    skos:exactMatch <http://purl.org/spar/datacite/orcid> ;
    skos:inScheme atold:notation-type ;
    skos:prefLabel "ORCID"@en,
        "ORCID"@et ;
    skos:topConceptOf atold:notation-type .

<http://publications.europa.eu/resource/authority/notation-type/PEGASE> a skos:Concept ;
    at:authority-code "PEGASE" ;
    at:deprecated "false" ;
    at:op-code "PEGASE" ;
    at:op-mapped-code [ a at:MappedCode ;
            at:affected-table "notation-type" ;
            at:legacy-code "Pegase" ;
            dc:source "MDR" ] ;
    at:start.use "2001-10-10" ;
    atold:op-code "PEGASE" ;
    dc:identifier "PEGASE" ;
    skos:altLabel "Pégase code"@en ;
    skos:definition "Code from Pégase, an application managed by the Secretariat-General of the European Commission which allows to encode the different information concerning the interinstitutional procedures with the aim to feed information systems such as SG Vista and Prelex."@en ;
    skos:inScheme atold:notation-type ;
    skos:prefLabel "Pégase"@en,
        "Pégase"@et ;
    skos:topConceptOf atold:notation-type .

<http://publications.europa.eu/resource/authority/notation-type/PHONE_PREFIX> a skos:Concept ;
    at:authority-code "PHONE_PREFIX" ;
    at:deprecated "false" ;
    at:op-code "PHONE_PREFIX" ;
    at:start.use "2021-12-08" ;
    atold:op-code "PHONE_PREFIX" ;
    dc:identifier "PHONE_PREFIX" ;
    skos:definition "Country calling codes or country dial-in codes are telephone number prefixes for reaching telephone subscribers in the networks of the member countries or regions of the International Telecommunication Union (ITU). Country codes are a component of the international telephone numbering plan, and are necessary only when dialing a telephone number to establish a call to another country. Country codes are dialed before the national telephone number."@en ;
    skos:inScheme atold:notation-type ;
    skos:prefLabel "Country calling code"@en ;
    skos:topConceptOf atold:notation-type .

<http://publications.europa.eu/resource/authority/notation-type/PII> a skos:Concept ;
    at:authority-code "PII" ;
    at:deprecated "false" ;
    at:op-code "PII" ;
    at:start.use "1996-01-01" ;
    atold:op-code "PII" ;
    dc:identifier "PII" ;
    skos:altLabel "Publisher Item Identifier"@en ;
    skos:definition "The Publisher Item Identifier (PII) is an alphanumeric string of characters using a pre-existing ISSN or ISBN. It uniquely identifies an article and can be used for future cataloging, searching, and electronic retrieval."@en ;
    skos:exactMatch <http://purl.org/spar/datacite/pii> ;
    skos:inScheme atold:notation-type ;
    skos:prefLabel "PII"@en,
        "PII"@et ;
    skos:topConceptOf atold:notation-type .

<http://publications.europa.eu/resource/authority/notation-type/PLANJO> a skos:Concept ;
    at:authority-code "PLANJO" ;
    at:deprecated "false" ;
    at:op-code "PLANJO" ;
    at:op-mapped-code [ a at:MappedCode ;
            at:affected-table "notation-type" ;
            at:legacy-code "PLANJO_CODES" ;
            dc:source "MDR" ] ;
    at:start.use "2002-04-25" ;
    atold:op-code "PLANJO" ;
    dc:identifier "PLANJO" ;
    skos:altLabel "PlanJO code"@en ;
    skos:definition "Code used by PlanJO, the internal workflow system used for the legal acts and documents published in the Official Journal L and C."@en ;
    skos:inScheme atold:notation-type ;
    skos:prefLabel "PlanJO"@en,
        "PlanJO"@et ;
    skos:topConceptOf atold:notation-type .

<http://publications.europa.eu/resource/authority/notation-type/PMCID> a skos:Concept ;
    at:authority-code "PMCID" ;
    at:deprecated "false" ;
    at:op-code "PMCID" ;
    at:start.use "2000-02-28" ;
    atold:op-code "PMCID" ;
    dc:identifier "PMCID" ;
    skos:altLabel "PubMed Central Identifier"@en ;
    skos:definition "The PMCID (PubMed Central Identifier), also known as the PMC reference number, is a bibliographic identifier assigned by the National Library of Medicine to each full-text paper in PubMed Central, a free archive of biomedical and life sciences journal literature."@en ;
    skos:exactMatch <http://purl.org/spar/datacite/pmcid> ;
    skos:inScheme atold:notation-type ;
    skos:prefLabel "PMCID"@en,
        "PMCID"@et ;
    skos:topConceptOf atold:notation-type .

<http://publications.europa.eu/resource/authority/notation-type/PMID> a skos:Concept ;
    at:authority-code "PMID" ;
    at:deprecated "false" ;
    at:op-code "PMID" ;
    at:start.use "1996-12-31" ;
    atold:op-code "PMID" ;
    dc:identifier "PMID" ;
    skos:altLabel "PubMed Identifier"@en ;
    skos:definition "The PMID (PubMed Identifier or PubMed Unique Identifier) is a unique identifier number assigned to each article record entering PubMed, index of the biomedical literature. PMIDs are not reused after records are deleted."@en ;
    skos:exactMatch <http://purl.org/spar/datacite/pmid> ;
    skos:inScheme atold:notation-type ;
    skos:prefLabel "PMID"@en,
        "PMID"@et ;
    skos:topConceptOf atold:notation-type .

<http://publications.europa.eu/resource/authority/notation-type/PUB_CORP> a skos:Concept ;
    at:authority-code "PUB_CORP" ;
    at:deprecated "false" ;
    at:op-code "PUB_CORP" ;
    at:start.use "2010-03-29" ;
    atold:op-code "PUB_CORP" ;
    dc:identifier "PUB_CORP" ;
    skos:altLabel "PUB_CORP code"@en ;
    skos:definition "Code used by PUB_CORP table of Publications domain in ATTO."@en ;
    skos:inScheme atold:notation-type ;
    skos:prefLabel "PUB_CORP"@en,
        "PUB_CORP"@et ;
    skos:topConceptOf atold:notation-type .

<http://publications.europa.eu/resource/authority/notation-type/PUB_DIV> a skos:Concept ;
    at:authority-code "PUB_DIV" ;
    at:deprecated "false" ;
    at:op-code "PUB_DIV" ;
    at:start.use "2010-03-29" ;
    atold:op-code "PUB_DIV" ;
    dc:identifier "PUB_DIV" ;
    skos:altLabel "PUB_DIV code"@en ;
    skos:definition "Code used by PUB_DIV of Publications domain in ATTO."@en ;
    skos:inScheme atold:notation-type ;
    skos:prefLabel "PUB_DIV"@en,
        "PUB_DIV"@et ;
    skos:topConceptOf atold:notation-type .

<http://publications.europa.eu/resource/authority/notation-type/PUB_FREQ> a skos:Concept ;
    at:authority-code "PUB_FREQ" ;
    at:deprecated "false" ;
    at:op-code "PUB_FREQ" ;
    at:start.use "2010-03-29" ;
    atold:op-code "PUB_FREQ" ;
    dc:identifier "PUB_FREQ" ;
    skos:altLabel "PUB_FREQ code"@en ;
    skos:definition "Code used by PUB_FREQ of Publications domain in ATTO."@en ;
    skos:inScheme atold:notation-type ;
    skos:prefLabel "PUB_FREQ"@en,
        "PUB_FREQ"@et ;
    skos:topConceptOf atold:notation-type .

<http://publications.europa.eu/resource/authority/notation-type/PUB_LANG> a skos:Concept ;
    at:authority-code "PUB_LANG" ;
    at:deprecated "false" ;
    at:op-code "PUB_LANG" ;
    at:start.use "2010-03-29" ;
    atold:op-code "PUB_LANG" ;
    dc:identifier "PUB_LANG" ;
    skos:altLabel "PUB_LANG code"@en ;
    skos:definition "Code used by PUB_LANG of Publications domain in ATTO."@en ;
    skos:inScheme atold:notation-type ;
    skos:prefLabel "PUB_LANG"@en,
        "PUB_LANG"@et ;
    skos:topConceptOf atold:notation-type .

<http://publications.europa.eu/resource/authority/notation-type/PUB_LNGISO> a skos:Concept ;
    at:authority-code "PUB_LNGISO" ;
    at:deprecated "false" ;
    at:op-code "PUB_LNGISO" ;
    at:start.use "2010-03-29" ;
    atold:op-code "PUB_LNGISO" ;
    dc:identifier "PUB_LNGISO" ;
    skos:altLabel "PUB_LNGISO code"@en ;
    skos:definition "Code used by PUB__LNGISO of Publications domain in ATTO."@en ;
    skos:inScheme atold:notation-type ;
    skos:prefLabel "PUB_LNGISO"@en,
        "PUB_LNGISO"@et ;
    skos:topConceptOf atold:notation-type .

<http://publications.europa.eu/resource/authority/notation-type/PUB_LOC> a skos:Concept ;
    at:authority-code "PUB_LOC" ;
    at:deprecated "false" ;
    at:op-code "PUB_LOC" ;
    at:start.use "2010-03-29" ;
    atold:op-code "PUB_LOC" ;
    dc:identifier "PUB_LOC" ;
    skos:altLabel "PUB_LOC code"@en ;
    skos:definition "Code used by PUB_LOC table of Publications domain in ATTO."@en ;
    skos:inScheme atold:notation-type ;
    skos:prefLabel "PUB_LOC"@en,
        "PUB_LOC"@et ;
    skos:topConceptOf atold:notation-type .

<http://publications.europa.eu/resource/authority/notation-type/PUB_NOT> a skos:Concept ;
    at:authority-code "PUB_NOT" ;
    at:deprecated "false" ;
    at:op-code "PUB_NOT" ;
    at:start.use "2010-03-29" ;
    atold:op-code "PUB_NOT" ;
    dc:identifier "PUB_NOT" ;
    skos:altLabel "PUB_NOT code"@en ;
    skos:definition "Code used by PUB_NOT of Publications domain in ATTO."@en ;
    skos:inScheme atold:notation-type ;
    skos:prefLabel "PUB_NOT"@en,
        "PUB_NOT"@et ;
    skos:topConceptOf atold:notation-type .

<http://publications.europa.eu/resource/authority/notation-type/PUB_ORDIN> a skos:Concept ;
    at:authority-code "PUB_ORDIN" ;
    at:deprecated "false" ;
    at:op-code "PUB_ORDIN" ;
    at:start.use "2010-03-29" ;
    atold:op-code "PUB_ORDIN" ;
    dc:identifier "PUB_ORDIN" ;
    skos:altLabel "PUB_ORDIN code"@en ;
    skos:definition "Code used by PUB_ORDIN of Publications domain in ATTO."@en ;
    skos:inScheme atold:notation-type ;
    skos:prefLabel "PUB_ORDIN"@en,
        "PUB_ORDIN"@et ;
    skos:topConceptOf atold:notation-type .

<http://publications.europa.eu/resource/authority/notation-type/PUB_QUAL> a skos:Concept ;
    at:authority-code "PUB_QUAL" ;
    at:deprecated "false" ;
    at:op-code "PUB_QUAL" ;
    at:start.use "2010-03-29" ;
    atold:op-code "PUB_QUAL" ;
    dc:identifier "PUB_QUAL" ;
    skos:altLabel "PUB_QUAL code"@en ;
    skos:definition "Code used by PUB_QUAL of Publications domain in ATTO."@en ;
    skos:inScheme atold:notation-type ;
    skos:prefLabel "PUB_QUAL"@en,
        "PUB_QUAL"@et ;
    skos:topConceptOf atold:notation-type .

<http://publications.europa.eu/resource/authority/notation-type/PUB_TARGET> a skos:Concept ;
    at:authority-code "PUB_TARGET" ;
    at:deprecated "false" ;
    at:op-code "PUB_TARGET" ;
    at:start.use "2010-03-29" ;
    atold:op-code "PUB_TARGET" ;
    dc:identifier "PUB_TARGET" ;
    skos:altLabel "PUB_TARGET code"@en ;
    skos:definition "Code used by PUB_TARGET of Publications domain in ATTO."@en ;
    skos:inScheme atold:notation-type ;
    skos:prefLabel "PUB_TARGET"@en,
        "PUB_TARGET"@et ;
    skos:topConceptOf atold:notation-type .

<http://publications.europa.eu/resource/authority/notation-type/PUB_THEM14> a skos:Concept ;
    at:authority-code "PUB_THEM14" ;
    at:deprecated "false" ;
    at:op-code "PUB_THEM14" ;
    at:start.use "2010-03-29" ;
    atold:op-code "PUB_THEM14" ;
    dc:identifier "PUB_THEM14" ;
    skos:altLabel "PUB_THEM14 code"@en ;
    skos:definition "Code used by PUB_THEM14 of Publications domain in ATTO."@en ;
    skos:inScheme atold:notation-type ;
    skos:prefLabel "PUB_THEM14"@en,
        "PUB_THEM14"@et ;
    skos:topConceptOf atold:notation-type .

<http://publications.europa.eu/resource/authority/notation-type/PURL> a skos:Concept ;
    at:authority-code "PURL" ;
    at:deprecated "false" ;
    at:op-code "PURL" ;
    at:start.use "1998-03-31" ;
    atold:op-code "PURL" ;
    dc:identifier "PURL" ;
    skos:altLabel "Persistent URL"@en ;
    skos:definition "A persistent URL (PURL) is a Uniform Resource Locator (URL) that is guaranteed by an organization to function for a long period of time."@en ;
    skos:exactMatch <http://purl.org/spar/datacite/purl> ;
    skos:inScheme atold:notation-type ;
    skos:prefLabel "PURL"@en,
        "PURL"@et ;
    skos:topConceptOf atold:notation-type .

<http://publications.europa.eu/resource/authority/notation-type/SICI> a skos:Concept ;
    at:authority-code "SICI" ;
    at:deprecated "false" ;
    at:op-code "SICI" ;
    at:start.use "1991-12-31" ;
    atold:op-code "SICI" ;
    dc:identifier "SICI" ;
    skos:altLabel "Serial Item and Contribution Identifier"@en ;
    skos:definition "An add-on to the ISSN, the Serial Item and Contribution Identifier (SICI) is a variable length code (ANSI/NISO standard Z39.56) that provides unique identification of serial issues (SII) and serial contributions (SCI)."@en ;
    skos:exactMatch <http://purl.org/spar/datacite/sici> ;
    skos:inScheme atold:notation-type ;
    skos:prefLabel "SICI"@en,
        "SICI"@et ;
    skos:topConceptOf atold:notation-type .

<http://publications.europa.eu/resource/authority/notation-type/TED> a skos:Concept ;
    at:authority-code "TED" ;
    at:deprecated "false" ;
    at:op-code "TED" ;
    at:start.use "1986-01-01" ;
    atold:op-code "TED" ;
    dc:identifier "TED" ;
    skos:altLabel "TED code"@en ;
    skos:definition "Code used in Tenders Electronic Daily, the online version of the 'Supplement to the Official Journal of the European Union', dedicated to European public procurement."@en ;
    skos:inScheme atold:notation-type ;
    skos:prefLabel "TED"@en,
        "TED"@et ;
    skos:topConceptOf atold:notation-type .

<http://publications.europa.eu/resource/authority/notation-type/TED_SCHEMA> a skos:Concept ;
    at:authority-code "TED_SCHEMA" ;
    at:deprecated "false" ;
    at:op-code "TED_SCHEMA" ;
    at:start.use "2019-09-18" ;
    atold:op-code "TED_SCHEMA" ;
    dc:identifier "TED_SCHEMA" ;
    skos:altLabel "TED Schema code"@en ;
    skos:definition "Code used in the schema of Tenders Electronic Daily, the online version of the 'Supplement to the Official Journal of the European Union', dedicated to European public procurement."@en ;
    skos:inScheme atold:notation-type ;
    skos:prefLabel "TED Schema"@en,
        "TED Schema"@et ;
    skos:topConceptOf atold:notation-type .

<http://publications.europa.eu/resource/authority/notation-type/TIR> a skos:Concept ;
    at:authority-code "TIR" ;
    at:deprecated "false" ;
    at:op-code "TIR" ;
    at:op-mapped-code [ a at:MappedCode ;
            at:affected-table "notation-type" ;
            at:legacy-code "code-tir" ;
            dc:source "MDR" ] ;
    at:start.use "1975-11-14" ;
    atold:op-code "TIR" ;
    dc:identifier "TIR" ;
    skos:altLabel "International Road Transport code"@en ;
    skos:definition "The TIR code is used for distinguishing signs of vehicles in international traffic."@en ;
    skos:inScheme atold:notation-type ;
    skos:prefLabel "TIR"@en,
        "TIR"@et ;
    skos:topConceptOf atold:notation-type .

<http://publications.europa.eu/resource/authority/notation-type/UNSD_GEOSCHEME> a skos:Concept ;
    at:authority-code "UNSD_GEOSCHEME" ;
    at:deprecated "false" ;
    at:op-code "UNSD_GEOSCHEME" ;
    at:start.use "1970-01-01" ;
    atold:op-code "UNSD_GEOSCHEME" ;
    dc:identifier "UNSD_GEOSCHEME" ;
    skos:altLabel "United Nations Statistics Division geoscheme"@en ;
    skos:definition "The United Nations geoscheme is a system which divides the countries of the world into regional and subregional groups. It was devised by the United Nations Statistics Division (UNSD) based on the M49 coding classification. The UNSD geoscheme notation uses two levels of this classification: intermediate region and subregion. The intermediate region name is used whenever it is available; in other cases the broader level, subregion, is used. The UNSD geoscheme notation is used in the Country authority table."@en ;
    skos:inScheme atold:notation-type ;
    skos:prefLabel "UNSD geoscheme"@en,
        "UNSD geoscheme"@et ;
    skos:topConceptOf atold:notation-type .

<http://publications.europa.eu/resource/authority/notation-type/UNSD_M49> a skos:Concept ;
    at:authority-code "UNSD_M49" ;
    at:deprecated "false" ;
    at:op-code "UNSD_M49" ;
    at:op-mapped-code [ a at:MappedCode ;
            at:affected-table "notation-type" ;
            at:legacy-code "code-M49" ;
            dc:source "MDR" ] ;
    at:start.use "1970-01-01" ;
    atold:op-code "UNSD_M49" ;
    dc:identifier "UNSD_M49" ;
    skos:altLabel "United Nations Statistics Division M49 code"@en ;
    skos:definition "The UNSD M49 codes are standard country or area codes for statistical purposes, developed and maintained by the United Nations Statistics Division (UNSD). Each area code is a three-digit number which can refer to a wide variety of geographical, political, or economic regions, like a continent, a country or a specific group of countries. Codes assigned in the system generally do not change when the country or area's name changes (unlike ISO 3166-1 alpha-2 or ISO 3166-1 alpha-3), but instead change when the territorial extent of the country or area changes significantly."@en ;
    skos:inScheme atold:notation-type ;
    skos:prefLabel "UNSD M49"@en,
        "UNSD M49"@et ;
    skos:topConceptOf atold:notation-type .

<http://publications.europa.eu/resource/authority/notation-type/UN_LOCODE> a skos:Concept ;
    at:authority-code "UN_LOCODE" ;
    at:deprecated "false" ;
    at:op-code "UN_LOCODE" ;
    at:op-mapped-code [ a at:MappedCode ;
            at:affected-table "notation-type" ;
            at:legacy-code "unlocode" ;
            dc:source "MDR" ] ;
    at:start.use "1981-01-01" ;
    atold:op-code "UN_LOCODE" ;
    dc:identifier "UN_LOCODE" ;
    skos:altLabel "United Nations Code for Trade and Transport Locations code"@en ;
    skos:definition "5-character code where the first two characters are the ISO 3166 country codes while the remaining three are derived from Recommendation 16 from the UNECE in Geneva, together with Eurostat supplied codes for ports not yet included in the UN system."@en ;
    skos:inScheme atold:notation-type ;
    skos:prefLabel "UN location"@en,
        "UN location"@et ;
    skos:topConceptOf atold:notation-type .

<http://publications.europa.eu/resource/authority/notation-type/UPC> a skos:Concept ;
    at:authority-code "UPC" ;
    at:deprecated "false" ;
    at:op-code "UPC" ;
    at:start.use "1973-01-01" ;
    atold:op-code "UPC" ;
    dc:identifier "UPC" ;
    skos:altLabel "Universal Product Code"@en ;
    skos:definition "The Universal Product Code (UPC) is a widely-used standard for barcodes. The barcode consists of a series of variable-width vertical bars and was created for tracking merchandise in stores, mainly at the point of sale."@en ;
    skos:exactMatch <http://purl.org/spar/datacite/upc> ;
    skos:inScheme atold:notation-type ;
    skos:prefLabel "UPC"@en,
        "UPC"@et ;
    skos:topConceptOf atold:notation-type .

<http://publications.europa.eu/resource/authority/notation-type/URI> a skos:Concept ;
    at:authority-code "URI" ;
    at:deprecated "false" ;
    at:op-code "URI" ;
    at:start.use "1998-12-31" ;
    atold:op-code "URI" ;
    dc:identifier "URI" ;
    skos:altLabel "Uniform Resource Identifier"@en ;
    skos:definition "A Uniform Resource Identifier (URI) is a compact sequence of characters that identifies an abstract or physical resource. A URI can be used as a locator, a name, or both. If a URI is a locator, it describes a resource’s primary access mechanism. If a URI is a name, it identifies a resource by giving it a unique name."@en ;
    skos:exactMatch <http://purl.org/spar/datacite/uri> ;
    skos:inScheme atold:notation-type ;
    skos:prefLabel "URI"@en,
        "URI"@et ;
    skos:topConceptOf atold:notation-type .

<http://publications.europa.eu/resource/authority/notation-type/URL> a skos:Concept ;
    at:authority-code "URL" ;
    at:deprecated "false" ;
    at:op-code "URL" ;
    at:start.use "1994-12-31" ;
    atold:op-code "URL" ;
    dc:identifier "URL" ;
    skos:altLabel "Uniform Resource Locator"@en ;
    skos:definition "A Uniform Resource Locator (URL) is a URI that, in addition to identifying a resource, provides a means of locating the resource by describing its primary access mechanism. As there is no exact definition of URL by means of a set of schemes, URL is a useful but informal concept, usually referring to a subset of URIs that do not contain URNs."@en ;
    skos:exactMatch <http://purl.org/spar/datacite/url> ;
    skos:inScheme atold:notation-type ;
    skos:prefLabel "URL"@en,
        "URL"@et ;
    skos:topConceptOf atold:notation-type .

<http://publications.europa.eu/resource/authority/notation-type/URN> a skos:Concept ;
    at:authority-code "URN" ;
    at:deprecated "false" ;
    at:op-code "URN" ;
    at:start.use "1997-05-31" ;
    atold:op-code "URN" ;
    dc:identifier "URN" ;
    skos:altLabel "Uniform Resource Name"@en ;
    skos:definition "A Uniform Resource Name (URN) is a URI that is assigned under the \"urn\" URI scheme and a particular URN namespace, with the intent that the URN will be a persistent, location-independent resource identifier."@en ;
    skos:exactMatch <http://purl.org/spar/datacite/urn> ;
    skos:inScheme atold:notation-type ;
    skos:prefLabel "URN"@en,
        "URN"@et ;
    skos:topConceptOf atold:notation-type .

<http://publications.europa.eu/resource/authority/notation-type/WHOISWHO> a skos:Concept ;
    at:authority-code "WHOISWHO" ;
    at:deprecated "false" ;
    at:op-code "WHOISWHO" ;
    at:start.use "1981-12-01" ;
    atold:op-code "WHOISWHO" ;
    dc:identifier "WHOISWHO" ;
    skos:altLabel "EU Whoiswho code"@en ;
    skos:definition "Code used in the EU Whoiswho, an electronic directory of managers and services in the EU institutions, bodies and agencies."@en ;
    skos:inScheme atold:notation-type ;
    skos:prefLabel "EU Whoiswho"@en,
        "EU Whoiswho"@et ;
    skos:topConceptOf atold:notation-type .

<http://publications.europa.eu/resource/authority/notation-type/XML_LNG> a skos:Concept ;
    at:authority-code "XML_LNG" ;
    at:deprecated "false" ;
    at:op-code "XML_LNG" ;
    at:op-mapped-code [ a at:MappedCode ;
            at:affected-table "notation-type" ;
            at:legacy-code "xml-lang" ;
            dc:source "MDR" ] ;
    at:start.use "1995-03-01" ;
    atold:op-code "XML_LNG" ;
    dc:identifier "XML_LNG" ;
    skos:altLabel "xml language"@en ;
    skos:definition "XML LANG codes are used to indicate the natural language in which xml content is expressed. The code is based on ISO 639 codes and RFC 5646 explains how those codes are structured."@en ;
    skos:inScheme atold:notation-type ;
    skos:prefLabel "xml lang"@en,
        "xml keel"@et ;
    skos:topConceptOf atold:notation-type .

atold:notation-type a skos:ConceptScheme ;
    rdfs:label "Notation type"@en ;
    at:prefLabel "Notation type"@en ;
    at:table.id "notation-type" ;
    at:table.version.number "20220615-0" ;
    owl:versionInfo "20220615-0" ;
    skos:prefLabel "Notation type"@en .

