<?xml version="1.0" encoding="UTF-8"?>
<rdf:RDF xmlns:rdf="http://www.w3.org/1999/02/22-rdf-syntax-ns#"
         xmlns:at="http://publications.europa.eu/ontology/authority/"
         xmlns:rdfs="http://www.w3.org/2000/01/rdf-schema#"
         xmlns:owl="http://www.w3.org/2002/07/owl#"
         xmlns:skos="http://www.w3.org/2004/02/skos/core#"
         xmlns:atold="http://publications.europa.eu/resource/authority/"
         xmlns:dc="http://purl.org/dc/elements/1.1/"
         xml:base="http://publications.europa.eu/resource/authority/notation-type">
   <skos:ConceptScheme rdf:about="http://publications.europa.eu/resource/authority/notation-type"
                       at:table.id="notation-type"
                       at:table.version.number="20220615-0">
      <at:prefLabel xml:lang="en">Notation type</at:prefLabel>
      <rdfs:label xml:lang="en">Notation type</rdfs:label>
      <owl:versionInfo>20220615-0</owl:versionInfo>
      <skos:prefLabel xml:lang="en">Notation type</skos:prefLabel>
   </skos:ConceptScheme>
   <skos:Concept rdf:about="http://publications.europa.eu/resource/authority/notation-type/AKN4EU"
                 at:deprecated="false">
      <skos:prefLabel xml:lang="en">AKN4EU</skos:prefLabel>
      <skos:prefLabel xml:lang="et">AKN4EU</skos:prefLabel>
      <at:authority-code>AKN4EU</at:authority-code>
      <at:op-code>AKN4EU</at:op-code>
      <at:start.use>2019-03-13</at:start.use>
      <atold:op-code>AKN4EU</atold:op-code>
      <dc:identifier>AKN4EU</dc:identifier>
      <skos:altLabel xml:lang="en">Akoma Ntoso for European Union</skos:altLabel>
      <skos:definition xml:lang="en">This concept identifies the Akoma Ntoso common XML schema. It is developed under the governance of the Interinstitutional Metadata and Formats Committee (IMFC). The specifications are based on the generic Akoma Ntoso standard maintained by OASIS but tailored to the requirements that the EU Institutions define for their legal documents.</skos:definition>
      <skos:inScheme rdf:resource="http://publications.europa.eu/resource/authority/notation-type"/>
      <skos:topConceptOf rdf:resource="http://publications.europa.eu/resource/authority/notation-type"/>
   </skos:Concept>
   <skos:Concept rdf:about="http://publications.europa.eu/resource/authority/notation-type/ARK"
                 at:deprecated="false">
      <skos:prefLabel xml:lang="en">ARK</skos:prefLabel>
      <skos:prefLabel xml:lang="et">ARK</skos:prefLabel>
      <at:authority-code>ARK</at:authority-code>
      <at:op-code>ARK</at:op-code>
      <at:start.use>2001-12-31</at:start.use>
      <atold:op-code>ARK</atold:op-code>
      <dc:identifier>ARK</dc:identifier>
      <skos:altLabel xml:lang="en">Archival Resource Key</skos:altLabel>
      <skos:definition xml:lang="en">The ARK (Archival Resource Key) identifier is a specially constructed, globally unique actionable URL (Uniform Resource Locator). It provides a naming scheme for persistent access to digital objects.</skos:definition>
      <skos:inScheme rdf:resource="http://publications.europa.eu/resource/authority/notation-type"/>
      <skos:topConceptOf rdf:resource="http://publications.europa.eu/resource/authority/notation-type"/>
      <skos:exactMatch rdf:resource="http://purl.org/spar/datacite/ark"/>
   </skos:Concept>
   <skos:Concept rdf:about="http://publications.europa.eu/resource/authority/notation-type/ARXIV"
                 at:deprecated="false">
      <skos:prefLabel xml:lang="en">arXiv</skos:prefLabel>
      <skos:prefLabel xml:lang="et">arXiv</skos:prefLabel>
      <at:authority-code>ARXIV</at:authority-code>
      <at:op-code>ARXIV</at:op-code>
      <at:start.use>1991-08-14</at:start.use>
      <atold:op-code>ARXIV</atold:op-code>
      <dc:identifier>ARXIV</dc:identifier>
      <skos:altLabel xml:lang="en">arXiv identifier</skos:altLabel>
      <skos:definition xml:lang="en">The ArXiv identifier is generated by ArXiv, an open access repository and distribution server for electronic preprints featuring, in particular, physics, mathematics, computer science, nonlinear sciences, quantitative biology, quantitative finance, statistics, electrical engineering and systems science and economics.</skos:definition>
      <skos:inScheme rdf:resource="http://publications.europa.eu/resource/authority/notation-type"/>
      <skos:topConceptOf rdf:resource="http://publications.europa.eu/resource/authority/notation-type"/>
      <skos:exactMatch rdf:resource="http://purl.org/spar/datacite/arxiv"/>
   </skos:Concept>
   <skos:Concept rdf:about="http://publications.europa.eu/resource/authority/notation-type/BIBCODE"
                 at:deprecated="false">
      <skos:prefLabel xml:lang="en">Bibcode</skos:prefLabel>
      <skos:prefLabel xml:lang="et">Bibcode</skos:prefLabel>
      <at:authority-code>BIBCODE</at:authority-code>
      <at:op-code>BIBCODE</at:op-code>
      <at:start.use>1995-12-31</at:start.use>
      <atold:op-code>BIBCODE</atold:op-code>
      <dc:identifier>BIBCODE</dc:identifier>
      <skos:altLabel xml:lang="en">Bibliographic Reference Code</skos:altLabel>
      <skos:definition xml:lang="en">The bibcode is a compact identifier used by several astronomical data systems to uniquely specify literature references. The Bibliographic Reference Code (REFCODE) is used widely, for example, by the NASA Astrophysics Data System who coined and prefer the term "bibcode".</skos:definition>
      <skos:inScheme rdf:resource="http://publications.europa.eu/resource/authority/notation-type"/>
      <skos:topConceptOf rdf:resource="http://publications.europa.eu/resource/authority/notation-type"/>
      <skos:exactMatch rdf:resource="http://purl.org/spar/datacite/bibcode"/>
   </skos:Concept>
   <skos:Concept rdf:about="http://publications.europa.eu/resource/authority/notation-type/CELEX"
                 at:deprecated="false">
      <skos:prefLabel xml:lang="en">CELEX id</skos:prefLabel>
      <skos:prefLabel xml:lang="et">CELEX id</skos:prefLabel>
      <at:authority-code>CELEX</at:authority-code>
      <at:op-code>CELEX</at:op-code>
      <at:start.use>1981-01-01</at:start.use>
      <atold:op-code>CELEX</atold:op-code>
      <dc:identifier>CELEX</dc:identifier>
      <skos:altLabel xml:lang="en">CELEX code</skos:altLabel>
      <skos:definition xml:lang="en">The unique identifier of each document in EUR-Lex, regardless of language.</skos:definition>
      <skos:inScheme rdf:resource="http://publications.europa.eu/resource/authority/notation-type"/>
      <skos:topConceptOf rdf:resource="http://publications.europa.eu/resource/authority/notation-type"/>
      <at:op-mapped-code>
         <at:MappedCode>
            <dc:source>MDR</dc:source>
            <at:affected-table>notation-type</at:affected-table>
            <at:legacy-code>celex_id</at:legacy-code>
         </at:MappedCode>
      </at:op-mapped-code>
   </skos:Concept>
   <skos:Concept rdf:about="http://publications.europa.eu/resource/authority/notation-type/CELEX_RT"
                 at:deprecated="false">
      <skos:prefLabel xml:lang="en">CELEX root</skos:prefLabel>
      <skos:prefLabel xml:lang="et">CELEX juurelement</skos:prefLabel>
      <at:authority-code>CELEX_RT</at:authority-code>
      <at:op-code>CELEX_RT</at:op-code>
      <at:start.use>1981-01-01</at:start.use>
      <atold:op-code>CELEX_RT</atold:op-code>
      <dc:identifier>CELEX_RT</dc:identifier>
      <skos:altLabel xml:lang="en">CELEX root code</skos:altLabel>
      <skos:definition xml:lang="en">Code used to identify the root of a CELEX code.</skos:definition>
      <skos:inScheme rdf:resource="http://publications.europa.eu/resource/authority/notation-type"/>
      <skos:topConceptOf rdf:resource="http://publications.europa.eu/resource/authority/notation-type"/>
      <at:op-mapped-code>
         <at:MappedCode>
            <dc:source>MDR</dc:source>
            <at:affected-table>notation-type</at:affected-table>
            <at:legacy-code>celex_root</at:legacy-code>
         </at:MappedCode>
      </at:op-mapped-code>
   </skos:Concept>
   <skos:Concept rdf:about="http://publications.europa.eu/resource/authority/notation-type/CELEX_SECT"
                 at:deprecated="false">
      <skos:prefLabel xml:lang="en">CELEX sector</skos:prefLabel>
      <skos:prefLabel xml:lang="et">CELEX sektor</skos:prefLabel>
      <at:authority-code>CELEX_SECT</at:authority-code>
      <at:op-code>CELEX_SECT</at:op-code>
      <at:start.use>1981-01-01</at:start.use>
      <atold:op-code>CELEX_SECT</atold:op-code>
      <dc:identifier>CELEX_SECT</dc:identifier>
      <skos:altLabel xml:lang="en">CELEX sector code</skos:altLabel>
      <skos:definition xml:lang="en">Code used to identify the sector, the first element (number or letter) of the CELEX code.</skos:definition>
      <skos:inScheme rdf:resource="http://publications.europa.eu/resource/authority/notation-type"/>
      <skos:topConceptOf rdf:resource="http://publications.europa.eu/resource/authority/notation-type"/>
      <at:op-mapped-code>
         <at:MappedCode>
            <dc:source>MDR</dc:source>
            <at:affected-table>notation-type</at:affected-table>
            <at:legacy-code>oj.celex.structure.id</at:legacy-code>
         </at:MappedCode>
      </at:op-mapped-code>
   </skos:Concept>
   <skos:Concept rdf:about="http://publications.europa.eu/resource/authority/notation-type/CELLAR_MANIFT"
                 at:deprecated="false">
      <skos:prefLabel xml:lang="en">CELLAR Manif MIME</skos:prefLabel>
      <skos:prefLabel xml:lang="et">CELLAR Manif MIME</skos:prefLabel>
      <at:authority-code>CELLAR_MANIFT</at:authority-code>
      <at:op-code>CELLAR_MANIFT</at:op-code>
      <at:start.use>2010-09-23</at:start.use>
      <atold:op-code>CELLAR_MANIFT</atold:op-code>
      <dc:identifier>CELLAR_MANIFT</dc:identifier>
      <skos:altLabel xml:lang="en">Media type (Cellar Manifestation) code</skos:altLabel>
      <skos:definition xml:lang="en">Code used in Cellar for manifestations of media types. Cellar is the information system storing all metadata and digital content managed by the Publications Office in a harmonised and standardised format.</skos:definition>
      <skos:inScheme rdf:resource="http://publications.europa.eu/resource/authority/notation-type"/>
      <skos:topConceptOf rdf:resource="http://publications.europa.eu/resource/authority/notation-type"/>
      <at:op-mapped-code>
         <at:MappedCode>
            <dc:source>MDR</dc:source>
            <at:affected-table>notation-type</at:affected-table>
            <at:legacy-code>manifestation-type-cellar</at:legacy-code>
         </at:MappedCode>
      </at:op-mapped-code>
   </skos:Concept>
   <skos:Concept rdf:about="http://publications.europa.eu/resource/authority/notation-type/CELLAR_MT"
                 at:deprecated="false">
      <skos:prefLabel xml:lang="en">CELLAR MIME</skos:prefLabel>
      <skos:prefLabel xml:lang="et">CELLAR MIME</skos:prefLabel>
      <at:authority-code>CELLAR_MT</at:authority-code>
      <at:op-code>CELLAR_MT</at:op-code>
      <at:start.use>2010-09-23</at:start.use>
      <atold:op-code>CELLAR_MT</atold:op-code>
      <dc:identifier>CELLAR_MT</dc:identifier>
      <skos:altLabel xml:lang="en">Media type (Cellar) code</skos:altLabel>
      <skos:definition xml:lang="en">Code used in Cellar for media types. Cellar is the information system storing all metadata and digital content managed by the Publications Office in a harmonised and standardised format.</skos:definition>
      <skos:inScheme rdf:resource="http://publications.europa.eu/resource/authority/notation-type"/>
      <skos:topConceptOf rdf:resource="http://publications.europa.eu/resource/authority/notation-type"/>
      <at:op-mapped-code>
         <at:MappedCode>
            <dc:source>MDR</dc:source>
            <at:affected-table>notation-type</at:affected-table>
            <at:legacy-code>mime-type-cellar</at:legacy-code>
         </at:MappedCode>
      </at:op-mapped-code>
   </skos:Concept>
   <skos:Concept rdf:about="http://publications.europa.eu/resource/authority/notation-type/CJ"
                 at:deprecated="false">
      <skos:prefLabel xml:lang="en">CJ</skos:prefLabel>
      <skos:prefLabel xml:lang="et">CJ</skos:prefLabel>
      <at:authority-code>CJ</at:authority-code>
      <at:op-code>CJ</at:op-code>
      <at:start.use>1952-07-24</at:start.use>
      <atold:op-code>CJ</atold:op-code>
      <dc:identifier>CJ</dc:identifier>
      <skos:altLabel xml:lang="en">CJ code</skos:altLabel>
      <skos:definition xml:lang="en">Code used by the Court of Justice.</skos:definition>
      <skos:inScheme rdf:resource="http://publications.europa.eu/resource/authority/notation-type"/>
      <skos:topConceptOf rdf:resource="http://publications.europa.eu/resource/authority/notation-type"/>
   </skos:Concept>
   <skos:Concept rdf:about="http://publications.europa.eu/resource/authority/notation-type/CODIF_DATA"
                 at:deprecated="false">
      <skos:prefLabel xml:lang="en">Codification data</skos:prefLabel>
      <skos:prefLabel xml:lang="et">Codification data</skos:prefLabel>
      <at:authority-code>CODIF_DATA</at:authority-code>
      <at:op-code>CODIF_DATA</at:op-code>
      <at:start.use>2022-06-15</at:start.use>
      <atold:op-code>CODIF_DATA</atold:op-code>
      <dc:identifier>CODIF_DATA</dc:identifier>
      <skos:definition xml:lang="en">Code used in several authority tables for codifying concepts in TED portal expert search and used in TED Schema (CODIF_DATA).</skos:definition>
      <skos:inScheme rdf:resource="http://publications.europa.eu/resource/authority/notation-type"/>
      <skos:topConceptOf rdf:resource="http://publications.europa.eu/resource/authority/notation-type"/>
   </skos:Concept>
   <skos:Concept rdf:about="http://publications.europa.eu/resource/authority/notation-type/COMREF"
                 at:deprecated="false">
      <skos:prefLabel xml:lang="en">COMREF</skos:prefLabel>
      <skos:prefLabel xml:lang="et">COMREF</skos:prefLabel>
      <at:authority-code>COMREF</at:authority-code>
      <at:op-code>COMREF</at:op-code>
      <at:start.use>1957-03-25</at:start.use>
      <atold:op-code>COMREF</atold:op-code>
      <dc:identifier>COMREF</dc:identifier>
      <skos:altLabel xml:lang="en">COMREF code</skos:altLabel>
      <skos:definition xml:lang="en">Code used by COMREF, the European Commission's Human Resources Database.</skos:definition>
      <skos:inScheme rdf:resource="http://publications.europa.eu/resource/authority/notation-type"/>
      <skos:topConceptOf rdf:resource="http://publications.europa.eu/resource/authority/notation-type"/>
   </skos:Concept>
   <skos:Concept rdf:about="http://publications.europa.eu/resource/authority/notation-type/CONSIL"
                 at:deprecated="false">
      <skos:prefLabel xml:lang="en">Council</skos:prefLabel>
      <skos:prefLabel xml:lang="et">Council</skos:prefLabel>
      <at:authority-code>CONSIL</at:authority-code>
      <at:op-code>CONSIL</at:op-code>
      <at:start.use>1993-11-01</at:start.use>
      <atold:op-code>CONSIL</atold:op-code>
      <dc:identifier>CONSIL</dc:identifier>
      <skos:altLabel xml:lang="en">Council code</skos:altLabel>
      <skos:definition xml:lang="en">Code used by the Council of the European Union.</skos:definition>
      <skos:inScheme rdf:resource="http://publications.europa.eu/resource/authority/notation-type"/>
      <skos:topConceptOf rdf:resource="http://publications.europa.eu/resource/authority/notation-type"/>
   </skos:Concept>
   <skos:Concept rdf:about="http://publications.europa.eu/resource/authority/notation-type/DEMED"
                 at:deprecated="false">
      <skos:prefLabel xml:lang="en">DEMED</skos:prefLabel>
      <skos:prefLabel xml:lang="et">DEMED</skos:prefLabel>
      <at:authority-code>DEMED</at:authority-code>
      <at:op-code>DEMED</at:op-code>
      <at:start.use>1969-01-18</at:start.use>
      <atold:op-code>DEMED</atold:op-code>
      <dc:identifier>DEMED</dc:identifier>
      <skos:altLabel xml:lang="en">DEMED code</skos:altLabel>
      <skos:definition xml:lang="en">Code used by the DEMED system.</skos:definition>
      <skos:inScheme rdf:resource="http://publications.europa.eu/resource/authority/notation-type"/>
      <skos:topConceptOf rdf:resource="http://publications.europa.eu/resource/authority/notation-type"/>
   </skos:Concept>
   <skos:Concept rdf:about="http://publications.europa.eu/resource/authority/notation-type/DOI"
                 at:deprecated="false">
      <skos:prefLabel xml:lang="en">DOI</skos:prefLabel>
      <skos:prefLabel xml:lang="et">DOI</skos:prefLabel>
      <at:authority-code>DOI</at:authority-code>
      <at:op-code>DOI</at:op-code>
      <at:start.use>2000-01-01</at:start.use>
      <atold:op-code>DOI</atold:op-code>
      <dc:identifier>DOI</dc:identifier>
      <skos:altLabel xml:lang="en">Digital Object Identifier code</skos:altLabel>
      <skos:definition xml:lang="en">DOI is a permanent identifier given to an electronic document. Similar to a URN, but in contrast to a URL, it is not dependent upon the electronic document's location. A typical use of a DOI is to give a scholarly paper or article a unique identifying number that anyone can use to obtain information about the publication's location on a digital network.</skos:definition>
      <skos:inScheme rdf:resource="http://publications.europa.eu/resource/authority/notation-type"/>
      <skos:topConceptOf rdf:resource="http://publications.europa.eu/resource/authority/notation-type"/>
      <skos:exactMatch rdf:resource="http://purl.org/spar/datacite/doi"/>
   </skos:Concept>
   <skos:Concept rdf:about="http://publications.europa.eu/resource/authority/notation-type/DOI_P"
                 at:deprecated="false">
      <skos:prefLabel xml:lang="en">DOI pref</skos:prefLabel>
      <skos:prefLabel xml:lang="et">DOI pref</skos:prefLabel>
      <at:authority-code>DOI_P</at:authority-code>
      <at:op-code>DOI_P</at:op-code>
      <at:start.use>1970-01-01</at:start.use>
      <atold:op-code>DOI_P</atold:op-code>
      <dc:identifier>DOI_P</dc:identifier>
      <skos:altLabel xml:lang="en">DOI prefix</skos:altLabel>
      <skos:definition xml:lang="en">The DOI prefix is composed of a directory indicator followed by a registrant code. The directory indicator shall be "10" and it distinguishes the entire set of character strings (prefix and suffix) as digital object identifiers within the resolution system. The second element of the DOI prefix shall be the registrant code. The registrant code is a unique string assigned to a registrant.</skos:definition>
      <skos:inScheme rdf:resource="http://publications.europa.eu/resource/authority/notation-type"/>
      <skos:topConceptOf rdf:resource="http://publications.europa.eu/resource/authority/notation-type"/>
      <at:op-mapped-code>
         <at:MappedCode>
            <dc:source>MDR</dc:source>
            <at:affected-table>notation-type</at:affected-table>
            <at:legacy-code>id-doi.old</at:legacy-code>
         </at:MappedCode>
      </at:op-mapped-code>
      <at:op-mapped-code>
         <at:MappedCode>
            <dc:source>MDR</dc:source>
            <at:affected-table>notation-type</at:affected-table>
            <at:legacy-code>id-doi</at:legacy-code>
         </at:MappedCode>
      </at:op-mapped-code>
   </skos:Concept>
   <skos:Concept rdf:about="http://publications.europa.eu/resource/authority/notation-type/EAN13"
                 at:deprecated="false">
      <skos:prefLabel xml:lang="en">EAN 13</skos:prefLabel>
      <skos:prefLabel xml:lang="et">EAN 13</skos:prefLabel>
      <at:authority-code>EAN13</at:authority-code>
      <at:op-code>EAN13</at:op-code>
      <at:start.use>1978-12-31</at:start.use>
      <atold:op-code>EAN13</atold:op-code>
      <dc:identifier>EAN13</dc:identifier>
      <skos:altLabel xml:lang="en">EAN 13 code</skos:altLabel>
      <skos:definition xml:lang="en">The EAN 13 code is the most widely used commercial distribution code in the world. It is shown on all marketed products. It is managed by GS1, an international agency located in Brussels.</skos:definition>
      <skos:inScheme rdf:resource="http://publications.europa.eu/resource/authority/notation-type"/>
      <skos:topConceptOf rdf:resource="http://publications.europa.eu/resource/authority/notation-type"/>
      <skos:exactMatch rdf:resource="http://purl.org/spar/datacite/ean13"/>
   </skos:Concept>
   <skos:Concept rdf:about="http://publications.europa.eu/resource/authority/notation-type/ECLI"
                 at:deprecated="false">
      <skos:prefLabel xml:lang="en">ECLI</skos:prefLabel>
      <skos:prefLabel xml:lang="et">ECLI</skos:prefLabel>
      <at:authority-code>ECLI</at:authority-code>
      <at:op-code>ECLI</at:op-code>
      <at:start.use>2011-04-29</at:start.use>
      <atold:op-code>ECLI</atold:op-code>
      <dc:identifier>ECLI</dc:identifier>
      <skos:altLabel xml:lang="en">European Case Law Identifier code</skos:altLabel>
      <skos:definition xml:lang="en">The European Case Law Identifier (ECLI) has been developed to facilitate the correct and unequivocal citation of judgments from European and national courts. ECLI is a uniform identifier that has the same recognizable format for all Member States and EU courts.</skos:definition>
      <skos:inScheme rdf:resource="http://publications.europa.eu/resource/authority/notation-type"/>
      <skos:topConceptOf rdf:resource="http://publications.europa.eu/resource/authority/notation-type"/>
      <at:op-mapped-code>
         <at:MappedCode>
            <dc:source>MDR</dc:source>
            <at:affected-table>notation-type</at:affected-table>
            <at:legacy-code>code-ecli</at:legacy-code>
         </at:MappedCode>
      </at:op-mapped-code>
      <skos:historyNote xml:lang="en">No time span</skos:historyNote>
   </skos:Concept>
   <skos:Concept rdf:about="http://publications.europa.eu/resource/authority/notation-type/EP"
                 at:deprecated="false">
      <skos:prefLabel xml:lang="en">EP</skos:prefLabel>
      <skos:prefLabel xml:lang="et">EP</skos:prefLabel>
      <at:authority-code>EP</at:authority-code>
      <at:op-code>EP</at:op-code>
      <at:start.use>1962-03-30</at:start.use>
      <atold:op-code>EP</atold:op-code>
      <dc:identifier>EP</dc:identifier>
      <skos:altLabel xml:lang="en">EP code</skos:altLabel>
      <skos:definition xml:lang="en">Code used by the European Parliament.</skos:definition>
      <skos:inScheme rdf:resource="http://publications.europa.eu/resource/authority/notation-type"/>
      <skos:topConceptOf rdf:resource="http://publications.europa.eu/resource/authority/notation-type"/>
   </skos:Concept>
   <skos:Concept rdf:about="http://publications.europa.eu/resource/authority/notation-type/ESPD"
                 at:deprecated="false">
      <skos:prefLabel xml:lang="en">ESPD</skos:prefLabel>
      <skos:prefLabel xml:lang="et">ESPD</skos:prefLabel>
      <at:authority-code>ESPD</at:authority-code>
      <at:op-code>ESPD</at:op-code>
      <at:start.use>2020-09-23</at:start.use>
      <atold:op-code>ESPD</atold:op-code>
      <dc:identifier>ESPD</dc:identifier>
      <skos:altLabel xml:lang="en">ESPD code</skos:altLabel>
      <skos:definition xml:lang="en">Code used in the European Single Procurement Document (ESPD).</skos:definition>
      <skos:inScheme rdf:resource="http://publications.europa.eu/resource/authority/notation-type"/>
      <skos:topConceptOf rdf:resource="http://publications.europa.eu/resource/authority/notation-type"/>
   </skos:Concept>
   <skos:Concept rdf:about="http://publications.europa.eu/resource/authority/notation-type/EUBOOKSHOP"
                 at:deprecated="false">
      <skos:prefLabel xml:lang="en">EU Bookshop</skos:prefLabel>
      <skos:prefLabel xml:lang="et">EU Bookshop</skos:prefLabel>
      <at:authority-code>EUBOOKSHOP</at:authority-code>
      <at:op-code>EUBOOKSHOP</at:op-code>
      <at:start.use>1952-07-24</at:start.use>
      <atold:op-code>EUBOOKSHOP</atold:op-code>
      <dc:identifier>EUBOOKSHOP</dc:identifier>
      <skos:altLabel xml:lang="en">EU Bookshop code</skos:altLabel>
      <skos:definition xml:lang="en">Code used by the EU Bookshop.</skos:definition>
      <skos:inScheme rdf:resource="http://publications.europa.eu/resource/authority/notation-type"/>
      <skos:topConceptOf rdf:resource="http://publications.europa.eu/resource/authority/notation-type"/>
   </skos:Concept>
   <skos:Concept rdf:about="http://publications.europa.eu/resource/authority/notation-type/EUDOR_LNG"
                 at:deprecated="false">
      <skos:prefLabel xml:lang="en">Eudor lang</skos:prefLabel>
      <skos:prefLabel xml:lang="et">Eudor keel</skos:prefLabel>
      <at:authority-code>EUDOR_LNG</at:authority-code>
      <at:op-code>EUDOR_LNG</at:op-code>
      <at:start.use>1998-12-04</at:start.use>
      <atold:op-code>EUDOR_LNG</atold:op-code>
      <dc:identifier>EUDOR_LNG</dc:identifier>
      <skos:altLabel xml:lang="en">Eudor language code</skos:altLabel>
      <skos:definition xml:lang="en">Code used in Eudor system for languages. Eudor supports Idol, a central repository that holds indexed data.</skos:definition>
      <skos:inScheme rdf:resource="http://publications.europa.eu/resource/authority/notation-type"/>
      <skos:topConceptOf rdf:resource="http://publications.europa.eu/resource/authority/notation-type"/>
      <at:op-mapped-code>
         <at:MappedCode>
            <dc:source>MDR</dc:source>
            <at:affected-table>notation-type</at:affected-table>
            <at:legacy-code>EUDOR</at:legacy-code>
         </at:MappedCode>
      </at:op-mapped-code>
   </skos:Concept>
   <skos:Concept rdf:about="http://publications.europa.eu/resource/authority/notation-type/EUDOR_MIME"
                 at:deprecated="false">
      <skos:prefLabel xml:lang="en">EUDOR MIME</skos:prefLabel>
      <skos:prefLabel xml:lang="et">EUDOR MIME</skos:prefLabel>
      <at:authority-code>EUDOR_MIME</at:authority-code>
      <at:op-code>EUDOR_MIME</at:op-code>
      <at:start.use>1998-12-04</at:start.use>
      <atold:op-code>EUDOR_MIME</atold:op-code>
      <dc:identifier>EUDOR_MIME</dc:identifier>
      <skos:altLabel xml:lang="en">Media type (Eudor) code</skos:altLabel>
      <skos:definition xml:lang="en">Code used in Eudor system for media types. Eudor supports Idol, a central repository that holds indexed data.</skos:definition>
      <skos:inScheme rdf:resource="http://publications.europa.eu/resource/authority/notation-type"/>
      <skos:topConceptOf rdf:resource="http://publications.europa.eu/resource/authority/notation-type"/>
      <at:op-mapped-code>
         <at:MappedCode>
            <dc:source>MDR</dc:source>
            <at:affected-table>notation-type</at:affected-table>
            <at:legacy-code>eudor-type-cellar</at:legacy-code>
         </at:MappedCode>
      </at:op-mapped-code>
   </skos:Concept>
   <skos:Concept rdf:about="http://publications.europa.eu/resource/authority/notation-type/EUROVOC"
                 at:deprecated="false">
      <skos:prefLabel xml:lang="en">EuroVoc</skos:prefLabel>
      <skos:prefLabel xml:lang="et">EuroVoc</skos:prefLabel>
      <at:authority-code>EUROVOC</at:authority-code>
      <at:op-code>EUROVOC</at:op-code>
      <at:start.use>1984-01-01</at:start.use>
      <atold:op-code>EUROVOC</atold:op-code>
      <dc:identifier>EUROVOC</dc:identifier>
      <skos:altLabel xml:lang="en">EuroVoc code</skos:altLabel>
      <skos:definition xml:lang="en">Code used in EU's multilingual thesaurus EuroVoc.</skos:definition>
      <skos:inScheme rdf:resource="http://publications.europa.eu/resource/authority/notation-type"/>
      <skos:topConceptOf rdf:resource="http://publications.europa.eu/resource/authority/notation-type"/>
   </skos:Concept>
   <skos:Concept rdf:about="http://publications.europa.eu/resource/authority/notation-type/E_ISSN"
                 at:deprecated="false">
      <skos:prefLabel xml:lang="en">e-ISSN</skos:prefLabel>
      <skos:prefLabel xml:lang="et">e-ISSN</skos:prefLabel>
      <at:authority-code>E_ISSN</at:authority-code>
      <at:op-code>E_ISSN</at:op-code>
      <at:start.use>2007-12-31</at:start.use>
      <atold:op-code>E_ISSN</atold:op-code>
      <dc:identifier>E_ISSN</dc:identifier>
      <skos:altLabel xml:lang="en">Electronic ISSN</skos:altLabel>
      <skos:definition xml:lang="en">A different ISSN from the print edition, the e-ISSN (Electronic ISSN) is used for the online edition of a journal. This is to enable librarians and other users to distinguish between their print and online holdings.</skos:definition>
      <skos:inScheme rdf:resource="http://publications.europa.eu/resource/authority/notation-type"/>
      <skos:topConceptOf rdf:resource="http://publications.europa.eu/resource/authority/notation-type"/>
      <skos:exactMatch rdf:resource="http://purl.org/spar/datacite/eissn"/>
   </skos:Concept>
   <skos:Concept rdf:about="http://publications.europa.eu/resource/authority/notation-type/FD_010"
                 at:deprecated="false">
      <skos:prefLabel xml:lang="en">FD_010</skos:prefLabel>
      <skos:prefLabel xml:lang="et">FD_010</skos:prefLabel>
      <at:authority-code>FD_010</at:authority-code>
      <at:op-code>FD_010</at:op-code>
      <at:start.use>2010-03-29</at:start.use>
      <atold:op-code>FD_010</atold:op-code>
      <dc:identifier>FD_010</dc:identifier>
      <skos:altLabel xml:lang="en">FD_Table010 code</skos:altLabel>
      <skos:definition xml:lang="en">Code used by FD_Table010 of Eurlex domain in ATTO.</skos:definition>
      <skos:inScheme rdf:resource="http://publications.europa.eu/resource/authority/notation-type"/>
      <skos:topConceptOf rdf:resource="http://publications.europa.eu/resource/authority/notation-type"/>
   </skos:Concept>
   <skos:Concept rdf:about="http://publications.europa.eu/resource/authority/notation-type/FD_020"
                 at:deprecated="false">
      <skos:prefLabel xml:lang="en">FD_020</skos:prefLabel>
      <skos:prefLabel xml:lang="et">FD_020</skos:prefLabel>
      <at:authority-code>FD_020</at:authority-code>
      <at:op-code>FD_020</at:op-code>
      <at:start.use>2010-03-29</at:start.use>
      <atold:op-code>FD_020</atold:op-code>
      <dc:identifier>FD_020</dc:identifier>
      <skos:altLabel xml:lang="en">FD_Table020 code</skos:altLabel>
      <skos:definition xml:lang="en">Code used by FD_Table020 of Eurlex domain in ATTO.</skos:definition>
      <skos:inScheme rdf:resource="http://publications.europa.eu/resource/authority/notation-type"/>
      <skos:topConceptOf rdf:resource="http://publications.europa.eu/resource/authority/notation-type"/>
   </skos:Concept>
   <skos:Concept rdf:about="http://publications.europa.eu/resource/authority/notation-type/FD_030"
                 at:deprecated="false">
      <skos:prefLabel xml:lang="en">FD_030</skos:prefLabel>
      <skos:prefLabel xml:lang="et">FD_030</skos:prefLabel>
      <at:authority-code>FD_030</at:authority-code>
      <at:op-code>FD_030</at:op-code>
      <at:start.use>2010-03-29</at:start.use>
      <atold:op-code>FD_030</atold:op-code>
      <dc:identifier>FD_030</dc:identifier>
      <skos:altLabel xml:lang="en">FD_Table030 code</skos:altLabel>
      <skos:definition xml:lang="en">Code used by FD_Table030 of Eurlex domain in ATTO.</skos:definition>
      <skos:inScheme rdf:resource="http://publications.europa.eu/resource/authority/notation-type"/>
      <skos:topConceptOf rdf:resource="http://publications.europa.eu/resource/authority/notation-type"/>
   </skos:Concept>
   <skos:Concept rdf:about="http://publications.europa.eu/resource/authority/notation-type/FD_040"
                 at:deprecated="false">
      <skos:prefLabel xml:lang="en">FD_040</skos:prefLabel>
      <skos:prefLabel xml:lang="et">FD_040</skos:prefLabel>
      <at:authority-code>FD_040</at:authority-code>
      <at:op-code>FD_040</at:op-code>
      <at:start.use>2010-03-29</at:start.use>
      <atold:op-code>FD_040</atold:op-code>
      <dc:identifier>FD_040</dc:identifier>
      <skos:altLabel xml:lang="en">FD_Table040 code</skos:altLabel>
      <skos:definition xml:lang="en">Code used by FD_Table040 of Eurlex domain in ATTO.</skos:definition>
      <skos:inScheme rdf:resource="http://publications.europa.eu/resource/authority/notation-type"/>
      <skos:topConceptOf rdf:resource="http://publications.europa.eu/resource/authority/notation-type"/>
   </skos:Concept>
   <skos:Concept rdf:about="http://publications.europa.eu/resource/authority/notation-type/FD_050"
                 at:deprecated="false">
      <skos:prefLabel xml:lang="en">FD_050</skos:prefLabel>
      <skos:prefLabel xml:lang="et">FD_050</skos:prefLabel>
      <at:authority-code>FD_050</at:authority-code>
      <at:op-code>FD_050</at:op-code>
      <at:start.use>2010-03-29</at:start.use>
      <atold:op-code>FD_050</atold:op-code>
      <dc:identifier>FD_050</dc:identifier>
      <skos:altLabel xml:lang="en">FD_Table050 code</skos:altLabel>
      <skos:definition xml:lang="en">Code used by FD_Table050 of Eurlex domain in ATTO.</skos:definition>
      <skos:inScheme rdf:resource="http://publications.europa.eu/resource/authority/notation-type"/>
      <skos:topConceptOf rdf:resource="http://publications.europa.eu/resource/authority/notation-type"/>
   </skos:Concept>
   <skos:Concept rdf:about="http://publications.europa.eu/resource/authority/notation-type/FD_060"
                 at:deprecated="false">
      <skos:prefLabel xml:lang="en">FD_060</skos:prefLabel>
      <skos:prefLabel xml:lang="et">FD_060</skos:prefLabel>
      <at:authority-code>FD_060</at:authority-code>
      <at:op-code>FD_060</at:op-code>
      <at:start.use>2010-03-29</at:start.use>
      <atold:op-code>FD_060</atold:op-code>
      <dc:identifier>FD_060</dc:identifier>
      <skos:altLabel xml:lang="en">FD_Table060 code</skos:altLabel>
      <skos:definition xml:lang="en">Code used by FD_Table060 of Eurlex domain in ATTO.</skos:definition>
      <skos:inScheme rdf:resource="http://publications.europa.eu/resource/authority/notation-type"/>
      <skos:topConceptOf rdf:resource="http://publications.europa.eu/resource/authority/notation-type"/>
   </skos:Concept>
   <skos:Concept rdf:about="http://publications.europa.eu/resource/authority/notation-type/FD_070"
                 at:deprecated="false">
      <skos:prefLabel xml:lang="en">FD_070</skos:prefLabel>
      <skos:prefLabel xml:lang="et">FD_070</skos:prefLabel>
      <at:authority-code>FD_070</at:authority-code>
      <at:op-code>FD_070</at:op-code>
      <at:start.use>2010-03-29</at:start.use>
      <atold:op-code>FD_070</atold:op-code>
      <dc:identifier>FD_070</dc:identifier>
      <skos:altLabel xml:lang="en">FD_Table070 code</skos:altLabel>
      <skos:definition xml:lang="en">Code used by FD_Table070 of Eurlex domain in ATTO.</skos:definition>
      <skos:inScheme rdf:resource="http://publications.europa.eu/resource/authority/notation-type"/>
      <skos:topConceptOf rdf:resource="http://publications.europa.eu/resource/authority/notation-type"/>
   </skos:Concept>
   <skos:Concept rdf:about="http://publications.europa.eu/resource/authority/notation-type/FD_100"
                 at:deprecated="false">
      <skos:prefLabel xml:lang="en">FD_100</skos:prefLabel>
      <skos:prefLabel xml:lang="et">FD_100</skos:prefLabel>
      <at:authority-code>FD_100</at:authority-code>
      <at:op-code>FD_100</at:op-code>
      <at:start.use>2010-03-29</at:start.use>
      <atold:op-code>FD_100</atold:op-code>
      <dc:identifier>FD_100</dc:identifier>
      <skos:altLabel xml:lang="en">FD_Table100 code</skos:altLabel>
      <skos:definition xml:lang="en">Code used by FD_Table100 of Eurlex domain in ATTO.</skos:definition>
      <skos:inScheme rdf:resource="http://publications.europa.eu/resource/authority/notation-type"/>
      <skos:topConceptOf rdf:resource="http://publications.europa.eu/resource/authority/notation-type"/>
   </skos:Concept>
   <skos:Concept rdf:about="http://publications.europa.eu/resource/authority/notation-type/FD_110"
                 at:deprecated="false">
      <skos:prefLabel xml:lang="en">FD_110</skos:prefLabel>
      <skos:prefLabel xml:lang="et">FD_110</skos:prefLabel>
      <at:authority-code>FD_110</at:authority-code>
      <at:op-code>FD_110</at:op-code>
      <at:start.use>2010-03-29</at:start.use>
      <atold:op-code>FD_110</atold:op-code>
      <dc:identifier>FD_110</dc:identifier>
      <skos:altLabel xml:lang="en">FD_Table110 code</skos:altLabel>
      <skos:definition xml:lang="en">Code used by FD_Table110 of Eurlex domain in ATTO.</skos:definition>
      <skos:inScheme rdf:resource="http://publications.europa.eu/resource/authority/notation-type"/>
      <skos:topConceptOf rdf:resource="http://publications.europa.eu/resource/authority/notation-type"/>
   </skos:Concept>
   <skos:Concept rdf:about="http://publications.europa.eu/resource/authority/notation-type/FD_140"
                 at:deprecated="false">
      <skos:prefLabel xml:lang="en">FD_140</skos:prefLabel>
      <skos:prefLabel xml:lang="et">FD_140</skos:prefLabel>
      <at:authority-code>FD_140</at:authority-code>
      <at:op-code>FD_140</at:op-code>
      <at:start.use>2010-03-29</at:start.use>
      <atold:op-code>FD_140</atold:op-code>
      <dc:identifier>FD_140</dc:identifier>
      <skos:altLabel xml:lang="en">FD_Table140 code</skos:altLabel>
      <skos:definition xml:lang="en">Code used by FD_Table140 of Eurlex domain in ATTO.</skos:definition>
      <skos:inScheme rdf:resource="http://publications.europa.eu/resource/authority/notation-type"/>
      <skos:topConceptOf rdf:resource="http://publications.europa.eu/resource/authority/notation-type"/>
   </skos:Concept>
   <skos:Concept rdf:about="http://publications.europa.eu/resource/authority/notation-type/FD_160"
                 at:deprecated="false">
      <skos:prefLabel xml:lang="en">FD_160</skos:prefLabel>
      <skos:prefLabel xml:lang="et">FD_160</skos:prefLabel>
      <at:authority-code>FD_160</at:authority-code>
      <at:op-code>FD_160</at:op-code>
      <at:start.use>2010-03-29</at:start.use>
      <atold:op-code>FD_160</atold:op-code>
      <dc:identifier>FD_160</dc:identifier>
      <skos:altLabel xml:lang="en">FD_Table160 code</skos:altLabel>
      <skos:definition xml:lang="en">Code used by FD_Table160 of Eurlex domain in ATTO.</skos:definition>
      <skos:inScheme rdf:resource="http://publications.europa.eu/resource/authority/notation-type"/>
      <skos:topConceptOf rdf:resource="http://publications.europa.eu/resource/authority/notation-type"/>
   </skos:Concept>
   <skos:Concept rdf:about="http://publications.europa.eu/resource/authority/notation-type/FD_290"
                 at:deprecated="false">
      <skos:prefLabel xml:lang="en">FD_290</skos:prefLabel>
      <skos:prefLabel xml:lang="et">FD_290</skos:prefLabel>
      <at:authority-code>FD_290</at:authority-code>
      <at:op-code>FD_290</at:op-code>
      <at:start.use>2010-03-29</at:start.use>
      <atold:op-code>FD_290</atold:op-code>
      <dc:identifier>FD_290</dc:identifier>
      <skos:altLabel xml:lang="en">FD_Table290 code</skos:altLabel>
      <skos:definition xml:lang="en">Code used by FD_Table290 of Eurlex domain in ATTO.</skos:definition>
      <skos:inScheme rdf:resource="http://publications.europa.eu/resource/authority/notation-type"/>
      <skos:topConceptOf rdf:resource="http://publications.europa.eu/resource/authority/notation-type"/>
   </skos:Concept>
   <skos:Concept rdf:about="http://publications.europa.eu/resource/authority/notation-type/FD_325"
                 at:deprecated="false">
      <skos:prefLabel xml:lang="en">FD_361</skos:prefLabel>
      <skos:prefLabel xml:lang="et">FD_361</skos:prefLabel>
      <at:authority-code>FD_325</at:authority-code>
      <at:op-code>FD_325</at:op-code>
      <at:start.use>2010-03-29</at:start.use>
      <atold:op-code>FD_325</atold:op-code>
      <dc:identifier>FD_325</dc:identifier>
      <skos:altLabel xml:lang="en">FD_Table361 code</skos:altLabel>
      <skos:definition xml:lang="en">Code used by FD_Table361 of Eurlex domain in ATTO.</skos:definition>
      <skos:inScheme rdf:resource="http://publications.europa.eu/resource/authority/notation-type"/>
      <skos:topConceptOf rdf:resource="http://publications.europa.eu/resource/authority/notation-type"/>
   </skos:Concept>
   <skos:Concept rdf:about="http://publications.europa.eu/resource/authority/notation-type/FD_361"
                 at:deprecated="false">
      <skos:prefLabel xml:lang="en">FD_325</skos:prefLabel>
      <skos:prefLabel xml:lang="et">FD_325</skos:prefLabel>
      <at:authority-code>FD_361</at:authority-code>
      <at:op-code>FD_361</at:op-code>
      <at:start.use>2010-03-29</at:start.use>
      <atold:op-code>FD_361</atold:op-code>
      <dc:identifier>FD_361</dc:identifier>
      <skos:altLabel xml:lang="en">FD_Table325 code</skos:altLabel>
      <skos:definition xml:lang="en">Code used by FD_Table325 of Eurlex domain in ATTO.</skos:definition>
      <skos:inScheme rdf:resource="http://publications.europa.eu/resource/authority/notation-type"/>
      <skos:topConceptOf rdf:resource="http://publications.europa.eu/resource/authority/notation-type"/>
   </skos:Concept>
   <skos:Concept rdf:about="http://publications.europa.eu/resource/authority/notation-type/FD_375"
                 at:deprecated="false">
      <skos:prefLabel xml:lang="en">FD_375</skos:prefLabel>
      <skos:prefLabel xml:lang="et">FD_375</skos:prefLabel>
      <at:authority-code>FD_375</at:authority-code>
      <at:op-code>FD_375</at:op-code>
      <at:start.use>2010-03-29</at:start.use>
      <atold:op-code>FD_375</atold:op-code>
      <dc:identifier>FD_375</dc:identifier>
      <skos:altLabel xml:lang="en">FD_Table375 code</skos:altLabel>
      <skos:definition xml:lang="en">Code used by FD_Table375 of Eurlex domain in ATTO.</skos:definition>
      <skos:inScheme rdf:resource="http://publications.europa.eu/resource/authority/notation-type"/>
      <skos:topConceptOf rdf:resource="http://publications.europa.eu/resource/authority/notation-type"/>
   </skos:Concept>
   <skos:Concept rdf:about="http://publications.europa.eu/resource/authority/notation-type/FD_380"
                 at:deprecated="false">
      <skos:prefLabel xml:lang="en">FD_380</skos:prefLabel>
      <skos:prefLabel xml:lang="et">FD_380</skos:prefLabel>
      <at:authority-code>FD_380</at:authority-code>
      <at:op-code>FD_380</at:op-code>
      <at:start.use>2010-03-29</at:start.use>
      <atold:op-code>FD_380</atold:op-code>
      <dc:identifier>FD_380</dc:identifier>
      <skos:altLabel xml:lang="en">FD_Table380 code</skos:altLabel>
      <skos:definition xml:lang="en">Code used by FD_Table380 of Eurlex domain in ATTO.</skos:definition>
      <skos:inScheme rdf:resource="http://publications.europa.eu/resource/authority/notation-type"/>
      <skos:topConceptOf rdf:resource="http://publications.europa.eu/resource/authority/notation-type"/>
   </skos:Concept>
   <skos:Concept rdf:about="http://publications.europa.eu/resource/authority/notation-type/FD_400"
                 at:deprecated="false">
      <skos:prefLabel xml:lang="en">FD_400</skos:prefLabel>
      <skos:prefLabel xml:lang="et">FD_400</skos:prefLabel>
      <at:authority-code>FD_400</at:authority-code>
      <at:op-code>FD_400</at:op-code>
      <at:start.use>2010-03-29</at:start.use>
      <atold:op-code>FD_400</atold:op-code>
      <dc:identifier>FD_400</dc:identifier>
      <skos:altLabel xml:lang="en">FD_Table400 code</skos:altLabel>
      <skos:definition xml:lang="en">Code used by FD_Table400 of Eurlex domain in ATTO.</skos:definition>
      <skos:inScheme rdf:resource="http://publications.europa.eu/resource/authority/notation-type"/>
      <skos:topConceptOf rdf:resource="http://publications.europa.eu/resource/authority/notation-type"/>
   </skos:Concept>
   <skos:Concept rdf:about="http://publications.europa.eu/resource/authority/notation-type/FD_499"
                 at:deprecated="false">
      <skos:prefLabel xml:lang="en">FD_499</skos:prefLabel>
      <skos:prefLabel xml:lang="et">FD_499</skos:prefLabel>
      <at:authority-code>FD_499</at:authority-code>
      <at:op-code>FD_499</at:op-code>
      <at:start.use>2010-03-29</at:start.use>
      <atold:op-code>FD_499</atold:op-code>
      <dc:identifier>FD_499</dc:identifier>
      <skos:altLabel xml:lang="en">FD_Table499 code</skos:altLabel>
      <skos:definition xml:lang="en">Code used by FD_Table499 of Eurlex domain in ATTO.</skos:definition>
      <skos:inScheme rdf:resource="http://publications.europa.eu/resource/authority/notation-type"/>
      <skos:topConceptOf rdf:resource="http://publications.europa.eu/resource/authority/notation-type"/>
   </skos:Concept>
   <skos:Concept rdf:about="http://publications.europa.eu/resource/authority/notation-type/FD_557"
                 at:deprecated="false">
      <skos:prefLabel xml:lang="en">FD_557</skos:prefLabel>
      <skos:prefLabel xml:lang="et">FD_557</skos:prefLabel>
      <at:authority-code>FD_557</at:authority-code>
      <at:op-code>FD_557</at:op-code>
      <at:start.use>2010-03-29</at:start.use>
      <atold:op-code>FD_557</atold:op-code>
      <dc:identifier>FD_557</dc:identifier>
      <skos:altLabel xml:lang="en">FD_Table557 code</skos:altLabel>
      <skos:definition xml:lang="en">Code used by FD_Table557 of Eurlex domain in ATTO.</skos:definition>
      <skos:inScheme rdf:resource="http://publications.europa.eu/resource/authority/notation-type"/>
      <skos:topConceptOf rdf:resource="http://publications.europa.eu/resource/authority/notation-type"/>
   </skos:Concept>
   <skos:Concept rdf:about="http://publications.europa.eu/resource/authority/notation-type/FD_601"
                 at:deprecated="false">
      <skos:prefLabel xml:lang="en">FD_601</skos:prefLabel>
      <skos:prefLabel xml:lang="et">FD_601</skos:prefLabel>
      <at:authority-code>FD_601</at:authority-code>
      <at:op-code>FD_601</at:op-code>
      <at:start.use>2011-06-09</at:start.use>
      <atold:op-code>FD_601</atold:op-code>
      <dc:identifier>FD_601</dc:identifier>
      <skos:altLabel xml:lang="en">FD_Table601 code</skos:altLabel>
      <skos:definition xml:lang="en">Code used by FD_Table601 of Eurlex domain in ATTO.</skos:definition>
      <skos:inScheme rdf:resource="http://publications.europa.eu/resource/authority/notation-type"/>
      <skos:topConceptOf rdf:resource="http://publications.europa.eu/resource/authority/notation-type"/>
   </skos:Concept>
   <skos:Concept rdf:about="http://publications.europa.eu/resource/authority/notation-type/FD_607"
                 at:deprecated="false">
      <skos:prefLabel xml:lang="en">FD_607</skos:prefLabel>
      <skos:prefLabel xml:lang="et">FD_607</skos:prefLabel>
      <at:authority-code>FD_607</at:authority-code>
      <at:op-code>FD_607</at:op-code>
      <at:start.use>2010-03-29</at:start.use>
      <atold:op-code>FD_607</atold:op-code>
      <dc:identifier>FD_607</dc:identifier>
      <skos:altLabel xml:lang="en">FD_Table607 code</skos:altLabel>
      <skos:definition xml:lang="en">Code used by FD_Table607 of Eurlex domain in ATTO.</skos:definition>
      <skos:inScheme rdf:resource="http://publications.europa.eu/resource/authority/notation-type"/>
      <skos:topConceptOf rdf:resource="http://publications.europa.eu/resource/authority/notation-type"/>
   </skos:Concept>
   <skos:Concept rdf:about="http://publications.europa.eu/resource/authority/notation-type/FD_608"
                 at:deprecated="false">
      <skos:prefLabel xml:lang="en">FD_608</skos:prefLabel>
      <skos:prefLabel xml:lang="et">FD_608</skos:prefLabel>
      <at:authority-code>FD_608</at:authority-code>
      <at:op-code>FD_608</at:op-code>
      <at:start.use>2010-03-29</at:start.use>
      <atold:op-code>FD_608</atold:op-code>
      <dc:identifier>FD_608</dc:identifier>
      <skos:altLabel xml:lang="en">FD_Table608 code</skos:altLabel>
      <skos:definition xml:lang="en">Code used by FD_Table608 of Eurlex domain in ATTO.</skos:definition>
      <skos:inScheme rdf:resource="http://publications.europa.eu/resource/authority/notation-type"/>
      <skos:topConceptOf rdf:resource="http://publications.europa.eu/resource/authority/notation-type"/>
   </skos:Concept>
   <skos:Concept rdf:about="http://publications.europa.eu/resource/authority/notation-type/FD_609"
                 at:deprecated="false">
      <skos:prefLabel xml:lang="en">FD_609</skos:prefLabel>
      <skos:prefLabel xml:lang="et">FD_609</skos:prefLabel>
      <at:authority-code>FD_609</at:authority-code>
      <at:op-code>FD_609</at:op-code>
      <at:start.use>2010-03-29</at:start.use>
      <atold:op-code>FD_609</atold:op-code>
      <dc:identifier>FD_609</dc:identifier>
      <skos:altLabel xml:lang="en">FD_Table609 code</skos:altLabel>
      <skos:definition xml:lang="en">Code used by FD_Table609 of Eurlex domain in ATTO.</skos:definition>
      <skos:inScheme rdf:resource="http://publications.europa.eu/resource/authority/notation-type"/>
      <skos:topConceptOf rdf:resource="http://publications.europa.eu/resource/authority/notation-type"/>
   </skos:Concept>
   <skos:Concept rdf:about="http://publications.europa.eu/resource/authority/notation-type/FD_610"
                 at:deprecated="false">
      <skos:prefLabel xml:lang="en">FD_610</skos:prefLabel>
      <skos:prefLabel xml:lang="et">FD_610</skos:prefLabel>
      <at:authority-code>FD_610</at:authority-code>
      <at:op-code>FD_610</at:op-code>
      <at:start.use>2011-06-09</at:start.use>
      <atold:op-code>FD_610</atold:op-code>
      <dc:identifier>FD_610</dc:identifier>
      <skos:altLabel xml:lang="en">FD_Table610 code</skos:altLabel>
      <skos:definition xml:lang="en">Code used by FD_Table610 of Eurlex domain in ATTO.</skos:definition>
      <skos:inScheme rdf:resource="http://publications.europa.eu/resource/authority/notation-type"/>
      <skos:topConceptOf rdf:resource="http://publications.europa.eu/resource/authority/notation-type"/>
   </skos:Concept>
   <skos:Concept rdf:about="http://publications.europa.eu/resource/authority/notation-type/FD_612"
                 at:deprecated="false">
      <skos:prefLabel xml:lang="en">FD_612</skos:prefLabel>
      <skos:prefLabel xml:lang="et">FD_612</skos:prefLabel>
      <at:authority-code>FD_612</at:authority-code>
      <at:op-code>FD_612</at:op-code>
      <at:start.use>2010-03-29</at:start.use>
      <atold:op-code>FD_612</atold:op-code>
      <dc:identifier>FD_612</dc:identifier>
      <skos:altLabel xml:lang="en">FD_Table612 code</skos:altLabel>
      <skos:definition xml:lang="en">Code used by FD_Table612 of Eurlex domain in ATTO.</skos:definition>
      <skos:inScheme rdf:resource="http://publications.europa.eu/resource/authority/notation-type"/>
      <skos:topConceptOf rdf:resource="http://publications.europa.eu/resource/authority/notation-type"/>
   </skos:Concept>
   <skos:Concept rdf:about="http://publications.europa.eu/resource/authority/notation-type/FD_613"
                 at:deprecated="false">
      <skos:prefLabel xml:lang="en">FD_613</skos:prefLabel>
      <skos:prefLabel xml:lang="et">FD_613</skos:prefLabel>
      <at:authority-code>FD_613</at:authority-code>
      <at:op-code>FD_613</at:op-code>
      <at:start.use>2010-03-29</at:start.use>
      <atold:op-code>FD_613</atold:op-code>
      <dc:identifier>FD_613</dc:identifier>
      <skos:altLabel xml:lang="en">FD_Table613 code</skos:altLabel>
      <skos:definition xml:lang="en">Code used by FD_Table613 of Eurlex domain in ATTO.</skos:definition>
      <skos:inScheme rdf:resource="http://publications.europa.eu/resource/authority/notation-type"/>
      <skos:topConceptOf rdf:resource="http://publications.europa.eu/resource/authority/notation-type"/>
   </skos:Concept>
   <skos:Concept rdf:about="http://publications.europa.eu/resource/authority/notation-type/FILE_EXT"
                 at:deprecated="false">
      <skos:prefLabel xml:lang="en">File ext</skos:prefLabel>
      <skos:prefLabel xml:lang="et">File ext</skos:prefLabel>
      <at:authority-code>FILE_EXT</at:authority-code>
      <at:op-code>FILE_EXT</at:op-code>
      <at:start.use>1973-01-01</at:start.use>
      <atold:op-code>FILE_EXT</atold:op-code>
      <dc:identifier>FILE_EXT</dc:identifier>
      <skos:altLabel xml:lang="en">File extensions code</skos:altLabel>
      <skos:definition xml:lang="en">A file extension is an identifier specified as a suffix to the name of a computer file. The extension indicates a characteristic of the file contents or its intended use. A file extension is typically delimited from the filename with a full stop.</skos:definition>
      <skos:inScheme rdf:resource="http://publications.europa.eu/resource/authority/notation-type"/>
      <skos:topConceptOf rdf:resource="http://publications.europa.eu/resource/authority/notation-type"/>
      <at:op-mapped-code>
         <at:MappedCode>
            <dc:source>MDR</dc:source>
            <at:affected-table>notation-type</at:affected-table>
            <at:legacy-code>file-extension</at:legacy-code>
         </at:MappedCode>
      </at:op-mapped-code>
   </skos:Concept>
   <skos:Concept rdf:about="http://publications.europa.eu/resource/authority/notation-type/FORMEX"
                 at:deprecated="false">
      <skos:prefLabel xml:lang="en">Formex</skos:prefLabel>
      <skos:prefLabel xml:lang="et">Formex</skos:prefLabel>
      <at:authority-code>FORMEX</at:authority-code>
      <at:op-code>FORMEX</at:op-code>
      <at:start.use>2004-05-01</at:start.use>
      <atold:op-code>FORMEX</atold:op-code>
      <dc:identifier>FORMEX</dc:identifier>
      <skos:altLabel xml:lang="en">Formex code</skos:altLabel>
      <skos:definition xml:lang="en">Code used by Formalized Exchange of Electronic Publications.</skos:definition>
      <skos:inScheme rdf:resource="http://publications.europa.eu/resource/authority/notation-type"/>
      <skos:topConceptOf rdf:resource="http://publications.europa.eu/resource/authority/notation-type"/>
   </skos:Concept>
   <skos:Concept rdf:about="http://publications.europa.eu/resource/authority/notation-type/FUNDREF"
                 at:deprecated="false">
      <skos:prefLabel xml:lang="en">FundRef</skos:prefLabel>
      <skos:prefLabel xml:lang="et">FundRef</skos:prefLabel>
      <at:authority-code>FUNDREF</at:authority-code>
      <at:op-code>FUNDREF</at:op-code>
      <at:start.use>2012-01-01</at:start.use>
      <atold:op-code>FUNDREF</atold:op-code>
      <dc:identifier>FUNDREF</dc:identifier>
      <skos:altLabel xml:lang="en">FundRef identifier</skos:altLabel>
      <skos:definition xml:lang="en">FundRef is an identifier for an organisation that funds research. It is assigned by Crossref and maintained in its global FundRef registry.</skos:definition>
      <skos:inScheme rdf:resource="http://publications.europa.eu/resource/authority/notation-type"/>
      <skos:topConceptOf rdf:resource="http://publications.europa.eu/resource/authority/notation-type"/>
      <skos:exactMatch rdf:resource="http://purl.org/spar/datacite/fundref"/>
   </skos:Concept>
   <skos:Concept rdf:about="http://publications.europa.eu/resource/authority/notation-type/HANDLE"
                 at:deprecated="false">
      <skos:prefLabel xml:lang="en">Handle</skos:prefLabel>
      <skos:prefLabel xml:lang="et">Handle</skos:prefLabel>
      <at:authority-code>HANDLE</at:authority-code>
      <at:op-code>HANDLE</at:op-code>
      <at:start.use>1994-12-31</at:start.use>
      <atold:op-code>HANDLE</atold:op-code>
      <dc:identifier>HANDLE</dc:identifier>
      <skos:altLabel xml:lang="en">Handle identifier</skos:altLabel>
      <skos:definition xml:lang="en">The Handle identifier is generated by the Handle System which allows secured name resolution and administration over the public Internet. A Handle is unique and can be retained over long time periods. The scheme is described in the RFC 1737.</skos:definition>
      <skos:inScheme rdf:resource="http://publications.europa.eu/resource/authority/notation-type"/>
      <skos:topConceptOf rdf:resource="http://publications.europa.eu/resource/authority/notation-type"/>
      <skos:exactMatch rdf:resource="http://purl.org/spar/datacite/handle"/>
   </skos:Concept>
   <skos:Concept rdf:about="http://publications.europa.eu/resource/authority/notation-type/IANA_DOMAIN"
                 at:deprecated="false">
      <skos:prefLabel xml:lang="en">IANA</skos:prefLabel>
      <skos:prefLabel xml:lang="et">IANA</skos:prefLabel>
      <at:authority-code>IANA_DOMAIN</at:authority-code>
      <at:op-code>IANA_DOMAIN</at:op-code>
      <at:start.use>1988-01-01</at:start.use>
      <atold:op-code>IANA_DOMAIN</atold:op-code>
      <dc:identifier>IANA_DOMAIN</dc:identifier>
      <skos:altLabel xml:lang="en">Internet Assigned Numbers Authority code</skos:altLabel>
      <skos:definition xml:lang="en">Internet Assigned Numbers Authority codes are two-letter codes for country-coded top-level domains in Internet addresses.</skos:definition>
      <skos:inScheme rdf:resource="http://publications.europa.eu/resource/authority/notation-type"/>
      <skos:topConceptOf rdf:resource="http://publications.europa.eu/resource/authority/notation-type"/>
      <at:op-mapped-code>
         <at:MappedCode>
            <dc:source>MDR</dc:source>
            <at:affected-table>notation-type</at:affected-table>
            <at:legacy-code>code-iana</at:legacy-code>
         </at:MappedCode>
      </at:op-mapped-code>
   </skos:Concept>
   <skos:Concept rdf:about="http://publications.europa.eu/resource/authority/notation-type/IANA_MT"
                 at:deprecated="false">
      <skos:prefLabel xml:lang="en">IANA MIME</skos:prefLabel>
      <skos:prefLabel xml:lang="et">IANA MIME</skos:prefLabel>
      <at:authority-code>IANA_MT</at:authority-code>
      <at:op-code>IANA_MT</at:op-code>
      <at:start.use>1988-01-01</at:start.use>
      <atold:op-code>IANA_MT</atold:op-code>
      <dc:identifier>IANA_MT</dc:identifier>
      <skos:altLabel xml:lang="en">Media Type (IANA) code</skos:altLabel>
      <skos:definition xml:lang="en">Code used by the Internet Assigned Numbers Authority (IANA) for media types.</skos:definition>
      <skos:inScheme rdf:resource="http://publications.europa.eu/resource/authority/notation-type"/>
      <skos:topConceptOf rdf:resource="http://publications.europa.eu/resource/authority/notation-type"/>
      <at:op-mapped-code>
         <at:MappedCode>
            <dc:source>MDR</dc:source>
            <at:affected-table>notation-type</at:affected-table>
            <at:legacy-code>internet-media-type</at:legacy-code>
         </at:MappedCode>
      </at:op-mapped-code>
   </skos:Concept>
   <skos:Concept rdf:about="http://publications.europa.eu/resource/authority/notation-type/IATE"
                 at:deprecated="false">
      <skos:prefLabel xml:lang="en">IATE</skos:prefLabel>
      <skos:prefLabel xml:lang="et">IATE</skos:prefLabel>
      <at:authority-code>IATE</at:authority-code>
      <at:op-code>IATE</at:op-code>
      <at:start.use>2004-06-01</at:start.use>
      <atold:op-code>IATE</atold:op-code>
      <dc:identifier>IATE</dc:identifier>
      <skos:altLabel xml:lang="en">IATE code</skos:altLabel>
      <skos:definition xml:lang="en">Code used in IATE, Inter-Active Terminology for Europe.</skos:definition>
      <skos:inScheme rdf:resource="http://publications.europa.eu/resource/authority/notation-type"/>
      <skos:topConceptOf rdf:resource="http://publications.europa.eu/resource/authority/notation-type"/>
      <at:op-mapped-code>
         <at:MappedCode>
            <dc:source>MDR</dc:source>
            <at:affected-table>notation-type</at:affected-table>
            <at:legacy-code>IATE.id</at:legacy-code>
         </at:MappedCode>
      </at:op-mapped-code>
   </skos:Concept>
   <skos:Concept rdf:about="http://publications.europa.eu/resource/authority/notation-type/IBAN_COU"
                 at:deprecated="false">
      <skos:prefLabel xml:lang="en">IBAN country code</skos:prefLabel>
      <at:authority-code>IBAN_COU</at:authority-code>
      <at:op-code>IBAN_COU</at:op-code>
      <at:start.use>2021-12-08</at:start.use>
      <atold:op-code>IBAN_COU</atold:op-code>
      <dc:identifier>IBAN_COU</dc:identifier>
      <skos:definition xml:lang="en">A two-letter country code (ISO 3166-1 alpha-2) used in the International Bank Account Number (IBAN) system. An IBAN consists of up to 34 alphanumeric characters comprising a country code; two check digits; and a number that includes the domestic bank account number, branch identifier, and potential routing information.</skos:definition>
      <skos:inScheme rdf:resource="http://publications.europa.eu/resource/authority/notation-type"/>
      <skos:topConceptOf rdf:resource="http://publications.europa.eu/resource/authority/notation-type"/>
   </skos:Concept>
   <skos:Concept rdf:about="http://publications.europa.eu/resource/authority/notation-type/IENI"
                 at:deprecated="false">
      <skos:prefLabel xml:lang="en">IENI</skos:prefLabel>
      <skos:prefLabel xml:lang="et">IENI</skos:prefLabel>
      <at:authority-code>IENI</at:authority-code>
      <at:op-code>IENI</at:op-code>
      <at:start.use>2022-04-29</at:start.use>
      <atold:op-code>IENI</atold:op-code>
      <dc:identifier>IENI</dc:identifier>
      <skos:altLabel xml:lang="en">IENI collection</skos:altLabel>
      <skos:definition xml:lang="en">Identifier used in the collection (“IENI collection”) of acts related to the Ireland and Northern Ireland, based on the Protocol annexed to the Agreement on the withdrawal of the United Kingdom of Great Britain and Northern Ireland.</skos:definition>
      <skos:inScheme rdf:resource="http://publications.europa.eu/resource/authority/notation-type"/>
      <skos:topConceptOf rdf:resource="http://publications.europa.eu/resource/authority/notation-type"/>
   </skos:Concept>
   <skos:Concept rdf:about="http://publications.europa.eu/resource/authority/notation-type/INFOURI"
                 at:deprecated="false">
      <skos:prefLabel xml:lang="en">INFO URI</skos:prefLabel>
      <skos:prefLabel xml:lang="et">INFO URI</skos:prefLabel>
      <at:authority-code>INFOURI</at:authority-code>
      <at:op-code>INFOURI</at:op-code>
      <at:start.use>2005-12-30</at:start.use>
      <atold:op-code>INFOURI</atold:op-code>
      <dc:identifier>INFOURI</dc:identifier>
      <skos:altLabel xml:lang="en">Info URI</skos:altLabel>
      <skos:definition xml:lang="en">The Info URI identifier is an URI conforming to the Info URI scheme which enables identifiers from public namespaces to be represented as URIs when they would otherwise have no canonical URL form.</skos:definition>
      <skos:inScheme rdf:resource="http://publications.europa.eu/resource/authority/notation-type"/>
      <skos:topConceptOf rdf:resource="http://publications.europa.eu/resource/authority/notation-type"/>
      <skos:exactMatch rdf:resource="http://purl.org/spar/datacite/infouri"/>
   </skos:Concept>
   <skos:Concept rdf:about="http://publications.europa.eu/resource/authority/notation-type/ISBN"
                 at:deprecated="false">
      <skos:prefLabel xml:lang="en">ISBN</skos:prefLabel>
      <skos:prefLabel xml:lang="et">ISBN</skos:prefLabel>
      <at:authority-code>ISBN</at:authority-code>
      <at:op-code>ISBN</at:op-code>
      <at:start.use>1970-01-01</at:start.use>
      <atold:op-code>ISBN</atold:op-code>
      <dc:identifier>ISBN</dc:identifier>
      <skos:altLabel xml:lang="en">International Standard Book Number code</skos:altLabel>
      <skos:definition xml:lang="en">An ISBN is essentially a product identifier used by publishers, booksellers, libraries, internet retailers and other supply chain participants for ordering, listing, sales records and stock control purposes. The ISBN identifies the registrant as well as the specific title, edition and format. ISBNs are calculated using a specific mathematical formula and include a check digit to validate the number. ISBN is an International Standard that is published by ISO.</skos:definition>
      <skos:inScheme rdf:resource="http://publications.europa.eu/resource/authority/notation-type"/>
      <skos:topConceptOf rdf:resource="http://publications.europa.eu/resource/authority/notation-type"/>
      <skos:exactMatch rdf:resource="http://purl.org/spar/datacite/isbn"/>
   </skos:Concept>
   <skos:Concept rdf:about="http://publications.europa.eu/resource/authority/notation-type/ISBN_RG"
                 at:deprecated="false">
      <skos:prefLabel xml:lang="en">ISBN reg ele</skos:prefLabel>
      <skos:prefLabel xml:lang="et">ISBN reg ele</skos:prefLabel>
      <at:authority-code>ISBN_RG</at:authority-code>
      <at:op-code>ISBN_RG</at:op-code>
      <at:start.use>2000-01-01</at:start.use>
      <atold:op-code>ISBN_RG</atold:op-code>
      <dc:identifier>ISBN_RG</dc:identifier>
      <skos:altLabel xml:lang="en">ISBN registrant element</skos:altLabel>
      <skos:definition xml:lang="en">Each ISBN consists of 5 elements with each section being separated by spaces or hyphens. The ISBN registrant element identifies the particular publisher or imprint.</skos:definition>
      <skos:inScheme rdf:resource="http://publications.europa.eu/resource/authority/notation-type"/>
      <skos:topConceptOf rdf:resource="http://publications.europa.eu/resource/authority/notation-type"/>
      <at:op-mapped-code>
         <at:MappedCode>
            <dc:source>MDR</dc:source>
            <at:affected-table>notation-type</at:affected-table>
            <at:legacy-code>id-isbn.old</at:legacy-code>
         </at:MappedCode>
      </at:op-mapped-code>
      <at:op-mapped-code>
         <at:MappedCode>
            <dc:source>MDR</dc:source>
            <at:affected-table>notation-type</at:affected-table>
            <at:legacy-code>id-isbn</at:legacy-code>
         </at:MappedCode>
      </at:op-mapped-code>
   </skos:Concept>
   <skos:Concept rdf:about="http://publications.europa.eu/resource/authority/notation-type/ISG_COU"
                 at:deprecated="false">
      <skos:prefLabel xml:lang="en">ISG COU</skos:prefLabel>
      <skos:prefLabel xml:lang="et">ISG COU</skos:prefLabel>
      <at:authority-code>ISG_COU</at:authority-code>
      <at:op-code>ISG_COU</at:op-code>
      <at:start.use>1993-01-01</at:start.use>
      <atold:op-code>ISG_COU</atold:op-code>
      <dc:identifier>ISG_COU</dc:identifier>
      <skos:altLabel xml:lang="en">ISG country code</skos:altLabel>
      <skos:definition xml:lang="en">Country code used in the Interinstitutional style guide.</skos:definition>
      <skos:inScheme rdf:resource="http://publications.europa.eu/resource/authority/notation-type"/>
      <skos:topConceptOf rdf:resource="http://publications.europa.eu/resource/authority/notation-type"/>
      <at:op-mapped-code>
         <at:MappedCode>
            <dc:source>MDR</dc:source>
            <at:affected-table>notation-type</at:affected-table>
            <at:legacy-code>op-styleguide</at:legacy-code>
         </at:MappedCode>
      </at:op-mapped-code>
   </skos:Concept>
   <skos:Concept rdf:about="http://publications.europa.eu/resource/authority/notation-type/ISNI"
                 at:deprecated="false">
      <skos:prefLabel xml:lang="en">ISNI</skos:prefLabel>
      <skos:prefLabel xml:lang="et">ISNI</skos:prefLabel>
      <at:authority-code>ISNI</at:authority-code>
      <at:op-code>ISNI</at:op-code>
      <at:start.use>2012-03-15</at:start.use>
      <atold:op-code>ISNI</atold:op-code>
      <dc:identifier>ISNI</dc:identifier>
      <skos:altLabel xml:lang="en">International Standard Name Identifier</skos:altLabel>
      <skos:definition xml:lang="en">ISNI is the ISO certified global standard number for identifying the millions of contributors to creative works and those active in their distribution, including researchers, inventors, writers, artists, visual creators, performers, producers, publishers, aggregators, and more.</skos:definition>
      <skos:inScheme rdf:resource="http://publications.europa.eu/resource/authority/notation-type"/>
      <skos:topConceptOf rdf:resource="http://publications.europa.eu/resource/authority/notation-type"/>
      <skos:exactMatch rdf:resource="http://purl.org/spar/datacite/isni"/>
   </skos:Concept>
   <skos:Concept rdf:about="http://publications.europa.eu/resource/authority/notation-type/ISO_15924_ALPHA_4"
                 at:deprecated="false">
      <skos:prefLabel xml:lang="en">ISO 15924 α-4</skos:prefLabel>
      <skos:prefLabel xml:lang="et">ISO 15924 α-4</skos:prefLabel>
      <at:authority-code>ISO_15924_ALPHA_4</at:authority-code>
      <at:op-code>ISO_15924_ALPHA_4</at:op-code>
      <at:start.use>2020-06-24</at:start.use>
      <atold:op-code>ISO_15924_ALPHA_4</atold:op-code>
      <dc:identifier>ISO_15924_ALPHA_4</dc:identifier>
      <skos:altLabel xml:lang="en">ISO 15924 alpha-4 code</skos:altLabel>
      <skos:definition xml:lang="en">ISO 15924 alpha-4 codes are four-letter script codes defined in ISO 15924 standard published by the International Organization for Standardization (ISO), to represent names of scripts. Script is defined as ‘set of graphic characters used for the written form of one or more languages’.</skos:definition>
      <skos:inScheme rdf:resource="http://publications.europa.eu/resource/authority/notation-type"/>
      <skos:topConceptOf rdf:resource="http://publications.europa.eu/resource/authority/notation-type"/>
      <at:op-mapped-code>
         <at:MappedCode>
            <dc:source>MDR</dc:source>
            <at:affected-table>notation-type</at:affected-table>
            <at:legacy-code>iso-15924-alpha-4</at:legacy-code>
         </at:MappedCode>
      </at:op-mapped-code>
   </skos:Concept>
   <skos:Concept rdf:about="http://publications.europa.eu/resource/authority/notation-type/ISO_15924_NUM"
                 at:deprecated="false">
      <skos:prefLabel xml:lang="en">ISO 15924 num</skos:prefLabel>
      <skos:prefLabel xml:lang="et">ISO 15924 num</skos:prefLabel>
      <at:authority-code>ISO_15924_NUM</at:authority-code>
      <at:op-code>ISO_15924_NUM</at:op-code>
      <at:start.use>2020-06-24</at:start.use>
      <atold:op-code>ISO_15924_NUM</atold:op-code>
      <dc:identifier>ISO_15924_NUM</dc:identifier>
      <skos:altLabel xml:lang="en">ISO 15924 numeric code</skos:altLabel>
      <skos:definition xml:lang="en">ISO 15924 numeric codes are three-digit script codes defined in ISO 15924 standard published by the International Organization for Standardization (ISO), to represent names of scripts. Script is defined as ‘set of graphic characters used for the written form of one or more languages’.</skos:definition>
      <skos:inScheme rdf:resource="http://publications.europa.eu/resource/authority/notation-type"/>
      <skos:topConceptOf rdf:resource="http://publications.europa.eu/resource/authority/notation-type"/>
      <at:op-mapped-code>
         <at:MappedCode>
            <dc:source>MDR</dc:source>
            <at:affected-table>notation-type</at:affected-table>
            <at:legacy-code>iso-15924-num</at:legacy-code>
         </at:MappedCode>
      </at:op-mapped-code>
   </skos:Concept>
   <skos:Concept rdf:about="http://publications.europa.eu/resource/authority/notation-type/ISO_3166_1_ALPHA_2"
                 at:deprecated="false">
      <skos:prefLabel xml:lang="en">ISO 3166-1 α-2</skos:prefLabel>
      <skos:prefLabel xml:lang="et">ISO 3166-1 α-2</skos:prefLabel>
      <at:authority-code>ISO_3166_1_ALPHA_2</at:authority-code>
      <at:op-code>ISO_3166_1_ALPHA_2</at:op-code>
      <at:start.use>1997-01-01</at:start.use>
      <atold:op-code>ISO_3166_1_ALPHA_2</atold:op-code>
      <dc:identifier>ISO_3166_1_ALPHA_2</dc:identifier>
      <skos:altLabel xml:lang="en">ISO 3166-1 alpha-2 code</skos:altLabel>
      <skos:definition xml:lang="en">ISO 3166-1 alpha-2 codes are two-letter country codes defined in ISO 3166-1, part of the ISO 3166 standard published by the International Organization for Standardization (ISO), to represent countries, dependent territories, and special areas of geographical interest.</skos:definition>
      <skos:inScheme rdf:resource="http://publications.europa.eu/resource/authority/notation-type"/>
      <skos:topConceptOf rdf:resource="http://publications.europa.eu/resource/authority/notation-type"/>
      <at:op-mapped-code>
         <at:MappedCode>
            <dc:source>MDR</dc:source>
            <at:affected-table>notation-type</at:affected-table>
            <at:legacy-code>code-3166-1-alpha-2</at:legacy-code>
         </at:MappedCode>
      </at:op-mapped-code>
   </skos:Concept>
   <skos:Concept rdf:about="http://publications.europa.eu/resource/authority/notation-type/ISO_3166_1_ALPHA_3"
                 at:deprecated="false">
      <skos:prefLabel xml:lang="en">ISO 3166-1 α-3</skos:prefLabel>
      <skos:prefLabel xml:lang="et">ISO 3166-1 α-3</skos:prefLabel>
      <at:authority-code>ISO_3166_1_ALPHA_3</at:authority-code>
      <at:op-code>ISO_3166_1_ALPHA_3</at:op-code>
      <at:start.use>1997-01-01</at:start.use>
      <atold:op-code>ISO_3166_1_ALPHA_3</atold:op-code>
      <dc:identifier>ISO_3166_1_ALPHA_3</dc:identifier>
      <skos:altLabel xml:lang="en">ISO 3166-1 alpha-3 code</skos:altLabel>
      <skos:definition xml:lang="en">ISO 3166-1 alpha-3 codes are three-letter country codes defined in ISO 3166-1, part of the ISO 3166 standard published by the International Organization for Standardization (ISO), to represent countries, dependent territories, and special areas of geographical interest.</skos:definition>
      <skos:inScheme rdf:resource="http://publications.europa.eu/resource/authority/notation-type"/>
      <skos:topConceptOf rdf:resource="http://publications.europa.eu/resource/authority/notation-type"/>
      <at:op-mapped-code>
         <at:MappedCode>
            <dc:source>MDR</dc:source>
            <at:affected-table>notation-type</at:affected-table>
            <at:legacy-code>code-3166-1-alpha-3</at:legacy-code>
         </at:MappedCode>
      </at:op-mapped-code>
   </skos:Concept>
   <skos:Concept rdf:about="http://publications.europa.eu/resource/authority/notation-type/ISO_3166_1_NUM"
                 at:deprecated="false">
      <skos:prefLabel xml:lang="en">ISO 3166-1 num</skos:prefLabel>
      <skos:prefLabel xml:lang="et">ISO 3166-1 num</skos:prefLabel>
      <at:authority-code>ISO_3166_1_NUM</at:authority-code>
      <at:op-code>ISO_3166_1_NUM</at:op-code>
      <at:start.use>1981-01-01</at:start.use>
      <atold:op-code>ISO_3166_1_NUM</atold:op-code>
      <dc:identifier>ISO_3166_1_NUM</dc:identifier>
      <skos:altLabel xml:lang="en">ISO 3166-1 numeric code</skos:altLabel>
      <skos:definition xml:lang="en">ISO 3166-1 numeric (or numeric-3) codes are three-digit country codes defined in ISO 3166-1, part of the ISO 3166 standard published by the International Organization for Standardization (ISO), to represent countries, dependent territories, and special areas of geographical interest. They are similar to the three-digit country codes developed and maintained by the United Nations Statistics Division, from which they originate in its UN M.49 standard.</skos:definition>
      <skos:inScheme rdf:resource="http://publications.europa.eu/resource/authority/notation-type"/>
      <skos:topConceptOf rdf:resource="http://publications.europa.eu/resource/authority/notation-type"/>
      <at:op-mapped-code>
         <at:MappedCode>
            <dc:source>MDR</dc:source>
            <at:affected-table>notation-type</at:affected-table>
            <at:legacy-code>code-3166-1-num</at:legacy-code>
         </at:MappedCode>
      </at:op-mapped-code>
   </skos:Concept>
   <skos:Concept rdf:about="http://publications.europa.eu/resource/authority/notation-type/ISO_3166_2"
                 at:deprecated="false">
      <skos:prefLabel xml:lang="en">ISO 3166-2</skos:prefLabel>
      <skos:prefLabel xml:lang="et">ISO 3166-2</skos:prefLabel>
      <at:authority-code>ISO_3166_2</at:authority-code>
      <at:op-code>ISO_3166_2</at:op-code>
      <at:start.use>1998-01-01</at:start.use>
      <atold:op-code>ISO_3166_2</atold:op-code>
      <dc:identifier>ISO_3166_2</dc:identifier>
      <skos:altLabel xml:lang="en">ISO 3166-2 code</skos:altLabel>
      <skos:definition xml:lang="en">ISO 3166-2 codes identify the principal subdivisions (e.g. provinces or states) of all countries coded in ISO 3166-1.</skos:definition>
      <skos:inScheme rdf:resource="http://publications.europa.eu/resource/authority/notation-type"/>
      <skos:topConceptOf rdf:resource="http://publications.europa.eu/resource/authority/notation-type"/>
      <at:op-mapped-code>
         <at:MappedCode>
            <dc:source>MDR</dc:source>
            <at:affected-table>notation-type</at:affected-table>
            <at:legacy-code>code-3166-2</at:legacy-code>
         </at:MappedCode>
      </at:op-mapped-code>
   </skos:Concept>
   <skos:Concept rdf:about="http://publications.europa.eu/resource/authority/notation-type/ISO_3166_3"
                 at:deprecated="false">
      <skos:prefLabel xml:lang="en">ISO 3166-3</skos:prefLabel>
      <skos:prefLabel xml:lang="et">ISO 3166-3</skos:prefLabel>
      <at:authority-code>ISO_3166_3</at:authority-code>
      <at:op-code>ISO_3166_3</at:op-code>
      <at:start.use>1999-01-01</at:start.use>
      <atold:op-code>ISO_3166_3</atold:op-code>
      <dc:identifier>ISO_3166_3</dc:identifier>
      <skos:altLabel xml:lang="en">ISO 3166-3 code</skos:altLabel>
      <skos:definition xml:lang="en">ISO 3166-3 is part of the ISO 3166 standard published by the International Organization for Standardization (ISO), and defines codes for country names which have been deleted from ISO 3166-1. Each former country name in ISO 3166-3 is assigned a four-letter alphabetic code.</skos:definition>
      <skos:inScheme rdf:resource="http://publications.europa.eu/resource/authority/notation-type"/>
      <skos:topConceptOf rdf:resource="http://publications.europa.eu/resource/authority/notation-type"/>
      <at:op-mapped-code>
         <at:MappedCode>
            <dc:source>MDR</dc:source>
            <at:affected-table>notation-type</at:affected-table>
            <at:legacy-code>code-3166-3</at:legacy-code>
         </at:MappedCode>
      </at:op-mapped-code>
   </skos:Concept>
   <skos:Concept rdf:about="http://publications.europa.eu/resource/authority/notation-type/ISO_4217"
                 at:deprecated="false">
      <skos:prefLabel xml:lang="en">ISO 4217</skos:prefLabel>
      <skos:prefLabel xml:lang="et">ISO 4217</skos:prefLabel>
      <at:authority-code>ISO_4217</at:authority-code>
      <at:op-code>ISO_4217</at:op-code>
      <at:start.use>1978-02-01</at:start.use>
      <atold:op-code>ISO_4217</atold:op-code>
      <dc:identifier>ISO_4217</dc:identifier>
      <skos:altLabel xml:lang="en">ISO 4217 code</skos:altLabel>
      <skos:definition xml:lang="en">ISO 4217 codes are used for the identification of currencies and funds organised in the following lists: current currency and funds code, current funds codes, codes for historic denominations of currencies and funds.</skos:definition>
      <skos:inScheme rdf:resource="http://publications.europa.eu/resource/authority/notation-type"/>
      <skos:topConceptOf rdf:resource="http://publications.europa.eu/resource/authority/notation-type"/>
      <at:op-mapped-code>
         <at:MappedCode>
            <dc:source>MDR</dc:source>
            <at:affected-table>notation-type</at:affected-table>
            <at:legacy-code>code-4217</at:legacy-code>
         </at:MappedCode>
      </at:op-mapped-code>
   </skos:Concept>
   <skos:Concept rdf:about="http://publications.europa.eu/resource/authority/notation-type/ISO_4217_NUM"
                 at:deprecated="false">
      <skos:prefLabel xml:lang="en">ISO 4217 num</skos:prefLabel>
      <skos:prefLabel xml:lang="et">ISO 4217 num</skos:prefLabel>
      <at:authority-code>ISO_4217_NUM</at:authority-code>
      <at:op-code>ISO_4217_NUM</at:op-code>
      <at:start.use>1978-02-01</at:start.use>
      <atold:op-code>ISO_4217_NUM</atold:op-code>
      <dc:identifier>ISO_4217_NUM</dc:identifier>
      <skos:altLabel xml:lang="en">ISO 4217 numeric code</skos:altLabel>
      <skos:definition xml:lang="en">ISO 4217 numeric codes are three-digit currency codes defined in ISO 4217 standard published by the International Organization for Standardization (ISO), to represent currencies and funds.</skos:definition>
      <skos:inScheme rdf:resource="http://publications.europa.eu/resource/authority/notation-type"/>
      <skos:topConceptOf rdf:resource="http://publications.europa.eu/resource/authority/notation-type"/>
   </skos:Concept>
   <skos:Concept rdf:about="http://publications.europa.eu/resource/authority/notation-type/ISO_5218_2"
                 at:deprecated="false">
      <skos:prefLabel xml:lang="en">ISO 5218-2</skos:prefLabel>
      <skos:prefLabel xml:lang="et">ISO 5218-2</skos:prefLabel>
      <at:authority-code>ISO_5218_2</at:authority-code>
      <at:op-code>ISO_5218_2</at:op-code>
      <at:start.use>1976-11-01</at:start.use>
      <atold:op-code>ISO_5218_2</atold:op-code>
      <dc:identifier>ISO_5218_2</dc:identifier>
      <skos:altLabel xml:lang="en">ISO 5218-2 code</skos:altLabel>
      <skos:definition xml:lang="en">ISO 5218-2 codes define a representation of human sexes through a language-neutral single-digit code.</skos:definition>
      <skos:inScheme rdf:resource="http://publications.europa.eu/resource/authority/notation-type"/>
      <skos:topConceptOf rdf:resource="http://publications.europa.eu/resource/authority/notation-type"/>
      <at:op-mapped-code>
         <at:MappedCode>
            <dc:source>MDR</dc:source>
            <at:affected-table>notation-type</at:affected-table>
            <at:legacy-code>code-5218-2</at:legacy-code>
         </at:MappedCode>
      </at:op-mapped-code>
   </skos:Concept>
   <skos:Concept rdf:about="http://publications.europa.eu/resource/authority/notation-type/ISO_639_1"
                 at:deprecated="false">
      <skos:prefLabel xml:lang="en">ISO 639-1</skos:prefLabel>
      <skos:prefLabel xml:lang="et">ISO 639-1</skos:prefLabel>
      <at:authority-code>ISO_639_1</at:authority-code>
      <at:op-code>ISO_639_1</at:op-code>
      <at:start.use>1967-01-01</at:start.use>
      <atold:op-code>ISO_639_1</atold:op-code>
      <dc:identifier>ISO_639_1</dc:identifier>
      <skos:altLabel xml:lang="en">ISO 639-1 code</skos:altLabel>
      <skos:definition xml:lang="en">A two-letter code that has been designed to represent most of the major languages of the world.</skos:definition>
      <skos:inScheme rdf:resource="http://publications.europa.eu/resource/authority/notation-type"/>
      <skos:topConceptOf rdf:resource="http://publications.europa.eu/resource/authority/notation-type"/>
      <at:op-mapped-code>
         <at:MappedCode>
            <dc:source>MDR</dc:source>
            <at:affected-table>notation-type</at:affected-table>
            <at:legacy-code>iso-639-1</at:legacy-code>
         </at:MappedCode>
      </at:op-mapped-code>
   </skos:Concept>
   <skos:Concept rdf:about="http://publications.europa.eu/resource/authority/notation-type/ISO_639_2B"
                 at:deprecated="false">
      <skos:prefLabel xml:lang="en">ISO 639-2 b</skos:prefLabel>
      <skos:prefLabel xml:lang="et">ISO 639-2 b</skos:prefLabel>
      <at:authority-code>ISO_639_2B</at:authority-code>
      <at:op-code>ISO_639_2B</at:op-code>
      <at:start.use>1989-01-01</at:start.use>
      <atold:op-code>ISO_639_2B</atold:op-code>
      <dc:identifier>ISO_639_2B</dc:identifier>
      <skos:altLabel xml:lang="en">ISO 639-2 – bibliographic code</skos:altLabel>
      <skos:definition xml:lang="en">A three-letter code which is derived from the English name for the language and gives more possible combinations, so ISO 639-2:1998 can cover more languages.</skos:definition>
      <skos:inScheme rdf:resource="http://publications.europa.eu/resource/authority/notation-type"/>
      <skos:topConceptOf rdf:resource="http://publications.europa.eu/resource/authority/notation-type"/>
      <at:op-mapped-code>
         <at:MappedCode>
            <dc:source>MDR</dc:source>
            <at:affected-table>notation-type</at:affected-table>
            <at:legacy-code>iso-639-2b</at:legacy-code>
         </at:MappedCode>
      </at:op-mapped-code>
   </skos:Concept>
   <skos:Concept rdf:about="http://publications.europa.eu/resource/authority/notation-type/ISO_639_2T"
                 at:deprecated="false">
      <skos:prefLabel xml:lang="en">ISO 639-2 t</skos:prefLabel>
      <skos:prefLabel xml:lang="et">ISO 639-2 t</skos:prefLabel>
      <at:authority-code>ISO_639_2T</at:authority-code>
      <at:op-code>ISO_639_2T</at:op-code>
      <at:start.use>1989-01-01</at:start.use>
      <atold:op-code>ISO_639_2T</atold:op-code>
      <dc:identifier>ISO_639_2T</dc:identifier>
      <skos:altLabel xml:lang="en">ISO 639-2 – terminological code</skos:altLabel>
      <skos:definition xml:lang="en">A three-letter code which is derived from the native name for the language and resembles the language's two-letter code in ISO 639-1 and which gives more possible combinations, so ISO 639-2:1998 can cover more languages.</skos:definition>
      <skos:inScheme rdf:resource="http://publications.europa.eu/resource/authority/notation-type"/>
      <skos:topConceptOf rdf:resource="http://publications.europa.eu/resource/authority/notation-type"/>
      <at:op-mapped-code>
         <at:MappedCode>
            <dc:source>MDR</dc:source>
            <at:affected-table>notation-type</at:affected-table>
            <at:legacy-code>iso-639-2t</at:legacy-code>
         </at:MappedCode>
      </at:op-mapped-code>
   </skos:Concept>
   <skos:Concept rdf:about="http://publications.europa.eu/resource/authority/notation-type/ISO_639_3"
                 at:deprecated="false">
      <skos:prefLabel xml:lang="en">ISO 639-3</skos:prefLabel>
      <skos:prefLabel xml:lang="et">ISO 639-3</skos:prefLabel>
      <at:authority-code>ISO_639_3</at:authority-code>
      <at:op-code>ISO_639_3</at:op-code>
      <at:start.use>2007-02-01</at:start.use>
      <atold:op-code>ISO_639_3</atold:op-code>
      <dc:identifier>ISO_639_3</dc:identifier>
      <skos:altLabel xml:lang="en">ISO 639-3 code</skos:altLabel>
      <skos:definition xml:lang="en">A three-letter code which aims to give as complete a listing of languages as possible, including living, extinct and ancient languages.</skos:definition>
      <skos:inScheme rdf:resource="http://publications.europa.eu/resource/authority/notation-type"/>
      <skos:topConceptOf rdf:resource="http://publications.europa.eu/resource/authority/notation-type"/>
      <at:op-mapped-code>
         <at:MappedCode>
            <dc:source>MDR</dc:source>
            <at:affected-table>notation-type</at:affected-table>
            <at:legacy-code>iso-639-3</at:legacy-code>
         </at:MappedCode>
      </at:op-mapped-code>
   </skos:Concept>
   <skos:Concept rdf:about="http://publications.europa.eu/resource/authority/notation-type/ISSN"
                 at:deprecated="false">
      <skos:prefLabel xml:lang="en">ISSN</skos:prefLabel>
      <skos:prefLabel xml:lang="et">ISSN</skos:prefLabel>
      <at:authority-code>ISSN</at:authority-code>
      <at:op-code>ISSN</at:op-code>
      <at:start.use>1975-01-01</at:start.use>
      <atold:op-code>ISSN</atold:op-code>
      <dc:identifier>ISSN</dc:identifier>
      <skos:altLabel xml:lang="en">International Standard Serial Number</skos:altLabel>
      <skos:definition xml:lang="en">Eight-digit number which identifies all periodical publications as such, including electronic serials. Each ISSN assigned to a serial publication is registered in an international database: the ISSN Register. It is the most comprehensive and authoritative source for the identification of serial publications world-wide.</skos:definition>
      <skos:inScheme rdf:resource="http://publications.europa.eu/resource/authority/notation-type"/>
      <skos:topConceptOf rdf:resource="http://publications.europa.eu/resource/authority/notation-type"/>
      <skos:exactMatch rdf:resource="http://purl.org/spar/datacite/issn"/>
   </skos:Concept>
   <skos:Concept rdf:about="http://publications.europa.eu/resource/authority/notation-type/ISSN_L"
                 at:deprecated="false">
      <skos:prefLabel xml:lang="en">ISSN-L</skos:prefLabel>
      <skos:prefLabel xml:lang="et">ISSN-L</skos:prefLabel>
      <at:authority-code>ISSN_L</at:authority-code>
      <at:op-code>ISSN_L</at:op-code>
      <at:start.use>2007-12-31</at:start.use>
      <atold:op-code>ISSN_L</atold:op-code>
      <dc:identifier>ISSN_L</dc:identifier>
      <skos:altLabel xml:lang="en">Linking ISSN</skos:altLabel>
      <skos:definition xml:lang="en">The linking ISSN (ISSN-L) is a specific ISSN that groups the different media of the same serial publication. A single ISSN-L is designated for all media of a serial publication, irrespective of how many there are.</skos:definition>
      <skos:inScheme rdf:resource="http://publications.europa.eu/resource/authority/notation-type"/>
      <skos:topConceptOf rdf:resource="http://publications.europa.eu/resource/authority/notation-type"/>
      <skos:exactMatch rdf:resource="http://purl.org/spar/datacite/lissn"/>
   </skos:Concept>
   <skos:Concept rdf:about="http://publications.europa.eu/resource/authority/notation-type/ISTC"
                 at:deprecated="false">
      <skos:prefLabel xml:lang="en">ISTC</skos:prefLabel>
      <skos:prefLabel xml:lang="et">ISTC</skos:prefLabel>
      <at:authority-code>ISTC</at:authority-code>
      <at:op-code>ISTC</at:op-code>
      <at:start.use>2009-03-01</at:start.use>
      <atold:op-code>ISTC</atold:op-code>
      <dc:identifier>ISTC</dc:identifier>
      <skos:altLabel xml:lang="en">International Standard Text Code</skos:altLabel>
      <skos:definition xml:lang="en">ISTC is a numbering system for the unique identification of text-based works; the term “work” can refer to any content appearing in conventional printed books, audio-books, static e-books or enhanced digital books, as well as content which might appear in a newspaper or journal.</skos:definition>
      <skos:inScheme rdf:resource="http://publications.europa.eu/resource/authority/notation-type"/>
      <skos:topConceptOf rdf:resource="http://publications.europa.eu/resource/authority/notation-type"/>
      <skos:exactMatch rdf:resource="http://purl.org/spar/datacite/istc"/>
   </skos:Concept>
   <skos:Concept rdf:about="http://publications.europa.eu/resource/authority/notation-type/LAC"
                 at:deprecated="false">
      <skos:prefLabel xml:lang="en">Legacy code</skos:prefLabel>
      <skos:prefLabel xml:lang="et">Aegunud kood (legacy)</skos:prefLabel>
      <at:authority-code>LAC</at:authority-code>
      <at:op-code>LAC</at:op-code>
      <at:start.use>1958-01-01</at:start.use>
      <atold:op-code>LAC</atold:op-code>
      <dc:identifier>LAC</dc:identifier>
      <skos:altLabel xml:lang="en">Legacy authority code</skos:altLabel>
      <skos:definition xml:lang="en">This concept identifies the mnemonic denotation of a concept used in authority tables.</skos:definition>
      <skos:inScheme rdf:resource="http://publications.europa.eu/resource/authority/notation-type"/>
      <skos:topConceptOf rdf:resource="http://publications.europa.eu/resource/authority/notation-type"/>
   </skos:Concept>
   <skos:Concept rdf:about="http://publications.europa.eu/resource/authority/notation-type/LITIGE"
                 at:deprecated="false">
      <skos:prefLabel xml:lang="en">Litige</skos:prefLabel>
      <skos:prefLabel xml:lang="et">Litige</skos:prefLabel>
      <at:authority-code>LITIGE</at:authority-code>
      <at:op-code>LITIGE</at:op-code>
      <at:start.use>1998-11-12</at:start.use>
      <atold:op-code>LITIGE</atold:op-code>
      <dc:identifier>LITIGE</dc:identifier>
      <skos:altLabel xml:lang="en">Litige code</skos:altLabel>
      <skos:definition xml:lang="en">Code used in the system Litige of the Court of Justice.</skos:definition>
      <skos:inScheme rdf:resource="http://publications.europa.eu/resource/authority/notation-type"/>
      <skos:topConceptOf rdf:resource="http://publications.europa.eu/resource/authority/notation-type"/>
   </skos:Concept>
   <skos:Concept rdf:about="http://publications.europa.eu/resource/authority/notation-type/LRIS"
                 at:deprecated="false">
      <skos:prefLabel xml:lang="en">LRIS</skos:prefLabel>
      <skos:prefLabel xml:lang="et">LRIS</skos:prefLabel>
      <at:authority-code>LRIS</at:authority-code>
      <at:op-code>LRIS</at:op-code>
      <at:start.use>2012-12-31</at:start.use>
      <atold:op-code>LRIS</atold:op-code>
      <dc:identifier>LRIS</dc:identifier>
      <skos:altLabel xml:lang="en">Local Resource Identifier</skos:altLabel>
      <skos:definition xml:lang="en">The Local Resource Identifier is generated by the resource identifier scheme that provides local resource identifiers that are unique in their local environment and understood by the person submitting the metadata.</skos:definition>
      <skos:inScheme rdf:resource="http://publications.europa.eu/resource/authority/notation-type"/>
      <skos:topConceptOf rdf:resource="http://publications.europa.eu/resource/authority/notation-type"/>
      <skos:exactMatch rdf:resource="http://purl.org/spar/datacite/local-resource-identifier-scheme"/>
   </skos:Concept>
   <skos:Concept rdf:about="http://publications.europa.eu/resource/authority/notation-type/LSID"
                 at:deprecated="false">
      <skos:prefLabel xml:lang="en">LSID</skos:prefLabel>
      <skos:prefLabel xml:lang="et">LSID</skos:prefLabel>
      <at:authority-code>LSID</at:authority-code>
      <at:op-code>LSID</at:op-code>
      <at:start.use>2003-09-30</at:start.use>
      <atold:op-code>LSID</atold:op-code>
      <dc:identifier>LSID</dc:identifier>
      <skos:altLabel xml:lang="en">Life Science Identifier</skos:altLabel>
      <skos:definition xml:lang="en">The Life Sciences Identifier (LSID) is a persistent, location-independent, globally unique identifier for biological objects in the life sciences domain specified by OMG Life Sciences Research. LSID is represented as a Uniform Resource Name (URN).</skos:definition>
      <skos:inScheme rdf:resource="http://publications.europa.eu/resource/authority/notation-type"/>
      <skos:topConceptOf rdf:resource="http://publications.europa.eu/resource/authority/notation-type"/>
      <skos:exactMatch rdf:resource="http://purl.org/spar/datacite/lsid"/>
   </skos:Concept>
   <skos:Concept rdf:about="http://publications.europa.eu/resource/authority/notation-type/MINIDOC"
                 at:deprecated="false">
      <skos:prefLabel xml:lang="en">Minidoc</skos:prefLabel>
      <skos:prefLabel xml:lang="et">Minidoc</skos:prefLabel>
      <at:authority-code>MINIDOC</at:authority-code>
      <at:op-code>MINIDOC</at:op-code>
      <at:start.use>1952-07-24</at:start.use>
      <atold:op-code>MINIDOC</atold:op-code>
      <dc:identifier>MINIDOC</dc:identifier>
      <skos:altLabel xml:lang="en">Minidoc code</skos:altLabel>
      <skos:definition xml:lang="en">Code used in the system Minidoc of the Court of Justice.</skos:definition>
      <skos:inScheme rdf:resource="http://publications.europa.eu/resource/authority/notation-type"/>
      <skos:topConceptOf rdf:resource="http://publications.europa.eu/resource/authority/notation-type"/>
   </skos:Concept>
   <skos:Concept rdf:about="http://publications.europa.eu/resource/authority/notation-type/MNE"
                 at:deprecated="false">
      <skos:prefLabel xml:lang="en">MNE</skos:prefLabel>
      <skos:prefLabel xml:lang="et">MNE</skos:prefLabel>
      <at:authority-code>MNE</at:authority-code>
      <at:op-code>MNE</at:op-code>
      <at:start.use>1969-01-18</at:start.use>
      <atold:op-code>MNE</atold:op-code>
      <dc:identifier>MNE</dc:identifier>
      <skos:altLabel xml:lang="en">MNE code</skos:altLabel>
      <skos:definition xml:lang="en">Code used by Procat for national transposing measures/mesures nationales de transposition.</skos:definition>
      <skos:inScheme rdf:resource="http://publications.europa.eu/resource/authority/notation-type"/>
      <skos:topConceptOf rdf:resource="http://publications.europa.eu/resource/authority/notation-type"/>
      <at:op-mapped-code>
         <at:MappedCode>
            <dc:source>MDR</dc:source>
            <at:affected-table>notation-type</at:affected-table>
            <at:legacy-code>VOLET_MNE</at:legacy-code>
         </at:MappedCode>
      </at:op-mapped-code>
   </skos:Concept>
   <skos:Concept rdf:about="http://publications.europa.eu/resource/authority/notation-type/NIHMSID"
                 at:deprecated="false">
      <skos:prefLabel xml:lang="en">NIHMSID</skos:prefLabel>
      <skos:prefLabel xml:lang="et">NIHMSID</skos:prefLabel>
      <at:authority-code>NIHMSID</at:authority-code>
      <at:op-code>NIHMSID</at:op-code>
      <at:start.use>2005-12-31</at:start.use>
      <atold:op-code>NIHMSID</atold:op-code>
      <dc:identifier>NIHMSID</dc:identifier>
      <skos:altLabel xml:lang="en">NIH Manuscript Submission Identifier</skos:altLabel>
      <skos:definition xml:lang="en">The NIHMSID is an ID used to identify publications which have been initially submitted into the NIH Manuscript Submission System for eventual deposit in PubMed Central. Once the web version of the publication is approved for inclusion in PMC and the corresponding citation is in PubMed, the article will also be assigned a PMCID.</skos:definition>
      <skos:inScheme rdf:resource="http://publications.europa.eu/resource/authority/notation-type"/>
      <skos:topConceptOf rdf:resource="http://publications.europa.eu/resource/authority/notation-type"/>
      <skos:exactMatch rdf:resource="http://purl.org/spar/datacite/nihmsid"/>
   </skos:Concept>
   <skos:Concept rdf:about="http://publications.europa.eu/resource/authority/notation-type/OCI"
                 at:deprecated="false">
      <skos:prefLabel xml:lang="en">OCI</skos:prefLabel>
      <skos:prefLabel xml:lang="et">OCI</skos:prefLabel>
      <at:authority-code>OCI</at:authority-code>
      <at:op-code>OCI</at:op-code>
      <at:start.use>2015-12-31</at:start.use>
      <atold:op-code>OCI</atold:op-code>
      <dc:identifier>OCI</dc:identifier>
      <skos:altLabel xml:lang="en">Open Citation Identifier</skos:altLabel>
      <skos:definition xml:lang="en">The Open Citation Identifier (OCI) is a globally unique persistent identifier for bibliographic citations. Within the OpenCitations Corpus, these bibliographic resource identifiers are unique, and every citation recorded in OCC has an OCI.</skos:definition>
      <skos:inScheme rdf:resource="http://publications.europa.eu/resource/authority/notation-type"/>
      <skos:topConceptOf rdf:resource="http://publications.europa.eu/resource/authority/notation-type"/>
      <skos:exactMatch rdf:resource="http://purl.org/spar/datacite/oci"/>
   </skos:Concept>
   <skos:Concept rdf:about="http://publications.europa.eu/resource/authority/notation-type/ODP"
                 at:deprecated="false">
      <skos:prefLabel xml:lang="en">ODP</skos:prefLabel>
      <skos:prefLabel xml:lang="et">ODP</skos:prefLabel>
      <at:authority-code>ODP</at:authority-code>
      <at:op-code>ODP</at:op-code>
      <at:start.use>2012-04-19</at:start.use>
      <atold:op-code>ODP</atold:op-code>
      <dc:identifier>ODP</dc:identifier>
      <skos:altLabel xml:lang="en">ODP code</skos:altLabel>
      <skos:definition xml:lang="en">Code used by the EU Open Data Portal which provides access to open public data produced by EU institutions, agencies and bodies.</skos:definition>
      <skos:inScheme rdf:resource="http://publications.europa.eu/resource/authority/notation-type"/>
      <skos:topConceptOf rdf:resource="http://publications.europa.eu/resource/authority/notation-type"/>
   </skos:Concept>
   <skos:Concept rdf:about="http://publications.europa.eu/resource/authority/notation-type/OJ"
                 at:deprecated="false">
      <skos:prefLabel xml:lang="en">OJ id</skos:prefLabel>
      <skos:prefLabel xml:lang="et">OJ id</skos:prefLabel>
      <at:authority-code>OJ</at:authority-code>
      <at:op-code>OJ</at:op-code>
      <at:start.use>1952-12-30</at:start.use>
      <atold:op-code>OJ</atold:op-code>
      <dc:identifier>OJ</dc:identifier>
      <skos:altLabel xml:lang="en">OJ code</skos:altLabel>
      <skos:definition xml:lang="en">Code used in the Official Journal.</skos:definition>
      <skos:inScheme rdf:resource="http://publications.europa.eu/resource/authority/notation-type"/>
      <skos:topConceptOf rdf:resource="http://publications.europa.eu/resource/authority/notation-type"/>
   </skos:Concept>
   <skos:Concept rdf:about="http://publications.europa.eu/resource/authority/notation-type/OJ_SECTION"
                 at:deprecated="false">
      <skos:prefLabel xml:lang="en">OJ section</skos:prefLabel>
      <skos:prefLabel xml:lang="et">OJ osa</skos:prefLabel>
      <at:authority-code>OJ_SECTION</at:authority-code>
      <at:op-code>OJ_SECTION</at:op-code>
      <at:start.use>1952-12-30</at:start.use>
      <atold:op-code>OJ_SECTION</atold:op-code>
      <dc:identifier>OJ_SECTION</dc:identifier>
      <skos:altLabel xml:lang="en">OJ section code</skos:altLabel>
      <skos:definition xml:lang="en">Code used to identify the section of the OJ.</skos:definition>
      <skos:inScheme rdf:resource="http://publications.europa.eu/resource/authority/notation-type"/>
      <skos:topConceptOf rdf:resource="http://publications.europa.eu/resource/authority/notation-type"/>
      <at:op-mapped-code>
         <at:MappedCode>
            <dc:source>MDR</dc:source>
            <at:affected-table>notation-type</at:affected-table>
            <at:legacy-code>oj.section</at:legacy-code>
         </at:MappedCode>
      </at:op-mapped-code>
   </skos:Concept>
   <skos:Concept rdf:about="http://publications.europa.eu/resource/authority/notation-type/ONIX"
                 at:deprecated="false">
      <skos:prefLabel xml:lang="en">ONIX</skos:prefLabel>
      <skos:prefLabel xml:lang="et">ONIX</skos:prefLabel>
      <at:authority-code>ONIX</at:authority-code>
      <at:op-code>ONIX</at:op-code>
      <at:start.use>2000-01-01</at:start.use>
      <atold:op-code>ONIX</atold:op-code>
      <dc:identifier>ONIX</dc:identifier>
      <skos:altLabel xml:lang="en">ONIX code</skos:altLabel>
      <skos:definition xml:lang="en">Code value from ONIX for Books.</skos:definition>
      <skos:inScheme rdf:resource="http://publications.europa.eu/resource/authority/notation-type"/>
      <skos:topConceptOf rdf:resource="http://publications.europa.eu/resource/authority/notation-type"/>
   </skos:Concept>
   <skos:Concept rdf:about="http://publications.europa.eu/resource/authority/notation-type/OP_CAT"
                 at:deprecated="false">
      <skos:prefLabel xml:lang="en">OP cat</skos:prefLabel>
      <skos:prefLabel xml:lang="et">OP cat</skos:prefLabel>
      <at:authority-code>OP_CAT</at:authority-code>
      <at:op-code>OP_CAT</at:op-code>
      <at:start.use>1969-01-18</at:start.use>
      <atold:op-code>OP_CAT</atold:op-code>
      <dc:identifier>OP_CAT</dc:identifier>
      <skos:altLabel xml:lang="en">OP catalogue number</skos:altLabel>
      <skos:definition xml:lang="en">An internal identifier assigned to all works created by the Publications Office. It is used to categorise publications in catalogues, amongst other things. It is also used as an identification key in various IT applications, as is the case for EU Bookshop, the European institutions’ online bookshop.</skos:definition>
      <skos:inScheme rdf:resource="http://publications.europa.eu/resource/authority/notation-type"/>
      <skos:topConceptOf rdf:resource="http://publications.europa.eu/resource/authority/notation-type"/>
      <at:op-mapped-code>
         <at:MappedCode>
            <dc:source>MDR</dc:source>
            <at:affected-table>notation-type</at:affected-table>
            <at:legacy-code>cat.no</at:legacy-code>
         </at:MappedCode>
      </at:op-mapped-code>
      <at:op-mapped-code>
         <at:MappedCode>
            <dc:source>MDR</dc:source>
            <at:affected-table>notation-type</at:affected-table>
            <at:legacy-code>cat.no.old</at:legacy-code>
         </at:MappedCode>
      </at:op-mapped-code>
   </skos:Concept>
   <skos:Concept rdf:about="http://publications.europa.eu/resource/authority/notation-type/OP_DATPRO"
                 at:deprecated="false">
      <skos:prefLabel xml:lang="bg">НЕОКОНЧАТЕЛНИ ДАННИ</skos:prefLabel>
      <skos:prefLabel xml:lang="cs">Předběžné údaje</skos:prefLabel>
      <skos:prefLabel xml:lang="da">Midlertidige data</skos:prefLabel>
      <skos:prefLabel xml:lang="de">Vorläufige Daten</skos:prefLabel>
      <skos:prefLabel xml:lang="el">Προσωρινά δεδομένα</skos:prefLabel>
      <skos:prefLabel xml:lang="en">Provisional data</skos:prefLabel>
      <skos:prefLabel xml:lang="es">Datos provisionales</skos:prefLabel>
      <skos:prefLabel xml:lang="et">Esialgsed andmed</skos:prefLabel>
      <skos:prefLabel xml:lang="fi">Alustavat tiedot</skos:prefLabel>
      <skos:prefLabel xml:lang="fr">Données provisoires</skos:prefLabel>
      <skos:prefLabel xml:lang="ga">Sonraí sealadacha</skos:prefLabel>
      <skos:prefLabel xml:lang="hr">Privremeni podaci</skos:prefLabel>
      <skos:prefLabel xml:lang="hu">Ideiglenes adatok</skos:prefLabel>
      <skos:prefLabel xml:lang="it">Dati provvisori</skos:prefLabel>
      <skos:prefLabel xml:lang="lt">Laikinieji duomenys</skos:prefLabel>
      <skos:prefLabel xml:lang="lv">Provizoriski dati</skos:prefLabel>
      <skos:prefLabel xml:lang="mt">Dejta provviżorja</skos:prefLabel>
      <skos:prefLabel xml:lang="nl">Voorlopige gegevens</skos:prefLabel>
      <skos:prefLabel xml:lang="pl">Dane tymczasowe</skos:prefLabel>
      <skos:prefLabel xml:lang="pt">Dados provisórios</skos:prefLabel>
      <skos:prefLabel xml:lang="ro">Date provizorii</skos:prefLabel>
      <skos:prefLabel xml:lang="sk">Predbežné údaje</skos:prefLabel>
      <skos:prefLabel xml:lang="sl">Začasni podatki</skos:prefLabel>
      <skos:prefLabel xml:lang="sv">Tillfälliga uppgifter</skos:prefLabel>
      <at:authority-code>OP_DATPRO</at:authority-code>
      <at:op-code>OP_DATPRO</at:op-code>
      <at:start.use>1952-07-23</at:start.use>
      <atold:op-code>OP_DATPRO</atold:op-code>
      <dc:identifier>OP_DATPRO</dc:identifier>
      <skos:inScheme rdf:resource="http://publications.europa.eu/resource/authority/notation-type"/>
      <skos:topConceptOf rdf:resource="http://publications.europa.eu/resource/authority/notation-type"/>
   </skos:Concept>
   <skos:Concept rdf:about="http://publications.europa.eu/resource/authority/notation-type/ORCID"
                 at:deprecated="false">
      <skos:prefLabel xml:lang="en">ORCID</skos:prefLabel>
      <skos:prefLabel xml:lang="et">ORCID</skos:prefLabel>
      <at:authority-code>ORCID</at:authority-code>
      <at:op-code>ORCID</at:op-code>
      <at:start.use>2012-10-16</at:start.use>
      <atold:op-code>ORCID</atold:op-code>
      <dc:identifier>ORCID</dc:identifier>
      <skos:altLabel xml:lang="en">ORCID identifier</skos:altLabel>
      <skos:definition xml:lang="en">ORCID is a non-proprietary persistent digital identifier that uniquely identifies researchers.</skos:definition>
      <skos:inScheme rdf:resource="http://publications.europa.eu/resource/authority/notation-type"/>
      <skos:topConceptOf rdf:resource="http://publications.europa.eu/resource/authority/notation-type"/>
      <skos:exactMatch rdf:resource="http://purl.org/spar/datacite/orcid"/>
   </skos:Concept>
   <skos:Concept rdf:about="http://publications.europa.eu/resource/authority/notation-type/PEGASE"
                 at:deprecated="false">
      <skos:prefLabel xml:lang="en">Pégase</skos:prefLabel>
      <skos:prefLabel xml:lang="et">Pégase</skos:prefLabel>
      <at:authority-code>PEGASE</at:authority-code>
      <at:op-code>PEGASE</at:op-code>
      <at:start.use>2001-10-10</at:start.use>
      <atold:op-code>PEGASE</atold:op-code>
      <dc:identifier>PEGASE</dc:identifier>
      <skos:altLabel xml:lang="en">Pégase code</skos:altLabel>
      <skos:definition xml:lang="en">Code from Pégase, an application managed by the Secretariat-General of the European Commission which allows to encode the different information concerning the interinstitutional procedures with the aim to feed information systems such as SG Vista and Prelex.</skos:definition>
      <skos:inScheme rdf:resource="http://publications.europa.eu/resource/authority/notation-type"/>
      <skos:topConceptOf rdf:resource="http://publications.europa.eu/resource/authority/notation-type"/>
      <at:op-mapped-code>
         <at:MappedCode>
            <dc:source>MDR</dc:source>
            <at:affected-table>notation-type</at:affected-table>
            <at:legacy-code>Pegase</at:legacy-code>
         </at:MappedCode>
      </at:op-mapped-code>
   </skos:Concept>
   <skos:Concept rdf:about="http://publications.europa.eu/resource/authority/notation-type/PHONE_PREFIX"
                 at:deprecated="false">
      <skos:prefLabel xml:lang="en">Country calling code</skos:prefLabel>
      <at:authority-code>PHONE_PREFIX</at:authority-code>
      <at:op-code>PHONE_PREFIX</at:op-code>
      <at:start.use>2021-12-08</at:start.use>
      <atold:op-code>PHONE_PREFIX</atold:op-code>
      <dc:identifier>PHONE_PREFIX</dc:identifier>
      <skos:definition xml:lang="en">Country calling codes or country dial-in codes are telephone number prefixes for reaching telephone subscribers in the networks of the member countries or regions of the International Telecommunication Union (ITU). Country codes are a component of the international telephone numbering plan, and are necessary only when dialing a telephone number to establish a call to another country. Country codes are dialed before the national telephone number.</skos:definition>
      <skos:inScheme rdf:resource="http://publications.europa.eu/resource/authority/notation-type"/>
      <skos:topConceptOf rdf:resource="http://publications.europa.eu/resource/authority/notation-type"/>
   </skos:Concept>
   <skos:Concept rdf:about="http://publications.europa.eu/resource/authority/notation-type/PII"
                 at:deprecated="false">
      <skos:prefLabel xml:lang="en">PII</skos:prefLabel>
      <skos:prefLabel xml:lang="et">PII</skos:prefLabel>
      <at:authority-code>PII</at:authority-code>
      <at:op-code>PII</at:op-code>
      <at:start.use>1996-01-01</at:start.use>
      <atold:op-code>PII</atold:op-code>
      <dc:identifier>PII</dc:identifier>
      <skos:altLabel xml:lang="en">Publisher Item Identifier</skos:altLabel>
      <skos:definition xml:lang="en">The Publisher Item Identifier (PII) is an alphanumeric string of characters using a pre-existing ISSN or ISBN. It uniquely identifies an article and can be used for future cataloging, searching, and electronic retrieval.</skos:definition>
      <skos:inScheme rdf:resource="http://publications.europa.eu/resource/authority/notation-type"/>
      <skos:topConceptOf rdf:resource="http://publications.europa.eu/resource/authority/notation-type"/>
      <skos:exactMatch rdf:resource="http://purl.org/spar/datacite/pii"/>
   </skos:Concept>
   <skos:Concept rdf:about="http://publications.europa.eu/resource/authority/notation-type/PLANJO"
                 at:deprecated="false">
      <skos:prefLabel xml:lang="en">PlanJO</skos:prefLabel>
      <skos:prefLabel xml:lang="et">PlanJO</skos:prefLabel>
      <at:authority-code>PLANJO</at:authority-code>
      <at:op-code>PLANJO</at:op-code>
      <at:start.use>2002-04-25</at:start.use>
      <atold:op-code>PLANJO</atold:op-code>
      <dc:identifier>PLANJO</dc:identifier>
      <skos:altLabel xml:lang="en">PlanJO code</skos:altLabel>
      <skos:definition xml:lang="en">Code used by PlanJO, the internal workflow system used for the legal acts and documents published in the Official Journal L and C.</skos:definition>
      <skos:inScheme rdf:resource="http://publications.europa.eu/resource/authority/notation-type"/>
      <skos:topConceptOf rdf:resource="http://publications.europa.eu/resource/authority/notation-type"/>
      <at:op-mapped-code>
         <at:MappedCode>
            <dc:source>MDR</dc:source>
            <at:affected-table>notation-type</at:affected-table>
            <at:legacy-code>PLANJO_CODES</at:legacy-code>
         </at:MappedCode>
      </at:op-mapped-code>
   </skos:Concept>
   <skos:Concept rdf:about="http://publications.europa.eu/resource/authority/notation-type/PMCID"
                 at:deprecated="false">
      <skos:prefLabel xml:lang="en">PMCID</skos:prefLabel>
      <skos:prefLabel xml:lang="et">PMCID</skos:prefLabel>
      <at:authority-code>PMCID</at:authority-code>
      <at:op-code>PMCID</at:op-code>
      <at:start.use>2000-02-28</at:start.use>
      <atold:op-code>PMCID</atold:op-code>
      <dc:identifier>PMCID</dc:identifier>
      <skos:altLabel xml:lang="en">PubMed Central Identifier</skos:altLabel>
      <skos:definition xml:lang="en">The PMCID (PubMed Central Identifier), also known as the PMC reference number, is a bibliographic identifier assigned by the National Library of Medicine to each full-text paper in PubMed Central, a free archive of biomedical and life sciences journal literature.</skos:definition>
      <skos:inScheme rdf:resource="http://publications.europa.eu/resource/authority/notation-type"/>
      <skos:topConceptOf rdf:resource="http://publications.europa.eu/resource/authority/notation-type"/>
      <skos:exactMatch rdf:resource="http://purl.org/spar/datacite/pmcid"/>
   </skos:Concept>
   <skos:Concept rdf:about="http://publications.europa.eu/resource/authority/notation-type/PMID"
                 at:deprecated="false">
      <skos:prefLabel xml:lang="en">PMID</skos:prefLabel>
      <skos:prefLabel xml:lang="et">PMID</skos:prefLabel>
      <at:authority-code>PMID</at:authority-code>
      <at:op-code>PMID</at:op-code>
      <at:start.use>1996-12-31</at:start.use>
      <atold:op-code>PMID</atold:op-code>
      <dc:identifier>PMID</dc:identifier>
      <skos:altLabel xml:lang="en">PubMed Identifier</skos:altLabel>
      <skos:definition xml:lang="en">The PMID (PubMed Identifier or PubMed Unique Identifier) is a unique identifier number assigned to each article record entering PubMed, index of the biomedical literature. PMIDs are not reused after records are deleted.</skos:definition>
      <skos:inScheme rdf:resource="http://publications.europa.eu/resource/authority/notation-type"/>
      <skos:topConceptOf rdf:resource="http://publications.europa.eu/resource/authority/notation-type"/>
      <skos:exactMatch rdf:resource="http://purl.org/spar/datacite/pmid"/>
   </skos:Concept>
   <skos:Concept rdf:about="http://publications.europa.eu/resource/authority/notation-type/PUB_CORP"
                 at:deprecated="false">
      <skos:prefLabel xml:lang="en">PUB_CORP</skos:prefLabel>
      <skos:prefLabel xml:lang="et">PUB_CORP</skos:prefLabel>
      <at:authority-code>PUB_CORP</at:authority-code>
      <at:op-code>PUB_CORP</at:op-code>
      <at:start.use>2010-03-29</at:start.use>
      <atold:op-code>PUB_CORP</atold:op-code>
      <dc:identifier>PUB_CORP</dc:identifier>
      <skos:altLabel xml:lang="en">PUB_CORP code</skos:altLabel>
      <skos:definition xml:lang="en">Code used by PUB_CORP table of Publications domain in ATTO.</skos:definition>
      <skos:inScheme rdf:resource="http://publications.europa.eu/resource/authority/notation-type"/>
      <skos:topConceptOf rdf:resource="http://publications.europa.eu/resource/authority/notation-type"/>
   </skos:Concept>
   <skos:Concept rdf:about="http://publications.europa.eu/resource/authority/notation-type/PUB_DIV"
                 at:deprecated="false">
      <skos:prefLabel xml:lang="en">PUB_DIV</skos:prefLabel>
      <skos:prefLabel xml:lang="et">PUB_DIV</skos:prefLabel>
      <at:authority-code>PUB_DIV</at:authority-code>
      <at:op-code>PUB_DIV</at:op-code>
      <at:start.use>2010-03-29</at:start.use>
      <atold:op-code>PUB_DIV</atold:op-code>
      <dc:identifier>PUB_DIV</dc:identifier>
      <skos:altLabel xml:lang="en">PUB_DIV code</skos:altLabel>
      <skos:definition xml:lang="en">Code used by PUB_DIV of Publications domain in ATTO.</skos:definition>
      <skos:inScheme rdf:resource="http://publications.europa.eu/resource/authority/notation-type"/>
      <skos:topConceptOf rdf:resource="http://publications.europa.eu/resource/authority/notation-type"/>
   </skos:Concept>
   <skos:Concept rdf:about="http://publications.europa.eu/resource/authority/notation-type/PUB_FREQ"
                 at:deprecated="false">
      <skos:prefLabel xml:lang="en">PUB_FREQ</skos:prefLabel>
      <skos:prefLabel xml:lang="et">PUB_FREQ</skos:prefLabel>
      <at:authority-code>PUB_FREQ</at:authority-code>
      <at:op-code>PUB_FREQ</at:op-code>
      <at:start.use>2010-03-29</at:start.use>
      <atold:op-code>PUB_FREQ</atold:op-code>
      <dc:identifier>PUB_FREQ</dc:identifier>
      <skos:altLabel xml:lang="en">PUB_FREQ code</skos:altLabel>
      <skos:definition xml:lang="en">Code used by PUB_FREQ of Publications domain in ATTO.</skos:definition>
      <skos:inScheme rdf:resource="http://publications.europa.eu/resource/authority/notation-type"/>
      <skos:topConceptOf rdf:resource="http://publications.europa.eu/resource/authority/notation-type"/>
   </skos:Concept>
   <skos:Concept rdf:about="http://publications.europa.eu/resource/authority/notation-type/PUB_LANG"
                 at:deprecated="false">
      <skos:prefLabel xml:lang="en">PUB_LANG</skos:prefLabel>
      <skos:prefLabel xml:lang="et">PUB_LANG</skos:prefLabel>
      <at:authority-code>PUB_LANG</at:authority-code>
      <at:op-code>PUB_LANG</at:op-code>
      <at:start.use>2010-03-29</at:start.use>
      <atold:op-code>PUB_LANG</atold:op-code>
      <dc:identifier>PUB_LANG</dc:identifier>
      <skos:altLabel xml:lang="en">PUB_LANG code</skos:altLabel>
      <skos:definition xml:lang="en">Code used by PUB_LANG of Publications domain in ATTO.</skos:definition>
      <skos:inScheme rdf:resource="http://publications.europa.eu/resource/authority/notation-type"/>
      <skos:topConceptOf rdf:resource="http://publications.europa.eu/resource/authority/notation-type"/>
   </skos:Concept>
   <skos:Concept rdf:about="http://publications.europa.eu/resource/authority/notation-type/PUB_LNGISO"
                 at:deprecated="false">
      <skos:prefLabel xml:lang="en">PUB_LNGISO</skos:prefLabel>
      <skos:prefLabel xml:lang="et">PUB_LNGISO</skos:prefLabel>
      <at:authority-code>PUB_LNGISO</at:authority-code>
      <at:op-code>PUB_LNGISO</at:op-code>
      <at:start.use>2010-03-29</at:start.use>
      <atold:op-code>PUB_LNGISO</atold:op-code>
      <dc:identifier>PUB_LNGISO</dc:identifier>
      <skos:altLabel xml:lang="en">PUB_LNGISO code</skos:altLabel>
      <skos:definition xml:lang="en">Code used by PUB__LNGISO of Publications domain in ATTO.</skos:definition>
      <skos:inScheme rdf:resource="http://publications.europa.eu/resource/authority/notation-type"/>
      <skos:topConceptOf rdf:resource="http://publications.europa.eu/resource/authority/notation-type"/>
   </skos:Concept>
   <skos:Concept rdf:about="http://publications.europa.eu/resource/authority/notation-type/PUB_LOC"
                 at:deprecated="false">
      <skos:prefLabel xml:lang="en">PUB_LOC</skos:prefLabel>
      <skos:prefLabel xml:lang="et">PUB_LOC</skos:prefLabel>
      <at:authority-code>PUB_LOC</at:authority-code>
      <at:op-code>PUB_LOC</at:op-code>
      <at:start.use>2010-03-29</at:start.use>
      <atold:op-code>PUB_LOC</atold:op-code>
      <dc:identifier>PUB_LOC</dc:identifier>
      <skos:altLabel xml:lang="en">PUB_LOC code</skos:altLabel>
      <skos:definition xml:lang="en">Code used by PUB_LOC table of Publications domain in ATTO.</skos:definition>
      <skos:inScheme rdf:resource="http://publications.europa.eu/resource/authority/notation-type"/>
      <skos:topConceptOf rdf:resource="http://publications.europa.eu/resource/authority/notation-type"/>
   </skos:Concept>
   <skos:Concept rdf:about="http://publications.europa.eu/resource/authority/notation-type/PUB_NOT"
                 at:deprecated="false">
      <skos:prefLabel xml:lang="en">PUB_NOT</skos:prefLabel>
      <skos:prefLabel xml:lang="et">PUB_NOT</skos:prefLabel>
      <at:authority-code>PUB_NOT</at:authority-code>
      <at:op-code>PUB_NOT</at:op-code>
      <at:start.use>2010-03-29</at:start.use>
      <atold:op-code>PUB_NOT</atold:op-code>
      <dc:identifier>PUB_NOT</dc:identifier>
      <skos:altLabel xml:lang="en">PUB_NOT code</skos:altLabel>
      <skos:definition xml:lang="en">Code used by PUB_NOT of Publications domain in ATTO.</skos:definition>
      <skos:inScheme rdf:resource="http://publications.europa.eu/resource/authority/notation-type"/>
      <skos:topConceptOf rdf:resource="http://publications.europa.eu/resource/authority/notation-type"/>
   </skos:Concept>
   <skos:Concept rdf:about="http://publications.europa.eu/resource/authority/notation-type/PUB_ORDIN"
                 at:deprecated="false">
      <skos:prefLabel xml:lang="en">PUB_ORDIN</skos:prefLabel>
      <skos:prefLabel xml:lang="et">PUB_ORDIN</skos:prefLabel>
      <at:authority-code>PUB_ORDIN</at:authority-code>
      <at:op-code>PUB_ORDIN</at:op-code>
      <at:start.use>2010-03-29</at:start.use>
      <atold:op-code>PUB_ORDIN</atold:op-code>
      <dc:identifier>PUB_ORDIN</dc:identifier>
      <skos:altLabel xml:lang="en">PUB_ORDIN code</skos:altLabel>
      <skos:definition xml:lang="en">Code used by PUB_ORDIN of Publications domain in ATTO.</skos:definition>
      <skos:inScheme rdf:resource="http://publications.europa.eu/resource/authority/notation-type"/>
      <skos:topConceptOf rdf:resource="http://publications.europa.eu/resource/authority/notation-type"/>
   </skos:Concept>
   <skos:Concept rdf:about="http://publications.europa.eu/resource/authority/notation-type/PUB_QUAL"
                 at:deprecated="false">
      <skos:prefLabel xml:lang="en">PUB_QUAL</skos:prefLabel>
      <skos:prefLabel xml:lang="et">PUB_QUAL</skos:prefLabel>
      <at:authority-code>PUB_QUAL</at:authority-code>
      <at:op-code>PUB_QUAL</at:op-code>
      <at:start.use>2010-03-29</at:start.use>
      <atold:op-code>PUB_QUAL</atold:op-code>
      <dc:identifier>PUB_QUAL</dc:identifier>
      <skos:altLabel xml:lang="en">PUB_QUAL code</skos:altLabel>
      <skos:definition xml:lang="en">Code used by PUB_QUAL of Publications domain in ATTO.</skos:definition>
      <skos:inScheme rdf:resource="http://publications.europa.eu/resource/authority/notation-type"/>
      <skos:topConceptOf rdf:resource="http://publications.europa.eu/resource/authority/notation-type"/>
   </skos:Concept>
   <skos:Concept rdf:about="http://publications.europa.eu/resource/authority/notation-type/PUB_TARGET"
                 at:deprecated="false">
      <skos:prefLabel xml:lang="en">PUB_TARGET</skos:prefLabel>
      <skos:prefLabel xml:lang="et">PUB_TARGET</skos:prefLabel>
      <at:authority-code>PUB_TARGET</at:authority-code>
      <at:op-code>PUB_TARGET</at:op-code>
      <at:start.use>2010-03-29</at:start.use>
      <atold:op-code>PUB_TARGET</atold:op-code>
      <dc:identifier>PUB_TARGET</dc:identifier>
      <skos:altLabel xml:lang="en">PUB_TARGET code</skos:altLabel>
      <skos:definition xml:lang="en">Code used by PUB_TARGET of Publications domain in ATTO.</skos:definition>
      <skos:inScheme rdf:resource="http://publications.europa.eu/resource/authority/notation-type"/>
      <skos:topConceptOf rdf:resource="http://publications.europa.eu/resource/authority/notation-type"/>
   </skos:Concept>
   <skos:Concept rdf:about="http://publications.europa.eu/resource/authority/notation-type/PUB_THEM14"
                 at:deprecated="false">
      <skos:prefLabel xml:lang="en">PUB_THEM14</skos:prefLabel>
      <skos:prefLabel xml:lang="et">PUB_THEM14</skos:prefLabel>
      <at:authority-code>PUB_THEM14</at:authority-code>
      <at:op-code>PUB_THEM14</at:op-code>
      <at:start.use>2010-03-29</at:start.use>
      <atold:op-code>PUB_THEM14</atold:op-code>
      <dc:identifier>PUB_THEM14</dc:identifier>
      <skos:altLabel xml:lang="en">PUB_THEM14 code</skos:altLabel>
      <skos:definition xml:lang="en">Code used by PUB_THEM14 of Publications domain in ATTO.</skos:definition>
      <skos:inScheme rdf:resource="http://publications.europa.eu/resource/authority/notation-type"/>
      <skos:topConceptOf rdf:resource="http://publications.europa.eu/resource/authority/notation-type"/>
   </skos:Concept>
   <skos:Concept rdf:about="http://publications.europa.eu/resource/authority/notation-type/PURL"
                 at:deprecated="false">
      <skos:prefLabel xml:lang="en">PURL</skos:prefLabel>
      <skos:prefLabel xml:lang="et">PURL</skos:prefLabel>
      <at:authority-code>PURL</at:authority-code>
      <at:op-code>PURL</at:op-code>
      <at:start.use>1998-03-31</at:start.use>
      <atold:op-code>PURL</atold:op-code>
      <dc:identifier>PURL</dc:identifier>
      <skos:altLabel xml:lang="en">Persistent URL</skos:altLabel>
      <skos:definition xml:lang="en">A persistent URL (PURL) is a Uniform Resource Locator (URL) that is guaranteed by an organization to function for a long period of time.</skos:definition>
      <skos:inScheme rdf:resource="http://publications.europa.eu/resource/authority/notation-type"/>
      <skos:topConceptOf rdf:resource="http://publications.europa.eu/resource/authority/notation-type"/>
      <skos:exactMatch rdf:resource="http://purl.org/spar/datacite/purl"/>
   </skos:Concept>
   <skos:Concept rdf:about="http://publications.europa.eu/resource/authority/notation-type/SICI"
                 at:deprecated="false">
      <skos:prefLabel xml:lang="en">SICI</skos:prefLabel>
      <skos:prefLabel xml:lang="et">SICI</skos:prefLabel>
      <at:authority-code>SICI</at:authority-code>
      <at:op-code>SICI</at:op-code>
      <at:start.use>1991-12-31</at:start.use>
      <atold:op-code>SICI</atold:op-code>
      <dc:identifier>SICI</dc:identifier>
      <skos:altLabel xml:lang="en">Serial Item and Contribution Identifier</skos:altLabel>
      <skos:definition xml:lang="en">An add-on to the ISSN, the Serial Item and Contribution Identifier (SICI) is a variable length code (ANSI/NISO standard Z39.56) that provides unique identification of serial issues (SII) and serial contributions (SCI).</skos:definition>
      <skos:inScheme rdf:resource="http://publications.europa.eu/resource/authority/notation-type"/>
      <skos:topConceptOf rdf:resource="http://publications.europa.eu/resource/authority/notation-type"/>
      <skos:exactMatch rdf:resource="http://purl.org/spar/datacite/sici"/>
   </skos:Concept>
   <skos:Concept rdf:about="http://publications.europa.eu/resource/authority/notation-type/TED"
                 at:deprecated="false">
      <skos:prefLabel xml:lang="en">TED</skos:prefLabel>
      <skos:prefLabel xml:lang="et">TED</skos:prefLabel>
      <at:authority-code>TED</at:authority-code>
      <at:op-code>TED</at:op-code>
      <at:start.use>1986-01-01</at:start.use>
      <atold:op-code>TED</atold:op-code>
      <dc:identifier>TED</dc:identifier>
      <skos:altLabel xml:lang="en">TED code</skos:altLabel>
      <skos:definition xml:lang="en">Code used in Tenders Electronic Daily, the online version of the 'Supplement to the Official Journal of the European Union', dedicated to European public procurement.</skos:definition>
      <skos:inScheme rdf:resource="http://publications.europa.eu/resource/authority/notation-type"/>
      <skos:topConceptOf rdf:resource="http://publications.europa.eu/resource/authority/notation-type"/>
   </skos:Concept>
   <skos:Concept rdf:about="http://publications.europa.eu/resource/authority/notation-type/TED_SCHEMA"
                 at:deprecated="false">
      <skos:prefLabel xml:lang="en">TED Schema</skos:prefLabel>
      <skos:prefLabel xml:lang="et">TED Schema</skos:prefLabel>
      <at:authority-code>TED_SCHEMA</at:authority-code>
      <at:op-code>TED_SCHEMA</at:op-code>
      <at:start.use>2019-09-18</at:start.use>
      <atold:op-code>TED_SCHEMA</atold:op-code>
      <dc:identifier>TED_SCHEMA</dc:identifier>
      <skos:altLabel xml:lang="en">TED Schema code</skos:altLabel>
      <skos:definition xml:lang="en">Code used in the schema of Tenders Electronic Daily, the online version of the 'Supplement to the Official Journal of the European Union', dedicated to European public procurement.</skos:definition>
      <skos:inScheme rdf:resource="http://publications.europa.eu/resource/authority/notation-type"/>
      <skos:topConceptOf rdf:resource="http://publications.europa.eu/resource/authority/notation-type"/>
   </skos:Concept>
   <skos:Concept rdf:about="http://publications.europa.eu/resource/authority/notation-type/TIR"
                 at:deprecated="false">
      <skos:prefLabel xml:lang="en">TIR</skos:prefLabel>
      <skos:prefLabel xml:lang="et">TIR</skos:prefLabel>
      <at:authority-code>TIR</at:authority-code>
      <at:op-code>TIR</at:op-code>
      <at:start.use>1975-11-14</at:start.use>
      <atold:op-code>TIR</atold:op-code>
      <dc:identifier>TIR</dc:identifier>
      <skos:altLabel xml:lang="en">International Road Transport code</skos:altLabel>
      <skos:definition xml:lang="en">The TIR code is used for distinguishing signs of vehicles in international traffic.</skos:definition>
      <skos:inScheme rdf:resource="http://publications.europa.eu/resource/authority/notation-type"/>
      <skos:topConceptOf rdf:resource="http://publications.europa.eu/resource/authority/notation-type"/>
      <at:op-mapped-code>
         <at:MappedCode>
            <dc:source>MDR</dc:source>
            <at:affected-table>notation-type</at:affected-table>
            <at:legacy-code>code-tir</at:legacy-code>
         </at:MappedCode>
      </at:op-mapped-code>
   </skos:Concept>
   <skos:Concept rdf:about="http://publications.europa.eu/resource/authority/notation-type/UNSD_GEOSCHEME"
                 at:deprecated="false">
      <skos:prefLabel xml:lang="en">UNSD geoscheme</skos:prefLabel>
      <skos:prefLabel xml:lang="et">UNSD geoscheme</skos:prefLabel>
      <at:authority-code>UNSD_GEOSCHEME</at:authority-code>
      <at:op-code>UNSD_GEOSCHEME</at:op-code>
      <at:start.use>1970-01-01</at:start.use>
      <atold:op-code>UNSD_GEOSCHEME</atold:op-code>
      <dc:identifier>UNSD_GEOSCHEME</dc:identifier>
      <skos:altLabel xml:lang="en">United Nations Statistics Division geoscheme</skos:altLabel>
      <skos:definition xml:lang="en">The United Nations geoscheme is a system which divides the countries of the world into regional and subregional groups. It was devised by the United Nations Statistics Division (UNSD) based on the M49 coding classification. The UNSD geoscheme notation uses two levels of this classification: intermediate region and subregion. The intermediate region name is used whenever it is available; in other cases the broader level, subregion, is used. The UNSD geoscheme notation is used in the Country authority table.</skos:definition>
      <skos:inScheme rdf:resource="http://publications.europa.eu/resource/authority/notation-type"/>
      <skos:topConceptOf rdf:resource="http://publications.europa.eu/resource/authority/notation-type"/>
   </skos:Concept>
   <skos:Concept rdf:about="http://publications.europa.eu/resource/authority/notation-type/UNSD_M49"
                 at:deprecated="false">
      <skos:prefLabel xml:lang="en">UNSD M49</skos:prefLabel>
      <skos:prefLabel xml:lang="et">UNSD M49</skos:prefLabel>
      <at:authority-code>UNSD_M49</at:authority-code>
      <at:op-code>UNSD_M49</at:op-code>
      <at:start.use>1970-01-01</at:start.use>
      <atold:op-code>UNSD_M49</atold:op-code>
      <dc:identifier>UNSD_M49</dc:identifier>
      <skos:altLabel xml:lang="en">United Nations Statistics Division M49 code</skos:altLabel>
      <skos:definition xml:lang="en">The UNSD M49 codes are standard country or area codes for statistical purposes, developed and maintained by the United Nations Statistics Division (UNSD). Each area code is a three-digit number which can refer to a wide variety of geographical, political, or economic regions, like a continent, a country or a specific group of countries. Codes assigned in the system generally do not change when the country or area's name changes (unlike ISO 3166-1 alpha-2 or ISO 3166-1 alpha-3), but instead change when the territorial extent of the country or area changes significantly.</skos:definition>
      <skos:inScheme rdf:resource="http://publications.europa.eu/resource/authority/notation-type"/>
      <skos:topConceptOf rdf:resource="http://publications.europa.eu/resource/authority/notation-type"/>
      <at:op-mapped-code>
         <at:MappedCode>
            <dc:source>MDR</dc:source>
            <at:affected-table>notation-type</at:affected-table>
            <at:legacy-code>code-M49</at:legacy-code>
         </at:MappedCode>
      </at:op-mapped-code>
   </skos:Concept>
   <skos:Concept rdf:about="http://publications.europa.eu/resource/authority/notation-type/UN_LOCODE"
                 at:deprecated="false">
      <skos:prefLabel xml:lang="en">UN location</skos:prefLabel>
      <skos:prefLabel xml:lang="et">UN location</skos:prefLabel>
      <at:authority-code>UN_LOCODE</at:authority-code>
      <at:op-code>UN_LOCODE</at:op-code>
      <at:start.use>1981-01-01</at:start.use>
      <atold:op-code>UN_LOCODE</atold:op-code>
      <dc:identifier>UN_LOCODE</dc:identifier>
      <skos:altLabel xml:lang="en">United Nations Code for Trade and Transport Locations code</skos:altLabel>
      <skos:definition xml:lang="en">5-character code where the first two characters are the ISO 3166 country codes while the remaining three are derived from Recommendation 16 from the UNECE in Geneva, together with Eurostat supplied codes for ports not yet included in the UN system.</skos:definition>
      <skos:inScheme rdf:resource="http://publications.europa.eu/resource/authority/notation-type"/>
      <skos:topConceptOf rdf:resource="http://publications.europa.eu/resource/authority/notation-type"/>
      <at:op-mapped-code>
         <at:MappedCode>
            <dc:source>MDR</dc:source>
            <at:affected-table>notation-type</at:affected-table>
            <at:legacy-code>unlocode</at:legacy-code>
         </at:MappedCode>
      </at:op-mapped-code>
   </skos:Concept>
   <skos:Concept rdf:about="http://publications.europa.eu/resource/authority/notation-type/UPC"
                 at:deprecated="false">
      <skos:prefLabel xml:lang="en">UPC</skos:prefLabel>
      <skos:prefLabel xml:lang="et">UPC</skos:prefLabel>
      <at:authority-code>UPC</at:authority-code>
      <at:op-code>UPC</at:op-code>
      <at:start.use>1973-01-01</at:start.use>
      <atold:op-code>UPC</atold:op-code>
      <dc:identifier>UPC</dc:identifier>
      <skos:altLabel xml:lang="en">Universal Product Code</skos:altLabel>
      <skos:definition xml:lang="en">The Universal Product Code (UPC) is a widely-used standard for barcodes. The barcode consists of a series of variable-width vertical bars and was created for tracking merchandise in stores, mainly at the point of sale.</skos:definition>
      <skos:inScheme rdf:resource="http://publications.europa.eu/resource/authority/notation-type"/>
      <skos:topConceptOf rdf:resource="http://publications.europa.eu/resource/authority/notation-type"/>
      <skos:exactMatch rdf:resource="http://purl.org/spar/datacite/upc"/>
   </skos:Concept>
   <skos:Concept rdf:about="http://publications.europa.eu/resource/authority/notation-type/URI"
                 at:deprecated="false">
      <skos:prefLabel xml:lang="en">URI</skos:prefLabel>
      <skos:prefLabel xml:lang="et">URI</skos:prefLabel>
      <at:authority-code>URI</at:authority-code>
      <at:op-code>URI</at:op-code>
      <at:start.use>1998-12-31</at:start.use>
      <atold:op-code>URI</atold:op-code>
      <dc:identifier>URI</dc:identifier>
      <skos:altLabel xml:lang="en">Uniform Resource Identifier</skos:altLabel>
      <skos:definition xml:lang="en">A Uniform Resource Identifier (URI) is a compact sequence of characters that identifies an abstract or physical resource. A URI can be used as a locator, a name, or both. If a URI is a locator, it describes a resource’s primary access mechanism. If a URI is a name, it identifies a resource by giving it a unique name.</skos:definition>
      <skos:inScheme rdf:resource="http://publications.europa.eu/resource/authority/notation-type"/>
      <skos:topConceptOf rdf:resource="http://publications.europa.eu/resource/authority/notation-type"/>
      <skos:exactMatch rdf:resource="http://purl.org/spar/datacite/uri"/>
   </skos:Concept>
   <skos:Concept rdf:about="http://publications.europa.eu/resource/authority/notation-type/URL"
                 at:deprecated="false">
      <skos:prefLabel xml:lang="en">URL</skos:prefLabel>
      <skos:prefLabel xml:lang="et">URL</skos:prefLabel>
      <at:authority-code>URL</at:authority-code>
      <at:op-code>URL</at:op-code>
      <at:start.use>1994-12-31</at:start.use>
      <atold:op-code>URL</atold:op-code>
      <dc:identifier>URL</dc:identifier>
      <skos:altLabel xml:lang="en">Uniform Resource Locator</skos:altLabel>
      <skos:definition xml:lang="en">A Uniform Resource Locator (URL) is a URI that, in addition to identifying a resource, provides a means of locating the resource by describing its primary access mechanism. As there is no exact definition of URL by means of a set of schemes, URL is a useful but informal concept, usually referring to a subset of URIs that do not contain URNs.</skos:definition>
      <skos:inScheme rdf:resource="http://publications.europa.eu/resource/authority/notation-type"/>
      <skos:topConceptOf rdf:resource="http://publications.europa.eu/resource/authority/notation-type"/>
      <skos:exactMatch rdf:resource="http://purl.org/spar/datacite/url"/>
   </skos:Concept>
   <skos:Concept rdf:about="http://publications.europa.eu/resource/authority/notation-type/URN"
                 at:deprecated="false">
      <skos:prefLabel xml:lang="en">URN</skos:prefLabel>
      <skos:prefLabel xml:lang="et">URN</skos:prefLabel>
      <at:authority-code>URN</at:authority-code>
      <at:op-code>URN</at:op-code>
      <at:start.use>1997-05-31</at:start.use>
      <atold:op-code>URN</atold:op-code>
      <dc:identifier>URN</dc:identifier>
      <skos:altLabel xml:lang="en">Uniform Resource Name</skos:altLabel>
      <skos:definition xml:lang="en">A Uniform Resource Name (URN) is a URI that is assigned under the "urn" URI scheme and a particular URN namespace, with the intent that the URN will be a persistent, location-independent resource identifier.</skos:definition>
      <skos:inScheme rdf:resource="http://publications.europa.eu/resource/authority/notation-type"/>
      <skos:topConceptOf rdf:resource="http://publications.europa.eu/resource/authority/notation-type"/>
      <skos:exactMatch rdf:resource="http://purl.org/spar/datacite/urn"/>
   </skos:Concept>
   <skos:Concept rdf:about="http://publications.europa.eu/resource/authority/notation-type/WHOISWHO"
                 at:deprecated="false">
      <skos:prefLabel xml:lang="en">EU Whoiswho</skos:prefLabel>
      <skos:prefLabel xml:lang="et">EU Whoiswho</skos:prefLabel>
      <at:authority-code>WHOISWHO</at:authority-code>
      <at:op-code>WHOISWHO</at:op-code>
      <at:start.use>1981-12-01</at:start.use>
      <atold:op-code>WHOISWHO</atold:op-code>
      <dc:identifier>WHOISWHO</dc:identifier>
      <skos:altLabel xml:lang="en">EU Whoiswho code</skos:altLabel>
      <skos:definition xml:lang="en">Code used in the EU Whoiswho, an electronic directory of managers and services in the EU institutions, bodies and agencies.</skos:definition>
      <skos:inScheme rdf:resource="http://publications.europa.eu/resource/authority/notation-type"/>
      <skos:topConceptOf rdf:resource="http://publications.europa.eu/resource/authority/notation-type"/>
   </skos:Concept>
   <skos:Concept rdf:about="http://publications.europa.eu/resource/authority/notation-type/XML_LNG"
                 at:deprecated="false">
      <skos:prefLabel xml:lang="en">xml lang</skos:prefLabel>
      <skos:prefLabel xml:lang="et">xml keel</skos:prefLabel>
      <at:authority-code>XML_LNG</at:authority-code>
      <at:op-code>XML_LNG</at:op-code>
      <at:start.use>1995-03-01</at:start.use>
      <atold:op-code>XML_LNG</atold:op-code>
      <dc:identifier>XML_LNG</dc:identifier>
      <skos:altLabel xml:lang="en">xml language</skos:altLabel>
      <skos:definition xml:lang="en">XML LANG codes are used to indicate the natural language in which xml content is expressed. The code is based on ISO 639 codes and RFC 5646 explains how those codes are structured.</skos:definition>
      <skos:inScheme rdf:resource="http://publications.europa.eu/resource/authority/notation-type"/>
      <skos:topConceptOf rdf:resource="http://publications.europa.eu/resource/authority/notation-type"/>
      <at:op-mapped-code>
         <at:MappedCode>
            <dc:source>MDR</dc:source>
            <at:affected-table>notation-type</at:affected-table>
            <at:legacy-code>xml-lang</at:legacy-code>
         </at:MappedCode>
      </at:op-mapped-code>
   </skos:Concept>
</rdf:RDF>
