@prefix at: <http://publications.europa.eu/ontology/authority/> .
@prefix atold: <http://publications.europa.eu/resource/authority/> .
@prefix dc: <http://purl.org/dc/elements/1.1/> .
@prefix owl: <http://www.w3.org/2002/07/owl#> .
@prefix rdfs: <http://www.w3.org/2000/01/rdf-schema#> .
@prefix skos: <http://www.w3.org/2004/02/skos/core#> .

<http://publications.europa.eu/resource/authority/licence/0BSD> a skos:Concept ;
    at:authority-code "0BSD" ;
    at:deprecated "false" ;
    at:op-code "0BSD" ;
    at:start.use "2006-07-01" ;
    atold:op-code "0BSD" ;
    dc:identifier "0BSD" ;
    skos:altLabel "0BSD"@bg,
        "0BSD"@cs,
        "0BSD"@da,
        "0BSD"@de,
        "0BSD"@el,
        "0BSD"@en,
        "0BSD"@es,
        "0BSD"@et,
        "0BSD"@fi,
        "0BSD"@fr,
        "0BSD"@ga,
        "0BSD"@hr,
        "0BSD"@hu,
        "0BSD"@it,
        "0BSD"@lt,
        "0BSD"@lv,
        "0BSD"@mt,
        "0BSD"@nl,
        "0BSD"@pl,
        "0BSD"@pt,
        "0BSD"@ro,
        "0BSD"@sk,
        "0BSD"@sl,
        "0BSD"@sv ;
    skos:changeNote "The source of the start-use date: https://spdx.org/licenses/0BSD.html"@en ;
    skos:definition "The BSD 0-clause licence, 0BSD, goes further than the 2-clause licence by dropping the requirements to include the copyright notice, licence text or disclaimer in either source or binary forms. Doing so forms a public-domain-equivalent licence. It is approved by the Open Source Initiative."@en ;
    skos:exactMatch <https://opensource.org/licenses/0BSD> ;
    skos:inScheme atold:licence ;
    skos:prefLabel "Zero-Clause BSD / Free Public License 1.0.0 (0BSD)"@en ;
    skos:topConceptOf atold:licence .

<http://publications.europa.eu/resource/authority/licence/AGPL_3_0> a skos:Concept ;
    at:authority-code "AGPL_3_0" ;
    at:deprecated "false" ;
    at:op-code "AGPL_3_0" ;
    at:start.use "2007-11-19" ;
    atold:op-code "AGPL_3_0" ;
    dc:identifier "AGPL_3_0" ;
    skos:altLabel "AGPL-3.0"@bg,
        "AGPL-3.0"@cs,
        "AGPL-3.0"@da,
        "AGPL-3.0"@de,
        "AGPL-3.0"@el,
        "AGPL-3.0"@en,
        "AGPL-3.0"@es,
        "AGPL-3.0"@et,
        "AGPL-3.0"@fi,
        "AGPL-3.0"@fr,
        "AGPL-3.0"@ga,
        "AGPL-3.0"@hr,
        "AGPL-3.0"@hu,
        "AGPL-3.0"@it,
        "AGPL-3.0"@lt,
        "AGPL-3.0"@lv,
        "AGPL-3.0"@mt,
        "AGPL-3.0"@nl,
        "AGPL-3.0"@pl,
        "AGPL-3.0"@pt,
        "AGPL-3.0"@ro,
        "AGPL-3.0"@sk,
        "AGPL-3.0"@sl,
        "AGPL-3.0"@sv ;
    skos:changeNote "The source of the start-use date: https://en.wikipedia.org/wiki/Affero_General_Public_License"@en ;
    skos:definition "AGPL-3.0 is a modified GPL-3.0 extended to network or Web services distribution (SaaS). Strong copyleft: copies and derivatives may be distributed under the same AGPL only. Need to document derivatives’ changes and dates. Incompatible with other licences except linking with code covered by the original GPL-3.0."@en ;
    skos:exactMatch <https://opensource.org/licenses/AGPL-3.0> ;
    skos:inScheme atold:licence ;
    skos:prefLabel "GNU Affero General Public License version 3"@en ;
    skos:topConceptOf atold:licence .

<http://publications.europa.eu/resource/authority/licence/APACHE_1_1> a skos:Concept ;
    at:authority-code "APACHE_1_1" ;
    at:deprecated "true" ;
    at:end.use "2004-01-01" ;
    at:op-code "APACHE_1_1" ;
    at:start.use "2000-01-01" ;
    atold:op-code "APACHE_1_1" ;
    dc:identifier "APACHE_1_1" ;
    skos:altLabel "Apache 1.1"@bg,
        "Apache 1.1"@cs,
        "Apache 1.1"@da,
        "Apache 1.1"@de,
        "Apache 1.1"@el,
        "Apache 1.1"@en,
        "Apache 1.1"@es,
        "Apache 1.1"@et,
        "Apache 1.1"@fi,
        "Apache 1.1"@fr,
        "Apache 1.1"@ga,
        "Apache 1.1"@hr,
        "Apache 1.1"@hu,
        "Apache 1.1"@it,
        "Apache 1.1"@lt,
        "Apache 1.1"@lv,
        "Apache 1.1"@mt,
        "Apache 1.1"@nl,
        "Apache 1.1"@pl,
        "Apache 1.1"@pt,
        "Apache 1.1"@ro,
        "Apache 1.1"@sk,
        "Apache 1.1"@sl,
        "Apache 1.1"@sv ;
    skos:changeNote "The source of the start-use date: https://opensource.org/licenses/Apache-1.1"@en ;
    skos:definition "Apache-1.1 is a permissive free software licence approved by the Open Source Initiative. It is superseded by Apache-2.0."@en ;
    skos:exactMatch <https://opensource.org/licenses/Apache-1.1> ;
    skos:inScheme atold:licence ;
    skos:prefLabel "Apache Software License, version 1.1 (Apache-1.1)"@en,
        "Apache tarkvara litsents, versioon 1.1 (Apache-1.1)"@et ;
    skos:topConceptOf atold:licence .

<http://publications.europa.eu/resource/authority/licence/APACHE_2_0> a skos:Concept ;
    at:authority-code "APACHE_2_0" ;
    at:deprecated "false" ;
    at:op-code "APACHE_2_0" ;
    at:start.use "2004-01-02" ;
    atold:op-code "APACHE_2_0" ;
    dc:identifier "APACHE_2_0" ;
    skos:altLabel "Apache 2.0"@bg,
        "Apache 2.0"@cs,
        "Apache 2.0"@da,
        "Apache 2.0"@de,
        "Apache 2.0"@el,
        "Apache 2.0"@en,
        "Apache 2.0"@es,
        "Apache 2.0"@et,
        "Apache 2.0"@fi,
        "Apache 2.0"@fr,
        "Apache 2.0"@ga,
        "Apache 2.0"@hr,
        "Apache 2.0"@hu,
        "Apache 2.0"@it,
        "Apache 2.0"@lt,
        "Apache 2.0"@lv,
        "Apache 2.0"@mt,
        "Apache 2.0"@nl,
        "Apache 2.0"@pl,
        "Apache 2.0"@pt,
        "Apache 2.0"@ro,
        "Apache 2.0"@sk,
        "Apache 2.0"@sl,
        "Apache 2.0"@sv ;
    skos:changeNote "The source of the start-use date: https://opensource.org/licenses/Apache-2.0"@en ;
    skos:definition "Apache-2.0 is a permissive free software licence approved by the Open Source Initiative. It gives complete freedom to use the given works, as long as the required notices are included. Compared with the MIT, recipients receive a patent licence from the contributors of the code."@en ;
    skos:exactMatch <https://opensource.org/licenses/Apache-2.0> ;
    skos:inScheme atold:licence ;
    skos:prefLabel "Apache License, Version 2.0"@en,
        "Apache litsents, versioon 2.0"@et ;
    skos:topConceptOf atold:licence .

<http://publications.europa.eu/resource/authority/licence/APL_1_0> a skos:Concept ;
    at:authority-code "APL_1_0" ;
    at:deprecated "false" ;
    at:op-code "APL_1_0" ;
    at:start.use "2003-07-01" ;
    atold:op-code "APL_1_0" ;
    dc:identifier "APL_1_0" ;
    skos:altLabel "APL-1.0"@bg,
        "APL-1.0"@cs,
        "APL-1.0"@da,
        "APL-1.0"@de,
        "APL-1.0"@el,
        "APL-1.0"@en,
        "APL-1.0"@es,
        "APL-1.0"@et,
        "APL-1.0"@fi,
        "APL-1.0"@fr,
        "APL-1.0"@ga,
        "APL-1.0"@hr,
        "APL-1.0"@hu,
        "APL-1.0"@it,
        "APL-1.0"@lt,
        "APL-1.0"@lv,
        "APL-1.0"@mt,
        "APL-1.0"@nl,
        "APL-1.0"@pl,
        "APL-1.0"@pt,
        "APL-1.0"@ro,
        "APL-1.0"@sk,
        "APL-1.0"@sl,
        "APL-1.0"@sv ;
    skos:changeNote "The source of the start-use date: http://www.worldlii.org/int/other/PubRL/2009/1.html"@en ;
    skos:definition "APL-1.0 is a copyleft-style, free software licence approved by the Open Source Initiative. It allows combining the covered code with other components not governed by the APL licence provided the APL requirements are fulfilled for the covered portion of the larger work."@en ;
    skos:exactMatch <https://opensource.org/licenses/APL-1.0> ;
    skos:inScheme atold:licence ;
    skos:prefLabel "Adaptive Public License 1.0"@en ;
    skos:topConceptOf atold:licence .

<http://publications.europa.eu/resource/authority/licence/APSL_2_0> a skos:Concept ;
    at:authority-code "APSL_2_0" ;
    at:deprecated "false" ;
    at:op-code "APSL_2_0" ;
    at:start.use "2003-08-06" ;
    atold:op-code "APSL_2_0" ;
    dc:identifier "APSL_2_0" ;
    skos:altLabel "APSL-2.0"@bg,
        "APSL-2.0"@cs,
        "APSL-2.0"@da,
        "APSL-2.0"@de,
        "APSL-2.0"@el,
        "APSL-2.0"@en,
        "APSL-2.0"@es,
        "APSL-2.0"@et,
        "APSL-2.0"@fi,
        "APSL-2.0"@fr,
        "APSL-2.0"@ga,
        "APSL-2.0"@hr,
        "APSL-2.0"@hu,
        "APSL-2.0"@it,
        "APSL-2.0"@lt,
        "APSL-2.0"@lv,
        "APSL-2.0"@mt,
        "APSL-2.0"@nl,
        "APSL-2.0"@pl,
        "APSL-2.0"@pt,
        "APSL-2.0"@ro,
        "APSL-2.0"@sk,
        "APSL-2.0"@sl,
        "APSL-2.0"@sv ;
    skos:changeNote "The source of the start-use date: https://en.wikipedia.org/wiki/Apple_Public_Source_License"@en ;
    skos:definition "APSL-2.0 is a copyleft-style, free software licence approved by the Open Source Initiative. Under this licence, it is possible to create a larger work by combining covered code with other code not governed by the terms of this licence and distribute the larger work as a single product. In each such instance, it must be ensured that requirements of this licence are fulfilled for the covered code or any portion thereof."@en ;
    skos:exactMatch <https://opensource.org/licenses/APSL-2.0> ;
    skos:inScheme atold:licence ;
    skos:prefLabel "Apple Public Source License 2.0"@en ;
    skos:topConceptOf atold:licence .

<http://publications.europa.eu/resource/authority/licence/ARTISTIC_1_0> a skos:Concept ;
    at:authority-code "ARTISTIC_1_0" ;
    at:deprecated "true" ;
    at:end.use "2000-06-30" ;
    at:op-code "ARTISTIC_1_0" ;
    at:start.use "1997-08-15" ;
    atold:op-code "ARTISTIC_1_0" ;
    dc:identifier "ARTISTIC_1_0" ;
    skos:altLabel "Artistic 1.0"@bg,
        "Artistic 1.0"@cs,
        "Artistic 1.0"@da,
        "Artistic 1.0"@de,
        "Artistic 1.0"@el,
        "Artistic 1.0"@en,
        "Artistic 1.0"@es,
        "Artistic 1.0"@et,
        "Artistic 1.0"@fi,
        "Artistic 1.0"@fr,
        "Artistic 1.0"@ga,
        "Artistic 1.0"@hr,
        "Artistic 1.0"@hu,
        "Artistic 1.0"@it,
        "Artistic 1.0"@lt,
        "Artistic 1.0"@lv,
        "Artistic 1.0"@mt,
        "Artistic 1.0"@nl,
        "Artistic 1.0"@pl,
        "Artistic 1.0"@pt,
        "Artistic 1.0"@ro,
        "Artistic 1.0"@sk,
        "Artistic 1.0"@sl,
        "Artistic 1.0"@sv ;
    skos:changeNote "The source of the start-use date: https://wiki.vvlibri.org/index.php?title=Artistic_License_Version_2.0"@en ;
    skos:definition "Artistic-1.0 is a copyleft-style, free software licence approved by the Open Source Initiative. It is superseded by Artistic 2.0."@en ;
    skos:exactMatch <https://opensource.org/licenses/Artistic-1.0> ;
    skos:inScheme atold:licence ;
    skos:prefLabel "Artistic License 1.0 (Artistic-1.0)"@en ;
    skos:topConceptOf atold:licence .

<http://publications.europa.eu/resource/authority/licence/ARTISTIC_2_0> a skos:Concept ;
    at:authority-code "ARTISTIC_2_0" ;
    at:deprecated "false" ;
    at:op-code "ARTISTIC_2_0" ;
    at:start.use "2000-07-01" ;
    atold:op-code "ARTISTIC_2_0" ;
    dc:identifier "ARTISTIC_2_0" ;
    skos:altLabel "Artistic 2.0"@bg,
        "Artistic 2.0"@cs,
        "Artistic 2.0"@da,
        "Artistic 2.0"@de,
        "Artistic 2.0"@el,
        "Artistic 2.0"@en,
        "Artistic 2.0"@es,
        "Artistic 2.0"@et,
        "Artistic 2.0"@fi,
        "Artistic 2.0"@fr,
        "Artistic 2.0"@ga,
        "Artistic 2.0"@hr,
        "Artistic 2.0"@hu,
        "Artistic 2.0"@it,
        "Artistic 2.0"@lt,
        "Artistic 2.0"@lv,
        "Artistic 2.0"@mt,
        "Artistic 2.0"@nl,
        "Artistic 2.0"@pl,
        "Artistic 2.0"@pt,
        "Artistic 2.0"@ro,
        "Artistic 2.0"@sk,
        "Artistic 2.0"@sl,
        "Artistic 2.0"@sv ;
    skos:changeNote "The source of the start-use date: https://www.appropedia.org/Open_software_licenses; http://www.linfo.org/artistic.html"@en ;
    skos:definition "Artistic-2.0 is a copyleft-style, free software licence approved by the Open Source Initiative. It preserves control of the original copyright holder: recipient can use, modify and distribute the original versions but other modified versions must document how far they are different and be reported to the original author, or be distributed under a different name, or otherwise be available under the Artistic licence or any other licence granting similar rights."@en ;
    skos:exactMatch <https://opensource.org/licenses/Artistic-2.0> ;
    skos:inScheme atold:licence ;
    skos:prefLabel "Artistic License 2.0"@en ;
    skos:topConceptOf atold:licence .

<http://publications.europa.eu/resource/authority/licence/BSD_2_CLAUSE> a skos:Concept ;
    at:authority-code "BSD_2_CLAUSE" ;
    at:deprecated "false" ;
    at:op-code "BSD_2_CLAUSE" ;
    at:start.use "1999-04-01" ;
    atold:op-code "BSD_2_CLAUSE" ;
    dc:identifier "BSD_2_CLAUSE" ;
    skos:altLabel "BSD-2-Clause"@bg,
        "BSD-2-Clause"@cs,
        "BSD-2-Clause"@da,
        "BSD-2-Clause"@de,
        "BSD-2-Clause"@el,
        "BSD-2-Clause"@en,
        "BSD-2-Clause"@es,
        "BSD-2-Clause"@et,
        "BSD-2-Clause"@fi,
        "BSD-2-Clause"@fr,
        "BSD-2-Clause"@ga,
        "BSD-2-Clause"@hr,
        "BSD-2-Clause"@hu,
        "BSD-2-Clause"@it,
        "BSD-2-Clause"@lt,
        "BSD-2-Clause"@lv,
        "BSD-2-Clause"@mt,
        "BSD-2-Clause"@nl,
        "BSD-2-Clause"@pl,
        "BSD-2-Clause"@pt,
        "BSD-2-Clause"@ro,
        "BSD-2-Clause"@sk,
        "BSD-2-Clause"@sl,
        "BSD-2-Clause"@sv ;
    skos:changeNote "The source of the start-use date: https://en.wikipedia.org/wiki/BSD_licenses"@en ;
    skos:definition "BSD-2-Clause permits redistribution and use in source and binary forms, with or without modification, provided that the certain conditions are met: redistributions of source code must retain the copyright notice, the specific list of conditions and the disclaimer."@en ;
    skos:exactMatch <https://opensource.org/licenses/BSD-2-Clause> ;
    skos:inScheme atold:licence ;
    skos:prefLabel "2-Clause BSD License"@en ;
    skos:topConceptOf atold:licence .

<http://publications.europa.eu/resource/authority/licence/BSD_3_CLAUSE> a skos:Concept ;
    at:authority-code "BSD_3_CLAUSE" ;
    at:deprecated "false" ;
    at:op-code "BSD_3_CLAUSE" ;
    at:start.use "1999-07-22" ;
    atold:op-code "BSD_3_CLAUSE" ;
    dc:identifier "BSD_3_CLAUSE" ;
    skos:altLabel "BSD-3-Clause"@bg,
        "BSD-3-Clause"@cs,
        "BSD-3-Clause"@da,
        "BSD-3-Clause"@de,
        "BSD-3-Clause"@el,
        "BSD-3-Clause"@en,
        "BSD-3-Clause"@es,
        "BSD-3-Clause"@et,
        "BSD-3-Clause"@fi,
        "BSD-3-Clause"@fr,
        "BSD-3-Clause"@ga,
        "BSD-3-Clause"@hr,
        "BSD-3-Clause"@hu,
        "BSD-3-Clause"@it,
        "BSD-3-Clause"@lt,
        "BSD-3-Clause"@lv,
        "BSD-3-Clause"@mt,
        "BSD-3-Clause"@nl,
        "BSD-3-Clause"@pl,
        "BSD-3-Clause"@pt,
        "BSD-3-Clause"@ro,
        "BSD-3-Clause"@sk,
        "BSD-3-Clause"@sl,
        "BSD-3-Clause"@sv ;
    skos:changeNote "The source of the start-use date: https://en.wikipedia.org/wiki/BSD_licenses"@en ;
    skos:definition "BSD-3-Clause permits redistribution and use in source and binary forms, with or without modification, provided that the certain conditions are met: redistributions of source code and in binary forms must retain the copyright notice, the specific list of conditions and the disclaimer. Neither the name of the copyright holder nor of its contributors may be used to promote derived products without prior written permission."@en ;
    skos:exactMatch <https://opensource.org/licenses/BSD-3-Clause> ;
    skos:inScheme atold:licence ;
    skos:prefLabel "3-Clause BSD License"@en ;
    skos:topConceptOf atold:licence .

<http://publications.europa.eu/resource/authority/licence/BSD_3_CLAUSE_LBNL> a skos:Concept ;
    at:authority-code "BSD_3_CLAUSE_LBNL" ;
    at:deprecated "false" ;
    at:op-code "BSD_3_CLAUSE_LBNL" ;
    at:start.use "2002-07-01" ;
    atold:op-code "BSD_3_CLAUSE_LBNL" ;
    dc:identifier "BSD_3_CLAUSE_LBNL" ;
    skos:altLabel "BSD-3-Clause-LBNL"@bg,
        "BSD-3-Clause-LBNL"@cs,
        "BSD-3-Clause-LBNL"@da,
        "BSD-3-Clause-LBNL"@de,
        "BSD-3-Clause-LBNL"@el,
        "BSD-3-Clause-LBNL"@en,
        "BSD-3-Clause-LBNL"@es,
        "BSD-3-Clause-LBNL"@et,
        "BSD-3-Clause-LBNL"@fi,
        "BSD-3-Clause-LBNL"@fr,
        "BSD-3-Clause-LBNL"@ga,
        "BSD-3-Clause-LBNL"@hr,
        "BSD-3-Clause-LBNL"@hu,
        "BSD-3-Clause-LBNL"@it,
        "BSD-3-Clause-LBNL"@lt,
        "BSD-3-Clause-LBNL"@lv,
        "BSD-3-Clause-LBNL"@mt,
        "BSD-3-Clause-LBNL"@nl,
        "BSD-3-Clause-LBNL"@pl,
        "BSD-3-Clause-LBNL"@pt,
        "BSD-3-Clause-LBNL"@ro,
        "BSD-3-Clause-LBNL"@sk,
        "BSD-3-Clause-LBNL"@sl,
        "BSD-3-Clause-LBNL"@sv ;
    skos:changeNote "The source of the start-use date: https://enterprise.dejacode.com/licenses/public/lbnl-bsd/?_list_filters=q%3Dbsd#essentials"@en ;
    skos:definition "BSD-3-Clause-LBNL is a BSD-style, permissive free software licence approved by the Open Source Initiative."@en ;
    skos:exactMatch <https://opensource.org/licenses/BSD-3-Clause-LBNL> ;
    skos:inScheme atold:licence ;
    skos:prefLabel "Lawrence Berkeley National Labs BSD Variant License (BSD-3-Clause-LBNL)"@en ;
    skos:topConceptOf atold:licence .

<http://publications.europa.eu/resource/authority/licence/BSD_PLUS_PATENT> a skos:Concept ;
    at:authority-code "BSD_PLUS_PATENT" ;
    at:deprecated "false" ;
    at:op-code "BSD_PLUS_PATENT" ;
    at:start.use "2017-07-01" ;
    atold:op-code "BSD_PLUS_PATENT" ;
    dc:identifier "BSD_PLUS_PATENT" ;
    skos:altLabel "BSD+Patent"@bg,
        "BSD+Patent"@cs,
        "BSD+Patent"@da,
        "BSD+Patent"@de,
        "BSD+Patent"@el,
        "BSD+Patent"@es,
        "BSD+Patent"@et,
        "BSD+Patent"@fi,
        "BSD+Patent"@fr,
        "BSD+Patent"@ga,
        "BSD+Patent"@hr,
        "BSD+Patent"@hu,
        "BSD+Patent"@it,
        "BSD+Patent"@lt,
        "BSD+Patent"@lv,
        "BSD+Patent"@mt,
        "BSD+Patent"@nl,
        "BSD+Patent"@pl,
        "BSD+Patent"@pt,
        "BSD+Patent"@ro,
        "BSD+Patent"@sk,
        "BSD+Patent"@sl,
        "BSD+Patent"@sv ;
    skos:changeNote "The source of the start-use date: https://enterprise.dejacode.com/licenses/public/bsd-plus-patent/?_list_filters=q%3Dbsd#essentials"@en ;
    skos:definition "BSD+Patent is a free software licence approved by the Open Source Initiative. It is a 2-clause license in which nothing restricts redistribution under any other license, but it requests to retain copyright notices and restrict the use of the BSD licensor name to promote derivative products."@en ;
    skos:exactMatch <https://opensource.org/licenses/BSDplusPatent> ;
    skos:inScheme atold:licence ;
    skos:prefLabel "BSD+Patent"@en ;
    skos:topConceptOf atold:licence .

<http://publications.europa.eu/resource/authority/licence/BSL_1_0> a skos:Concept ;
    at:authority-code "BSL_1_0" ;
    at:deprecated "false" ;
    at:op-code "BSL_1_0" ;
    at:start.use "2003-08-17" ;
    atold:op-code "BSL_1_0" ;
    dc:identifier "BSL_1_0" ;
    skos:altLabel "BSL-1.0"@bg,
        "BSL-1.0"@cs,
        "BSL-1.0"@da,
        "BSL-1.0"@de,
        "BSL-1.0"@el,
        "BSL-1.0"@en,
        "BSL-1.0"@es,
        "BSL-1.0"@et,
        "BSL-1.0"@fi,
        "BSL-1.0"@fr,
        "BSL-1.0"@ga,
        "BSL-1.0"@hr,
        "BSL-1.0"@hu,
        "BSL-1.0"@it,
        "BSL-1.0"@lt,
        "BSL-1.0"@lv,
        "BSL-1.0"@mt,
        "BSL-1.0"@nl,
        "BSL-1.0"@pl,
        "BSL-1.0"@pt,
        "BSL-1.0"@ro,
        "BSL-1.0"@sk,
        "BSL-1.0"@sl,
        "BSL-1.0"@sv ;
    skos:changeNote "The source of the start-use date: https://en.wikipedia.org/wiki/Boost_(C%2B%2B_libraries)#License"@en ;
    skos:definition "BSL-1.0 is a simple permissive licence only requiring preservation of copyright and licence notices for source (and not binary) distribution. Licenced works, modifications, and larger works may be distributed under different terms and without source code."@en ;
    skos:exactMatch <https://opensource.org/licenses/BSL-1.0> ;
    skos:inScheme atold:licence ;
    skos:prefLabel "Boost Software License 1.0"@en ;
    skos:topConceptOf atold:licence .

<http://publications.europa.eu/resource/authority/licence/CATOSL_1_1> a skos:Concept ;
    at:authority-code "CATOSL_1_1" ;
    at:deprecated "false" ;
    at:op-code "CATOSL_1_1" ;
    at:start.use "2004-07-31" ;
    atold:op-code "CATOSL_1_1" ;
    dc:identifier "CATOSL_1_1" ;
    skos:altLabel "CATOSL-1.1"@bg,
        "CATOSL-1.1"@cs,
        "CATOSL-1.1"@da,
        "CATOSL-1.1"@de,
        "CATOSL-1.1"@el,
        "CATOSL-1.1"@en,
        "CATOSL-1.1"@es,
        "CATOSL-1.1"@et,
        "CATOSL-1.1"@fi,
        "CATOSL-1.1"@fr,
        "CATOSL-1.1"@ga,
        "CATOSL-1.1"@hr,
        "CATOSL-1.1"@hu,
        "CATOSL-1.1"@it,
        "CATOSL-1.1"@lt,
        "CATOSL-1.1"@lv,
        "CATOSL-1.1"@mt,
        "CATOSL-1.1"@nl,
        "CATOSL-1.1"@pl,
        "CATOSL-1.1"@pt,
        "CATOSL-1.1"@ro,
        "CATOSL-1.1"@sk,
        "CATOSL-1.1"@sl,
        "CATOSL-1.1"@sv ;
    skos:changeNote "The source of the start-use date: https://webcache.googleusercontent.com/search?q=cache:7pbd65y1OUYJ:https://www.theinquirer.net/inquirer/news/1022762/computer-associates-open-source-guru-speaks-out+&cd=1&hl=en&ct=clnk&gl=lu"@en ;
    skos:definition "CATOSL-1.1 is a copyleft-style, free software licence approved by the Open Source Initiative. Under this licence, it is possible to create a larger work by combining the program with other software code not governed by the terms of this licence, and distribute the larger work as a single product."@en ;
    skos:exactMatch <https://opensource.org/licenses/CATOSL-1.1> ;
    skos:inScheme atold:licence ;
    skos:prefLabel "Computer Associates Trusted Open Source License 1.1 (CATOSL-1.1)"@en ;
    skos:topConceptOf atold:licence .

<http://publications.europa.eu/resource/authority/licence/CC0> a skos:Concept ;
    at:authority-code "CC0" ;
    at:deprecated "false" ;
    at:op-code "CC0" ;
    at:start.use "2009-03-11" ;
    atold:op-code "CC0" ;
    dc:identifier "CC0" ;
    skos:altLabel "CC0 1.0"@bg,
        "CC0 1.0"@cs,
        "CC0 1.0"@da,
        "CC0 1.0"@de,
        "CC0 1.0"@el,
        "CC0 1.0"@en,
        "CC0 1.0"@es,
        "CC0 1.0"@et,
        "CC0 1.0"@fi,
        "CC0 1.0"@fr,
        "CC0 1.0"@ga,
        "CC0 1.0"@hr,
        "CC0 1.0"@hu,
        "CC0 1.0"@it,
        "CC0 1.0"@lt,
        "CC0 1.0"@lv,
        "CC0 1.0"@mt,
        "CC0 1.0"@nl,
        "CC0 1.0"@pl,
        "CC0 1.0"@pt,
        "CC0 1.0"@ro,
        "CC0 1.0"@sk,
        "CC0 1.0"@sl,
        "CC0 1.0"@sv ;
    skos:definition "The person who associated a work with CC0 1.0 has dedicated the work to the public domain by waiving all of his or her rights to the work worldwide under copyright law, including all related and neighboring rights, to the extent allowed by law. One can copy, modify, distribute and perform the work, even for commercial purposes, all without asking permission."@en,
        "La personne qui a associé une œuvre à CC0 1.0 a dédié l’œuvre au domaine public en renonçant dans le monde entier à ses droits sur l’œuvre selon les lois sur le droit d’auteur, droit voisin et connexes, dans la mesure permise par la loi. On peut copier, modifier, distribuer et représenter l’œuvre, même à des fins commerciales, sans avoir besoin de demander l’autorisation."@fr ;
    skos:exactMatch <http://creativecommons.org/publicdomain/zero/1.0/> ;
    skos:inScheme atold:licence ;
    skos:prefLabel "Creative Commons CC0 1.0 Универсален"@bg,
        "Creative Commons CC0 1.0 Univerzální"@cs,
        "Creative Commons CC0 1.0 Universelt"@da,
        "Creative Commons CC0 1.0 Universell"@de,
        "Creative Commons CC0 1.0 Παγκόσμια"@el,
        "Creative Commons CC0 1.0 Universal"@en,
        "Creative Commons CC0 1.0 Universal"@es,
        "Creative Commons CC0 1.0 Üldine"@et,
        "Creative Commons CC0 1.0 Yleismaailmallinen"@fi,
        "Creative Commons CC0 1.0 Universel"@fr,
        "Creative Commons CC0 1.0 Univerzalno"@hr,
        "Creative Commons CC0 1.0 Univerzális"@hu,
        "Creative Commons CC0 1.0 Universal"@it,
        "Creative Commons CC0 1.0 Universali"@lt,
        "Creative Commons CC0 1.0 Universāls"@lv,
        "Creative Commons CC0 1.0 Universali"@mt,
        "Creative Commons CC0 1.0 Universeel"@nl,
        "Creative Commons CC0 1.0 Universal"@pl,
        "Creative Commons CC0 1.0 Universal"@pt,
        "Creative Commons CC0 1.0 Universal"@ro,
        "Creative Commons CC0 1.0 Univerzálne"@sk,
        "Creative Commons CC0 1.0 Univerzalna"@sl,
        "Creative Commons CC0 1.0 universell"@sv ;
    skos:topConceptOf atold:licence .

<http://publications.europa.eu/resource/authority/licence/CC_BY> a skos:Concept ;
    at:authority-code "CC_BY" ;
    at:deprecated "true" ;
    at:end.use "2013-11-26" ;
    at:op-code "CC_BY" ;
    at:start.use "2013-11-25" ;
    atold:op-code "CC_BY" ;
    dc:identifier "CC_BY" ;
    skos:altLabel "CC BY 4.0"@bg,
        "CC BY 4.0"@cs,
        "CC BY 4.0"@da,
        "CC BY 4.0"@de,
        "CC BY 4.0"@el,
        "CC BY 4.0"@en,
        "CC BY 4.0"@es,
        "CC BY 4.0"@et,
        "CC BY 4.0"@fi,
        "CC BY 4.0"@fr,
        "CC BY 4.0"@ga,
        "CC BY 4.0"@hr,
        "CC BY 4.0"@hu,
        "CC BY 4.0"@it,
        "CC BY 4.0"@lt,
        "CC BY 4.0"@lv,
        "CC BY 4.0"@mt,
        "CC BY 4.0"@nl,
        "CC BY 4.0"@pl,
        "CC BY 4.0"@pt,
        "CC BY 4.0"@ro,
        "CC BY 4.0"@sk,
        "CC BY 4.0"@sl,
        "CC BY 4.0"@sv ;
    skos:definition "This licence lets others distribute, remix, tweak, and build upon the author's work, even commercially, as long as they credit the author for the original creation. This is the most accommodating of licences offered. Recommended for maximum dissemination and use of licenced materials."@en,
        "Cette licence permet aux autres de distribuer, remixer, arranger, et adapter l’œuvre de l’auteur/autrice, même à des fins commerciales, tant qu’on accorde le mérite de la création originale à l’auteur/l’autrice en citant son nom. C’est le contrat le plus souple proposé. Recommandé pour la diffusion et l’utilisation maximales d’œuvres licenciées sous CC."@fr ;
    skos:inScheme atold:licence ;
    skos:prefLabel "Creative Commons Uveďte původ 4.0 Mezinárodní"@cs,
        "Creative Commons Navngivelse 4.0 International"@da,
        "Creative Commons Namensnennung 4.0 International"@de,
        "Creative Commons Αναφορά Δημιουργού 4.0 Διεθνές"@el,
        "Creative Commons Attribution 4.0 International"@en,
        "Creative Commons Atribución 4.0 Internacional"@es,
        "Creative Commons Nimeä 4.0 Kansainvälinen"@fi,
        "Creative Commons Attribution 4.0 International"@fr,
        "Creative Commons Imenovanje 4.0 međunarodna"@hr,
        "Creative Commons Nevezd meg! 4.0 Nemzetközi"@hu,
        "Creative Commons Attribuzione 4.0 Internazionale"@it,
        "Creative Commons Priskyrimas 4.0 Tarptautinė"@lt,
        "Creative Commons Atsaucoties 4.0 Internacionāls"@lv,
        "Creative Commons Naamsvermelding 4.0 Internationaal"@nl,
        "Creative Commons Uznanie autorstwa 4.0 Międzynarodowe"@pl,
        "Creative Commons Atribuição 4.0 Internacional"@pt,
        "Creative Commons Atribuire 4.0 Internațional"@ro,
        "Creative Commons Erkännande 4.0 Internationell"@sv ;
    skos:topConceptOf atold:licence .

<http://publications.europa.eu/resource/authority/licence/CC_BYNC> a skos:Concept ;
    at:authority-code "CC_BYNC" ;
    at:deprecated "true" ;
    at:end.use "2013-11-26" ;
    at:op-code "CC_BYNC" ;
    at:start.use "2013-11-25" ;
    atold:op-code "CC_BYNC" ;
    dc:identifier "CC_BYNC" ;
    skos:altLabel "CC BY-NC 4.0"@bg,
        "CC BY-NC 4.0"@cs,
        "CC BY-NC 4.0"@da,
        "CC BY-NC 4.0"@de,
        "CC BY-NC 4.0"@el,
        "CC BY-NC 4.0"@en,
        "CC BY-NC 4.0"@es,
        "CC BY-NC 4.0"@et,
        "CC BY-NC 4.0"@fi,
        "CC BY-NC 4.0"@fr,
        "CC BY-NC 4.0"@ga,
        "CC BY-NC 4.0"@hr,
        "CC BY-NC 4.0"@hu,
        "CC BY-NC 4.0"@it,
        "CC BY-NC 4.0"@lt,
        "CC BY-NC 4.0"@lv,
        "CC BY-NC 4.0"@mt,
        "CC BY-NC 4.0"@nl,
        "CC BY-NC 4.0"@pl,
        "CC BY-NC 4.0"@pt,
        "CC BY-NC 4.0"@ro,
        "CC BY-NC 4.0"@sk,
        "CC BY-NC 4.0"@sl,
        "CC BY-NC 4.0"@sv ;
    skos:definition "This licence lets others remix, tweak, and build upon the author's work non-commercially, and although their new works must also acknowledge the author and be non-commercial, they don’t have to licence their derivative works on the same terms."@en,
        "Cette licence permet aux autres de remixer, arranger, et adapter l’œuvre de l’auteur/autrice à des fins non commerciales et, bien que les nouvelles œuvres doivent créditer l’auteur/autrice en citant son nom et ne pas constituer une utilisation commerciale, elles n’ont pas à être diffusées selon les mêmes conditions."@fr ;
    skos:inScheme atold:licence ;
    skos:prefLabel "Creative Commons Uveďte původ–Neužívejte komerčně 4.0 Mezinárodní"@cs,
        "Creative Commons Navngivelse–IkkeKommerciel 4.0 International"@da,
        "Creative Commons Namensnennung – Nicht kommerziell 4.0 International"@de,
        "Creative Commons Αναφορά Δημιουργού – Μη Εμπορική Χρήση 4.0 Διεθνές"@el,
        "Creative Commons Attribution–NonCommercial 4.0 International"@en,
        "Creative Commons Atribución–NoComercial 4.0 Internacional"@es,
        "Creative Commons Nimeä–EiKaupallinen 4.0 Kansainvälinen"@fi,
        "Creative Commons Attribution – Pas d’Utilisation Commerciale 4.0 International"@fr,
        "Creative Commons Imenovanje–Nekomercijalno 4.0 međunarodna"@hr,
        "Creative Commons Nevezd meg! – Ne add el! 4.0 Nemzetközi"@hu,
        "Creative Commons Attribuzione – Non commerciale 4.0 Internazionale"@it,
        "Creative Commons Priskyrimas – Nekomercinis platinimas 4.0 Tarptautinė"@lt,
        "Creative Commons Atsaucoties–Nekomerciāli 4.0 Internacionāls"@lv,
        "Creative Commons Naamsvermelding–NietCommercieel 4.0 Internationaal"@nl,
        "Creative Commons Uznanie autorstwa–Użycie niekomercyjne 4.0 Międzynarodowe"@pl,
        "Creative Commons Atribuição–NãoComercial 4.0 Internacional"@pt,
        "Creative Commons Atribuire–Necomercial 4.0 Internațional"@ro,
        "Creative Commons Erkännande–IckeKommersiell 4.0 Internationell"@sv ;
    skos:topConceptOf atold:licence .

<http://publications.europa.eu/resource/authority/licence/CC_BYNCND> a skos:Concept ;
    at:authority-code "CC_BYNCND" ;
    at:deprecated "true" ;
    at:end.use "2013-11-26" ;
    at:op-code "CC_BYNCND" ;
    at:start.use "2013-11-25" ;
    atold:op-code "CC_BYNCND" ;
    dc:identifier "CC_BYNCND" ;
    skos:altLabel "CC BY-NC-ND 4.0"@bg,
        "CC BY-NC-ND 4.0"@cs,
        "CC BY-NC-ND 4.0"@da,
        "CC BY-NC-ND 4.0"@de,
        "CC BY-NC-ND 4.0"@el,
        "CC BY-NC-ND 4.0"@en,
        "CC BY-NC-ND 4.0"@es,
        "CC BY-NC-ND 4.0"@et,
        "CC BY-NC-ND 4.0"@fi,
        "CC BY-NC-ND 4.0"@fr,
        "CC BY-NC-ND 4.0"@ga,
        "CC BY-NC-ND 4.0"@hr,
        "CC BY-NC-ND 4.0"@hu,
        "CC BY-NC-ND 4.0"@it,
        "CC BY-NC-ND 4.0"@lt,
        "CC BY-NC-ND 4.0"@lv,
        "CC BY-NC-ND 4.0"@mt,
        "CC BY-NC-ND 4.0"@nl,
        "CC BY-NC-ND 4.0"@pl,
        "CC BY-NC-ND 4.0"@pt,
        "CC BY-NC-ND 4.0"@ro,
        "CC BY-NC-ND 4.0"@sk,
        "CC BY-NC-ND 4.0"@sl,
        "CC BY-NC-ND 4.0"@sv ;
    skos:definition "This licence is the most restrictive of the six main licences of Creative Commons, only allowing others to download the works and share them with others as long as they credit the author, but they can’t change them in any way or use them commercially."@en,
        "Cette licence est la plus restrictive des six licences principales de Creative Commons, n’autorisant les autres qu’à télécharger les œuvres de l’auteur/autrice et à les partager qu’on le/la crédite en citant son nom, mais on ne peut les modifier de quelque façon que ce soit ni les utiliser à des fins commerciales."@fr ;
    skos:inScheme atold:licence ;
    skos:prefLabel "Creative Commons Uveďte původ–Neužívejte komerčně–Nezpracovávejte 4.0 Mezinárodní"@cs,
        "Creative Commons Navngivelse–IkkeKommerciel–IngenBearbejdelse 4.0 International"@da,
        "Creative Commons Namensnennung – Nicht kommerziell – Keine Bearbeitungen 4.0 International"@de,
        "Creative Commons Αναφορά Δημιουργού – Μη Εμπορική Χρήση – Όχι Παράγωγα Έργα 4.0 Διεθνές"@el,
        "Creative Commons Attribution–NonCommercial–NoDerivatives 4.0 International"@en,
        "Creative Commons Atribución–NoComercial–SinDerivar 4.0 Internacional"@es,
        "Creative Commons Nimeä–EiKaupallinen–EiMuutoksia 4.0 Kansainvälinen"@fi,
        "Creative Commons Attribution – Pas d'Utilisation Commerciale – Pas de Modification 4.0 International"@fr,
        "Creative Commons Imenovanje–Nekomercijalno–Bez prerada 4.0 međunarodna"@hr,
        "Creative Commons Nevezd meg! – Ne add el! – Ne változtasd! 4.0 Nemzetközi"@hu,
        "Creative Commons Attribuzione – Non commerciale – Non opere derivate 4.0 Internazionale"@it,
        "Creative Commons Priskyrimas – Nekomercinis platinimas – Jokių išvestinių darbų 4.0 Tarptautinė"@lt,
        "Creative Commons Atsaucoties, nekomerciāli, nepārveidojot 4.0 Internacionāls"@lv,
        "Creative Commons Naamsvermelding–NietCommercieel–GeenAfgeleideWerken 4.0 Internationaal"@nl,
        "Creative Commons Uznanie autorstwa–Użycie niekomercyjne–Bez utworów zależnych 4.0 Międzynarodowe"@pl,
        "Creative Commons Atribuição–NãoComercial–SemDerivações 4.0 Internacional"@pt,
        "Creative Commons Atribuire–Necomercial–FărăDerivate 4.0 Internațional"@ro,
        "Creative Commons Erkännande–Ickekommersiell–IngaBearbetningar 4.0 Internationell"@sv ;
    skos:topConceptOf atold:licence .

<http://publications.europa.eu/resource/authority/licence/CC_BYNCND_1_0> a skos:Concept ;
    at:authority-code "CC_BYNCND_1_0" ;
    at:deprecated "true" ;
    at:end.use "2004-05-24" ;
    at:op-code "CC_BYNCND_1_0" ;
    at:start.use "2002-12-15" ;
    atold:op-code "CC_BYNCND_1_0" ;
    dc:identifier "CC_BYNCND_1_0" ;
    skos:altLabel "CC BY-ND-NC 1.0"@bg,
        "CC BY-ND-NC 1.0"@cs,
        "CC BY-ND-NC 1.0"@da,
        "CC BY-ND-NC 1.0"@de,
        "CC BY-ND-NC 1.0"@el,
        "CC BY-ND-NC 1.0"@en,
        "CC BY-ND-NC 1.0"@es,
        "CC BY-ND-NC 1.0"@et,
        "CC BY-ND-NC 1.0"@fi,
        "CC BY-ND-NC 1.0"@fr,
        "CC BY-ND-NC 1.0"@ga,
        "CC BY-ND-NC 1.0"@hr,
        "CC BY-ND-NC 1.0"@hu,
        "CC BY-ND-NC 1.0"@it,
        "CC BY-ND-NC 1.0"@lt,
        "CC BY-ND-NC 1.0"@lv,
        "CC BY-ND-NC 1.0"@mt,
        "CC BY-ND-NC 1.0"@nl,
        "CC BY-ND-NC 1.0"@pl,
        "CC BY-ND-NC 1.0"@pt,
        "CC BY-ND-NC 1.0"@ro,
        "CC BY-ND-NC 1.0"@sk,
        "CC BY-ND-NC 1.0"@sl,
        "CC BY-ND-NC 1.0"@sv ;
    skos:definition "CC BY-ND-NC 1.0 is the most restrictive of the six main licences of Creative Commons, only allowing others to download the works and share them with others as long as they credit the author, but they can’t change them in any way or use them commercially."@en,
        "CC BY-ND-NC 1.0 est la plus restrictive des six licences principales de Creative Commons, n’autorisant les autres qu’à télécharger les œuvres de l’auteur/autrice et à les partager tant qu’on le/la crédite en citant son nom, mais on ne peut les modifier de quelque façon que ce soit ni les utiliser à des fins commerciales."@fr ;
    skos:exactMatch <http://creativecommons.org/licenses/by-nd-nc/1.0/> ;
    skos:inScheme atold:licence ;
    skos:prefLabel "Creative Commons Признание-Без производни-Некомерсиално 1.0 Неадаптиран"@bg,
        "Creative Commons Uveďte původ–Nezpracovávejte–Neužívejte komerčně 1.0 Generic"@cs,
        "Creative Commons Navngivelse–IngenBearbejdelse–IkkeKommerciel 1.0 Generisk"@da,
        "Creative Commons Namensnennung – Keine Bearbeitungen – Nicht-kommerziell 1.0 Generic"@de,
        "Creative Commons Αναφορά Δημιουργού – Όχι Παράγωγα Έργα – Μη Εμπορική Χρήση 1.0 Γενικό"@el,
        "Creative Commons Attribution–NoDerivs–NonCommercial 1.0 Generic"@en,
        "Creative Commons Atribución–SinDerivadas–NoComercial 1.0 Genérica"@es,
        "Creative Commons Autorile viitamine–Tuletatud teoste keeld–Mitteäriline eesmärk 1.0 Üldine"@et,
        "Creative Commons Nimeä–EiMuutoksia–EiKaupallinen 1.0 Yleinen"@fi,
        "Creative Commons Attribution – Pas de Modification – Pas d’Utilisation Commerciale 1.0 Générique"@fr,
        "Creative Commons Imenovanje–Bez prerada–Nekomercijalno 1.0 nelokalizirana licenca"@hr,
        "Creative Commons Nevezd meg! – Ne változtasd! – Ne add el! 1.0 Általános"@hu,
        "Creative Commons Attribuzione – Non opere derivate – Non commerciale 1.0 Generico"@it,
        "Creative Commons Priskyrimas – Jokių išvestinių darbų – Nekomercinis platinimas 1.0 Bendrasis"@lt,
        "Creative Commons Atsaucoties–Nepārveidojot–Nekomerciāli 1.0 Vispārīgs"@lv,
        "Creative Commons Attribuzzjoni-EbdaDerivattivi-MhuxKummerċjali 1.0 Generic"@mt,
        "Creative Commons Naamsvermelding–GeenAfgeleideWerken–NietCommercieel 1.0 Unported"@nl,
        "Creative Commons Uznanie autorstwa–Bez utworów zależnych–Użycie Niekomercyjne 1.0 Ogólny"@pl,
        "Creative Commons Atribuição–SemDerivações–NãoComercial 1.0 Genérica"@pt,
        "Creative Commons Atribuire–FărăModificări–Necomercial 1.0 Generică"@ro,
        "Creative Commons Uvedenie Autora-Bez Odvodeného Obsahu-Nekomerčné Použitie 1.0 Generic"@sk,
        "Creative Commons Priznanje avtorstva-Brez predelav-Nekomercialno 1.0 Generična"@sl,
        "Creative Commons Erkännande–IngaBearbetningar–IckeKommersiell 1.0 Generisk"@sv ;
    skos:topConceptOf atold:licence .

<http://publications.europa.eu/resource/authority/licence/CC_BYNCND_2_0> a skos:Concept ;
    at:authority-code "CC_BYNCND_2_0" ;
    at:deprecated "false" ;
    at:op-code "CC_BYNCND_2_0" ;
    at:start.use "2004-05-25" ;
    atold:op-code "CC_BYNCND_2_0" ;
    dc:identifier "CC_BYNCND_2_0" ;
    skos:altLabel "CC BY-NC-ND 2.0"@bg,
        "CC BY-NC-ND 2.0"@cs,
        "CC BY-NC-ND 2.0"@da,
        "CC BY-NC-ND 2.0"@de,
        "CC BY-NC-ND 2.0"@el,
        "CC BY-NC-ND 2.0"@en,
        "CC BY-NC-ND 2.0"@es,
        "CC BY-NC-ND 2.0"@et,
        "CC BY-NC-ND 2.0"@fi,
        "CC BY-NC-ND 2.0"@fr,
        "CC BY-NC-ND 2.0"@ga,
        "CC BY-NC-ND 2.0"@hr,
        "CC BY-NC-ND 2.0"@hu,
        "CC BY-NC-ND 2.0"@it,
        "CC BY-NC-ND 2.0"@lt,
        "CC BY-NC-ND 2.0"@lv,
        "CC BY-NC-ND 2.0"@mt,
        "CC BY-NC-ND 2.0"@nl,
        "CC BY-NC-ND 2.0"@pl,
        "CC BY-NC-ND 2.0"@pt,
        "CC BY-NC-ND 2.0"@ro,
        "CC BY-NC-ND 2.0"@sk,
        "CC BY-NC-ND 2.0"@sl,
        "CC BY-NC-ND 2.0"@sv ;
    skos:definition "CC BY-ND-NC 2.0 is the most restrictive of the six main licences of Creative Commons, only allowing others to download the works and share them with others as long as they credit the author, but they can’t change them in any way or use them commercially."@en,
        "CC BY-ND-NC 2.0 est la plus restrictive des six licences principales de Creative Commons, n’autorisant les autres qu’à télécharger les œuvres de l’auteur/autrice et à les partager tant qu’on le/la crédite en citant son nom, mais on ne peut les modifier de quelque façon que ce soit ni les utiliser à des fins commerciales."@fr ;
    skos:exactMatch <http://creativecommons.org/licenses/by-nc-nd/2.0/> ;
    skos:inScheme atold:licence ;
    skos:prefLabel "Creative Commons Признание-Без производни-Некомерсиално 2.0 Неадаптиран"@bg,
        "Creative Commons Uveďte původ–Neužívejte komerčně–Nezpracovávejte 2.0 Generic"@cs,
        "Creative Commons Navngivelse–IkkeKommerciel–IngenBearbejdelse 2.0 Generisk"@da,
        "Creative Commons Namensnennung – Nicht-kommerziell – Keine Bearbeitung 2.0 Generic"@de,
        "Creative Commons Αναφορά Δημιουργού – Μη Εμπορική Χρήση – Όχι Παράγωγα Έργα 2.0 Γενικό"@el,
        "Creative Commons Attribution–NonCommercial–NoDerivs 2.0 Generic"@en,
        "Creative Commons Atribución–NoComercial–SinDerivadas 2.0 Genérica"@es,
        "Creative Commons Autorile viitamine–Mitteäriline eesmärk–Tuletatud teoste keeld 2.0 Üldine"@et,
        "Creative Commons Nimeä–EiKaupallinen–EiMuutoksia 2.0 Yleinen"@fi,
        "Creative Commons Attribution – Pas d’Utilisation Commerciale – Pas de Modification 2.0 Générique"@fr,
        "Creative Commons Imenovanje–Nekomercijalno–Bez prerada 2.0 nelokalizirana licenca"@hr,
        "Creative Commons Nevezd meg! – Ne add el! – Ne változtasd! 2.0 Általános"@hu,
        "Creative Commons Attribuzione – Non commerciale – Non opere derivate 2.0 Generico"@it,
        "Creative Commons Priskyrimas – Nekomercinis platinimas – Jokių išvestinių darbų 2.0 Bendrasis"@lt,
        "Creative Commons Atsaucoties–Nekomerciāli–Nepārveidojot 2.0 Vispārīgs"@lv,
        "Creative Commons Attribuzzjoni-MhuxKummerċjali-EbdaDerivattivi 2.0 Generic"@mt,
        "Creative Commons Naamsvermelding–NietCommercieel–GeenAfgeleideWerken 2.0 Unported"@nl,
        "Creative Commons Uznanie autorstwa–Użycie niekomercyjne–Bez utworów zależnych 2.0 Ogólny"@pl,
        "Creative Commons Atribuição–NãoComercial–SemDerivações 2.0 Genérica"@pt,
        "Creative Commons Atribuire–Necomercial–FărăModificări 2.0 Generică"@ro,
        "Creative Commons Uvedenie Autora-Nekomerčné Použitie-Bez Odvodeného Obsahu 2.0 Generic"@sk,
        "Creative Commons Priznanje avtorstva-Nekomercialno-Brez predelav 2.0 Generična"@sl,
        "Creative Commons Erkännande–Ickekommersiell–IngaBearbetningar 2.0 Generisk"@sv ;
    skos:topConceptOf atold:licence .

<http://publications.europa.eu/resource/authority/licence/CC_BYNCND_2_5> a skos:Concept ;
    at:authority-code "CC_BYNCND_2_5" ;
    at:deprecated "false" ;
    at:op-code "CC_BYNCND_2_5" ;
    at:start.use "2005-06-01" ;
    atold:op-code "CC_BYNCND_2_5" ;
    dc:identifier "CC_BYNCND_2_5" ;
    skos:altLabel "CC BY-NC-ND 2.5"@bg,
        "CC BY-NC-ND 2.5"@cs,
        "CC BY-NC-ND 2.5"@da,
        "CC BY-NC-ND 2.5"@de,
        "CC BY-NC-ND 2.5"@el,
        "CC BY-NC-ND 2.5"@en,
        "CC BY-NC-ND 2.5"@es,
        "CC BY-NC-ND 2.5"@et,
        "CC BY-NC-ND 2.5"@fi,
        "CC BY-NC-ND 2.5"@fr,
        "CC BY-NC-ND 2.5"@ga,
        "CC BY-NC-ND 2.5"@hr,
        "CC BY-NC-ND 2.5"@hu,
        "CC BY-NC-ND 2.5"@it,
        "CC BY-NC-ND 2.5"@lt,
        "CC BY-NC-ND 2.5"@lv,
        "CC BY-NC-ND 2.5"@mt,
        "CC BY-NC-ND 2.5"@nl,
        "CC BY-NC-ND 2.5"@pl,
        "CC BY-NC-ND 2.5"@pt,
        "CC BY-NC-ND 2.5"@ro,
        "CC BY-NC-ND 2.5"@sk,
        "CC BY-NC-ND 2.5"@sl,
        "CC BY-NC-ND 2.5"@sv ;
    skos:definition "CC BY-ND-NC 2.5 is the most restrictive of the six main licences of Creative Commons, only allowing others to download the works and share them with others as long as they credit the author, but they can’t change them in any way or use them commercially."@en,
        "CC BY-ND-NC 2.5 est la plus restrictive des six licences principales de Creative Commons, n’autorisant les autres qu’à télécharger les œuvres de l’auteur/autrice et à les partager tant qu’on le/la crédite en citant son nom, mais on ne peut les modifier de quelque façon que ce soit ni les utiliser à des fins commerciales."@fr ;
    skos:exactMatch <http://creativecommons.org/licenses/by-nc-nd/2.5/> ;
    skos:inScheme atold:licence ;
    skos:prefLabel "Creative Commons Признание-Без производни-Некомерсиално 2.5 Неадаптиран"@bg,
        "Creative Commons Uveďte původ–Neužívejte komerčně–Nezpracovávejte 2.5 Generic"@cs,
        "Creative Commons Navngivelse–IkkeKommerciel–IngenBearbejdelse 2.5 Generisk"@da,
        "Creative Commons Namensnennung – Nicht-kommerziell – Keine Bearbeitung 2.5 Generic"@de,
        "Creative Commons Αναφορά Δημιουργού – Μη Εμπορική Χρήση – Όχι Παράγωγα Έργα 2.5 Γενικό"@el,
        "Creative Commons Attribution–NonCommercial–NoDerivs 2.5 Generic"@en,
        "Creative Commons Atribución–NoComercial–SinDerivadas 2.5 Genérica"@es,
        "Creative Commons Autorile viitamine–Mitteäriline eesmärk–Tuletatud teoste keeld 2.5 Üldine"@et,
        "Creative Commons Nimeä–EiKaupallinen–EiMuutoksia 2.5 Yleinen"@fi,
        "Creative Commons Attribution – Pas d’Utilisation Commerciale – Pas de Modification 2.5 Générique"@fr,
        "Creative Commons Imenovanje–Nekomercijalno–Bez prerada 2.5 nelokalizirana licenca"@hr,
        "Creative Commons Nevezd meg! – Ne add el! – Ne változtasd! 2.5 Általános"@hu,
        "Creative Commons Attribuzione – Non commerciale – Non opere derivate 2.5 Generico"@it,
        "Creative Commons Priskyrimas – Nekomercinis platinimas – Jokių išvestinių darbų 2.5 Bendrasis"@lt,
        "Creative Commons Atsaucoties–Nekomerciāli–Nepārveidojot 2.5 Vispārīgs"@lv,
        "Creative Commons Attribuzzjoni-MhuxKummerċjali-EbdaDerivattivi 2.5 Generic"@mt,
        "Creative Commons Naamsvermelding–NietCommercieel–GeenAfgeleideWerken 2.5 Unported"@nl,
        "Creative Commons Uznanie autorstwa–Użycie niekomercyjne–Bez utworów zależnych 2.5 Ogólny"@pl,
        "Creative Commons Atribuição–NãoComercial–SemDerivações 2.5 Genérica"@pt,
        "Creative Commons Atribuire–Necomercial–FărăModificări 2.5 Generică"@ro,
        "Creative Commons Uvedenie Autora-Nekomerčné Použitie-Bez Odvodeného Obsahu 2.5 Generic"@sk,
        "Creative Commons Priznanje avtorstva-Nekomercialno-Brez predelav 2.5 Generična"@sl,
        "Creative Commons Erkännande–Ickekommersiell–IngaBearbetningar 2.5 Generisk"@sv ;
    skos:topConceptOf atold:licence .

<http://publications.europa.eu/resource/authority/licence/CC_BYNCND_3_0> a skos:Concept ;
    at:authority-code "CC_BYNCND_3_0" ;
    at:deprecated "false" ;
    at:op-code "CC_BYNCND_3_0" ;
    at:start.use "2007-02-23" ;
    atold:op-code "CC_BYNCND_3_0" ;
    dc:identifier "CC_BYNCND_3_0" ;
    skos:altLabel "CC BY-NC-ND 3.0"@bg,
        "CC BY-NC-ND 3.0"@cs,
        "CC BY-NC-ND 3.0"@da,
        "CC BY-NC-ND 3.0"@de,
        "CC BY-NC-ND 3.0"@el,
        "CC BY-NC-ND 3.0"@en,
        "CC BY-NC-ND 3.0"@es,
        "CC BY-NC-ND 3.0"@et,
        "CC BY-NC-ND 3.0"@fi,
        "CC BY-NC-ND 3.0"@fr,
        "CC BY-NC-ND 3.0"@ga,
        "CC BY-NC-ND 3.0"@hr,
        "CC BY-NC-ND 3.0"@hu,
        "CC BY-NC-ND 3.0"@it,
        "CC BY-NC-ND 3.0"@lt,
        "CC BY-NC-ND 3.0"@lv,
        "CC BY-NC-ND 3.0"@mt,
        "CC BY-NC-ND 3.0"@nl,
        "CC BY-NC-ND 3.0"@pl,
        "CC BY-NC-ND 3.0"@pt,
        "CC BY-NC-ND 3.0"@ro,
        "CC BY-NC-ND 3.0"@sk,
        "CC BY-NC-ND 3.0"@sl,
        "CC BY-NC-ND 3.0"@sv ;
    skos:definition "CC BY-ND-NC 3.0 is the most restrictive of the six main licences of Creative Commons, only allowing others to download the works and share them with others as long as they credit the author, but they can’t change them in any way or use them commercially."@en,
        "CC BY-ND-NC 3.0 est la plus restrictive des six licences principales de Creative Commons, n’autorisant les autres qu’à télécharger les œuvres de l’auteur/autrice et à les partager tant qu’on le/la crédite en citant son nom, mais on ne peut les modifier de quelque façon que ce soit ni les utiliser à des fins commerciales."@fr ;
    skos:exactMatch <http://creativecommons.org/licenses/by-nc-nd/3.0/> ;
    skos:historyNote "Unported licences are licences that are not associated with any specific jurisdiction, e.g. country."@en ;
    skos:inScheme atold:licence ;
    skos:prefLabel "Creative Commons Признание-Некомерсиално-Без производни 3.0 Нелокализиран"@bg,
        "Creative Commons Uveďte původ–Neužívejte komerčně–Nezpracovávejte 3.0 Unported"@cs,
        "Creative Commons Navngivelse–IkkeKommerciel–IngenBearbejdelse 3.0 Unported"@da,
        "Creative Commons Namensnennung – Nicht-kommerziell – Keine Bearbeitung 3.0 Unported"@de,
        "Creative Commons Αναφορά Δημιουργού – Μη Εμπορική Χρήση – Όχι Παράγωγα Έργα 3.0 Μη εισαγόμενο"@el,
        "Creative Commons Attribution–NonCommercial–NoDerivs 3.0 Unported"@en,
        "Creative Commons Atribución–NoComercial–SinDerivadas 3.0 Unported"@es,
        "Creative Commons Autorile viitamine–Mitteäriline eesmärk–Tuletatud teoste keeld 3.0 Jurisdiktsiooniga sidumata"@et,
        "Creative Commons Nimeä–EiKaupallinen–EiMuutoksia 3.0 Ei sovitettu"@fi,
        "Creative Commons Attribution – Pas d’Utilisation Commerciale – Pas de Modification 3.0 non transposé"@fr,
        "Creative Commons Imenovanje–Nekomercijalno–Bez prerada 3.0 nelokalizirana licenca"@hr,
        "Creative Commons Nevezd meg! – Ne add el! – Ne változtasd! 3.0 Unported"@hu,
        "Creative Commons Attribuzione – Non commerciale – Non opere derivate 3.0 Unported"@it,
        "Creative Commons Priskyrimas – Nekomercinis platinimas – Jokių išvestinių darbų 3.0 Nepritaikyta jurisdikcijai"@lt,
        "Creative Commons Atsaucoties–Nekomerciāli–Nepārveidojot 3.0 Nepārnesta"@lv,
        "Creative Commons Attribuzzjoni-MhuxKummerċjali-EbdaDerivattivi 3.0 Unported"@mt,
        "Creative Commons Naamsvermelding–NietCommercieel–GeenAfgeleideWerken 3.0 Unported"@nl,
        "Creative Commons Uznanie autorstwa–Użycie niekomercyjne–Bez utworów zależnych 3.0 Unported"@pl,
        "Creative Commons Atribuição–NãoComercial–SemDerivações 3.0 Não Adaptada"@pt,
        "Creative Commons Atribuire–Necomercial–FărăModificări 3.0 Ne-adaptată"@ro,
        "Creative Commons Uvedenie Autora-Nekomerčné Použitie-Bez Odvodeného Obsahu 3.0 Unported"@sk,
        "Creative Commons Priznanje avtorstva-Nekomercialno-Brez predelav 3.0 Nedoločena"@sl,
        "Creative Commons Erkännande–Ickekommersiell–IngaBearbetningar 3.0 Unported"@sv ;
    skos:topConceptOf atold:licence .

<http://publications.europa.eu/resource/authority/licence/CC_BYNCND_4_0> a skos:Concept ;
    at:authority-code "CC_BYNCND_4_0" ;
    at:deprecated "false" ;
    at:op-code "CC_BYNCND_4_0" ;
    at:start.use "2013-11-26" ;
    atold:op-code "CC_BYNCND_4_0" ;
    dc:identifier "CC_BYNCND_4_0" ;
    skos:altLabel "CC BY-NC-ND 4.0"@bg,
        "CC BY-NC-ND 4.0"@cs,
        "CC BY-NC-ND 4.0"@da,
        "CC BY-NC-ND 4.0"@de,
        "CC BY-NC-ND 4.0"@el,
        "CC BY-NC-ND 4.0"@en,
        "CC BY-NC-ND 4.0"@es,
        "CC BY-NC-ND 4.0"@et,
        "CC BY-NC-ND 4.0"@fi,
        "CC BY-NC-ND 4.0"@fr,
        "CC BY-NC-ND 4.0"@ga,
        "CC BY-NC-ND 4.0"@hr,
        "CC BY-NC-ND 4.0"@hu,
        "CC BY-NC-ND 4.0"@it,
        "CC BY-NC-ND 4.0"@lt,
        "CC BY-NC-ND 4.0"@lv,
        "CC BY-NC-ND 4.0"@mt,
        "CC BY-NC-ND 4.0"@nl,
        "CC BY-NC-ND 4.0"@pl,
        "CC BY-NC-ND 4.0"@pt,
        "CC BY-NC-ND 4.0"@ro,
        "CC BY-NC-ND 4.0"@sk,
        "CC BY-NC-ND 4.0"@sl,
        "CC BY-NC-ND 4.0"@sv ;
    skos:definition "CC BY-ND-NC 4.0 is the most restrictive of the six main licences of Creative Commons, only allowing others to download the works and share them with others as long as they credit the author, but they can’t change them in any way or use them commercially."@en,
        "CC BY-ND-NC 4.0 est la plus restrictive des six licences principales de Creative Commons, n’autorisant les autres qu’à télécharger les œuvres de l’auteur/autrice et à les partager tant qu’on le/la crédite en citant son nom, mais on ne peut les modifier de quelque façon que ce soit ni les utiliser à des fins commerciales."@fr ;
    skos:exactMatch <http://creativecommons.org/licenses/by-nc-nd/4.0/> ;
    skos:inScheme atold:licence ;
    skos:prefLabel "Creative Commons Признание-Некомерсиално-Без производни 4.0 Международен"@bg,
        "Creative Commons Uveďte původ–Neužívejte komerčně–Nezpracovávejte 4.0 Mezinárodní"@cs,
        "Creative Commons Navngivelse–IkkeKommerciel–IngenBearbejdelse 4.0 International"@da,
        "Creative Commons Namensnennung – Nicht kommerziell – Keine Bearbeitungen 4.0 International"@de,
        "Creative Commons Αναφορά Δημιουργού – Μη Εμπορική Χρήση – Όχι Παράγωγα Έργα 4.0 Διεθνές"@el,
        "Creative Commons Attribution–NonCommercial–NoDerivatives 4.0 International"@en,
        "Creative Commons Atribución–NoComercial–SinDerivar 4.0 Internacional"@es,
        "Creative Commons Autorile viitamine–Mitteäriline eesmärk–Tuletatud teoste keeld 4.0 Rahvusvaheline"@et,
        "Creative Commons Nimeä–EiKaupallinen–EiMuutoksia 4.0 Kansainvälinen"@fi,
        "Creative Commons Attribution – Pas d'Utilisation Commerciale – Pas de Modification 4.0 International"@fr,
        "Creative Commons Imenovanje–Nekomercijalno–Bez prerada 4.0 međunarodna"@hr,
        "Creative Commons Nevezd meg! – Ne add el! – Ne változtasd! 4.0 Nemzetközi"@hu,
        "Creative Commons Attribuzione – Non commerciale – Non opere derivate 4.0 Internazionale"@it,
        "Creative Commons Priskyrimas – Nekomercinis platinimas – Jokių išvestinių darbų 4.0 Tarptautinė"@lt,
        "Creative Commons Atsaucoties, nekomerciāli, nepārveidojot 4.0 Internacionāls"@lv,
        "Creative Commons Attribuzzjoni-MhuxKummerċjali-EbdaDerivattivi 4.0 Unported"@mt,
        "Creative Commons Naamsvermelding–NietCommercieel–GeenAfgeleideWerken 4.0 Internationaal"@nl,
        "Creative Commons Uznanie autorstwa–Użycie niekomercyjne–Bez utworów zależnych 4.0 Międzynarodowe"@pl,
        "Creative Commons Atribuição–NãoComercial–SemDerivações 4.0 Internacional"@pt,
        "Creative Commons Atribuire–Necomercial–FărăDerivate 4.0 Internațional"@ro,
        "Creative Commons Uvedenie Autora-Nekomerčné Použitie-Žiadne Odvodené Diela 4.0 Medzinárodný"@sk,
        "Creative Commons Priznanje avtorstva-Nekomercialno-Brez predelav 4.0 Mednarodna"@sl,
        "Creative Commons Erkännande–Ickekommersiell–IngaBearbetningar 4.0 Internationell"@sv ;
    skos:topConceptOf atold:licence .

<http://publications.europa.eu/resource/authority/licence/CC_BYNCSA> a skos:Concept ;
    at:authority-code "CC_BYNCSA" ;
    at:deprecated "true" ;
    at:end.use "2013-11-26" ;
    at:op-code "CC_BYNCSA" ;
    at:start.use "2013-11-25" ;
    atold:op-code "CC_BYNCSA" ;
    dc:identifier "CC_BYNCSA" ;
    skos:altLabel "CC BY-NC-SA 4.0"@bg,
        "CC BY-NC-SA 4.0"@cs,
        "CC BY-NC-SA 4.0"@da,
        "CC BY-NC-SA 4.0"@de,
        "CC BY-NC-SA 4.0"@el,
        "CC BY-NC-SA 4.0"@en,
        "CC BY-NC-SA 4.0"@es,
        "CC BY-NC-SA 4.0"@et,
        "CC BY-NC-SA 4.0"@fi,
        "CC BY-NC-SA 4.0"@fr,
        "CC BY-NC-SA 4.0"@ga,
        "CC BY-NC-SA 4.0"@hr,
        "CC BY-NC-SA 4.0"@hu,
        "CC BY-NC-SA 4.0"@it,
        "CC BY-NC-SA 4.0"@lt,
        "CC BY-NC-SA 4.0"@lv,
        "CC BY-NC-SA 4.0"@mt,
        "CC BY-NC-SA 4.0"@nl,
        "CC BY-NC-SA 4.0"@pl,
        "CC BY-NC-SA 4.0"@pt,
        "CC BY-NC-SA 4.0"@ro,
        "CC BY-NC-SA 4.0"@sk,
        "CC BY-NC-SA 4.0"@sl,
        "CC BY-NC-SA 4.0"@sv ;
    skos:definition "This licence lets others remix, tweak, and build upon the author’s work non-commercially, as long as they credit the author and licence their new creations under the identical terms."@en,
        "Cette licence permet aux autres de remixer, arranger, et adapter l’œuvre de l’auteur/autrice à des fins non commerciales tant qu’on le/la crédite en citant son nom et que les nouvelles œuvres sont diffusées selon les mêmes conditions."@fr ;
    skos:inScheme atold:licence ;
    skos:prefLabel "Creative Commons Uveďte původ–Neužívejte dílo komerčně–Zachovejte licenci 4.0 Mezinárodní"@cs,
        "Creative Commons Navngivelse–IkkeKommerciel–DelPåSammeVilkår 4.0 International"@da,
        "Creative Commons Namensnennung – Nicht-kommerziell – Weitergabe unter gleichen Bedingungen 4.0 International"@de,
        "Creative Commons Αναφορά Δημιουργού – Μη Εμπορική Χρήση – Παρόμοια Διανομή 4.0 Διεθνές"@el,
        "Creative Commons Attribution–NonCommercial–ShareAlike 4.0 International"@en,
        "Creative Commons Atribución–NoComercial–CompartirIgual 4.0 Internacional"@es,
        "Creative Commons Nimeä–EiKaupallinen–JaaSamoin 4.0 Kansainvälinen"@fi,
        "Creative Commons Attribution – Pas d’Utilisation Commerciale – Partage dans les Mêmes Conditions 4.0 International"@fr,
        "Creative Commons Imenovanje–Nekomercijalno–Dijeli pod istim uvjetima 4.0 međunarodna"@hr,
        "Creative Commons Nevezd meg! – Ne add el! – Így add tovább! 4.0 Nemzetközi"@hu,
        "Creative Commons Attribuzione – Non commerciale – Condividi allo stesso modo 4.0 Internazionale"@it,
        "Creative Commons Priskyrimas – Nekomercinis platinimas – Analogiškas platinimas 4.0 Tarptautinė"@lt,
        "Creative Commons Atsaucoties–Nekomerciāli–Nemainot licenci 4.0 Internacionāls"@lv,
        "Creative Commons Naamsvermelding–NietCommercieel–GelijkDelen 4.0 Internationaal"@nl,
        "Creative Commons Uznanie autorstwa–Użycie niekomercyjne–Na tych samych warunkach 4.0 Międzynarodowe"@pl,
        "Creative Commons Atribuição–NãoComercial–CompartilhaIgual 4.0 Internacional"@pt,
        "Creative Commons Atribuire–Necomercial–Distribuire în Condiţii Identice 4.0 Internațional"@ro,
        "Creative Commons Erkännande–IckeKommersiell–DelaLika 4.0 Internationell"@sv ;
    skos:topConceptOf atold:licence .

<http://publications.europa.eu/resource/authority/licence/CC_BYNCSA_1_0> a skos:Concept ;
    at:authority-code "CC_BYNCSA_1_0" ;
    at:deprecated "true" ;
    at:end.use "2004-05-24" ;
    at:op-code "CC_BYNCSA_1_0" ;
    at:start.use "2002-12-15" ;
    atold:op-code "CC_BYNCSA_1_0" ;
    dc:identifier "CC_BYNCSA_1_0" ;
    skos:altLabel "CC BY-NC-SA 1.0"@bg,
        "CC BY-NC-SA 1.0"@cs,
        "CC BY-NC-SA 1.0"@da,
        "CC BY-NC-SA 1.0"@de,
        "CC BY-NC-SA 1.0"@el,
        "CC BY-NC-SA 1.0"@en,
        "CC BY-NC-SA 1.0"@es,
        "CC BY-NC-SA 1.0"@et,
        "CC BY-NC-SA 1.0"@fi,
        "CC BY-NC-SA 1.0"@fr,
        "CC BY-NC-SA 1.0"@ga,
        "CC BY-NC-SA 1.0"@hr,
        "CC BY-NC-SA 1.0"@hu,
        "CC BY-NC-SA 1.0"@it,
        "CC BY-NC-SA 1.0"@lt,
        "CC BY-NC-SA 1.0"@lv,
        "CC BY-NC-SA 1.0"@mt,
        "CC BY-NC-SA 1.0"@nl,
        "CC BY-NC-SA 1.0"@pl,
        "CC BY-NC-SA 1.0"@pt,
        "CC BY-NC-SA 1.0"@ro,
        "CC BY-NC-SA 1.0"@sk,
        "CC BY-NC-SA 1.0"@sl,
        "CC BY-NC-SA 1.0"@sv ;
    skos:definition "CC BY-NC-SA 1.0 lets others remix, tweak, and build upon the author’s work non-commercially, as long as they credit the author and licence their new creations under the identical terms."@en,
        "CC BY-NC-SA 1.0 permet aux autres de remixer, arranger, et adapter l’œuvre de l’auteur/autrice à des fins non commerciales tant qu’on le/la crédite en citant son nom et que les nouvelles œuvres sont diffusées selon les mêmes conditions."@fr ;
    skos:exactMatch <http://creativecommons.org/licenses/by-nc-sa/1.0/> ;
    skos:inScheme atold:licence ;
    skos:prefLabel "Creative Commons Признание-Некомерсиално-Споделяне на споделеното 1.0 Неадаптиран"@bg,
        "Creative Commons Uveďte původ–Neužívejte dílo komerčně–Zachovejte licenci 1.0 Generic"@cs,
        "Creative Commons Navngivelse–IkkeKommerciel–DelPåSammeVilkår 1.0 Generisk"@da,
        "Creative Commons Namensnennung – Nicht-kommerziell – Weitergabe unter gleichen Bedingungen 1.0 Generic"@de,
        "Creative Commons Αναφορά Δημιουργού – Μη Εμπορική Χρήση – Παρόμοια Διανομή 1.0 Γενικό"@el,
        "Creative Commons Attribution–NonCommercial–ShareAlike 1.0 Generic"@en,
        "Creative Commons Atribución–NoComercial–CompartirIgual 1.0 Genérica"@es,
        "Creative Commons Autorile viitamine–Mitteäriline eesmärk–Jagamine samadel tingimustel 1.0 Üldine"@et,
        "Creative Commons Nimeä–EiKaupallinen–JaaSamoin 1.0 Yleinen"@fi,
        "Creative Commons Attribution – Pas d’Utilisation Commerciale – Partage dans les Mêmes Conditions 1.0 Générique"@fr,
        "Creative Commons Imenovanje–Nekomercijalno–Dijeli pod istim uvjetima 1.0 nelokalizirana licenca"@hr,
        "Creative Commons Nevezd meg! – Ne add el! – Így add tovább! 1.0 Általános"@hu,
        "Creative Commons Attribuzione – Non commerciale – Condividi allo stesso modo 1.0 Generico"@it,
        "Creative Commons Priskyrimas – Nekomercinis platinimas – Analogiškas platinimas 1.0 Bendrasis"@lt,
        "Creative Commons Atsaucoties–Nekomerciāli–Nemainot licenci 1.0 Vispārīgs"@lv,
        "Creative Commons Attribuzzjoni-MhuxKummerċjali-KondiviżjoniUgwali 1.0 Generic"@mt,
        "Creative Commons Naamsvermelding–NietCommercieel–GelijkDelen 1.0 Unported"@nl,
        "Creative Commons Uznanie autorstwa–Użycie niekomercyjne–Na tych samych warunkach 1.0 Ogólny"@pl,
        "Creative Commons Atribuição–NãoComercial–CompartilhaIgual 1.0 Genérica"@pt,
        "Creative Commons Atribuire–Necomercial–Distribuire în Condiţii Identice 1.0 Generică"@ro,
        "Creative Commons Uvedenie Autora-Nekomerčné Použitie-Rovnaké Šírenie 1.0 Generic"@sk,
        "Creative Commons Priznanje avtorstva-Nekomercialno-Deljenje pod enakimi pogoji 1.0 Generična"@sl,
        "Creative Commons Erkännande–IckeKommersiell–DelaLika 1.0 Generisk"@sv ;
    skos:topConceptOf atold:licence .

<http://publications.europa.eu/resource/authority/licence/CC_BYNCSA_2_0> a skos:Concept ;
    at:authority-code "CC_BYNCSA_2_0" ;
    at:deprecated "false" ;
    at:op-code "CC_BYNCSA_2_0" ;
    at:start.use "2004-05-25" ;
    atold:op-code "CC_BYNCSA_2_0" ;
    dc:identifier "CC_BYNCSA_2_0" ;
    skos:altLabel "CC BY-NC-SA 2.0"@bg,
        "CC BY-NC-SA 2.0"@cs,
        "CC BY-NC-SA 2.0"@da,
        "CC BY-NC-SA 2.0"@de,
        "CC BY-NC-SA 2.0"@el,
        "CC BY-NC-SA 2.0"@en,
        "CC BY-NC-SA 2.0"@es,
        "CC BY-NC-SA 2.0"@et,
        "CC BY-NC-SA 2.0"@fi,
        "CC BY-NC-SA 2.0"@fr,
        "CC BY-NC-SA 2.0"@ga,
        "CC BY-NC-SA 2.0"@hr,
        "CC BY-NC-SA 2.0"@hu,
        "CC BY-NC-SA 2.0"@it,
        "CC BY-NC-SA 2.0"@lt,
        "CC BY-NC-SA 2.0"@lv,
        "CC BY-NC-SA 2.0"@mt,
        "CC BY-NC-SA 2.0"@nl,
        "CC BY-NC-SA 2.0"@pl,
        "CC BY-NC-SA 2.0"@pt,
        "CC BY-NC-SA 2.0"@ro,
        "CC BY-NC-SA 2.0"@sk,
        "CC BY-NC-SA 2.0"@sl,
        "CC BY-NC-SA 2.0"@sv ;
    skos:definition "CC BY-NC-SA 2.0 lets others remix, tweak, and build upon the author’s work non-commercially, as long as they credit the author and licence their new creations under the identical terms."@en,
        "CC BY-NC-SA 2.0 permet aux autres de remixer, arranger, et adapter l’œuvre de l’auteur/autrice à des fins non commerciales tant qu’on le/la crédite en citant son nom et que les nouvelles œuvres sont diffusées selon les mêmes conditions."@fr ;
    skos:exactMatch <http://creativecommons.org/licenses/by-nc-sa/2.0/> ;
    skos:inScheme atold:licence ;
    skos:prefLabel "Creative Commons Признание-Некомерсиално-Споделяне на споделеното 2.0 Неадаптиран"@bg,
        "Creative Commons Uveďte původ–Neužívejte dílo komerčně–Zachovejte licenci 2.0 Generic"@cs,
        "Creative Commons Navngivelse–IkkeKommerciel–DelPåSammeVilkår 2.0 Generisk"@da,
        "Creative Commons Namensnennung – Nicht-kommerziell – Weitergabe unter gleichen Bedingungen 2.0 Generic"@de,
        "Creative Commons Αναφορά Δημιουργού – Μη Εμπορική Χρήση – Παρόμοια Διανομή 2.0 Γενικό"@el,
        "Creative Commons Attribution–NonCommercial–ShareAlike 2.0 Generic"@en,
        "Creative Commons Atribución–NoComercial–CompartirIgual 2.0 Genérica"@es,
        "Creative Commons Autorile viitamine–Mitteäriline eesmärk–Jagamine samadel tingimustel 2.0 Üldine"@et,
        "Creative Commons Nimeä–EiKaupallinen–JaaSamoin 2.0 Yleinen"@fi,
        "Creative Commons Attribution – Pas d’Utilisation Commerciale – Partage dans les Mêmes Conditions 2.0 Générique"@fr,
        "Creative Commons Imenovanje–Nekomercijalno–Dijeli pod istim uvjetima 2.0 nelokalizirana licenca"@hr,
        "Creative Commons Nevezd meg! – Ne add el! – Így add tovább! 2.0 Általános"@hu,
        "Creative Commons Attribuzione – Non commerciale – Condividi allo stesso modo 2.0 Generico"@it,
        "Creative Commons Priskyrimas – Nekomercinis platinimas – Analogiškas platinimas 2.0 Bendrasis"@lt,
        "Creative Commons Atsaucoties–Nekomerciāli–Nemainot licenci 2.0 Vispārīgs"@lv,
        "Creative Commons Attribuzzjoni-MhuxKummerċjali-KondiviżjoniUgwali 2.0 Generic"@mt,
        "Creative Commons Naamsvermelding–NietCommercieel–GelijkDelen 2.0 Unported"@nl,
        "Creative Commons Uznanie autorstwa–Użycie niekomercyjne–Na tych samych warunkach 2.0 Ogólny"@pl,
        "Creative Commons Atribuição–NãoComercial–CompartilhaIgual 2.0 Genérica"@pt,
        "Creative Commons Atribuire–Necomercial–Distribuire în Condiţii Identice 2.0 Generică"@ro,
        "Creative Commons Uvedenie Autora-Nekomerčné Použitie-Rovnaké Šírenie 2.0 Generic"@sk,
        "Creative Commons Priznanje avtorstva-Nekomercialno-Deljenje pod enakimi pogoji 2.0 Generična"@sl,
        "Creative Commons Erkännande–IckeKommersiell–DelaLika 2.0 Generisk"@sv ;
    skos:topConceptOf atold:licence .

<http://publications.europa.eu/resource/authority/licence/CC_BYNCSA_2_5> a skos:Concept ;
    at:authority-code "CC_BYNCSA_2_5" ;
    at:deprecated "false" ;
    at:op-code "CC_BYNCSA_2_5" ;
    at:start.use "2005-06-01" ;
    atold:op-code "CC_BYNCSA_2_5" ;
    dc:identifier "CC_BYNCSA_2_5" ;
    skos:altLabel "CC BY-NC-SA 2.5"@bg,
        "CC BY-NC-SA 2.5"@cs,
        "CC BY-NC-SA 2.5"@da,
        "CC BY-NC-SA 2.5"@de,
        "CC BY-NC-SA 2.5"@el,
        "CC BY-NC-SA 2.5"@en,
        "CC BY-NC-SA 2.5"@es,
        "CC BY-NC-SA 2.5"@et,
        "CC BY-NC-SA 2.5"@fi,
        "CC BY-NC-SA 2.5"@fr,
        "CC BY-NC-SA 2.5"@ga,
        "CC BY-NC-SA 2.5"@hr,
        "CC BY-NC-SA 2.5"@hu,
        "CC BY-NC-SA 2.5"@it,
        "CC BY-NC-SA 2.5"@lt,
        "CC BY-NC-SA 2.5"@lv,
        "CC BY-NC-SA 2.5"@mt,
        "CC BY-NC-SA 2.5"@nl,
        "CC BY-NC-SA 2.5"@pl,
        "CC BY-NC-SA 2.5"@pt,
        "CC BY-NC-SA 2.5"@ro,
        "CC BY-NC-SA 2.5"@sk,
        "CC BY-NC-SA 2.5"@sl,
        "CC BY-NC-SA 2.5"@sv ;
    skos:definition "CC BY-NC-SA 2.5 lets others remix, tweak, and build upon the author’s work non-commercially, as long as they credit the author and licence their new creations under the identical terms."@en,
        "CC BY-NC-SA 2.5 permet aux autres de remixer, arranger, et adapter l’œuvre de l’auteur/autrice à des fins non commerciales tant qu’on le/la crédite en citant son nom et que les nouvelles œuvres sont diffusées selon les mêmes conditions."@fr ;
    skos:exactMatch <http://creativecommons.org/licenses/by-nc-sa/2.5/> ;
    skos:inScheme atold:licence ;
    skos:prefLabel "Creative Commons Признание-Некомерсиално-Споделяне на споделеното 2.5 Неадаптиран"@bg,
        "Creative Commons Uveďte původ–Neužívejte dílo komerčně–Zachovejte licenci 2.5 Generic"@cs,
        "Creative Commons Navngivelse–IkkeKommerciel–DelPåSammeVilkår 2.5 Generisk"@da,
        "Creative Commons Namensnennung – Nicht-kommerziell – Weitergabe unter gleichen Bedingungen 2.5 Generic"@de,
        "Creative Commons Αναφορά Δημιουργού – Μη Εμπορική Χρήση – Παρόμοια Διανομή 2.5 Γενικό"@el,
        "Creative Commons Attribution–NonCommercial–ShareAlike 2.5 Generic"@en,
        "Creative Commons Atribución–NoComercial–CompartirIgual 2.5 Genérica"@es,
        "Creative Commons Autorile viitamine–Mitteäriline eesmärk–Jagamine samadel tingimustel 2.5 Üldine"@et,
        "Creative Commons Nimeä–EiKaupallinen–JaaSamoin 2.5 Yleinen"@fi,
        "Creative Commons Attribution – Pas d’Utilisation Commerciale – Partage dans les Mêmes Conditions 2.5 Générique"@fr,
        "Creative Commons Imenovanje–Nekomercijalno–Dijeli pod istim uvjetima 2.5 nelokalizirana licenca"@hr,
        "Creative Commons Nevezd meg! – Ne add el! – Így add tovább! 2.5 Általános"@hu,
        "Creative Commons Attribuzione – Non commerciale – Condividi allo stesso modo 2.5 Generico"@it,
        "Creative Commons Priskyrimas – Nekomercinis platinimas – Analogiškas platinimas 2.5 Bendrasis"@lt,
        "Creative Commons Atsaucoties–Nekomerciāli–Nemainot licenci 2.5 Vispārīgs"@lv,
        "Creative Commons Attribuzzjoni-MhuxKummerċjali-KondiviżjoniUgwali 2.5 Generic"@mt,
        "Creative Commons Naamsvermelding–NietCommercieel–GelijkDelen 2.5 Unported"@nl,
        "Creative Commons Uznanie autorstwa–Użycie niekomercyjne–Na tych samych warunkach 2.5 Ogólny"@pl,
        "Creative Commons Atribuição–NãoComercial–CompartilhaIgual 2.5 Genérica"@pt,
        "Creative Commons Atribuire–Necomercial–Distribuire în Condiţii Identice 2.5 Generică"@ro,
        "Creative Commons Uvedenie Autora-Nekomerčné Použitie-Rovnaké Šírenie 2.5 Generic"@sk,
        "Creative Commons Priznanje avtorstva-Nekomercialno-Deljenje pod enakimi pogoji 2.5 Generična"@sl,
        "Creative Commons Erkännande–IckeKommersiell–DelaLika 2.5 Generisk"@sv ;
    skos:topConceptOf atold:licence .

<http://publications.europa.eu/resource/authority/licence/CC_BYNCSA_3_0> a skos:Concept ;
    at:authority-code "CC_BYNCSA_3_0" ;
    at:deprecated "false" ;
    at:op-code "CC_BYNCSA_3_0" ;
    at:start.use "2007-02-23" ;
    atold:op-code "CC_BYNCSA_3_0" ;
    dc:identifier "CC_BYNCSA_3_0" ;
    skos:altLabel "CC BY-NC-SA 3.0"@bg,
        "CC BY-NC-SA 3.0"@cs,
        "CC BY-NC-SA 3.0"@da,
        "CC BY-NC-SA 3.0"@de,
        "CC BY-NC-SA 3.0"@el,
        "CC BY-NC-SA 3.0"@en,
        "CC BY-NC-SA 3.0"@es,
        "CC BY-NC-SA 3.0"@et,
        "CC BY-NC-SA 3.0"@fi,
        "CC BY-NC-SA 3.0"@fr,
        "CC BY-NC-SA 3.0"@ga,
        "CC BY-NC-SA 3.0"@hr,
        "CC BY-NC-SA 3.0"@hu,
        "CC BY-NC-SA 3.0"@it,
        "CC BY-NC-SA 3.0"@lt,
        "CC BY-NC-SA 3.0"@lv,
        "CC BY-NC-SA 3.0"@mt,
        "CC BY-NC-SA 3.0"@nl,
        "CC BY-NC-SA 3.0"@pl,
        "CC BY-NC-SA 3.0"@pt,
        "CC BY-NC-SA 3.0"@ro,
        "CC BY-NC-SA 3.0"@sk,
        "CC BY-NC-SA 3.0"@sl,
        "CC BY-NC-SA 3.0"@sv ;
    skos:definition "CC BY-NC-SA 3.0 lets others remix, tweak, and build upon the author’s work non-commercially, as long as they credit the author and licence their new creations under the identical terms."@en,
        "CC BY-NC-SA 3.0 permet aux autres de remixer, arranger, et adapter l’œuvre de l’auteur/autrice à des fins non commerciales tant qu’on le/la crédite en citant son nom et que les nouvelles œuvres sont diffusées selon les mêmes conditions."@fr ;
    skos:exactMatch <http://creativecommons.org/licenses/by-nc-sa/3.0/> ;
    skos:historyNote "Unported licences are licences that are not associated with any specific jurisdiction, e.g. country."@en ;
    skos:inScheme atold:licence ;
    skos:prefLabel "Creative Commons Признание-Некомерсиално-Споделяне на споделеното 3.0 Нелокализиран"@bg,
        "Creative Commons Uveďte původ–Neužívejte dílo komerčně–Zachovejte licenci 3.0 Unported"@cs,
        "Creative Commons Navngivelse–IkkeKommerciel–DelPåSammeVilkår 3.0 Unported"@da,
        "Creative Commons Namensnennung – Nicht-kommerziell – Weitergabe unter gleichen Bedingungen 3.0 Unported"@de,
        "Creative Commons Αναφορά Δημιουργού – Μη Εμπορική Χρήση – Παρόμοια Διανομή 3.0 Μη εισαγόμενο"@el,
        "Creative Commons Attribution–NonCommercial–ShareAlike 3.0 Unported"@en,
        "Creative Commons Atribución–NoComercial–CompartirIgual 3.0 Unported"@es,
        "Creative Commons Autorile viitamine–Mitteäriline eesmärk–Jagamine samadel tingimustel 3.0 Jurisdiktsiooniga sidumata"@et,
        "Creative Commons Nimeä–EiKaupallinen–JaaSamoin 3.0 Ei sovitettu"@fi,
        "Creative Commons Attribution – Pas d’Utilisation Commerciale – Partage dans les Mêmes Conditions 3.0 non transposé"@fr,
        "Creative Commons Imenovanje–Nekomercijalno–Dijeli pod istim uvjetima 3.0 nelokalizirana licenca"@hr,
        "Creative Commons Nevezd meg! – Ne add el! – Így add tovább! 3.0 Unported"@hu,
        "Creative Commons Attribuzione – Non commerciale – Condividi allo stesso modo 3.0 Unported"@it,
        "Creative Commons Priskyrimas – Nekomercinis platinimas – Analogiškas platinimas 3.0 Nepritaikyta jurisdikcijai"@lt,
        "Creative Commons Atsaucoties–Nekomerciāli–Nemainot licenci 3.0 Nepārnesta"@lv,
        "Creative Commons Attribuzzjoni-MhuxKummerċjali-KondiviżjoniUgwali 3.0 Unported"@mt,
        "Creative Commons Naamsvermelding–NietCommercieel–GelijkDelen 3.0 Unported"@nl,
        "Creative Commons Uznanie autorstwa–Użycie niekomercyjne–Na tych samych warunkach 3.0 Unported"@pl,
        "Creative Commons Atribuição–NãoComercial–CompartilhaIgual 3.0 Não Adaptada"@pt,
        "Creative Commons Atribuire–Necomercial–Distribuire în Condiţii Identice 3.0 Ne-adaptată"@ro,
        "Creative Commons Uvedenie Autora-Nekomerčné Použitie-Rovnaké Šírenie 3.0 Unported"@sk,
        "Creative Commons Priznanje avtorstva-Nekomercialno-Deljenje pod enakimi pogoji 3.0 Nedoločena"@sl,
        "Creative Commons Erkännande–IckeKommersiell–DelaLika 3.0 Unported"@sv ;
    skos:topConceptOf atold:licence .

<http://publications.europa.eu/resource/authority/licence/CC_BYNCSA_4_0> a skos:Concept ;
    at:authority-code "CC_BYNCSA_4_0" ;
    at:deprecated "false" ;
    at:op-code "CC_BYNCSA_4_0" ;
    at:start.use "2013-11-26" ;
    atold:op-code "CC_BYNCSA_4_0" ;
    dc:identifier "CC_BYNCSA_4_0" ;
    skos:altLabel "CC BY-NC-SA 4.0"@bg,
        "CC BY-NC-SA 4.0"@cs,
        "CC BY-NC-SA 4.0"@da,
        "CC BY-NC-SA 4.0"@de,
        "CC BY-NC-SA 4.0"@el,
        "CC BY-NC-SA 4.0"@en,
        "CC BY-NC-SA 4.0"@es,
        "CC BY-NC-SA 4.0"@et,
        "CC BY-NC-SA 4.0"@fi,
        "CC BY-NC-SA 4.0"@fr,
        "CC BY-NC-SA 4.0"@ga,
        "CC BY-NC-SA 4.0"@hr,
        "CC BY-NC-SA 4.0"@hu,
        "CC BY-NC-SA 4.0"@it,
        "CC BY-NC-SA 4.0"@lt,
        "CC BY-NC-SA 4.0"@lv,
        "CC BY-NC-SA 4.0"@mt,
        "CC BY-NC-SA 4.0"@nl,
        "CC BY-NC-SA 4.0"@pl,
        "CC BY-NC-SA 4.0"@pt,
        "CC BY-NC-SA 4.0"@ro,
        "CC BY-NC-SA 4.0"@sk,
        "CC BY-NC-SA 4.0"@sl,
        "CC BY-NC-SA 4.0"@sv ;
    skos:definition "CC BY-NC-SA 4.0 lets others remix, tweak, and build upon the author’s work non-commercially, as long as they credit the author and licence their new creations under the identical terms."@en,
        "CC BY-NC-SA 4.0 permet aux autres de remixer, arranger, et adapter l’œuvre de l’auteur/autrice à des fins non commerciales tant qu’on le/la crédite en citant son nom et que les nouvelles œuvres sont diffusées selon les mêmes conditions."@fr ;
    skos:exactMatch <http://creativecommons.org/licenses/by-nc-sa/4.0/> ;
    skos:inScheme atold:licence ;
    skos:prefLabel "Creative Commons Признание-Некомерсиално-Споделяне на споделеното 4.0 Международен"@bg,
        "Creative Commons Uveďte původ–Neužívejte dílo komerčně–Zachovejte licenci 4.0 Mezinárodní"@cs,
        "Creative Commons Navngivelse–IkkeKommerciel–DelPåSammeVilkår 4.0 International"@da,
        "Creative Commons Namensnennung – Nicht-kommerziell – Weitergabe unter gleichen Bedingungen 4.0 International"@de,
        "Creative Commons Αναφορά Δημιουργού – Μη Εμπορική Χρήση – Παρόμοια Διανομή 4.0 Διεθνές"@el,
        "Creative Commons Attribution–NonCommercial–ShareAlike 4.0 International"@en,
        "Creative Commons Atribución–NoComercial–CompartirIgual 4.0 Internacional"@es,
        "Creative Commons Autorile viitamine–Mitteäriline eesmärk–Jagamine samadel tingimustel 4.0 Rahvusvaheline"@et,
        "Creative Commons Nimeä–EiKaupallinen–JaaSamoin 4.0 Kansainvälinen"@fi,
        "Creative Commons Attribution – Pas d’Utilisation Commerciale – Partage dans les Mêmes Conditions 4.0 International"@fr,
        "Creative Commons Imenovanje–Nekomercijalno–Dijeli pod istim uvjetima 4.0 međunarodna"@hr,
        "Creative Commons Nevezd meg! – Ne add el! – Így add tovább! 4.0 Nemzetközi"@hu,
        "Creative Commons Attribuzione – Non commerciale – Condividi allo stesso modo 4.0 Internazionale"@it,
        "Creative Commons Priskyrimas – Nekomercinis platinimas – Analogiškas platinimas 4.0 Tarptautinė"@lt,
        "Creative Commons Atsaucoties–Nekomerciāli–Nemainot licenci 4.0 Internacionāls"@lv,
        "Creative Commons Attribuzzjoni-MhuxKummerċjali-KondiviżjoniUgwali 4.0 Internazzjonali"@mt,
        "Creative Commons Naamsvermelding–NietCommercieel–GelijkDelen 4.0 Internationaal"@nl,
        "Creative Commons Uznanie autorstwa–Użycie niekomercyjne–Na tych samych warunkach 4.0 Międzynarodowe"@pl,
        "Creative Commons Atribuição–NãoComercial–CompartilhaIgual 4.0 Internacional"@pt,
        "Creative Commons Atribuire–Necomercial–Distribuire în Condiţii Identice 4.0 Internațional"@ro,
        "Creative Commons Uvedenie Autora-Nekomerčné Použitie-Rovnaké Šírenie 4.0 Medzinárodný"@sk,
        "Creative Commons Priznanje avtorstva-Nekomercialno-Deljenje pod enakimi pogoji 4.0 Mednarodna"@sl,
        "Creative Commons Erkännande–IckeKommersiell–DelaLika 4.0 Internationell"@sv ;
    skos:topConceptOf atold:licence .

<http://publications.europa.eu/resource/authority/licence/CC_BYNC_1_0> a skos:Concept ;
    at:authority-code "CC_BYNC_1_0" ;
    at:deprecated "true" ;
    at:end.use "2004-05-24" ;
    at:op-code "CC_BYNC_1_0" ;
    at:start.use "2002-12-15" ;
    atold:op-code "CC_BYNC_1_0" ;
    dc:identifier "CC_BYNC_1_0" ;
    skos:altLabel "CC BY-NC 1.0"@bg,
        "CC BY-NC 1.0"@cs,
        "CC BY-NC 1.0"@da,
        "CC BY-NC 1.0"@de,
        "CC BY-NC 1.0"@el,
        "CC BY-NC 1.0"@en,
        "CC BY-NC 1.0"@es,
        "CC BY-NC 1.0"@et,
        "CC BY-NC 1.0"@fi,
        "CC BY-NC 1.0"@fr,
        "CC BY-NC 1.0"@ga,
        "CC BY-NC 1.0"@hr,
        "CC BY-NC 1.0"@hu,
        "CC BY-NC 1.0"@it,
        "CC BY-NC 1.0"@lt,
        "CC BY-NC 1.0"@lv,
        "CC BY-NC 1.0"@mt,
        "CC BY-NC 1.0"@nl,
        "CC BY-NC 1.0"@pl,
        "CC BY-NC 1.0"@pt,
        "CC BY-NC 1.0"@ro,
        "CC BY-NC 1.0"@sk,
        "CC BY-NC 1.0"@sl,
        "CC BY-NC 1.0"@sv ;
    skos:definition "CC BY-NC 1.0 lets others remix, tweak, and build upon the author’s work non-commercially, and although their new works must also acknowledge the author and be non-commercial, they don’t have to licence their derivative works on the same terms."@en,
        "CC BY-NC 1.0 permet aux autres de remixer, arranger, et adapter l’œuvre de l’auteur/autrice à des fins non commerciales et, bien que les nouvelles œuvres doivent créditer l’auteur/autrice en citant son nom et ne pas constituer une utilisation commerciale, elles n’ont pas à être diffusées selon les mêmes conditions."@fr ;
    skos:exactMatch <http://creativecommons.org/licenses/by-nc/1.0/> ;
    skos:inScheme atold:licence ;
    skos:prefLabel "Creative Commons Признание-Некомерсиално 1.0 Неадаптиран"@bg,
        "Creative Commons Uveďte původ–Neužívejte komerčně 1.0 Generic"@cs,
        "Creative Commons Navngivelse–IkkeKommerciel 1.0 Generisk"@da,
        "Creative Commons Namensnennung – Nicht kommerziell 1.0 Generic"@de,
        "Creative Commons Αναφορά Δημιουργού – Μη Εμπορική Χρήση 1.0 Γενικό"@el,
        "Creative Commons Attribution–NonCommercial 1.0 Generic"@en,
        "Creative Commons Atribución–NoComercial 1.0 Genérica"@es,
        "Creative Commons Autorile viitamine–Mitteäriline eesmärk 1.0 Üldine"@et,
        "Creative Commons Nimeä–EiKaupallinen 1.0 Yleinen"@fi,
        "Creative Commons Attribution – Pas d’Utilisation Commerciale 1.0 Générique"@fr,
        "Creative Commons Imenovanje–Nekomercijalno 1.0 nelokalizirana licenca"@hr,
        "Creative Commons Nevezd meg! – Ne add el! 1.0 Általános"@hu,
        "Creative Commons Attribuzione – Non commerciale 1.0 Generico"@it,
        "Creative Commons Priskyrimas – Nekomercinis platinimas 1.0 Bendrasis"@lt,
        "Creative Commons Atsaucoties–Nekomerciāli 1.0 Vispārīgs"@lv,
        "Creative Commons Attribuzzjoni-MhuxKummerċjali 1.0 Generic"@mt,
        "Creative Commons Naamsvermelding–NietCommercieel 1.0 Unported"@nl,
        "Creative Commons Uznanie autorstwa–Użycie niekomercyjne 1.0 Ogólny"@pl,
        "Creative Commons Atribuição–NãoComercial 1.0 Genérica"@pt,
        "Creative Commons Atribuire–Necomercial 1.0 Generică"@ro,
        "Creative Commons Uvedenie Autora-Nekomerčné Použitie 1.0 Generic"@sk,
        "Creative Commons Priznanje avtorstva-Nekomercialno 1.0 Generična"@sl,
        "Creative Commons Erkännande–IckeKommersiell 1.0 Generisk"@sv ;
    skos:topConceptOf atold:licence .

<http://publications.europa.eu/resource/authority/licence/CC_BYNC_2_0> a skos:Concept ;
    at:authority-code "CC_BYNC_2_0" ;
    at:deprecated "false" ;
    at:op-code "CC_BYNC_2_0" ;
    at:start.use "2004-05-25" ;
    atold:op-code "CC_BYNC_2_0" ;
    dc:identifier "CC_BYNC_2_0" ;
    skos:altLabel "CC BY-NC 2.0"@bg,
        "CC BY-NC 2.0"@cs,
        "CC BY-NC 2.0"@da,
        "CC BY-NC 2.0"@de,
        "CC BY-NC 2.0"@el,
        "CC BY-NC 2.0"@en,
        "CC BY-NC 2.0"@es,
        "CC BY-NC 2.0"@et,
        "CC BY-NC 2.0"@fi,
        "CC BY-NC 2.0"@fr,
        "CC BY-NC 2.0"@ga,
        "CC BY-NC 2.0"@hr,
        "CC BY-NC 2.0"@hu,
        "CC BY-NC 2.0"@it,
        "CC BY-NC 2.0"@lt,
        "CC BY-NC 2.0"@lv,
        "CC BY-NC 2.0"@mt,
        "CC BY-NC 2.0"@nl,
        "CC BY-NC 2.0"@pl,
        "CC BY-NC 2.0"@pt,
        "CC BY-NC 2.0"@ro,
        "CC BY-NC 2.0"@sk,
        "CC BY-NC 2.0"@sl,
        "CC BY-NC 2.0"@sv ;
    skos:definition "CC BY-NC 2.0 lets others remix, tweak, and build upon the author’s work non-commercially, and although their new works must also acknowledge the author and be non-commercial, they don’t have to licence their derivative works on the same terms."@en,
        "CC BY-NC 2.0 permet aux autres de remixer, arranger, et adapter l’œuvre de l’auteur/autrice à des fins non commerciales et, bien que les nouvelles œuvres doivent créditer l’auteur/autrice en citant son nom et ne pas constituer une utilisation commerciale, elles n’ont pas à être diffusées selon les mêmes conditions."@fr ;
    skos:exactMatch <http://creativecommons.org/licenses/by-nc/2.0/> ;
    skos:inScheme atold:licence ;
    skos:prefLabel "Creative Commons Признание-Некомерсиално 2.0 Неадаптиран"@bg,
        "Creative Commons Uveďte původ–Neužívejte komerčně 2.0 Generic"@cs,
        "Creative Commons Navngivelse–IkkeKommerciel 2.0 Generisk"@da,
        "Creative Commons Namensnennung – Nicht kommerziell 2.0 Generic"@de,
        "Creative Commons Αναφορά Δημιουργού – Μη Εμπορική Χρήση 2.0 Γενικό"@el,
        "Creative Commons Attribution–NonCommercial 2.0 Generic"@en,
        "Creative Commons Atribución–NoComercial 2.0 Genérica"@es,
        "Creative Commons Autorile viitamine–Mitteäriline eesmärk 2.0 Üldine"@et,
        "Creative Commons Nimeä–EiKaupallinen 2.0 Yleinen"@fi,
        "Creative Commons Attribution – Pas d’Utilisation Commerciale 2.0 Générique"@fr,
        "Creative Commons Imenovanje–Nekomercijalno 2.0 nelokalizirana licenca"@hr,
        "Creative Commons Nevezd meg! – Ne add el! 2.0 Általános"@hu,
        "Creative Commons Attribuzione – Non commerciale 2.0 Generico"@it,
        "Creative Commons Priskyrimas – Nekomercinis platinimas 2.0 Bendrasis"@lt,
        "Creative Commons Atsaucoties–Nekomerciāli 2.0 Vispārīgs"@lv,
        "Creative Commons Attribuzzjoni-MhuxKummerċjali 2.0 Generic"@mt,
        "Creative Commons Naamsvermelding–NietCommercieel 2.0 Unported"@nl,
        "Creative Commons Uznanie autorstwa–Użycie niekomercyjne 2.0 Ogólny"@pl,
        "Creative Commons Atribuição–NãoComercial 2.0 Genérica"@pt,
        "Creative Commons Atribuire–Necomercial 2.0 Generică"@ro,
        "Creative Commons Uvedenie Autora-Nekomerčné Použitie 2.0 Generic"@sk,
        "Creative Commons Priznanje avtorstva-Nekomercialno 2.0 Generična"@sl,
        "Creative Commons Erkännande–IckeKommersiell 2.0 Generisk"@sv ;
    skos:topConceptOf atold:licence .

<http://publications.europa.eu/resource/authority/licence/CC_BYNC_2_5> a skos:Concept ;
    at:authority-code "CC_BYNC_2_5" ;
    at:deprecated "false" ;
    at:op-code "CC_BYNC_2_5" ;
    at:start.use "2005-06-01" ;
    atold:op-code "CC_BYNC_2_5" ;
    dc:identifier "CC_BYNC_2_5" ;
    skos:altLabel "CC BY-NC 2.5"@bg,
        "CC BY-NC 2.5"@cs,
        "CC BY-NC 2.5"@da,
        "CC BY-NC 2.5"@de,
        "CC BY-NC 2.5"@el,
        "CC BY-NC 2.5"@en,
        "CC BY-NC 2.5"@es,
        "CC BY-NC 2.5"@et,
        "CC BY-NC 2.5"@fi,
        "CC BY-NC 2.5"@fr,
        "CC BY-NC 2.5"@ga,
        "CC BY-NC 2.5"@hr,
        "CC BY-NC 2.5"@hu,
        "CC BY-NC 2.5"@it,
        "CC BY-NC 2.5"@lt,
        "CC BY-NC 2.5"@lv,
        "CC BY-NC 2.5"@mt,
        "CC BY-NC 2.5"@nl,
        "CC BY-NC 2.5"@pl,
        "CC BY-NC 2.5"@pt,
        "CC BY-NC 2.5"@ro,
        "CC BY-NC 2.5"@sk,
        "CC BY-NC 2.5"@sl,
        "CC BY-NC 2.5"@sv ;
    skos:definition "CC BY-NC 2.5 lets others remix, tweak, and build upon the author’s work non-commercially, and although their new works must also acknowledge the author and be non-commercial, they don’t have to licence their derivative works on the same terms."@en,
        "CC BY-NC 2.5 permet aux autres de remixer, arranger, et adapter l’œuvre de l’auteur/autrice à des fins non commerciales et, bien que les nouvelles œuvres doivent créditer l’auteur/autrice en citant son nom et ne pas constituer une utilisation commerciale, elles n’ont pas à être diffusées selon les mêmes conditions."@fr ;
    skos:exactMatch <http://creativecommons.org/licenses/by-nc/2.5/> ;
    skos:inScheme atold:licence ;
    skos:prefLabel "Creative Commons Признание-Некомерсиално 2.5 Неадаптиран"@bg,
        "Creative Commons Uveďte původ–Neužívejte komerčně 2.5 Generic"@cs,
        "Creative Commons Navngivelse–IkkeKommerciel 2.5 Generisk"@da,
        "Creative Commons Namensnennung – Nicht kommerziell 2.5 Generic"@de,
        "Creative Commons Αναφορά Δημιουργού – Μη Εμπορική Χρήση 2.5 Γενικό"@el,
        "Creative Commons Attribution–NonCommercial 2.5 Generic"@en,
        "Creative Commons Atribución–NoComercial 2.5 Genérica"@es,
        "Creative Commons Autorile viitamine–Mitteäriline eesmärk 2.5 Üldine"@et,
        "Creative Commons Nimeä–EiKaupallinen 2.5 Yleinen"@fi,
        "Creative Commons Attribution – Pas d’Utilisation Commerciale 2.5 Générique"@fr,
        "Creative Commons Imenovanje–Nekomercijalno 2.5 nelokalizirana licenca"@hr,
        "Creative Commons Nevezd meg! – Ne add el! 2.5 Általános"@hu,
        "Creative Commons Attribuzione – Non commerciale 2.5 Generico"@it,
        "Creative Commons Priskyrimas – Nekomercinis platinimas 2.5 Bendrasis"@lt,
        "Creative Commons Atsaucoties–Nekomerciāli 2.5 Vispārīgs"@lv,
        "Creative Commons Attribuzzjoni-MhuxKummerċjali 2.5 Generic"@mt,
        "Creative Commons Naamsvermelding–NietCommercieel 2.5 Unported"@nl,
        "Creative Commons Uznanie autorstwa–Użycie niekomercyjne 2.5 Ogólny"@pl,
        "Creative Commons Atribuição–NãoComercial 2.5 Genérica"@pt,
        "Creative Commons Atribuire–Necomercial 2.5 Generică"@ro,
        "Creative Commons Uvedenie Autora-Nekomerčné Použitie 2.5 Generic"@sk,
        "Creative Commons Priznanje avtorstva-Nekomercialno 2.5 Generična"@sl,
        "Creative Commons Erkännande–IckeKommersiell 2.5 Generisk"@sv ;
    skos:topConceptOf atold:licence .

<http://publications.europa.eu/resource/authority/licence/CC_BYNC_3_0> a skos:Concept ;
    at:authority-code "CC_BYNC_3_0" ;
    at:deprecated "false" ;
    at:op-code "CC_BYNC_3_0" ;
    at:start.use "2007-02-23" ;
    atold:op-code "CC_BYNC_3_0" ;
    dc:identifier "CC_BYNC_3_0" ;
    skos:altLabel "CC BY-NC 3.0"@bg,
        "CC BY-NC 3.0"@cs,
        "CC BY-NC 3.0"@da,
        "CC BY-NC 3.0"@de,
        "CC BY-NC 3.0"@el,
        "CC BY-NC 3.0"@en,
        "CC BY-NC 3.0"@es,
        "CC BY-NC 3.0"@et,
        "CC BY-NC 3.0"@fi,
        "CC BY-NC 3.0"@fr,
        "CC BY-NC 3.0"@ga,
        "CC BY-NC 3.0"@hr,
        "CC BY-NC 3.0"@hu,
        "CC BY-NC 3.0"@it,
        "CC BY-NC 3.0"@lt,
        "CC BY-NC 3.0"@lv,
        "CC BY-NC 3.0"@mt,
        "CC BY-NC 3.0"@nl,
        "CC BY-NC 3.0"@pl,
        "CC BY-NC 3.0"@pt,
        "CC BY-NC 3.0"@ro,
        "CC BY-NC 3.0"@sk,
        "CC BY-NC 3.0"@sl,
        "CC BY-NC 3.0"@sv ;
    skos:definition "CC BY-NC 3.0 lets others remix, tweak, and build upon the author’s work non-commercially, and although their new works must also acknowledge the author and be non-commercial, they don’t have to licence their derivative works on the same terms."@en,
        "CC BY-NC 3.0 permet aux autres de remixer, arranger, et adapter l’œuvre de l’auteur/autrice à des fins non commerciales et, bien que les nouvelles œuvres doivent créditer l’auteur/autrice en citant son nom et ne pas constituer une utilisation commerciale, elles n’ont pas à être diffusées selon les mêmes conditions."@fr ;
    skos:exactMatch <http://creativecommons.org/licenses/by-nc/3.0/> ;
    skos:historyNote "Unported licences are licences that are not associated with any specific jurisdiction, e.g. country."@en ;
    skos:inScheme atold:licence ;
    skos:prefLabel "Creative Commons Признание-Некомерсиално 3.0 Нелокализиран"@bg,
        "Creative Commons Uveďte původ–Neužívejte komerčně 3.0 Unported"@cs,
        "Creative Commons Navngivelse–IkkeKommerciel 3.0 Unported"@da,
        "Creative Commons Namensnennung – Nicht kommerziell 3.0 Unported"@de,
        "Creative Commons Αναφορά Δημιουργού – Μη Εμπορική Χρήση 3.0 Μη εισαγόμενο"@el,
        "Creative Commons Attribution–NonCommercial 3.0 Unported"@en,
        "Creative Commons Atribución–NoComercial 3.0 Unported"@es,
        "Creative Commons Autorile viitamine–Mitteäriline eesmärk 3.0 Jurisdiktsiooniga sidumata"@et,
        "Creative Commons Nimeä–EiKaupallinen 3.0 Ei sovitettu"@fi,
        "Creative Commons Attribution – Pas d’Utilisation Commerciale 3.0 non transposé"@fr,
        "Creative Commons Imenovanje–Nekomercijalno 3.0 nelokalizirana licenca"@hr,
        "Creative Commons Nevezd meg! – Ne add el! 3.0 Unported"@hu,
        "Creative Commons Attribuzione – Non commerciale 3.0 Unported"@it,
        "Creative Commons Priskyrimas – Nekomercinis platinimas 3.0 Nepritaikyta jurisdikcijai"@lt,
        "Creative Commons Atsaucoties–Nekomerciāli 3.0 Nepārnesta"@lv,
        "Creative Commons Attribuzzjoni-MhuxKummerċjali 3.0 Unported"@mt,
        "Creative Commons Naamsvermelding–NietCommercieel 3.0 Unported"@nl,
        "Creative Commons Uznanie autorstwa–Użycie niekomercyjne 3.0 Unported"@pl,
        "Creative Commons Atribuição–NãoComercial 3.0 Não Adaptada"@pt,
        "Creative Commons Atribuire–Necomercial 3.0 Ne-adaptată"@ro,
        "Creative Commons Uvedenie Autora-Nekomerčné Použitie 3.0 Unported"@sk,
        "Creative Commons Priznanje avtorstva-Nekomercialno 3.0 Nedoločena"@sl,
        "Creative Commons Erkännande–IckeKommersiell 3.0 Unported"@sv ;
    skos:topConceptOf atold:licence .

<http://publications.europa.eu/resource/authority/licence/CC_BYNC_4_0> a skos:Concept ;
    at:authority-code "CC_BYNC_4_0" ;
    at:deprecated "false" ;
    at:op-code "CC_BYNC_4_0" ;
    at:start.use "2013-11-26" ;
    atold:op-code "CC_BYNC_4_0" ;
    dc:identifier "CC_BYNC_4_0" ;
    skos:altLabel "CC BY-NC 4.0"@bg,
        "CC BY-NC 4.0"@cs,
        "CC BY-NC 4.0"@da,
        "CC BY-NC 4.0"@de,
        "CC BY-NC 4.0"@el,
        "CC BY-NC 4.0"@en,
        "CC BY-NC 4.0"@es,
        "CC BY-NC 4.0"@et,
        "CC BY-NC 4.0"@fi,
        "CC BY-NC 4.0"@fr,
        "CC BY-NC 4.0"@ga,
        "CC BY-NC 4.0"@hr,
        "CC BY-NC 4.0"@hu,
        "CC BY-NC 4.0"@it,
        "CC BY-NC 4.0"@lt,
        "CC BY-NC 4.0"@lv,
        "CC BY-NC 4.0"@mt,
        "CC BY-NC 4.0"@nl,
        "CC BY-NC 4.0"@pl,
        "CC BY-NC 4.0"@pt,
        "CC BY-NC 4.0"@ro,
        "CC BY-NC 4.0"@sk,
        "CC BY-NC 4.0"@sl,
        "CC BY-NC 4.0"@sv ;
    skos:definition "CC BY-NC 4.0 lets others remix, tweak, and build upon the author’s work non-commercially, and although their new works must also acknowledge the author and be non-commercial, they don’t have to licence their derivative works on the same terms."@en,
        "CC BY-NC 4.0 permet aux autres de remixer, arranger, et adapter l’œuvre de l’auteur/autrice à des fins non commerciales et, bien que les nouvelles œuvres doivent créditer l’auteur/autrice en citant son nom et ne pas constituer une utilisation commerciale, elles n’ont pas à être diffusées selon les mêmes conditions."@fr ;
    skos:exactMatch <http://creativecommons.org/licenses/by-nc/4.0/> ;
    skos:inScheme atold:licence ;
    skos:prefLabel "Creative Commons Признание-Некомерсиално 4.0 Международен"@bg,
        "Creative Commons Uveďte původ–Neužívejte komerčně 4.0 Mezinárodní"@cs,
        "Creative Commons Navngivelse–IkkeKommerciel 4.0 International"@da,
        "Creative Commons Namensnennung – Nicht kommerziell 4.0 International"@de,
        "Creative Commons Αναφορά Δημιουργού – Μη Εμπορική Χρήση 4.0 Διεθνές"@el,
        "Creative Commons Attribution–NonCommercial 4.0 International"@en,
        "Creative Commons Atribución–NoComercial 4.0 Internacional"@es,
        "Creative Commons Autorile viitamine–Mitteäriline eesmärk 4.0 Rahvusvaheline"@et,
        "Creative Commons Nimeä–EiKaupallinen 4.0 Kansainvälinen"@fi,
        "Creative Commons Attribution – Pas d’Utilisation Commerciale 4.0 International"@fr,
        "Creative Commons Imenovanje–Nekomercijalno 4.0 međunarodna"@hr,
        "Creative Commons Nevezd meg! – Ne add el! 4.0 Nemzetközi"@hu,
        "Creative Commons Attribuzione – Non commerciale 4.0 Internazionale"@it,
        "Creative Commons Priskyrimas – Nekomercinis platinimas 4.0 Tarptautinė"@lt,
        "Creative Commons Atsaucoties–Nekomerciāli 4.0 Internacionāls"@lv,
        "Creative Commons Attribuzzjoni-MhuxKummerċjali 4.0 Internazzjonali"@mt,
        "Creative Commons Naamsvermelding–NietCommercieel 4.0 Internationaal"@nl,
        "Creative Commons Uznanie autorstwa–Użycie niekomercyjne 4.0 Międzynarodowe"@pl,
        "Creative Commons Atribuição–NãoComercial 4.0 Internacional"@pt,
        "Creative Commons Atribuire–Necomercial 4.0 Internațional"@ro,
        "Creative Commons Uvedenie Autora-Nekomerčné Použitie 4.0 Medzinárodný"@sk,
        "Creative Commons Priznanje avtorstva-Nekomercialno 4.0 Mednarodna"@sl,
        "Creative Commons Erkännande–IckeKommersiell 4.0 Internationell"@sv ;
    skos:topConceptOf atold:licence .

<http://publications.europa.eu/resource/authority/licence/CC_BYND> a skos:Concept ;
    at:authority-code "CC_BYND" ;
    at:deprecated "true" ;
    at:end.use "2013-11-26" ;
    at:op-code "CC_BYND" ;
    at:start.use "2013-11-25" ;
    atold:op-code "CC_BYND" ;
    dc:identifier "CC_BYND" ;
    skos:altLabel "CC BY-ND 4.0"@bg,
        "CC BY-ND 4.0"@cs,
        "CC BY-ND 4.0"@da,
        "CC BY-ND 4.0"@de,
        "CC BY-ND 4.0"@el,
        "CC BY-ND 4.0"@en,
        "CC BY-ND 4.0"@es,
        "CC BY-ND 4.0"@et,
        "CC BY-ND 4.0"@fi,
        "CC BY-ND 4.0"@fr,
        "CC BY-ND 4.0"@ga,
        "CC BY-ND 4.0"@hr,
        "CC BY-ND 4.0"@hu,
        "CC BY-ND 4.0"@it,
        "CC BY-ND 4.0"@lt,
        "CC BY-ND 4.0"@lv,
        "CC BY-ND 4.0"@mt,
        "CC BY-ND 4.0"@nl,
        "CC BY-ND 4.0"@pl,
        "CC BY-ND 4.0"@pt,
        "CC BY-ND 4.0"@ro,
        "CC BY-ND 4.0"@sk,
        "CC BY-ND 4.0"@sl,
        "CC BY-ND 4.0"@sv ;
    skos:definition "This licence allows for redistribution, commercial and non-commercial, as long as it is passed along unchanged and in whole, with credit to the author."@en,
        "Cette licence autorise la redistribution, à des fins commerciales ou non, tant que l’œuvre est diffusée sans modification et dans son intégralité, avec attribution et citation du nom de l’auteur/autrice."@fr ;
    skos:inScheme atold:licence ;
    skos:prefLabel "Creative Commons Uveďte původ–Nezpracovávejte 4.0 Mezinárodní"@cs,
        "Creative Commons Navngivelse–IngenBearbejdelse 4.0 International"@da,
        "Creative Commons Namensnennung – Keine Bearbeitungen 4.0 International"@de,
        "Creative Commons Αναφορά Δημιουργού – Όχι Παράγωγα Έργα 4.0 Διεθνές"@el,
        "Creative Commons Attribution–NoDerivatives 4.0 International"@en,
        "Creative Commons Atribución–SinDerivar 4.0 Internacional"@es,
        "Creative Commons Nimeä–EiMuutoksia 4.0 Kansainvälinen"@fi,
        "Creative Commons Attribution – Pas de Modification 4.0 International"@fr,
        "Creative Commons Imenovanje–Bez prerada 4.0 međunarodna"@hr,
        "Creative Commons Nevezd meg! – Ne változtasd! 4.0 Nemzetközi"@hu,
        "Creative Commons Attribuzione – Non opere derivate 4.0 Internazionale"@it,
        "Creative Commons Priskyrimas – Jokių išvestinių darbų 4.0 Tarptautinė"@lt,
        "Creative Commons Atsaucoties, nepārveidojot 4.0 Internacionāls"@lv,
        "Creative Commons Naamsvermelding–GeenAfgeleideWerken 4.0 Internationaal"@nl,
        "Creative Commons Uznanie autorstwa – Bez utworów zależnych 4.0 Międzynarodowe"@pl,
        "Creative Commons Atribuição–SemDerivações 4.0 Internacional"@pt,
        "Creative Commons Atribuire–FărăDerivate 4.0 Internațional"@ro,
        "Creative Commons Erkännande–IngaBearbetningar 4.0 Internationell"@sv ;
    skos:topConceptOf atold:licence .

<http://publications.europa.eu/resource/authority/licence/CC_BYND_1_0> a skos:Concept ;
    at:authority-code "CC_BYND_1_0" ;
    at:deprecated "true" ;
    at:end.use "2004-05-24" ;
    at:op-code "CC_BYND_1_0" ;
    at:start.use "2002-12-15" ;
    atold:op-code "CC_BYND_1_0" ;
    dc:identifier "CC_BYND_1_0" ;
    skos:altLabel "CC BY-ND 1.0"@bg,
        "CC BY-ND 1.0"@cs,
        "CC BY-ND 1.0"@da,
        "CC BY-ND 1.0"@de,
        "CC BY-ND 1.0"@el,
        "CC BY-ND 1.0"@en,
        "CC BY-ND 1.0"@es,
        "CC BY-ND 1.0"@et,
        "CC BY-ND 1.0"@fi,
        "CC BY-ND 1.0"@fr,
        "CC BY-ND 1.0"@ga,
        "CC BY-ND 1.0"@hr,
        "CC BY-ND 1.0"@hu,
        "CC BY-ND 1.0"@it,
        "CC BY-ND 1.0"@lt,
        "CC BY-ND 1.0"@lv,
        "CC BY-ND 1.0"@mt,
        "CC BY-ND 1.0"@nl,
        "CC BY-ND 1.0"@pl,
        "CC BY-ND 1.0"@pt,
        "CC BY-ND 1.0"@ro,
        "CC BY-ND 1.0"@sk,
        "CC BY-ND 1.0"@sl,
        "CC BY-ND 1.0"@sv ;
    skos:definition "CC BY-ND 1.0 allows for redistribution, commercial and non-commercial, as long as it is passed along unchanged and in whole, with credit to the author."@en,
        "CC BY-ND 1.0 autorise la redistribution, à des fins commerciales ou non, tant que l’œuvre est diffusée sans modification et dans son intégralité, avec attribution et citation du nom de l’auteur/autrice."@fr ;
    skos:exactMatch <http://creativecommons.org/licenses/by-nd/1.0/> ;
    skos:inScheme atold:licence ;
    skos:prefLabel "Creative Commons Признание-Без производни 1.0 Неадаптиран"@bg,
        "Creative Commons Uveďte původ–Nezpracovávejte 1.0 Generic"@cs,
        "Creative Commons Navngivelse–IngenBearbejdelse 1.0 Generisk"@da,
        "Creative Commons Namensnennung – Keine Bearbeitung 1.0 Generic"@de,
        "Creative Commons Αναφορά Δημιουργού – Όχι Παράγωγα Έργα 1.0 Γενικό"@el,
        "Creative Commons Attribution–NoDerivs 1.0 Generic"@en,
        "Creative Commons Atribución–SinDerivadas 1.0 Genérica"@es,
        "Creative Commons Autorile viitamine–Tuletatud teoste keeld 1.0 Üldine"@et,
        "Creative Commons Nimeä–EiMuutoksia 1.0 Yleinen"@fi,
        "Creative Commons Attribution – Pas de Modification 1.0 Générique"@fr,
        "Creative Commons Imenovanje–Bez prerada 1.0 nelokalizirana licenca"@hr,
        "Creative Commons Nevezd meg! – Ne változtasd! 1.0 Általános"@hu,
        "Creative Commons Attribuzione – Non opere derivate 1.0 Generico"@it,
        "Creative Commons Priskyrimas – Jokių išvestinių darbų 1.0 Bendrasis"@lt,
        "Creative Commons Atsaucoties–Nepārveidojot 1.0 Vispārīgs"@lv,
        "Creative Commons Attribuzzjoni-EbdaDerivattivi 1.0 Generic"@mt,
        "Creative Commons Naamsvermelding–GeenAfgeleideWerken 1.0 Unported"@nl,
        "Creative Commons Uznanie autorstwa–Bez utworów zależnych 1.0 Ogólny"@pl,
        "Creative Commons Atribuição–SemDerivações 1.0 Genérica"@pt,
        "Creative Commons Atribuire–FărăModificări 1.0 Generică"@ro,
        "Creative Commons Uvedenie Autora-Bez Odvodeného Obsahu 1.0 Generic"@sk,
        "Creative Commons Priznanje avtorstva-Brez predelav 1.0 Generična"@sl,
        "Creative Commons Erkännande–IngaBearbetningar 1.0 Generisk"@sv ;
    skos:topConceptOf atold:licence .

<http://publications.europa.eu/resource/authority/licence/CC_BYND_2_0> a skos:Concept ;
    at:authority-code "CC_BYND_2_0" ;
    at:deprecated "false" ;
    at:op-code "CC_BYND_2_0" ;
    at:start.use "2004-05-25" ;
    atold:op-code "CC_BYND_2_0" ;
    dc:identifier "CC_BYND_2_0" ;
    skos:altLabel "CC BY-ND 2.0"@bg,
        "CC BY-ND 2.0"@cs,
        "CC BY-ND 2.0"@da,
        "CC BY-ND 2.0"@de,
        "CC BY-ND 2.0"@el,
        "CC BY-ND 2.0"@en,
        "CC BY-ND 2.0"@es,
        "CC BY-ND 2.0"@et,
        "CC BY-ND 2.0"@fi,
        "CC BY-ND 2.0"@fr,
        "CC BY-ND 2.0"@ga,
        "CC BY-ND 2.0"@hr,
        "CC BY-ND 2.0"@hu,
        "CC BY-ND 2.0"@it,
        "CC BY-ND 2.0"@lt,
        "CC BY-ND 2.0"@lv,
        "CC BY-ND 2.0"@mt,
        "CC BY-ND 2.0"@nl,
        "CC BY-ND 2.0"@pl,
        "CC BY-ND 2.0"@pt,
        "CC BY-ND 2.0"@ro,
        "CC BY-ND 2.0"@sk,
        "CC BY-ND 2.0"@sl,
        "CC BY-ND 2.0"@sv ;
    skos:definition "CC BY-ND 2.0 allows for redistribution, commercial and non-commercial, as long as it is passed along unchanged and in whole, with credit to the author."@en,
        "CC BY-ND 2.0 autorise la redistribution, à des fins commerciales ou non, tant que l’œuvre est diffusée sans modification et dans son intégralité, avec attribution et citation du nom de l’auteur."@fr ;
    skos:exactMatch <http://creativecommons.org/licenses/by-nd/2.0/> ;
    skos:inScheme atold:licence ;
    skos:prefLabel "Creative Commons Признание-Без производни 2.0 Неадаптиран"@bg,
        "Creative Commons Uveďte původ–Nezpracovávejte 2.0 Generic"@cs,
        "Creative Commons Navngivelse–IngenBearbejdelse 2.0 Generisk"@da,
        "Creative Commons Namensnennung – Keine Bearbeitung 2.0 Generic"@de,
        "Creative Commons Αναφορά Δημιουργού – Όχι Παράγωγα Έργα 2.0 Γενικό"@el,
        "Creative Commons Attribution–NoDerivs 2.0 Generic"@en,
        "Creative Commons Atribución–SinDerivadas 2.0 Genérica"@es,
        "Creative Commons Autorile viitamine–Tuletatud teoste keeld 2.0 Üldine"@et,
        "Creative Commons Nimeä–EiMuutoksia 2.0 Yleinen"@fi,
        "Creative Commons Attribution – Pas de Modification 2.0 Générique"@fr,
        "Creative Commons Imenovanje–Bez prerada 2.0 nelokalizirana licenca"@hr,
        "Creative Commons Nevezd meg! – Ne változtasd! 2.0 Általános"@hu,
        "Creative Commons Attribuzione – Non opere derivate 2.0 Generico"@it,
        "Creative Commons Priskyrimas – Jokių išvestinių darbų 2.0 Bendrasis"@lt,
        "Creative Commons Atsaucoties–Nepārveidojot 2.0 Vispārīgs"@lv,
        "Creative Commons Attribuzzjoni-EbdaDerivattivi 2.0 Generic"@mt,
        "Creative Commons Naamsvermelding–GeenAfgeleideWerken 2.0 Unported"@nl,
        "Creative Commons Uznanie autorstwa–Bez utworów zależnych 2.0 Ogólny"@pl,
        "Creative Commons Atribuição–SemDerivações 2.0 Genérica"@pt,
        "Creative Commons Atribuire–FărăModificări 2.0 Generică"@ro,
        "Creative Commons Uvedenie Autora-Bez Odvodeného Obsahu 2.0 Generic"@sk,
        "Creative Commons Priznanje avtorstva-Brez predelav 2.0 Generična"@sl,
        "Creative Commons Erkännande–IngaBearbetningar 2.0 Generisk"@sv ;
    skos:topConceptOf atold:licence .

<http://publications.europa.eu/resource/authority/licence/CC_BYND_2_5> a skos:Concept ;
    at:authority-code "CC_BYND_2_5" ;
    at:deprecated "false" ;
    at:op-code "CC_BYND_2_5" ;
    at:start.use "2005-06-01" ;
    atold:op-code "CC_BYND_2_5" ;
    dc:identifier "CC_BYND_2_5" ;
    skos:altLabel "CC BY-ND 2.5"@bg,
        "CC BY-ND 2.5"@cs,
        "CC BY-ND 2.5"@da,
        "CC BY-ND 2.5"@de,
        "CC BY-ND 2.5"@el,
        "CC BY-ND 2.5"@en,
        "CC BY-ND 2.5"@es,
        "CC BY-ND 2.5"@et,
        "CC BY-ND 2.5"@fi,
        "CC BY-ND 2.5"@fr,
        "CC BY-ND 2.5"@ga,
        "CC BY-ND 2.5"@hr,
        "CC BY-ND 2.5"@hu,
        "CC BY-ND 2.5"@it,
        "CC BY-ND 2.5"@lt,
        "CC BY-ND 2.5"@lv,
        "CC BY-ND 2.5"@mt,
        "CC BY-ND 2.5"@nl,
        "CC BY-ND 2.5"@pl,
        "CC BY-ND 2.5"@pt,
        "CC BY-ND 2.5"@ro,
        "CC BY-ND 2.5"@sk,
        "CC BY-ND 2.5"@sl,
        "CC BY-ND 2.5"@sv ;
    skos:definition "CC BY-ND 2.5 allows for redistribution, commercial and non-commercial, as long as it is passed along unchanged and in whole, with credit to the author."@en,
        "CC BY-ND 2.5 autorise la redistribution, à des fins commerciales ou non, tant que l’œuvre est diffusée sans modification et dans son intégralité, avec attribution et citation du nom de l’auteur/autrice."@fr ;
    skos:exactMatch <http://creativecommons.org/licenses/by-nd/2.5/> ;
    skos:inScheme atold:licence ;
    skos:prefLabel "Creative Commons Признание-Без производни 2.5 Неадаптиран"@bg,
        "Creative Commons Uveďte původ–Nezpracovávejte 2.5 Generic"@cs,
        "Creative Commons Navngivelse–IngenBearbejdelse 2.5 Generisk"@da,
        "Creative Commons Namensnennung – Keine Bearbeitung 2.5 Generic"@de,
        "Creative Commons Αναφορά Δημιουργού – Όχι Παράγωγα Έργα 2.5 Γενικό"@el,
        "Creative Commons Attribution–NoDerivs 2.5 Generic"@en,
        "Creative Commons Atribución–SinDerivadas 2.5 Genérica"@es,
        "Creative Commons Autorile viitamine–Tuletatud teoste keeld 2.5 Üldine"@et,
        "Creative Commons Nimeä–EiMuutoksia 2.5 Yleinen"@fi,
        "Creative Commons Attribution – Pas de Modification 2.5 Générique"@fr,
        "Creative Commons Imenovanje–Bez prerada 2.5 nelokalizirana licenca"@hr,
        "Creative Commons Nevezd meg! – Ne változtasd! 2.5 Általános"@hu,
        "Creative Commons Attribuzione – Non opere derivate 2.5 Generico"@it,
        "Creative Commons Priskyrimas – Jokių išvestinių darbų 2.5 Bendrasis"@lt,
        "Creative Commons Atsaucoties–Nepārveidojot 2.5 Vispārīgs"@lv,
        "Creative Commons Attribuzzjoni-EbdaDerivattivi 2.5 Generic"@mt,
        "Creative Commons Naamsvermelding–GeenAfgeleideWerken 2.5 Unported"@nl,
        "Creative Commons Uznanie autorstwa–Bez utworów zależnych 2.5 Ogólny"@pl,
        "Creative Commons Atribuição–SemDerivações 2.5 Genérica"@pt,
        "Creative Commons Atribuire–FărăModificări 2.5 Generică"@ro,
        "Creative Commons Uvedenie Autora-Bez Odvodeného Obsahu 2.5 Generic"@sk,
        "Creative Commons Priznanje avtorstva-Brez predelav 2.5 Generična"@sl,
        "Creative Commons Erkännande–IngaBearbetningar 2.5 Generisk"@sv ;
    skos:topConceptOf atold:licence .

<http://publications.europa.eu/resource/authority/licence/CC_BYND_3_0> a skos:Concept ;
    at:authority-code "CC_BYND_3_0" ;
    at:deprecated "false" ;
    at:op-code "CC_BYND_3_0" ;
    at:start.use "2007-02-23" ;
    atold:op-code "CC_BYND_3_0" ;
    dc:identifier "CC_BYND_3_0" ;
    skos:altLabel "CC BY-ND 3.0"@bg,
        "CC BY-ND 3.0"@cs,
        "CC BY-ND 3.0"@da,
        "CC BY-ND 3.0"@de,
        "CC BY-ND 3.0"@el,
        "CC BY-ND 3.0"@en,
        "CC BY-ND 3.0"@es,
        "CC BY-ND 3.0"@et,
        "CC BY-ND 3.0"@fi,
        "CC BY-ND 3.0"@fr,
        "CC BY-ND 3.0"@ga,
        "CC BY-ND 3.0"@hr,
        "CC BY-ND 3.0"@hu,
        "CC BY-ND 3.0"@it,
        "CC BY-ND 3.0"@lt,
        "CC BY-ND 3.0"@lv,
        "CC BY-ND 3.0"@mt,
        "CC BY-ND 3.0"@nl,
        "CC BY-ND 3.0"@pl,
        "CC BY-ND 3.0"@pt,
        "CC BY-ND 3.0"@ro,
        "CC BY-ND 3.0"@sk,
        "CC BY-ND 3.0"@sl,
        "CC BY-ND 3.0"@sv ;
    skos:definition "CC BY-ND 3.0 allows for redistribution, commercial and non-commercial, as long as it is passed along unchanged and in whole, with credit to the author."@en,
        "CC BY-ND 3.0 autorise la redistribution, à des fins commerciales ou non, tant que l’œuvre est diffusée sans modification et dans son intégralité, avec attribution et citation du nom de l’auteur/autrice."@fr ;
    skos:exactMatch <http://creativecommons.org/licenses/by-nd/3.0/> ;
    skos:historyNote "Unported licences are licences that are not associated with any specific jurisdiction, e.g. country."@en ;
    skos:inScheme atold:licence ;
    skos:prefLabel "Creative Commons Признание-Без производни 3.0 Нелокализиран"@bg,
        "Creative Commons Uveďte původ–Nezpracovávejte 3.0 Unported"@cs,
        "Creative Commons Navngivelse–IngenBearbejdelse 3.0 Unported"@da,
        "Creative Commons Namensnennung – Keine Bearbeitung 3.0 Unported"@de,
        "Creative Commons Αναφορά Δημιουργού – Όχι Παράγωγα Έργα 3.0 Μη εισαγόμενο"@el,
        "Creative Commons Attribution–NoDerivs 3.0 Unported"@en,
        "Creative Commons Atribución–SinDerivadas 3.0 Unported"@es,
        "Creative Commons Autorile viitamine–Tuletatud teoste keeld 3.0 Jurisdiktsiooniga sidumata"@et,
        "Creative Commons Nimeä–EiMuutoksia 3.0 Ei sovitettu"@fi,
        "Creative Commons Attribution – Pas de Modification 3.0 non transposé"@fr,
        "Creative Commons Imenovanje–Bez prerada 3.0 nelokalizirana licenca"@hr,
        "Creative Commons Nevezd meg! – Ne változtasd! 3.0 Unported"@hu,
        "Creative Commons Attribuzione – Non opere derivate 3.0 Unported"@it,
        "Creative Commons Priskyrimas – Jokių išvestinių darbų 3.0 Nepritaikyta jurisdikcijai"@lt,
        "Creative Commons Atsaucoties–Nepārveidojot 3.0 Nepārnesta"@lv,
        "Creative Commons Attribuzzjoni-EbdaDerivattivi 3.0 Unported"@mt,
        "Creative Commons Naamsvermelding–GeenAfgeleideWerken 3.0 Unported"@nl,
        "Creative Commons Uznanie autorstwa–Bez utworów zależnych 3.0 Unported"@pl,
        "Creative Commons Atribuição–SemDerivações 3.0 Não Adaptada"@pt,
        "Creative Commons Atribuire-FărăModificări 3.0 Ne-adaptată"@ro,
        "Creative Commons Uvedenie Autora-Bez Odvodeného Obsahu 3.0 Unported"@sk,
        "Creative Commons Priznanje avtorstva-Brez predelav 3.0 Nedoločena"@sl,
        "Creative Commons Erkännande–IngaBearbetningar 3.0 Unported"@sv ;
    skos:topConceptOf atold:licence .

<http://publications.europa.eu/resource/authority/licence/CC_BYND_4_0> a skos:Concept ;
    at:authority-code "CC_BYND_4_0" ;
    at:deprecated "false" ;
    at:op-code "CC_BYND_4_0" ;
    at:start.use "2013-11-26" ;
    atold:op-code "CC_BYND_4_0" ;
    dc:identifier "CC_BYND_4_0" ;
    skos:altLabel "CC BY-ND 4.0"@bg,
        "CC BY-ND 4.0"@cs,
        "CC BY-ND 4.0"@da,
        "CC BY-ND 4.0"@de,
        "CC BY-ND 4.0"@el,
        "CC BY-ND 4.0"@en,
        "CC BY-ND 4.0"@es,
        "CC BY-ND 4.0"@et,
        "CC BY-ND 4.0"@fi,
        "CC BY-ND 4.0"@fr,
        "CC BY-ND 4.0"@ga,
        "CC BY-ND 4.0"@hr,
        "CC BY-ND 4.0"@hu,
        "CC BY-ND 4.0"@it,
        "CC BY-ND 4.0"@lt,
        "CC BY-ND 4.0"@lv,
        "CC BY-ND 4.0"@mt,
        "CC BY-ND 4.0"@nl,
        "CC BY-ND 4.0"@pl,
        "CC BY-ND 4.0"@pt,
        "CC BY-ND 4.0"@ro,
        "CC BY-ND 4.0"@sk,
        "CC BY-ND 4.0"@sl,
        "CC BY-ND 4.0"@sv ;
    skos:definition "CC BY-ND 4.0 allows for redistribution, commercial and non-commercial, as long as it is passed along unchanged and in whole, with credit to the author."@en,
        "CC BY-ND 4.0 autorise la redistribution, à des fins commerciales ou non, tant que l’œuvre est diffusée sans modification et dans son intégralité, avec attribution et citation du nom de l’auteur/autrice."@fr ;
    skos:exactMatch <http://creativecommons.org/licenses/by-nd/4.0/> ;
    skos:inScheme atold:licence ;
    skos:prefLabel "Creative Commons Признание-Без производни 4.0 Международен"@bg,
        "Creative Commons Uveďte původ–Nezpracovávejte 4.0 Mezinárodní"@cs,
        "Creative Commons Navngivelse–IngenBearbejdelse 4.0 International"@da,
        "Creative Commons Namensnennung – Keine Bearbeitungen 4.0 International"@de,
        "Creative Commons Αναφορά Δημιουργού – Όχι Παράγωγα Έργα 4.0 Διεθνές"@el,
        "Creative Commons Attribution–NoDerivatives 4.0 International"@en,
        "Creative Commons Atribución–SinDerivar 4.0 Internacional"@es,
        "Creative Commons Autorile viitamine–Tuletatud teoste keeld 4.0 Rahvusvaheline"@et,
        "Creative Commons Nimeä–EiMuutoksia 4.0 Kansainvälinen"@fi,
        "Creative Commons Attribution – Pas de Modification 4.0 International"@fr,
        "Creative Commons Imenovanje–Bez prerada 4.0 međunarodna"@hr,
        "Creative Commons Nevezd meg! – Ne változtasd! 4.0 Nemzetközi"@hu,
        "Creative Commons Attribuzione – Non opere derivate 4.0 Internazionale"@it,
        "Creative Commons Priskyrimas – Jokių išvestinių darbų 4.0 Tarptautinė"@lt,
        "Creative Commons Atsaucoties, nepārveidojot 4.0 Internacionāls"@lv,
        "Creative Commons Attribuzzjoni-EbdaDerivattivi 4.0 Internazzjonali"@mt,
        "Creative Commons Naamsvermelding–GeenAfgeleideWerken 4.0 Internationaal"@nl,
        "Creative Commons Uznanie autorstwa – Bez utworów zależnych 4.0 Międzynarodowe"@pl,
        "Creative Commons Atribuição–SemDerivações 4.0 Internacional"@pt,
        "Creative Commons Atribuire–FărăDerivate 4.0 Internațional"@ro,
        "Creative Commons Uvedenie Autora-Žiadne Odvodené Diela 4.0 Medzinárodný"@sk,
        "Creative Commons Priznanje avtorstva-Brez predelav 4.0 Mednarodna"@sl,
        "Creative Commons Erkännande–IngaBearbetningar 4.0 Internationell"@sv ;
    skos:topConceptOf atold:licence .

<http://publications.europa.eu/resource/authority/licence/CC_BYSA> a skos:Concept ;
    at:authority-code "CC_BYSA" ;
    at:deprecated "true" ;
    at:end.use "2013-11-26" ;
    at:op-code "CC_BYSA" ;
    at:start.use "2013-11-25" ;
    atold:op-code "CC_BYSA" ;
    dc:identifier "CC_BYSA" ;
    skos:altLabel "CC BY-SA 4.0"@bg,
        "CC BY-SA 4.0"@cs,
        "CC BY-SA 4.0"@da,
        "CC BY-SA 4.0"@de,
        "CC BY-SA 4.0"@el,
        "CC BY-SA 4.0"@en,
        "CC BY-SA 4.0"@es,
        "CC BY-SA 4.0"@et,
        "CC BY-SA 4.0"@fi,
        "CC BY-SA 4.0"@fr,
        "CC BY-SA 4.0"@ga,
        "CC BY-SA 4.0"@hr,
        "CC BY-SA 4.0"@hu,
        "CC BY-SA 4.0"@it,
        "CC BY-SA 4.0"@lt,
        "CC BY-SA 4.0"@lv,
        "CC BY-SA 4.0"@mt,
        "CC BY-SA 4.0"@nl,
        "CC BY-SA 4.0"@pl,
        "CC BY-SA 4.0"@pt,
        "CC BY-SA 4.0"@ro,
        "CC BY-SA 4.0"@sk,
        "CC BY-SA 4.0"@sl,
        "CC BY-SA 4.0"@sv ;
    skos:definition "This licence lets others remix, tweak, and build upon the author's work even for commercial purposes, as long as they credit the author and licence their new creations under the identical terms. This licence is often compared to “copyleft” free and open source software licences. All new works based on the original work will carry the same licence, so any derivatives will also allow commercial use. This is the licence used by Wikipedia, and is recommended for materials that would benefit from incorporating content from Wikipedia and similarly licenced projects."@en,
        "Cette licence permet aux autres de remixer, arranger, et adapter l’œuvre de l’auteur/l’autrice, même à des fins commerciales, tant qu’on accorde le mérite de la création originale à l’auteur/l’autrice en citant son nom et qu’on diffuse les nouvelles créations selon des conditions identiques. Cette licence est souvent comparée aux licences de logiciels libres, «open source» ou «copyleft». Toutes les nouvelles œuvres basées sur celles de l’auteur/autrice auront la même licence, et toute œuvre dérivée pourra être utilisée même à des fins commerciales. C’est la licence utilisée par Wikipédia; elle est recommandée pour des œuvres qui pourraient bénéficier de l’incorporation de contenu depuis Wikipédia et d’autres projets sous licence similaire."@fr ;
    skos:inScheme atold:licence ;
    skos:prefLabel "Creative Commons Uveďte původ–Zachovejte licenci 4.0 Mezinárodní"@cs,
        "Creative Commons Navngivelse–DelPåSammeVilkår 4.0 International"@da,
        "Creative Commons Namensnennung – Weitergabe unter gleichen Bedingungen 4.0 International"@de,
        "Creative Commons Αναφορά Δημιουργού – Παρόμοια Διανομή 4.0 Διεθνές"@el,
        "Creative Commons Attribution–ShareAlike 4.0 International"@en,
        "Creative Commons Atribución–CompartirIgual 4.0 Internacional"@es,
        "Creative Commons Nimeä–JaaSamoin 4.0 Kansainvälinen"@fi,
        "Creative Commons Attribution – Partage dans les Mêmes Conditions 4.0 International"@fr,
        "Creative Commons Imenovanje–Dijeli pod istim uvjetima 4.0 međunarodna"@hr,
        "Creative Commons Nevezd meg! – Így add tovább! 4.0 Nemzetközi"@hu,
        "Creative Commons Attribuzione – Condividi allo stesso modo 4.0 Internazionale"@it,
        "Creative Commons Priskyrimas – Analogiškas platinimas 4.0 Tarptautinė"@lt,
        "Creative Commons Atsaucoties–Nemainot licenci 4.0 Internacionāls"@lv,
        "Creative Commons Naamsvermelding–GelijkDelen 4.0 Internationaal"@nl,
        "Creative Commons Uznanie autorstwa–Na tych samych warunkach 4.0 Międzynarodowe"@pl,
        "Creative Commons Atribuição–CompartilhaIgual 4.0 Internacional"@pt,
        "Creative Commons Atribuire–Distribuire în condiţii identice 4.0 Internațional"@ro,
        "Creative Commons Erkännande–DelaLika 4.0 Internationell"@sv ;
    skos:topConceptOf atold:licence .

<http://publications.europa.eu/resource/authority/licence/CC_BYSA_1_0> a skos:Concept ;
    at:authority-code "CC_BYSA_1_0" ;
    at:deprecated "true" ;
    at:end.use "2004-05-24" ;
    at:op-code "CC_BYSA_1_0" ;
    at:start.use "2002-12-15" ;
    atold:op-code "CC_BYSA_1_0" ;
    dc:identifier "CC_BYSA_1_0" ;
    skos:altLabel "CC BY-SA 1.0"@bg,
        "CC BY-SA 1.0"@cs,
        "CC BY-SA 1.0"@da,
        "CC BY-SA 1.0"@de,
        "CC BY-SA 1.0"@el,
        "CC BY-SA 1.0"@en,
        "CC BY-SA 1.0"@es,
        "CC BY-SA 1.0"@et,
        "CC BY-SA 1.0"@fi,
        "CC BY-SA 1.0"@fr,
        "CC BY-SA 1.0"@ga,
        "CC BY-SA 1.0"@hr,
        "CC BY-SA 1.0"@hu,
        "CC BY-SA 1.0"@it,
        "CC BY-SA 1.0"@lt,
        "CC BY-SA 1.0"@lv,
        "CC BY-SA 1.0"@mt,
        "CC BY-SA 1.0"@nl,
        "CC BY-SA 1.0"@pl,
        "CC BY-SA 1.0"@pt,
        "CC BY-SA 1.0"@ro,
        "CC BY-SA 1.0"@sk,
        "CC BY-SA 1.0"@sl,
        "CC BY-SA 1.0"@sv ;
    skos:definition "CC BY-SA 1.0 lets others remix, tweak, and build upon the author’s work even for commercial purposes, as long as they credit the author and licence their new creations under the identical terms. This licence is often compared to “copyleft” free and open source software licences. All new works based on the original work will carry the same licence, so any derivatives will also allow commercial use. This is the licence used by Wikipedia, and is recommended for materials that would benefit from incorporating content from Wikipedia and similarly licenced projects."@en,
        "CC BY-SA 1.0 permet aux autres de remixer, arranger, et adapter l’œuvre de l’auteur/autrice, même à des fins commerciales, tant qu’on accorde le mérite de la création originale à l’auteur/autrice en citant son nom et qu’on diffuse les nouvelles créations selon des conditions identiques. Cette licence est souvent comparée aux licences de logiciels libres, «open source» ou «copyleft». Toutes les nouvelles œuvres basées sur celles de l’auteur/autrice auront la même licence, et toute œuvre dérivée pourra être utilisée même à des fins commerciales. C’est la licence utilisée par Wikipédia; elle est recommandée pour des œuvres qui pourraient bénéficier de l’incorporation de contenu depuis Wikipédia et d’autres projets sous licence similaire."@fr ;
    skos:exactMatch <http://creativecommons.org/licenses/by-sa/1.0/> ;
    skos:inScheme atold:licence ;
    skos:prefLabel "Creative Commons Признание-Споделяне на споделеното 1.0 Неадаптира"@bg,
        "Creative Commons Uveďte původ–Zachovejte licenci 1.0 Generic"@cs,
        "Creative Commons Navngivelse–DelPåSammeVilkår 1.0 Generisk"@da,
        "Creative Commons Namensnennung – Weitergabe unter gleichen Bedingungen 1.0 Generic"@de,
        "Creative Commons Αναφορά Δημιουργού – Παρόμοια Διανομή 1.0 Μη εισαγόμενο"@el,
        "Creative Commons Attribution–ShareAlike 1.0 Generic"@en,
        "Creative Commons Atribución–CompartirIgual 1.0 Genérica"@es,
        "Creative Commons Autorile viitamine–Jagamine samadel tingimustel 1.0 Üldine"@et,
        "Creative Commons Nimeä–JaaSamoin 1.0 Yleinen"@fi,
        "Creative Commons Attribution – Partage dans les Mêmes Conditions 1.0 Générique"@fr,
        "Creative Commons Imenovanje–Dijeli pod istim uvjetima 1.0 nelokalizirana licenca"@hr,
        "Creative Commons Nevezd meg! – Így add tovább! 1.0 Általános"@hu,
        "Creative Commons Attribuzione – Condividi allo stesso modo 1.0 Generico"@it,
        "Creative Commons Priskyrimas – Analogiškas platinimas 1.0 Bendrasis"@lt,
        "Creative Commons Atsaucoties–Nemainot licenci 1.0 Vispārīgs"@lv,
        "Creative Commons Attribuzzjoni-KondiviżjoniUgwali 1.0 Generic"@mt,
        "Creative Commons Naamsvermelding–GelijkDelen 1.0 Unported"@nl,
        "Creative Commons Uznanie autorstwa–Na tych samych warunkach 1.0 Ogólny"@pl,
        "Creative Commons Atribuição–CompartilhaIgual 1.0 Genérica"@pt,
        "Creative Commons Atribuire–Distribuire în condiţii identice 1.0 Generică"@ro,
        "Creative Commons Uvedenie Autora-Rovnaké Šírenie 1.0 Generic"@sk,
        "Creative Commons Priznanje avtorstva-Deljenje pod enakimi pogoji 1.0 Generična"@sl,
        "Creative Commons Erkännande–DelaLika 1.0 Generisk"@sv ;
    skos:topConceptOf atold:licence .

<http://publications.europa.eu/resource/authority/licence/CC_BYSA_2_0> a skos:Concept ;
    at:authority-code "CC_BYSA_2_0" ;
    at:deprecated "false" ;
    at:op-code "CC_BYSA_2_0" ;
    at:start.use "2004-05-25" ;
    atold:op-code "CC_BYSA_2_0" ;
    dc:identifier "CC_BYSA_2_0" ;
    skos:altLabel "CC BY-SA 2.0"@bg,
        "CC BY-SA 2.0"@cs,
        "CC BY-SA 2.0"@da,
        "CC BY-SA 2.0"@de,
        "CC BY-SA 2.0"@el,
        "CC BY-SA 2.0"@en,
        "CC BY-SA 2.0"@es,
        "CC BY-SA 2.0"@et,
        "CC BY-SA 2.0"@fi,
        "CC BY-SA 2.0"@fr,
        "CC BY-SA 2.0"@ga,
        "CC BY-SA 2.0"@hr,
        "CC BY-SA 2.0"@hu,
        "CC BY-SA 2.0"@it,
        "CC BY-SA 2.0"@lt,
        "CC BY-SA 2.0"@lv,
        "CC BY-SA 2.0"@mt,
        "CC BY-SA 2.0"@nl,
        "CC BY-SA 2.0"@pl,
        "CC BY-SA 2.0"@pt,
        "CC BY-SA 2.0"@ro,
        "CC BY-SA 2.0"@sk,
        "CC BY-SA 2.0"@sl,
        "CC BY-SA 2.0"@sv ;
    skos:definition "CC BY-SA 2.0 lets others remix, tweak, and build upon the author’s work even for commercial purposes, as long as they credit the author and licence their new creations under the identical terms. This licence is often compared to “copyleft” free and open source software licences. All new works based on the original work will carry the same licence, so any derivatives will also allow commercial use. This is the licence used by Wikipedia, and is recommended for materials that would benefit from incorporating content from Wikipedia and similarly licenced projects."@en,
        "CC BY-SA 2.0 permet aux autres de remixer, arranger, et adapter l’œuvre de l’auteur/autrice, même à des fins commerciales, tant qu’on accorde le mérite de la création originale à l’auteur/autrice en citant son nom et qu’on diffuse les nouvelles créations selon des conditions identiques. Cette licence est souvent comparée aux licences de logiciels libres, «open source» ou «copyleft». Toutes les nouvelles œuvres basées sur celles de l’auteur/autrice auront la même licence, et toute œuvre dérivée pourra être utilisée même à des fins commerciales. C’est la licence utilisée par Wikipédia; elle est recommandée pour des œuvres qui pourraient bénéficier de l’incorporation de contenu depuis Wikipédia et d’autres projets sous licence similaire."@fr ;
    skos:exactMatch <http://creativecommons.org/licenses/by-sa/2.0/> ;
    skos:inScheme atold:licence ;
    skos:prefLabel "Creative Commons Признание-Споделяне на споделеното 2.0 Неадаптиран"@bg,
        "Creative Commons Uveďte původ–Zachovejte licenci 2.0 Generic"@cs,
        "Creative Commons Navngivelse–DelPåSammeVilkår 2.0 Generisk"@da,
        "Creative Commons Namensnennung – Weitergabe unter gleichen Bedingungen 2.0 Generic"@de,
        "Creative Commons Αναφορά Δημιουργού – Παρόμοια Διανομή 2.0 Μη εισαγόμενο"@el,
        "Creative Commons Attribution–ShareAlike 2.0 Generic"@en,
        "Creative Commons Atribución–CompartirIgual 2.0 Genérica"@es,
        "Creative Commons Autorile viitamine–Jagamine samadel tingimustel 2.0 Üldine"@et,
        "Creative Commons Nimeä–JaaSamoin 2.0 Yleinen"@fi,
        "Creative Commons Attribution – Partage dans les Mêmes Conditions 2.0 Générique"@fr,
        "Creative Commons Imenovanje–Dijeli pod istim uvjetima 2.0 nelokalizirana licenca"@hr,
        "Creative Commons Nevezd meg! – Így add tovább! 2.0 Általános"@hu,
        "Creative Commons Attribuzione – Condividi allo stesso modo 2.0 Generico"@it,
        "Creative Commons Priskyrimas – Analogiškas platinimas 2.0 Bendrasis"@lt,
        "Creative Commons Atsaucoties–Nemainot licenci 2.0 Vispārīgs"@lv,
        "Creative Commons Attribuzzjoni-KondiviżjoniUgwali 2.0 Generic"@mt,
        "Creative Commons Naamsvermelding–GelijkDelen 2.0 Unported"@nl,
        "Creative Commons Uznanie autorstwa–Na tych samych warunkach 2.0 Ogólny"@pl,
        "Creative Commons Atribuição–CompartilhaIgual 2.0 Genérica"@pt,
        "Creative Commons Atribuire–Distribuire în condiţii identice 2.0 Generică"@ro,
        "Creative Commons Uvedenie Autora-Rovnaké Šírenie 2.0 Generic"@sk,
        "Creative Commons Priznanje avtorstva-Deljenje pod enakimi pogoji 2.0 Generična"@sl,
        "Creative Commons Erkännande–DelaLika 2.0 Generisk"@sv ;
    skos:topConceptOf atold:licence .

<http://publications.europa.eu/resource/authority/licence/CC_BYSA_2_5> a skos:Concept ;
    at:authority-code "CC_BYSA_2_5" ;
    at:deprecated "false" ;
    at:op-code "CC_BYSA_2_5" ;
    at:start.use "2005-06-01" ;
    atold:op-code "CC_BYSA_2_5" ;
    dc:identifier "CC_BYSA_2_5" ;
    skos:altLabel "CC BY-SA 2.5"@bg,
        "CC BY-SA 2.5"@cs,
        "CC BY-SA 2.5"@da,
        "CC BY-SA 2.5"@de,
        "CC BY-SA 2.5"@el,
        "CC BY-SA 2.5"@en,
        "CC BY-SA 2.5"@es,
        "CC BY-SA 2.5"@et,
        "CC BY-SA 2.5"@fi,
        "CC BY-SA 2.5"@fr,
        "CC BY-SA 2.5"@ga,
        "CC BY-SA 2.5"@hr,
        "CC BY-SA 2.5"@hu,
        "CC BY-SA 2.5"@it,
        "CC BY-SA 2.5"@lt,
        "CC BY-SA 2.5"@lv,
        "CC BY-SA 2.5"@mt,
        "CC BY-SA 2.5"@nl,
        "CC BY-SA 2.5"@pl,
        "CC BY-SA 2.5"@pt,
        "CC BY-SA 2.5"@ro,
        "CC BY-SA 2.5"@sk,
        "CC BY-SA 2.5"@sl,
        "CC BY-SA 2.5"@sv ;
    skos:definition "CC BY-SA 2.5 lets others remix, tweak, and build upon the author’s work even for commercial purposes, as long as they credit the author and licence their new creations under the identical terms. This licence is often compared to “copyleft” free and open source software licences. All new works based on the original work will carry the same licence, so any derivatives will also allow commercial use. This is the licence used by Wikipedia, and is recommended for materials that would benefit from incorporating content from Wikipedia and similarly licenced projects."@en,
        "CC BY-SA 2.5 permet aux autres de remixer, arranger, et adapter l’œuvre de l’auteur/autrice, même à des fins commerciales, tant qu’on accorde le mérite de la création originale à l’auteur/autrice en citant son nom et qu’on diffuse les nouvelles créations selon des conditions identiques. Cette licence est souvent comparée aux licences de logiciels libres, «open source» ou «copyleft». Toutes les nouvelles œuvres basées sur celles de l’auteur/autrice auront la même licence, et toute œuvre dérivée pourra être utilisée même à des fins commerciales. C’est la licence utilisée par Wikipédia; elle est recommandée pour des œuvres qui pourraient bénéficier de l’incorporation de contenu depuis Wikipédia et d’autres projets sous licence similaire."@fr ;
    skos:exactMatch <http://creativecommons.org/licenses/by-sa/2.5/> ;
    skos:inScheme atold:licence ;
    skos:prefLabel "Creative Commons Признание-Споделяне на споделеното 2.5 Неадаптиран"@bg,
        "Creative Commons Uveďte původ–Zachovejte licenci 2.5 Generic"@cs,
        "Creative Commons Navngivelse–DelPåSammeVilkår 2.5 Generisk"@da,
        "Creative Commons Namensnennung – Weitergabe unter gleichen Bedingungen 2.5 Generic"@de,
        "Creative Commons Αναφορά Δημιουργού – Παρόμοια Διανομή 2.5 Μη εισαγόμενο"@el,
        "Creative Commons Attribution–ShareAlike 2.5 Generic"@en,
        "Creative Commons Atribución–CompartirIgual 2.5 Genérica"@es,
        "Creative Commons Autorile viitamine–Jagamine samadel tingimustel 2.5 Üldine"@et,
        "Creative Commons Nimeä–JaaSamoin 2.5 Yleinen"@fi,
        "Creative Commons Attribution – Partage dans les Mêmes Conditions 2.5 Générique"@fr,
        "Creative Commons Imenovanje–Dijeli pod istim uvjetima 2.5 nelokalizirana licenca"@hr,
        "Creative Commons Nevezd meg! – Így add tovább! 2.5 Általános"@hu,
        "Creative Commons Attribuzione – Condividi allo stesso modo 2.5 Generico"@it,
        "Creative Commons Priskyrimas – Analogiškas platinimas 2.5 Bendrasis"@lt,
        "Creative Commons Atsaucoties–Nemainot licenci 2.5 Vispārīgs"@lv,
        "Creative Commons Attribuzzjoni-KondiviżjoniUgwali 2.5 Generic"@mt,
        "Creative Commons Naamsvermelding–GelijkDelen 2.5 Unported"@nl,
        "Creative Commons Uznanie autorstwa–Na tych samych warunkach 2.5 Ogólny"@pl,
        "Creative Commons Atribuição–CompartilhaIgual 2.5 Genérica"@pt,
        "Creative Commons Atribuire–Distribuire în condiţii identice 2.5 Generică"@ro,
        "Creative Commons Uvedenie Autora-Rovnaké Šírenie 2.5 Generic"@sk,
        "Creative Commons Priznanje avtorstva-Deljenje pod enakimi pogoji 2.5 Generična"@sl,
        "Creative Commons Erkännande–DelaLika 2.5 Generisk"@sv ;
    skos:topConceptOf atold:licence .

<http://publications.europa.eu/resource/authority/licence/CC_BYSA_3_0> a skos:Concept ;
    at:authority-code "CC_BYSA_3_0" ;
    at:deprecated "false" ;
    at:op-code "CC_BYSA_3_0" ;
    at:start.use "2007-02-23" ;
    atold:op-code "CC_BYSA_3_0" ;
    dc:identifier "CC_BYSA_3_0" ;
    skos:altLabel "CC BY-SA 3.0"@bg,
        "CC BY-SA 3.0"@cs,
        "CC BY-SA 3.0"@da,
        "CC BY-SA 3.0"@de,
        "CC BY-SA 3.0"@el,
        "CC BY-SA 3.0"@en,
        "CC BY-SA 3.0"@es,
        "CC BY-SA 3.0"@et,
        "CC BY-SA 3.0"@fi,
        "CC BY-SA 3.0"@fr,
        "CC BY-SA 3.0"@ga,
        "CC BY-SA 3.0"@hr,
        "CC BY-SA 3.0"@hu,
        "CC BY-SA 3.0"@it,
        "CC BY-SA 3.0"@lt,
        "CC BY-SA 3.0"@lv,
        "CC BY-SA 3.0"@mt,
        "CC BY-SA 3.0"@nl,
        "CC BY-SA 3.0"@pl,
        "CC BY-SA 3.0"@pt,
        "CC BY-SA 3.0"@ro,
        "CC BY-SA 3.0"@sk,
        "CC BY-SA 3.0"@sl,
        "CC BY-SA 3.0"@sv ;
    skos:definition "CC BY-SA 3.0 lets others remix, tweak, and build upon the author’s work even for commercial purposes, as long as they credit the author and licence their new creations under the identical terms. This licence is often compared to “copyleft” free and open source software licences. All new works based on the original work will carry the same licence, so any derivatives will also allow commercial use. This is the licence used by Wikipedia, and is recommended for materials that would benefit from incorporating content from Wikipedia and similarly licenced projects."@en,
        "CC BY-SA 3.0 permet aux autres de remixer, arranger, et adapter l’œuvre de l’auteur/autrice, même à des fins commerciales, tant qu’on accorde le mérite de la création originale à l’auteur/autrice en citant son nom et qu’on diffuse les nouvelles créations selon des conditions identiques. Cette licence est souvent comparée aux licences de logiciels libres, «open source» ou «copyleft». Toutes les nouvelles œuvres basées sur les œuvres de l’auteur/autrice auront la même licence, et toute œuvre dérivée pourra être utilisée même à des fins commerciales. C’est la licence utilisée par Wikipédia; elle est recommandée pour des œuvres qui pourraient bénéficier de l’incorporation de contenu depuis Wikipédia et d’autres projets sous licence similaire."@fr ;
    skos:exactMatch <http://creativecommons.org/licenses/by-sa/3.0/> ;
    skos:historyNote "Unported licences are licences that are not associated with any specific jurisdiction, e.g. country."@en ;
    skos:inScheme atold:licence ;
    skos:prefLabel "Creative Commons Признание-Споделяне на споделеното 3.0 Нелокализиран"@bg,
        "Creative Commons Uveďte původ–Zachovejte licenci 3.0 Unported"@cs,
        "Creative Commons Navngivelse–DelPåSammeVilkår 3.0 Unported"@da,
        "Creative Commons Namensnennung – Weitergabe unter gleichen Bedingungen 3.0 Unported"@de,
        "Creative Commons Αναφορά Δημιουργού – Παρόμοια Διανομή 3.0 Μη εισαγόμενο"@el,
        "Creative Commons Attribution–ShareAlike 3.0 Unported"@en,
        "Creative Commons Atribución–CompartirIgual 3.0 Unported"@es,
        "Creative Commons Autorile viitamine–Jagamine samadel tingimustel 3.0 Jurisdiktsiooniga sidumata"@et,
        "Creative Commons Nimeä–JaaSamoin 3.0 Ei sovitettu"@fi,
        "Creative Commons Attribution – Partage dans les Mêmes Conditions 3.0 non transposé"@fr,
        "Creative Commons Imenovanje–Dijeli pod istim uvjetima 3.0 nelokalizirana licenca"@hr,
        "Creative Commons Nevezd meg! – Így add tovább! 3.0 Unported"@hu,
        "Creative Commons Attribuzione – Condividi allo stesso modo 3.0 Unported"@it,
        "Creative Commons Priskyrimas – Analogiškas platinimas 3.0 Nepritaikyta jurisdikcijai"@lt,
        "Creative Commons Atsaucoties–Nemainot licenci 3.0 Nepārnesta"@lv,
        "Creative Commons Attribuzzjoni-KondiviżjoniUgwali 3.0 Unported"@mt,
        "Creative Commons Naamsvermelding–GelijkDelen 3.0 Unported"@nl,
        "Creative Commons Uznanie autorstwa–Na tych samych warunkach 3.0 Unported"@pl,
        "Creative Commons Atribuição–CompartilhaIgual 3.0 Não Adaptada"@pt,
        "Creative Commons Atribuire–Distribuire în condiţii identice 3.0 Ne-adaptată"@ro,
        "Creative Commons Uvedenie Autora-Rovnaké Šírenie 3.0 Unported"@sk,
        "Creative Commons Priznanje avtorstva-Deljenje pod enakimi pogoji 3.0 Nedoločena"@sl,
        "Creative Commons Erkännande–DelaLika 3.0 Unported"@sv ;
    skos:topConceptOf atold:licence .

<http://publications.europa.eu/resource/authority/licence/CC_BYSA_3_0_NL> a skos:Concept ;
    at:authority-code "CC_BYSA_3_0_NL" ;
    at:deprecated "false" ;
    at:op-code "CC_BYSA_3_0_NL" ;
    at:start.use "2007-02-23" ;
    atold:op-code "CC_BYSA_3_0_NL" ;
    dc:identifier "CC_BYSA_3_0_NL" ;
    skos:altLabel "CC BY-SA 3.0 NL"@bg,
        "CC BY-SA 3.0 NL"@cs,
        "CC BY-SA 3.0 NL"@da,
        "CC BY-SA 3.0 NL"@de,
        "CC BY-SA 3.0 NL"@el,
        "CC BY-SA 3.0 NL"@en,
        "CC BY-SA 3.0 NL"@es,
        "CC BY-SA 3.0 NL"@et,
        "CC BY-SA 3.0 NL"@fi,
        "CC BY-SA 3.0 NL"@fr,
        "CC BY-SA 3.0 NL"@ga,
        "CC BY-SA 3.0 NL"@hr,
        "CC BY-SA 3.0 NL"@hu,
        "CC BY-SA 3.0 NL"@it,
        "CC BY-SA 3.0 NL"@lt,
        "CC BY-SA 3.0 NL"@lv,
        "CC BY-SA 3.0 NL"@mt,
        "CC BY-SA 3.0 NL"@nl,
        "CC BY-SA 3.0 NL"@pl,
        "CC BY-SA 3.0 NL"@pt,
        "CC BY-SA 3.0 NL"@ro,
        "CC BY-SA 3.0 NL"@sk,
        "CC BY-SA 3.0 NL"@sl,
        "CC BY-SA 3.0 NL"@sv ;
    skos:definition "Published by Creative Commons for Netherlands, Naamsvermelding-GelijkDelen 3.0 Nederland (CC BY-SA 3.0 NL) is a licence permitting any commercial and non-commercial use, as long as credit is given to the author for the original creation and new creations are licenced under the identical terms. All new works based on the original work will carry the same licence, so any derivatives will also allow commercial use."@en ;
    skos:exactMatch <http://creativecommons.org/licenses/by-sa/3.0/nl/legalcode/> ;
    skos:inScheme atold:licence ;
    skos:prefLabel "Признание-Споделяне на споделеното 3.0 Холандия"@bg,
        "Uveďte původ–Zachovejte licenci 3.0 Nizozemí"@cs,
        "Kreditering–Deling på samme vilkår 3.0 Holland"@da,
        "Namensnennung – Weitergabe unter gleichen Bedingungen 3.0 Niederlande"@de,
        "Αναφορά Δημιουργού – Παρόμοια Διανομή 3.0 Ολλανδία"@el,
        "Naamsvermelding–GelijkDelen 3.0 Nederland"@en,
        "Reconocimiento–CompartirIgual 3.0 Países Bajos"@es,
        "Autorile viitamine–Jagamine samadel tingimustel 3.0 Holland"@et,
        "Nimeä–JaaSamoin 3.0 Hollanti"@fi,
        "Attribution – Partage dans les Mêmes Conditions 3.0 Pays-Bas"@fr,
        "Imenovanje–Dijeli pod istim uvjetima 3.0 Nizozemska"@hr,
        "Nevezd meg! – Így add tovább! 3.0 Hollandia"@hu,
        "Attribuzione – Condividi allo stesso modo 3.0 Olanda"@it,
        "Priskyrimas – Analogiškas platinimas 3.0 Nyderlandai"@lt,
        "Attiecinājums–Dalīties līdzīgi 3.0 Nīderlande"@lv,
        "Attribuzzjoni-KondiviżjoniUgwali 3.0 Pajjiżi l-Baxxi"@mt,
        "Naamsvermelding–GelijkDelen 3.0 Nederland"@nl,
        "Uznanie autorstwa–Na tych samych warunkach 3.0 Holandia"@pl,
        "Atribuição–CompartilhaIgual 3.0 Holanda"@pt,
        "Atribuire – Distribuire în condiţii identice 3.0 Olanda"@ro,
        "Uvedenie Autora-Rovnaké Šírenie 3.0 Holandsko"@sk,
        "Priznanje avtorstva-Deljenje pod enakimi pogoji 3.0 Nizozemska"@sl,
        "Erkännande–DelaLika 3.0 Nederländerna"@sv ;
    skos:topConceptOf atold:licence .

<http://publications.europa.eu/resource/authority/licence/CC_BYSA_4_0> a skos:Concept ;
    at:authority-code "CC_BYSA_4_0" ;
    at:deprecated "false" ;
    at:op-code "CC_BYSA_4_0" ;
    at:start.use "2013-11-26" ;
    atold:op-code "CC_BYSA_4_0" ;
    dc:identifier "CC_BYSA_4_0" ;
    skos:altLabel "CC BY-SA 4.0"@bg,
        "CC BY-SA 4.0"@cs,
        "CC BY-SA 4.0"@da,
        "CC BY-SA 4.0"@de,
        "CC BY-SA 4.0"@el,
        "CC BY-SA 4.0"@en,
        "CC BY-SA 4.0"@es,
        "CC BY-SA 4.0"@et,
        "CC BY-SA 4.0"@fi,
        "CC BY-SA 4.0"@fr,
        "CC BY-SA 4.0"@ga,
        "CC BY-SA 4.0"@hr,
        "CC BY-SA 4.0"@hu,
        "CC BY-SA 4.0"@it,
        "CC BY-SA 4.0"@lt,
        "CC BY-SA 4.0"@lv,
        "CC BY-SA 4.0"@mt,
        "CC BY-SA 4.0"@nl,
        "CC BY-SA 4.0"@pl,
        "CC BY-SA 4.0"@pt,
        "CC BY-SA 4.0"@ro,
        "CC BY-SA 4.0"@sk,
        "CC BY-SA 4.0"@sl,
        "CC BY-SA 4.0"@sv ;
    skos:definition "CC BY-SA 4.0 lets others remix, tweak, and build upon the author’s work even for commercial purposes, as long as they credit the author and licence their new creations under the identical terms. This licence is often compared to “copyleft” free and open source software licences. All new works based on the original work will carry the same licence, so any derivatives will also allow commercial use. This is the licence used by Wikipedia, and is recommended for materials that would benefit from incorporating content from Wikipedia and similarly licenced projects."@en,
        "CC BY-SA 4.0 permet aux autres de remixer, arranger, et adapter l’œuvre de l’auteur/autrice, même à des fins commerciales, tant qu’on accorde le mérite de la création originale à l’auteur/autrice en citant son nom et qu’on diffuse les nouvelles créations selon des conditions identiques. Cette licence est souvent comparée aux licences de logiciels libres, «open source» ou «copyleft». Toutes les nouvelles œuvres basées sur celles de l’auteur/autrice auront la même licence, et toute œuvre dérivée pourra être utilisée même à des fins commerciales. C’est la licence utilisée par Wikipédia; elle est recommandée pour des œuvres qui pourraient bénéficier de l’incorporation de contenu depuis Wikipédia et d’autres projets sous licence similaire."@fr ;
    skos:exactMatch <http://creativecommons.org/licenses/by-sa/4.0/> ;
    skos:inScheme atold:licence ;
    skos:prefLabel "Creative Commons Признание-Споделяне на споделеното 4.0 Международен"@bg,
        "Creative Commons Uveďte původ–Zachovejte licenci 4.0 Mezinárodní"@cs,
        "Creative Commons Navngivelse–DelPåSammeVilkår 4.0 International"@da,
        "Creative Commons Namensnennung – Weitergabe unter gleichen Bedingungen 4.0 International"@de,
        "Creative Commons Αναφορά Δημιουργού – Παρόμοια Διανομή 4.0 Διεθνές"@el,
        "Creative Commons Attribution–ShareAlike 4.0 International"@en,
        "Creative Commons Atribución–CompartirIgual 4.0 Internacional"@es,
        "Creative Commons Autorile viitamine–Jagamine samadel tingimustel 4.0 Rahvusvaheline"@et,
        "Creative Commons Nimeä–JaaSamoin 4.0 Kansainvälinen"@fi,
        "Creative Commons Attribution – Partage dans les Mêmes Conditions 4.0 International"@fr,
        "Creative Commons Imenovanje–Dijeli pod istim uvjetima 4.0 međunarodna"@hr,
        "Creative Commons Nevezd meg! – Így add tovább! 4.0 Nemzetközi"@hu,
        "Creative Commons Attribuzione – Condividi allo stesso modo 4.0 Internazionale"@it,
        "Creative Commons Priskyrimas – Analogiškas platinimas 4.0 Tarptautinė"@lt,
        "Creative Commons Atsaucoties–Nemainot licenci 4.0 Internacionāls"@lv,
        "Creative Commons Attribuzzjoni-KondiviżjoniUgwali 4.0 Internazzjonali"@mt,
        "Creative Commons Naamsvermelding–GelijkDelen 4.0 Internationaal"@nl,
        "Creative Commons Uznanie autorstwa–Na tych samych warunkach 4.0 Międzynarodowe"@pl,
        "Creative Commons Atribuição–CompartilhaIgual 4.0 Internacional"@pt,
        "Creative Commons Atribuire–Distribuire în condiţii identice 4.0 Internațional"@ro,
        "Creative Commons Uvedenie Autora-Rovnaké Šírenie 4.0 Medzinárodný"@sk,
        "Creative Commons Priznanje avtorstva-Deljenje pod enakimi pogoji 4.0 Mednarodna"@sl,
        "Creative Commons Erkännande–DelaLika 4.0 Internationell"@sv ;
    skos:topConceptOf atold:licence .

<http://publications.europa.eu/resource/authority/licence/CC_BY_1_0> a skos:Concept ;
    at:authority-code "CC_BY_1_0" ;
    at:deprecated "true" ;
    at:end.use "2004-05-24" ;
    at:op-code "CC_BY_1_0" ;
    at:start.use "2002-12-15" ;
    atold:op-code "CC_BY_1_0" ;
    dc:identifier "CC_BY_1_0" ;
    skos:altLabel "CC BY 1.0"@bg,
        "CC BY 1.0"@cs,
        "CC BY 1.0"@da,
        "CC BY 1.0"@de,
        "CC BY 1.0"@el,
        "CC BY 1.0"@en,
        "CC BY 1.0"@es,
        "CC BY 1.0"@et,
        "CC BY 1.0"@fi,
        "CC BY 1.0"@fr,
        "CC BY 1.0"@ga,
        "CC BY 1.0"@hr,
        "CC BY 1.0"@hu,
        "CC BY 1.0"@it,
        "CC BY 1.0"@lt,
        "CC BY 1.0"@lv,
        "CC BY 1.0"@mt,
        "CC BY 1.0"@nl,
        "CC BY 1.0"@pl,
        "CC BY 1.0"@pt,
        "CC BY 1.0"@ro,
        "CC BY 1.0"@sk,
        "CC BY 1.0"@sl,
        "CC BY 1.0"@sv ;
    skos:definition "CC BY 1.0 lets others distribute, remix, tweak, and build upon the author’s work, even commercially, as long as they credit the author for the original creation. This is the most accommodating of licences offered. Recommended for maximum dissemination and use of licenced materials."@en,
        "CC BY 1.0 permet aux autres de distribuer, remixer, arranger, et adapter l’œuvre de l’auteur/autrice, même à des fins commerciales, tant qu’on accorde le mérite de la création originale à l’auteur/autrice en citant son nom. C’est le contrat le plus souple proposé. Recommandé pour la diffusion et l’utilisation maximales d’œuvres licenciées sous CC."@fr ;
    skos:exactMatch <http://creativecommons.org/licenses/by/1.0/> ;
    skos:inScheme atold:licence ;
    skos:prefLabel "Creative Commons Признание 1.0 Неадаптиран"@bg,
        "Creative Commons Uveďte původ 1.0 Generic"@cs,
        "Creative Commons Navngivelse 1.0 Generisk"@da,
        "Creative Commons Namensnennung 1.0 Generic"@de,
        "Creative Commons Αναφορά Δημιουργού 1.0 Γενικό"@el,
        "Creative Commons Attribution 1.0 Generic"@en,
        "Creative Commons Atribución 1.0 Genérica"@es,
        "Creative Commons Autorile viitamine 1.0 Üldine"@et,
        "Creative Commons Nimeä 1.0 Yleinen"@fi,
        "Creative Commons Attribution 1.0 Générique"@fr,
        "Creative Commons Imenovanje 1.0 nelokalizirana licenca"@hr,
        "Creative Commons Nevezd meg! 1.0 Általános"@hu,
        "Creative Commons Attribuzione 1.0 Generico"@it,
        "Creative Commons Priskyrimas 1.0 Bendrasis"@lt,
        "Creative Commons Atsaucoties 1.0 Vispārīgs"@lv,
        "Creative Commons Attribuzzjoni 1.0 Generic"@mt,
        "Creative Commons Naamsvermelding 1.0 Unported"@nl,
        "Creative Commons Uznanie autorstwa 1.0 Ogólny"@pl,
        "Creative Commons Atribuição 1.0 Genérica"@pt,
        "Creative Commons Atribuire 1.0 Generică"@ro,
        "Creative Commons Uvedenie Autora 1.0 Generic"@sk,
        "Creative Commons Priznanje avtorstva 1.0 Generična"@sl,
        "Creative Commons Erkännande 1.0 Generisk"@sv ;
    skos:topConceptOf atold:licence .

<http://publications.europa.eu/resource/authority/licence/CC_BY_2_0> a skos:Concept ;
    at:authority-code "CC_BY_2_0" ;
    at:deprecated "false" ;
    at:op-code "CC_BY_2_0" ;
    at:start.use "2004-05-25" ;
    atold:op-code "CC_BY_2_0" ;
    dc:identifier "CC_BY_2_0" ;
    skos:altLabel "CC BY 2.0"@bg,
        "CC BY 2.0"@cs,
        "CC BY 2.0"@da,
        "CC BY 2.0"@de,
        "CC BY 2.0"@el,
        "CC BY 2.0"@en,
        "CC BY 2.0"@es,
        "CC BY 2.0"@et,
        "CC BY 2.0"@fi,
        "CC BY 2.0"@fr,
        "CC BY 2.0"@ga,
        "CC BY 2.0"@hr,
        "CC BY 2.0"@hu,
        "CC BY 2.0"@it,
        "CC BY 2.0"@lt,
        "CC BY 2.0"@lv,
        "CC BY 2.0"@mt,
        "CC BY 2.0"@nl,
        "CC BY 2.0"@pl,
        "CC BY 2.0"@pt,
        "CC BY 2.0"@ro,
        "CC BY 2.0"@sk,
        "CC BY 2.0"@sl,
        "CC BY 2.0"@sv ;
    skos:definition "CC BY 2.0 lets others distribute, remix, tweak, and build upon the author’s work, even commercially, as long as they credit the author for the original creation. This is the most accommodating of licences offered. Recommended for maximum dissemination and use of licenced materials."@en,
        "CC BY 2.0 permet aux autres de distribuer, remixer, arranger, et adapter l’œuvre de l’auteur/autrice, même à des fins commerciales, tant qu’on accorde le mérite de la création originale à l’auteur/autrice en citant son nom. C’est le contrat le plus souple proposé. Recommandé pour la diffusion et l’utilisation maximales d’œuvres licenciées sous CC."@fr ;
    skos:exactMatch <http://creativecommons.org/licenses/by/2.0/> ;
    skos:inScheme atold:licence ;
    skos:prefLabel "Creative Commons Признание 2.0 Неадаптиран"@bg,
        "Creative Commons Uveďte původ 2.0 Generic"@cs,
        "Creative Commons Navngivelse 2.0 Generisk"@da,
        "Creative Commons Namensnennung 2.0 Generic"@de,
        "Creative Commons Αναφορά Δημιουργού 2.0 Γενικό"@el,
        "Creative Commons Attribution 2.0 Generic"@en,
        "Creative Commons Atribución 2.0 Genérica"@es,
        "Creative Commons Autorile viitamine 2.0 Üldine"@et,
        "Creative Commons Nimeä 2.0 Yleinen"@fi,
        "Creative Commons Attribution 2.0 Générique"@fr,
        "Creative Commons Imenovanje 2.0 nelokalizirana licenca"@hr,
        "Creative Commons Nevezd meg! 2.0 Általános"@hu,
        "Creative Commons Attribuzione 2.0 Generico"@it,
        "Creative Commons Priskyrimas 2.0 Bendrasis"@lt,
        "Creative Commons Atsaucoties 2.0 Vispārīgs"@lv,
        "Creative Commons Attribuzzjoni 2.0 Generic"@mt,
        "Creative Commons Naamsvermelding 2.0 Unported"@nl,
        "Creative Commons Uznanie autorstwa 2.0 Ogólny"@pl,
        "Creative Commons Atribuição 2.0 Genérica"@pt,
        "Creative Commons Atribuire 2.0 Generică"@ro,
        "Creative Commons Uvedenie Autora 2.0 Generic"@sk,
        "Creative Commons Priznanje avtorstva 2.0 Generična"@sl,
        "Creative Commons Erkännande 2.0 Generisk"@sv ;
    skos:topConceptOf atold:licence .

<http://publications.europa.eu/resource/authority/licence/CC_BY_2_5> a skos:Concept ;
    at:authority-code "CC_BY_2_5" ;
    at:deprecated "false" ;
    at:op-code "CC_BY_2_5" ;
    at:start.use "2005-06-01" ;
    atold:op-code "CC_BY_2_5" ;
    dc:identifier "CC_BY_2_5" ;
    skos:altLabel "CC BY 2.5"@bg,
        "CC BY 2.5"@cs,
        "CC BY 2.5"@da,
        "CC BY 2.5"@de,
        "CC BY 2.5"@el,
        "CC BY 2.5"@en,
        "CC BY 2.5"@es,
        "CC BY 2.5"@et,
        "CC BY 2.5"@fi,
        "CC BY 2.5"@fr,
        "CC BY 2.5"@ga,
        "CC BY 2.5"@hr,
        "CC BY 2.5"@hu,
        "CC BY 2.5"@it,
        "CC BY 2.5"@lt,
        "CC BY 2.5"@lv,
        "CC BY 2.5"@mt,
        "CC BY 2.5"@nl,
        "CC BY 2.5"@pl,
        "CC BY 2.5"@pt,
        "CC BY 2.5"@ro,
        "CC BY 2.5"@sk,
        "CC BY 2.5"@sl,
        "CC BY 2.5"@sv ;
    skos:definition "CC BY 2.5 lets others distribute, remix, tweak, and build upon the author’s work, even commercially, as long as they credit the author for the original creation. This is the most accommodating of licences offered. Recommended for maximum dissemination and use of licenced materials."@en,
        "CC BY 2.5 permet aux autres de distribuer, remixer, arranger, et adapter l’œuvre de l’auteur/autrice, même à des fins commerciales, tant qu’on accorde le mérite de la création originale à l’auteur/autrice en citant son nom. C’est le contrat le plus souple proposé. Recommandé pour la diffusion et l’utilisation maximales d’œuvres licenciées sous CC."@fr ;
    skos:exactMatch <http://creativecommons.org/licenses/by/2.5/> ;
    skos:inScheme atold:licence ;
    skos:prefLabel "Creative Commons Признание 2.5 Неадаптиран"@bg,
        "Creative Commons Uveďte původ 2.5 Generic"@cs,
        "Creative Commons Navngivelse 2.5 Generisk"@da,
        "Creative Commons Namensnennung – Weitergabe unter gleichen Bedingungen 2.5 Generic"@de,
        "Creative Commons Αναφορά Δημιουργού 2.5 Γενικό"@el,
        "Creative Commons Attribution 2.5 Generic"@en,
        "Creative Commons Atribución 2.5 Genérica"@es,
        "Creative Commons Autorile viitamine 2.5 Üldine"@et,
        "Creative Commons Nimeä 2.5 Yleinen"@fi,
        "Creative Commons Attribution 2.5 Générique"@fr,
        "Creative Commons Imenovanje 2.5 nelokalizirana licenca"@hr,
        "Creative Commons Nevezd meg! 2.5 Általános"@hu,
        "Creative Commons Attribuzione 2.5 Generico"@it,
        "Creative Commons Priskyrimas 2.5 Bendrasis"@lt,
        "Creative Commons Atsaucoties 2.5 Vispārīgs"@lv,
        "Creative Commons Attribuzzjoni 2.5 Generic"@mt,
        "Creative Commons Naamsvermelding 2.5 Unported"@nl,
        "Creative Commons Uznanie autorstwa 2.5 Ogólny"@pl,
        "Creative Commons Atribuição 2.5 Genérica"@pt,
        "Creative Commons Atribuire 2.5 Generică"@ro,
        "Creative Commons Uvedenie Autora 2.5 Generic"@sk,
        "Creative Commons Priznanje avtorstva 2.5 Generična"@sl,
        "Creative Commons Erkännande 2.5 Generisk"@sv ;
    skos:topConceptOf atold:licence .

<http://publications.europa.eu/resource/authority/licence/CC_BY_3_0> a skos:Concept ;
    at:authority-code "CC_BY_3_0" ;
    at:deprecated "false" ;
    at:op-code "CC_BY_3_0" ;
    at:start.use "2007-02-23" ;
    atold:op-code "CC_BY_3_0" ;
    dc:identifier "CC_BY_3_0" ;
    skos:altLabel "CC BY 3.0"@bg,
        "CC BY 3.0"@cs,
        "CC BY 3.0"@da,
        "CC BY 3.0"@de,
        "CC BY 3.0"@el,
        "CC BY 3.0"@en,
        "CC BY 3.0"@es,
        "CC BY 3.0"@et,
        "CC BY 3.0"@fi,
        "CC BY 3.0"@fr,
        "CC BY 3.0"@ga,
        "CC BY 3.0"@hr,
        "CC BY 3.0"@hu,
        "CC BY 3.0"@it,
        "CC BY 3.0"@lt,
        "CC BY 3.0"@lv,
        "CC BY 3.0"@mt,
        "CC BY 3.0"@nl,
        "CC BY 3.0"@pl,
        "CC BY 3.0"@pt,
        "CC BY 3.0"@ro,
        "CC BY 3.0"@sk,
        "CC BY 3.0"@sl,
        "CC BY 3.0"@sv ;
    skos:definition "CC BY 3.0 lets others distribute, remix, tweak, and build upon the author’s work, even commercially, as long as they credit the author for the original creation. This is the most accommodating of licences offered. Recommended for maximum dissemination and use of licenced materials."@en,
        "CC BY 3.0 permet aux autres de distribuer, remixer, arranger, et adapter l’œuvre de l’auteur/autrice, même à des fins commerciales, tant qu’on accorde le mérite de la création originale à l’auteur/autrice en citant son nom. C’est le contrat le plus souple proposé. Recommandé pour la diffusion et l’utilisation maximales d’œuvres licenciées sous CC."@fr ;
    skos:exactMatch <http://creativecommons.org/licenses/by/3.0/> ;
    skos:historyNote "Unported licences are licences that are not associated with any specific jurisdiction, e.g. country."@en ;
    skos:inScheme atold:licence ;
    skos:prefLabel "Creative Commons Признание 3.0 Нелокализиран"@bg,
        "Creative Commons Uveďte původ 3.0 Unported"@cs,
        "Creative Commons Navngivelse 3.0 Unported"@da,
        "Creative Commons Namensnennung 3.0 Unported"@de,
        "Creative Commons Αναφορά Δημιουργού 3.0 Μη εισαγόμενο"@el,
        "Creative Commons Attribution 3.0 Unported"@en,
        "Creative Commons Atribución 3.0 Unported"@es,
        "Creative Commons Autorile viitamine 3.0 Jurisdiktsiooniga sidumata"@et,
        "Creative Commons Nimeä 3.0 Ei sovitettu"@fi,
        "Creative Commons Attribution 3.0 non transposé"@fr,
        "Creative Commons Imenovanje 3.0 nelokalizirana licenca"@hr,
        "Creative Commons Nevezd meg! 3.0 Unported"@hu,
        "Creative Commons Attribuzione 3.0 Unported"@it,
        "Creative Commons Priskyrimas 3.0 Nepritaikyta jurisdikcijai"@lt,
        "Creative Commons Atsaucoties 3.0 Nepārnesta"@lv,
        "Creative Commons Attribuzzjoni 3.0 Unported"@mt,
        "Creative Commons Naamsvermelding 3.0 Unported"@nl,
        "Creative Commons Uznanie autorstwa 3.0 Unported"@pl,
        "Creative Commons Atribuição 3.0 Não Adaptada"@pt,
        "Creative Commons Atribuire 3.0 Ne-adaptată"@ro,
        "Creative Commons Uvedenie Autora 3.0 Unported"@sk,
        "Creative Commons Priznanje avtorstva 3.0 Nedoločena"@sl,
        "Creative Commons Erkännande 3.0 Unported"@sv ;
    skos:topConceptOf atold:licence .

<http://publications.europa.eu/resource/authority/licence/CC_BY_3_0_AT> a skos:Concept ;
    at:authority-code "CC_BY_3_0_AT" ;
    at:deprecated "false" ;
    at:op-code "CC_BY_3_0_AT" ;
    at:start.use "2007-02-23" ;
    atold:op-code "CC_BY_3_0_AT" ;
    dc:identifier "CC_BY_3_0_AT" ;
    skos:altLabel "CC BY 3.0 AT"@bg,
        "CC BY 3.0 AT"@cs,
        "CC BY 3.0 AT"@da,
        "CC BY 3.0 AT"@de,
        "CC BY 3.0 AT"@el,
        "CC BY 3.0 AT"@en,
        "CC BY 3.0 NL"@es,
        "CC BY 3.0 AT"@et,
        "CC BY 3.0 AT"@fi,
        "CC BY 3.0 AT"@fr,
        "CC BY 3.0 AT"@ga,
        "CC BY 3.0 AT"@hr,
        "CC BY 3.0 AT"@hu,
        "CC BY 3.0 AT"@it,
        "CC BY 3.0 AT"@lt,
        "CC BY 3.0 AT"@lv,
        "CC BY 3.0 AT"@mt,
        "CC BY 3.0 AT"@nl,
        "CC BY 3.0 AT"@pl,
        "CC BY 3.0 AT"@pt,
        "CC BY 3.0 AT"@ro,
        "CC BY 3.0 AT"@sk,
        "CC BY 3.0 AT"@sl,
        "CC BY 3.0 AT"@sv ;
    skos:definition "Published by Creative Commons for Austria, Namensnennung 3.0 Österreich (CC BY 3.0 AT) is a licence permitting any commercial and non-commercial use as long as credit is given to the author for the original creation."@en ;
    skos:exactMatch <https://creativecommons.org/licenses/by/3.0/at/legalcode> ;
    skos:inScheme atold:licence ;
    skos:prefLabel "Признание 3.0 Австрия"@bg,
        "Uveďte původ 3.0 Rakousko"@cs,
        "Kreditering 3.0 Østrig"@da,
        "Namensnennung 3.0 Österreich"@de,
        "Αναφορά Δημιουργού 3.0"@el,
        "Attribution 3.0 Austria"@en,
        "Atribución 3.0 Austria"@es,
        "Autorile viitamine 3.0 Austria"@et,
        "Nimeä 3.0 Itävalta"@fi,
        "Attribution 3.0 Autriche"@fr,
        "Imenovanje 3.0 Austrija"@hr,
        "Nevezd meg! 3.0 Ausztria"@hu,
        "Attribuzione 3.0 Austria"@it,
        "Priskyrimas 3.0 Austrija"@lt,
        "Attiecinājums 3.0 Austrija"@lv,
        "Attribuzzjoni 3.0 Awstrija"@mt,
        "Naamsvermelding 3.0 Oostenrijk"@nl,
        "Uznanie autorstwa 3.0 Austria"@pl,
        "Atribuição 3.0 Áustria"@pt,
        "Atribuire 3.0 Austria"@ro,
        "Uvedenie Autora 3.0 Rakúsko"@sk,
        "Priznanje avtorstva 3.0 Avstrija"@sl,
        "Erkännande 3.0 Österrike"@sv ;
    skos:topConceptOf atold:licence .

<http://publications.europa.eu/resource/authority/licence/CC_BY_3_0_NL> a skos:Concept ;
    at:authority-code "CC_BY_3_0_NL" ;
    at:deprecated "false" ;
    at:op-code "CC_BY_3_0_NL" ;
    at:start.use "2007-02-23" ;
    atold:op-code "CC_BY_3_0_NL" ;
    dc:identifier "CC_BY_3_0_NL" ;
    skos:altLabel "CC BY 3.0 NL"@bg,
        "CC BY 3.0 NL"@cs,
        "CC BY 3.0 NL"@da,
        "CC BY 3.0 NL"@de,
        "CC BY 3.0 NL"@el,
        "CC BY 3.0 NL"@en,
        "CC BY 3.0 NL"@es,
        "CC BY 3.0 NL"@et,
        "CC BY 3.0 NL"@fi,
        "CC BY 3.0 NL"@fr,
        "CC BY 3.0 NL"@ga,
        "CC BY 3.0 NL"@hr,
        "CC BY 3.0 NL"@hu,
        "CC BY 3.0 NL"@it,
        "CC BY 3.0 NL"@lt,
        "CC BY 3.0 NL"@lv,
        "CC BY 3.0 NL"@mt,
        "CC BY 3.0 NL"@nl,
        "CC BY 3.0 NL"@pl,
        "CC BY 3.0 NL"@pt,
        "CC BY 3.0 NL"@ro,
        "CC BY 3.0 NL"@sk,
        "CC BY 3.0 NL"@sl,
        "CC BY 3.0 NL"@sv ;
    skos:definition "Published by Creative Commons for Netherlands, Naamsvermelding 3.0 Nederland (CC BY 3.0 NL) is a licence permitting any commercial and non-commercial use as long as credit is given to the author for the original creation."@en ;
    skos:exactMatch <http://creativecommons.org/licenses/by/3.0/nl/legalcode> ;
    skos:inScheme atold:licence ;
    skos:prefLabel "Признание 3.0 Холандия"@bg,
        "Uveďte původ 3.0 Nizozemí"@cs,
        "Kreditering 3.0 Holland"@da,
        "Namensnennung 3.0 Niederlande"@de,
        "Αναφορά Δημιουργού 3.0 Ολλανδία"@el,
        "Attribution 3.0 Netherlands"@en,
        "Atribución 3.0 Países Bajos"@es,
        "Autorile viitamine 3.0 Holland"@et,
        "Nimeä 3.0 Hollanti"@fi,
        "Attribution 3.0 Pays-Bas"@fr,
        "Imenovanje 3.0 Nizozemska"@hr,
        "Nevezd meg! 3.0 Hollandia"@hu,
        "Attribuzione 3.0 Olanda"@it,
        "Priskyrimas 3.0 Nyderlandai"@lt,
        "Attiecinājums 3.0 Nīderlande"@lv,
        "Attribuzzjoni 3.0 Pajjiżi l-Baxxi"@mt,
        "Naamsvermelding 3.0 Nederland"@nl,
        "Uznanie autorstwa 3.0 Holandia"@pl,
        "Atribuição 3.0 Holanda"@pt,
        "Atribuire 3.0 Olanda"@ro,
        "Uvedenie Autora 3.0 Holandsko"@sk,
        "Priznanje avtorstva 3.0 Nizozemska"@sl,
        "Erkännande 3.0 Nederländerna"@sv ;
    skos:topConceptOf atold:licence .

<http://publications.europa.eu/resource/authority/licence/CC_BY_4_0> a skos:Concept ;
    at:authority-code "CC_BY_4_0" ;
    at:deprecated "false" ;
    at:op-code "CC_BY_4_0" ;
    at:start.use "2013-11-26" ;
    atold:op-code "CC_BY_4_0" ;
    dc:identifier "CC_BY_4_0" ;
    skos:altLabel "CC BY 4.0"@bg,
        "CC BY 4.0"@cs,
        "CC BY 4.0"@da,
        "CC BY 4.0"@de,
        "CC BY 4.0"@el,
        "CC BY 4.0"@en,
        "CC BY 4.0"@es,
        "CC BY 4.0"@et,
        "CC BY 4.0"@fi,
        "CC BY 4.0"@fr,
        "CC BY 4.0"@ga,
        "CC BY 4.0"@hr,
        "CC BY 4.0"@hu,
        "CC BY 4.0"@it,
        "CC BY 4.0"@lt,
        "CC BY 4.0"@lv,
        "CC BY 4.0"@mt,
        "CC BY 4.0"@nl,
        "CC BY 4.0"@pl,
        "CC BY 4.0"@pt,
        "CC BY 4.0"@ro,
        "CC BY 4.0"@sk,
        "CC BY 4.0"@sl,
        "CC BY 4.0"@sv ;
    skos:definition "CC BY 4.0 lets others distribute, remix, tweak, and build upon the author’s work, even commercially, as long as they credit the author for the original creation. This is the most accommodating of licences offered. Recommended for maximum dissemination and use of licenced materials."@en,
        "CC BY 4.0 permet aux autres de distribuer, remixer, arranger, et adapter l’œuvre de l’auteur/autrice, même à des fins commerciales, tant qu’on accorde le mérite de la création originale à l’auteur/autrice en citant son nom. C’est le contrat le plus souple proposé. Recommandé pour la diffusion et l’utilisation maximales d’œuvres licenciées sous CC."@fr ;
    skos:exactMatch <http://creativecommons.org/licenses/by/4.0/> ;
    skos:inScheme atold:licence ;
    skos:prefLabel "Creative Commons Признание 4.0 Международен"@bg,
        "Creative Commons Uveďte původ 4.0 Mezinárodní"@cs,
        "Creative Commons Navngivelse 4.0 International"@da,
        "Creative Commons Namensnennung 4.0 International"@de,
        "Creative Commons Αναφορά Δημιουργού 4.0 Διεθνές"@el,
        "Creative Commons Attribution 4.0 International"@en,
        "Creative Commons Atribución 4.0 Internacional"@es,
        "Creative Commons Autorile viitamine 4.0 Rahvusvaheline"@et,
        "Creative Commons Nimeä 4.0 Kansainvälinen"@fi,
        "Creative Commons Attribution 4.0 International"@fr,
        "Creative Commons Imenovanje 4.0 međunarodna"@hr,
        "Creative Commons Nevezd meg! 4.0 Nemzetközi"@hu,
        "Creative Commons Attribuzione 4.0 Internazionale"@it,
        "Creative Commons Priskyrimas 4.0 Tarptautinė"@lt,
        "Creative Commons Atsaucoties 4.0 Internacionāls"@lv,
        "Creative Commons Attribuzzjoni 4.0 Internazzjonali"@mt,
        "Creative Commons Naamsvermelding 4.0 Internationaal"@nl,
        "Creative Commons Uznanie autorstwa 4.0 Międzynarodowe"@pl,
        "Creative Commons Atribuição 4.0 Internacional"@pt,
        "Creative Commons Atribuire 4.0 Internațional"@ro,
        "Creative Commons Uvedenie Autora 4.0 Medzinárodný"@sk,
        "Creative Commons Priznanje avtorstva 4.0 Mednarodna"@sl,
        "Creative Commons Erkännande 4.0 Internationell"@sv ;
    skos:topConceptOf atold:licence .

<http://publications.europa.eu/resource/authority/licence/CC_PDM_1_0> a skos:Concept ;
    at:authority-code "CC_PDM_1_0" ;
    at:deprecated "false" ;
    at:op-code "CC_PDM_1_0" ;
    at:start.use "2010-10-01" ;
    atold:op-code "CC_PDM_1_0" ;
    dc:identifier "CC_PDM_1_0" ;
    skos:altLabel "CC PDM 1.0"@bg,
        "CC PDM 1.0"@cs,
        "CC PDM 1.0"@da,
        "CC PDM 1.0"@de,
        "CC PDM 1.0"@el,
        "CC PDM 1.0"@en,
        "CC PDM 1.0"@es,
        "CC PDM 1.0"@et,
        "CC PDM 1.0"@fi,
        "CC PDM 1.0"@fr,
        "CC PDM 1.0"@ga,
        "CC PDM 1.0"@hr,
        "CC PDM 1.0"@hu,
        "CC PDM 1.0"@it,
        "CC PDM 1.0"@lt,
        "CC PDM 1.0"@lv,
        "CC PDM 1.0"@mt,
        "CC PDM 1.0"@nl,
        "CC PDM 1.0"@pl,
        "CC PDM 1.0"@pt,
        "CC PDM 1.0"@ro,
        "CC PDM 1.0"@sk,
        "CC PDM 1.0"@sl,
        "CC PDM 1.0"@sv ;
    skos:changeNote "The source of the start-use date: https://wiki.openmod-initiative.org/images/6/63/Jens-opendata_govdata.de_FraunhoferFokus.pdf"@en ;
    skos:definition "Published by Creative Commons, Public Domain Mark (CC PDM 1.0) identifies a work as being free of known restrictions under copyright law, including all related and neighboring rights. The user can copy, modify, distribute and perform the work, even for commercial purposes, all without asking permission."@en ;
    skos:exactMatch <http://creativecommons.org/publicdomain/mark/1.0/> ;
    skos:inScheme atold:licence ;
    skos:prefLabel "Public Domain Mark 1.0"@bg,
        "Označení volného díla 1.0"@cs,
        "Public domain-mærke 1.0"@da,
        "Public Domain Mark 1.0"@de,
        "Σήμα Δημόσιου Τομέα 1.0"@el,
        "Public Domain Mark 1.0"@en,
        "Etiqueta de Dominio Público 1.0"@es,
        "Avaliku omandi märge 1.0"@et,
        "Public Domain -merkintä 1.0"@fi,
        "Marque du Domaine Public 1.0"@fr,
        "Oznaka javnog dobra 1.0"@hr,
        "Közkincs megjelölés 1.0"@hu,
        "Marchio di pubblico dominio 1.0"@it,
        "Viešosios srities žymuo 1.0"@lt,
        "Sabiedrības īpašuma iezīme 1.0"@lv,
        "Public Domain Mark 1.0"@mt,
        "Public Domain Mark 1.0"@nl,
        "Znak domeny publicznej 1.0"@pl,
        "Marca de Domínio Público 1.0"@pt,
        "Marca Domeniului Public 1.0"@ro,
        "Public Domain Mark 1.0"@sk,
        "Oznaka javne domene 1.0"@sl,
        "Public domain-märke 1.0"@sv ;
    skos:topConceptOf atold:licence .

<http://publications.europa.eu/resource/authority/licence/CDDL_1_0> a skos:Concept ;
    at:authority-code "CDDL_1_0" ;
    at:deprecated "false" ;
    at:op-code "CDDL_1_0" ;
    at:start.use "2004-01-24" ;
    atold:op-code "CDDL_1_0" ;
    dc:identifier "CDDL_1_0" ;
    skos:altLabel "CDDL-1.0"@bg,
        "CDDL-1.0"@cs,
        "CDDL-1.0"@da,
        "CDDL-1.0"@de,
        "CDDL-1.0"@el,
        "CDDL-1.0"@en,
        "CDDL-1.0"@es,
        "CDDL-1.0"@et,
        "CDDL-1.0"@fi,
        "CDDL-1.0"@fr,
        "CDDL-1.0"@ga,
        "CDDL-1.0"@hr,
        "CDDL-1.0"@hu,
        "CDDL-1.0"@it,
        "CDDL-1.0"@lt,
        "CDDL-1.0"@lv,
        "CDDL-1.0"@mt,
        "CDDL-1.0"@nl,
        "CDDL-1.0"@pl,
        "CDDL-1.0"@pt,
        "CDDL-1.0"@ro,
        "CDDL-1.0"@sk,
        "CDDL-1.0"@sl,
        "CDDL-1.0"@sv ;
    skos:changeNote "The source of the start-use date: https://spdx.org/licenses/CDDL-1.0.html"@en ;
    skos:definition "CDDL-1.0 is a free software licence approved by the Open Source Initiative. A moderated (or weak) copyleft licence used by SUN, including explicit patent grants, it is similar to MPL and EPL. Compiled object code can be distributed under any licence, but the original source code (and modified derivatives) must be made available, under the CDDL."@en ;
    skos:exactMatch <https://opensource.org/licenses/CDDL-1.0> ;
    skos:inScheme atold:licence ;
    skos:prefLabel "Common Development and Distribution License 1.0"@en ;
    skos:topConceptOf atold:licence .

<http://publications.europa.eu/resource/authority/licence/CECILL_2_1> a skos:Concept ;
    at:authority-code "CECILL_2_1" ;
    at:deprecated "false" ;
    at:op-code "CECILL_2_1" ;
    at:start.use "2013-06-21" ;
    atold:op-code "CECILL_2_1" ;
    dc:identifier "CECILL_2_1" ;
    skos:altLabel "CECILL-2.1"@bg,
        "CECILL-2.1"@cs,
        "CECILL-2.1"@da,
        "CECILL-2.1"@de,
        "CECILL-2.1"@el,
        "CECILL-2.1"@en,
        "CECILL-2.1"@es,
        "CECILL-2.1"@et,
        "CECILL-2.1"@fi,
        "CECILL-2.1"@fr,
        "CECILL-2.1"@ga,
        "CECILL-2.1"@hr,
        "CECILL-2.1"@hu,
        "CECILL-2.1"@it,
        "CECILL-2.1"@lt,
        "CECILL-2.1"@lv,
        "CECILL-2.1"@mt,
        "CECILL-2.1"@nl,
        "CECILL-2.1"@pl,
        "CECILL-2.1"@pt,
        "CECILL-2.1"@ro,
        "CECILL-2.1"@sk,
        "CECILL-2.1"@sl,
        "CECILL-2.1"@sv ;
    skos:changeNote "The source of the start-use date: https://en.wikipedia.org/wiki/CeCILL"@en ;
    skos:definition "CECILL-2.1 is a moderate copyleft licence initiated in France by CEA, CNRS and Inria and approved by the Open Source Initiative. It has a working value in English/French. It is widely compatible, since only the specific files source code must stay covered, and not the other files or components of a solution. It is therefore designed for components or libraries. Governed by French law."@en ;
    skos:exactMatch <https://opensource.org/licenses/CECILL-2.1> ;
    skos:inScheme atold:licence ;
    skos:prefLabel "CEA CNRS Inria Free Software License Agreement, v2.1 (CECILL-2.1)"@en,
        "CEA CNRS Inria Logiciel Libre License, version 2.1 (CECILL-2.1)"@fr ;
    skos:topConceptOf atold:licence .

<http://publications.europa.eu/resource/authority/licence/CLARIN_ACA_1_0> a skos:Concept ;
    at:authority-code "CLARIN_ACA_1_0" ;
    at:deprecated "false" ;
    at:op-code "CLARIN_ACA_1_0" ;
    at:start.use "2014-12-12" ;
    atold:op-code "CLARIN_ACA_1_0" ;
    dc:identifier "CLARIN_ACA_1_0" ;
    skos:altLabel "CLARIN-EULA-ACA-v1.0"@bg,
        "CLARIN-EULA-ACA-v1.0"@cs,
        "CLARIN-EULA-ACA-v1.0"@da,
        "CLARIN-EULA-ACA-v1.0"@de,
        "CLARIN-EULA-ACA-v1.0"@el,
        "CLARIN-EULA-ACA-v1.0"@en,
        "CLARIN-EULA-ACA-v1.0"@es,
        "CLARIN-EULA-ACA-v1.0"@et,
        "CLARIN-EULA-ACA-v1.0"@fi,
        "CLARIN-EULA-ACA-v1.0"@fr,
        "CLARIN-EULA-ACA-v1.0"@ga,
        "CLARIN-EULA-ACA-v1.0"@hr,
        "CLARIN-EULA-ACA-v1.0"@hu,
        "CLARIN-EULA-ACA-v1.0"@it,
        "CLARIN-EULA-ACA-v1.0"@lt,
        "CLARIN-EULA-ACA-v1.0"@lv,
        "CLARIN-EULA-ACA-v1.0"@mt,
        "CLARIN-EULA-ACA-v1.0"@nl,
        "CLARIN-EULA-ACA-v1.0"@pl,
        "CLARIN-EULA-ACA-v1.0"@pt,
        "CLARIN-EULA-ACA-v1.0"@ro,
        "CLARIN-EULA-ACA-v1.0"@sk,
        "CLARIN-EULA-ACA-v1.0"@sl,
        "CLARIN-EULA-ACA-v1.0"@sv ;
    skos:definition "The copyright holder grants the end-user a free, non-exclusive and perpetual (for the duration of the copyright) right to use and make copies of the resource for educational, teaching or research purposes as such, as modified, or as part of a compilation or derived work."@en ;
    skos:exactMatch <https://www.clarin.eu/content/licenses-and-clarin-categories> ;
    skos:inScheme atold:licence ;
    skos:prefLabel "Clarin Academic End-User Licence (ACA) 1.0"@en,
        "Clarin akadeemiline lõppkasutaja litsents (ACA) 1.0"@et ;
    skos:topConceptOf atold:licence .

<http://publications.europa.eu/resource/authority/licence/CNRI_PYTHON> a skos:Concept ;
    at:authority-code "CNRI_PYTHON" ;
    at:deprecated "false" ;
    at:op-code "CNRI_PYTHON" ;
    at:start.use "2001-03-06" ;
    atold:op-code "CNRI_PYTHON" ;
    dc:identifier "CNRI_PYTHON" ;
    skos:altLabel "CNRI-Python"@bg,
        "CNRI-Python"@cs,
        "CNRI-Python"@da,
        "CNRI-Python"@de,
        "CNRI-Python"@el,
        "CNRI-Python"@en,
        "CNRI-Python"@es,
        "CNRI-Python"@et,
        "CNRI-Python"@fi,
        "CNRI-Python"@fr,
        "CNRI-Python"@ga,
        "CNRI-Python"@hr,
        "CNRI-Python"@hu,
        "CNRI-Python"@it,
        "CNRI-Python"@lt,
        "CNRI-Python"@lv,
        "CNRI-Python"@mt,
        "CNRI-Python"@nl,
        "CNRI-Python"@pl,
        "CNRI-Python"@pt,
        "CNRI-Python"@ro,
        "CNRI-Python"@sk,
        "CNRI-Python"@sl,
        "CNRI-Python"@sv ;
    skos:changeNote "The source of the start-use date: https://en.wikipedia.org/wiki/Python_Software_Foundation"@en ;
    skos:definition "CNRI-Python is a permissive free software licence approved by the Open Source Initiative."@en ;
    skos:exactMatch <https://opensource.org/licenses/CNRI-Python> ;
    skos:inScheme atold:licence ;
    skos:prefLabel "The CNRI portion of the multi-part Python License (CNRI-Python)"@en ;
    skos:topConceptOf atold:licence .

<http://publications.europa.eu/resource/authority/licence/COM_REUSE> a skos:Concept ;
    at:authority-code "COM_REUSE" ;
    at:deprecated "false" ;
    at:op-code "COM_REUSE" ;
    at:start.use "2011-12-14" ;
    atold:op-code "COM_REUSE" ;
    dc:identifier "COM_REUSE" ;
    skos:definition "According to the European Commission reuse notice, reuse is authorised, provided the source is acknowledged. The reuse policy of the European Commission is implemented by the Decision of 12 December 2011. The general principle of reuse can be subject to conditions which may be specified in individual copyright notices. Therefore users are advised to refer to the copyright notices of the individual websites maintained under Europa and of the individual documents. Reuse is not applicable to documents subject to intellectual property rights of third parties."@en ;
    skos:exactMatch <http://data.europa.eu/eli/dec/2011/833/oj> ;
    skos:inScheme atold:licence ;
    skos:prefLabel "European Commission reuse notice"@en ;
    skos:topConceptOf atold:licence .

<http://publications.europa.eu/resource/authority/licence/CPAL_1_0> a skos:Concept ;
    at:authority-code "CPAL_1_0" ;
    at:deprecated "false" ;
    at:op-code "CPAL_1_0" ;
    at:start.use "2007-07-26" ;
    atold:op-code "CPAL_1_0" ;
    dc:identifier "CPAL_1_0" ;
    skos:altLabel "CPAL-1.0"@bg,
        "CPAL-1.0"@cs,
        "CPAL-1.0"@da,
        "CPAL-1.0"@de,
        "CPAL-1.0"@el,
        "CPAL-1.0"@en,
        "CPAL-1.0"@es,
        "CPAL-1.0"@et,
        "CPAL-1.0"@fi,
        "CPAL-1.0"@fr,
        "CPAL-1.0"@ga,
        "CPAL-1.0"@hr,
        "CPAL-1.0"@hu,
        "CPAL-1.0"@it,
        "CPAL-1.0"@lt,
        "CPAL-1.0"@lv,
        "CPAL-1.0"@mt,
        "CPAL-1.0"@nl,
        "CPAL-1.0"@pl,
        "CPAL-1.0"@pt,
        "CPAL-1.0"@ro,
        "CPAL-1.0"@sk,
        "CPAL-1.0"@sl,
        "CPAL-1.0"@sv ;
    skos:changeNote "The source of the start-use date: https://en.wikipedia.org/wiki/Common_Public_Attribution_License; https://www.socialtext.net/open/cpal"@en ;
    skos:definition "CPAL-1.0 is a copyleft-style, free software licence approved by the Open Source Initiative. Under this licence, it is possible to create a larger work by combining the program with other software code not governed by the terms of this licence, and distribute the larger work as a single product."@en ;
    skos:exactMatch <https://opensource.org/licenses/CPAL-1.0> ;
    skos:inScheme atold:licence ;
    skos:prefLabel "Common Public Attribution License Version 1.0 (CPAL-1.0)"@en ;
    skos:topConceptOf atold:licence .

<http://publications.europa.eu/resource/authority/licence/CPL_1_0> a skos:Concept ;
    at:authority-code "CPL_1_0" ;
    at:deprecated "true" ;
    at:end.use "2005-06-27" ;
    at:op-code "CPL_1_0" ;
    at:start.use "2001-05-01" ;
    atold:op-code "CPL_1_0" ;
    dc:identifier "CPL_1_0" ;
    skos:altLabel "CPL-1.0"@bg,
        "CPL-1.0"@cs,
        "CPL-1.0"@da,
        "CPL-1.0"@de,
        "CPL-1.0"@el,
        "CPL-1.0"@en,
        "CPL-1.0"@es,
        "CPL-1.0"@et,
        "CPL-1.0"@fi,
        "CPL-1.0"@fr,
        "CPL-1.0"@ga,
        "CPL-1.0"@hr,
        "CPL-1.0"@hu,
        "CPL-1.0"@it,
        "CPL-1.0"@lt,
        "CPL-1.0"@lv,
        "CPL-1.0"@mt,
        "CPL-1.0"@nl,
        "CPL-1.0"@pl,
        "CPL-1.0"@pt,
        "CPL-1.0"@ro,
        "CPL-1.0"@sk,
        "CPL-1.0"@sl,
        "CPL-1.0"@sv ;
    skos:changeNote "The source of the start-use date: https://en.wikipedia.org/wiki/Common_Public_License"@en ;
    skos:definition "CPL-1.0 is a copyleft-style, free software licence approved by the Open Source Initiative. It is superseded by EPL-1.0."@en ;
    skos:exactMatch <https://opensource.org/licenses/CPL-1.0> ;
    skos:inScheme atold:licence ;
    skos:prefLabel "Common Public License, version 1.0 (CPL-1.0)"@en ;
    skos:topConceptOf atold:licence .

<http://publications.europa.eu/resource/authority/licence/DLDE_BYNC_1_0> a skos:Concept ;
    at:authority-code "DLDE_BYNC_1_0" ;
    at:deprecated "false" ;
    at:op-code "DLDE_BYNC_1_0" ;
    at:start.use "2012-01-01" ;
    atold:op-code "DLDE_BYNC_1_0" ;
    dc:identifier "DLDE_BYNC_1_0" ;
    skos:altLabel "DL-DE BY-NC 1.0"@bg,
        "DL-DE BY-NC 1.0"@cs,
        "DL-DE BY-NC 1.0"@da,
        "DL-DE BY-NC 1.0"@de,
        "DL-DE BY-NC 1.0"@el,
        "DL-DE BY-NC 1.0"@en,
        "DL-DE BY-NC 1.0"@es,
        "DL-DE BY-NC 1.0"@et,
        "DL-DE BY-NC 1.0"@fi,
        "DL-DE BY-NC 1.0"@fr,
        "DL-DE BY-NC 1.0"@ga,
        "DL-DE BY-NC 1.0"@hr,
        "DL-DE BY-NC 1.0"@hu,
        "DL-DE BY-NC 1.0"@it,
        "DL-DE BY-NC 1.0"@lt,
        "DL-DE BY-NC 1.0"@lv,
        "DL-DE BY-NC 1.0"@mt,
        "DL-DE BY-NC 1.0"@nl,
        "DL-DE BY-NC 1.0"@pl,
        "DL-DE BY-NC 1.0"@pt,
        "DL-DE BY-NC 1.0"@ro,
        "DL-DE BY-NC 1.0"@sk,
        "DL-DE BY-NC 1.0"@sl,
        "DL-DE BY-NC 1.0"@sv ;
    skos:changeNote "The source of the start-use date: https://wiki.openmod-initiative.org/images/6/63/Jens-opendata_govdata.de_FraunhoferFokus.pdf"@en ;
    skos:definition "Published by Germany, DL-DE BY-NC 1.0 is a data licence permitting any non-commercial use, as long as credit is given to the author for the original creation. Changes must be marked as such in the source note. The provider mus make available the data, contents and services with the diligence necessary for the discharge of its public tasks."@en ;
    skos:exactMatch <https://www.govdata.de/dl-de/by-nc-1-0> ;
    skos:inScheme atold:licence ;
    skos:prefLabel "Datenlizenz Deutschland – Namensnennung – Version 1.0"@de,
        "Data licence Germany – attribution – non-commercial – Version 1.0"@en ;
    skos:topConceptOf atold:licence .

<http://publications.europa.eu/resource/authority/licence/DLDE_BY_1_0> a skos:Concept ;
    at:authority-code "DLDE_BY_1_0" ;
    at:deprecated "false" ;
    at:op-code "DLDE_BY_1_0" ;
    at:start.use "2013-01-31" ;
    atold:op-code "DLDE_BY_1_0" ;
    dc:identifier "DLDE_BY_1_0" ;
    skos:altLabel "DL-DE BY 1.0"@bg,
        "DL-DE BY 1.0"@cs,
        "DL-DE BY 1.0"@da,
        "DL-DE BY 1.0"@de,
        "DL-DE BY 1.0"@el,
        "DL-DE BY 1.0"@en,
        "DL-DE BY 1.0"@es,
        "DL-DE BY 1.0"@et,
        "DL-DE BY 1.0"@fi,
        "DL-DE BY 1.0"@fr,
        "DL-DE BY 1.0"@ga,
        "DL-DE BY 1.0"@hr,
        "DL-DE BY 1.0"@hu,
        "DL-DE BY 1.0"@it,
        "DL-DE BY 1.0"@lt,
        "DL-DE BY 1.0"@lv,
        "DL-DE BY 1.0"@mt,
        "DL-DE BY 1.0"@nl,
        "DL-DE BY 1.0"@pl,
        "DL-DE BY 1.0"@pt,
        "DL-DE BY 1.0"@ro,
        "DL-DE BY 1.0"@sk,
        "DL-DE BY 1.0"@sl,
        "DL-DE BY 1.0"@sv ;
    skos:changeNote "The source of the start-use date: https://wiki.openmod-initiative.org/images/6/63/Jens-opendata_govdata.de_FraunhoferFokus.pdf"@en ;
    skos:definition "Published by Germany, DL-DE BY 1.0 is a data licence permitting any use commercially and non-commercially, as long as credit is given to the author for the original creation. Changes must be marked as such in the source note. The provider mus make available the data, contents and services with the diligence necessary for the discharge of its public tasks."@en ;
    skos:exactMatch <https://www.govdata.de/dl-de/by-1-0> ;
    skos:inScheme atold:licence ;
    skos:prefLabel "Datenlizenz Deutschland – Namensnennung – Version 1.0"@de,
        "Data licence Germany – attribution – Version 1.0"@en ;
    skos:topConceptOf atold:licence .

<http://publications.europa.eu/resource/authority/licence/DLDE_BY_2_0> a skos:Concept ;
    at:authority-code "DLDE_BY_2_0" ;
    at:deprecated "false" ;
    at:op-code "DLDE_BY_2_0" ;
    at:start.use "2014-07-01" ;
    atold:op-code "DLDE_BY_2_0" ;
    dc:identifier "DLDE_BY_2_0" ;
    skos:altLabel "DL-DE BY 2.0"@bg,
        "DL-DE BY 2.0"@cs,
        "DL-DE BY 2.0"@da,
        "DL-DE BY 2.0"@de,
        "DL-DE BY 2.0"@el,
        "DL-DE BY 2.0"@en,
        "DL-DE BY 2.0"@es,
        "DL-DE BY 2.0"@et,
        "DL-DE BY 2.0"@fi,
        "DL-DE BY 2.0"@fr,
        "DL-DE BY 2.0"@ga,
        "DL-DE BY 2.0"@hr,
        "DL-DE BY 2.0"@hu,
        "DL-DE BY 2.0"@it,
        "DL-DE BY 2.0"@lt,
        "DL-DE BY 2.0"@lv,
        "DL-DE BY 2.0"@mt,
        "DL-DE BY 2.0"@nl,
        "DL-DE BY 2.0"@pl,
        "DL-DE BY 2.0"@pt,
        "DL-DE BY 2.0"@ro,
        "DL-DE BY 2.0"@sk,
        "DL-DE BY 2.0"@sl,
        "DL-DE BY 2.0"@sv ;
    skos:changeNote "The source of the start-use date: https://wiki.openmod-initiative.org/images/6/63/Jens-opendata_govdata.de_FraunhoferFokus.pdf"@en ;
    skos:definition "Published by Germany, DL-DE BY 2.0 is a data licence permitting any use commercially and non-commercially, as long as credit is given to the author for the original creation. Changes must be marked as such in the source note."@en ;
    skos:exactMatch <https://www.govdata.de/dl-de/by-2-0> ;
    skos:inScheme atold:licence ;
    skos:prefLabel "Datenlizenz Deutschland – Namensnennung – Version 2.0"@de,
        "Data licence Germany – attribution – Version 2.0"@en ;
    skos:topConceptOf atold:licence .

<http://publications.europa.eu/resource/authority/licence/DLDE_ZERO_2_0> a skos:Concept ;
    at:authority-code "DLDE_ZERO_2_0" ;
    at:deprecated "false" ;
    at:op-code "DLDE_ZERO_2_0" ;
    at:start.use "2014-07-01" ;
    atold:op-code "DLDE_ZERO_2_0" ;
    dc:identifier "DLDE_ZERO_2_0" ;
    skos:altLabel "DL-DE ZERO 2.0"@bg,
        "DL-DE ZERO 2.0"@cs,
        "DL-DE ZERO 2.0"@da,
        "DL-DE ZERO 2.0"@de,
        "DL-DE ZERO 2.0"@el,
        "DL-DE ZERO 2.0"@en,
        "DL-DE ZERO 2.0"@es,
        "DL-DE ZERO 2.0"@et,
        "DL-DE ZERO 2.0"@fi,
        "DL-DE ZERO 2.0"@fr,
        "DL-DE ZERO 2.0"@ga,
        "DL-DE ZERO 2.0"@hr,
        "DL-DE ZERO 2.0"@hu,
        "DL-DE ZERO 2.0"@it,
        "DL-DE ZERO 2.0"@lt,
        "DL-DE ZERO 2.0"@lv,
        "DL-DE ZERO 2.0"@mt,
        "DL-DE ZERO 2.0"@nl,
        "DL-DE ZERO 2.0"@pl,
        "DL-DE ZERO 2.0"@pt,
        "DL-DE ZERO 2.0"@ro,
        "DL-DE ZERO 2.0"@sk,
        "DL-DE ZERO 2.0"@sl,
        "DL-DE ZERO 2.0"@sv ;
    skos:changeNote "The source of the start-use date: https://wiki.openmod-initiative.org/images/6/63/Jens-opendata_govdata.de_FraunhoferFokus.pdf"@en ;
    skos:definition "Published by Germany, DL-DE ZERO 2.0 is a data licence permitting any use without restrictions or conditions. The data and meta-data provided may be for commercial and non-commercial use."@en ;
    skos:exactMatch <https://www.govdata.de/dl-de/by-2-0> ;
    skos:inScheme atold:licence ;
    skos:prefLabel "Datenlizenz Deutschland – Zero – Version 2.0"@de,
        "Data licence Germany – Zero – Version 2.0"@en ;
    skos:topConceptOf atold:licence .

<http://publications.europa.eu/resource/authority/licence/ECL_1_0> a skos:Concept ;
    at:authority-code "ECL_1_0" ;
    at:deprecated "true" ;
    at:end.use "2007-04-14" ;
    at:op-code "ECL_1_0" ;
    at:start.use "2005-03-15" ;
    atold:op-code "ECL_1_0" ;
    dc:identifier "ECL_1_0" ;
    skos:altLabel "ECL-1.0"@bg,
        "ECL-1.0"@cs,
        "ECL-1.0"@da,
        "ECL-1.0"@de,
        "ECL-1.0"@el,
        "ECL-1.0"@en,
        "ECL-1.0"@es,
        "ECL-1.0"@et,
        "ECL-1.0"@fi,
        "ECL-1.0"@fr,
        "ECL-1.0"@ga,
        "ECL-1.0"@hr,
        "ECL-1.0"@hu,
        "ECL-1.0"@it,
        "ECL-1.0"@lt,
        "ECL-1.0"@lv,
        "ECL-1.0"@mt,
        "ECL-1.0"@nl,
        "ECL-1.0"@pl,
        "ECL-1.0"@pt,
        "ECL-1.0"@ro,
        "ECL-1.0"@sk,
        "ECL-1.0"@sl,
        "ECL-1.0"@sv ;
    skos:changeNote "The source of the start-use date: https://en.wikipedia.org/wiki/Sakai_(software"@en ;
    skos:definition "ECL-1.0 is a permissive free software licence approved by the Open Source Initiative. It is similar to the Apache 1.2. It is superseded by ECL-2.0."@en ;
    skos:exactMatch <https://opensource.org/licenses/ECL-1.0> ;
    skos:inScheme atold:licence ;
    skos:prefLabel "Educational Community License version 1.0 (ECL-1.0)"@en ;
    skos:topConceptOf atold:licence .

<http://publications.europa.eu/resource/authority/licence/ECL_2_0> a skos:Concept ;
    at:authority-code "ECL_2_0" ;
    at:deprecated "false" ;
    at:op-code "ECL_2_0" ;
    at:start.use "2007-04-15" ;
    atold:op-code "ECL_2_0" ;
    dc:identifier "ECL_2_0" ;
    skos:altLabel "ECL-2.0"@bg,
        "ECL-2.0"@cs,
        "ECL-2.0"@da,
        "ECL-2.0"@de,
        "ECL-2.0"@el,
        "ECL-2.0"@en,
        "ECL-2.0"@es,
        "ECL-2.0"@et,
        "ECL-2.0"@fi,
        "ECL-2.0"@fr,
        "ECL-2.0"@ga,
        "ECL-2.0"@hr,
        "ECL-2.0"@hu,
        "ECL-2.0"@it,
        "ECL-2.0"@lt,
        "ECL-2.0"@lv,
        "ECL-2.0"@mt,
        "ECL-2.0"@nl,
        "ECL-2.0"@pl,
        "ECL-2.0"@pt,
        "ECL-2.0"@ro,
        "ECL-2.0"@sk,
        "ECL-2.0"@sl,
        "ECL-2.0"@sv ;
    skos:changeNote "The source of the start-use date: https://tldrlegal.com/license/educational-community-license,-version-2.0-(ecl-2.0)#fulltext"@en ;
    skos:definition "ECL-2.0 is a permissive free software licence approved by the Open Source Initiative. It is similar to the Apache 1.2. Nothing in the licence prohibits re-licencing of a larger work under the EUPL."@en ;
    skos:exactMatch <https://opensource.org/licenses/ECL-2.0> ;
    skos:inScheme atold:licence ;
    skos:prefLabel "Educational Community License version 2.0 (ECL-2.0)"@en ;
    skos:topConceptOf atold:licence .

<http://publications.europa.eu/resource/authority/licence/ECOS_2_0> a skos:Concept ;
    at:authority-code "ECOS_2_0" ;
    at:deprecated "false" ;
    at:op-code "ECOS_2_0" ;
    at:start.use "2002-05-15" ;
    atold:op-code "ECOS_2_0" ;
    dc:identifier "ECOS_2_0" ;
    skos:altLabel "eCos-2.0"@bg,
        "eCos-2.0"@cs,
        "eCos-2.0"@da,
        "eCos-2.0"@de,
        "eCos-2.0"@el,
        "eCos-2.0"@en,
        "eCos-2.0"@es,
        "eCos-2.0"@et,
        "eCos-2.0"@fi,
        "eCos-2.0"@fr,
        "eCos-2.0"@ga,
        "eCos-2.0"@hr,
        "eCos-2.0"@hu,
        "eCos-2.0"@it,
        "eCos-2.0"@lt,
        "eCos-2.0"@lv,
        "eCos-2.0"@mt,
        "eCos-2.0"@nl,
        "eCos-2.0"@pl,
        "eCos-2.0"@pt,
        "eCos-2.0"@ro,
        "eCos-2.0"@sk,
        "eCos-2.0"@sl,
        "eCos-2.0"@sv ;
    skos:changeNote "The source of the start-use date: http://ecos.sourceware.org/license-overview.html"@en ;
    skos:definition "Owned by the Free Software Foundation, eCos-2.0 is a copyleft-style, free software licence approved by the Open Source Initiative."@en ;
    skos:exactMatch <https://opensource.org/licenses/eCos-2.0> ;
    skos:inScheme atold:licence ;
    skos:prefLabel "eCos License version 2.0"@en ;
    skos:topConceptOf atold:licence .

<http://publications.europa.eu/resource/authority/licence/EFL_1_0> a skos:Concept ;
    at:authority-code "EFL_1_0" ;
    at:deprecated "true" ;
    at:end.use "2008-01-01" ;
    at:op-code "EFL_1_0" ;
    at:start.use "2002-07-01" ;
    atold:op-code "EFL_1_0" ;
    dc:identifier "EFL_1_0" ;
    skos:altLabel "EFL-1.0"@bg,
        "EFL-1.0"@cs,
        "EFL-1.0"@da,
        "EFL-1.0"@de,
        "EFL-1.0"@el,
        "EFL-1.0"@en,
        "EFL-1.0"@es,
        "EFL-1.0"@et,
        "EFL-1.0"@fi,
        "EFL-1.0"@fr,
        "EFL-1.0"@ga,
        "EFL-1.0"@hr,
        "EFL-1.0"@hu,
        "EFL-1.0"@it,
        "EFL-1.0"@lt,
        "EFL-1.0"@lv,
        "EFL-1.0"@mt,
        "EFL-1.0"@nl,
        "EFL-1.0"@pl,
        "EFL-1.0"@pt,
        "EFL-1.0"@ro,
        "EFL-1.0"@sk,
        "EFL-1.0"@sl,
        "EFL-1.0"@sv ;
    skos:changeNote "The source of the start-use date: https://en.wikipedia.org/wiki/Eiffel_Forum_License"@en ;
    skos:definition "EFL-1.0 is a BSD-style, permissive free software licence approved by the Open Source Initiative. It is superseded by 2.0."@en ;
    skos:exactMatch <https://opensource.org/licenses/EFL-1.0> ;
    skos:inScheme atold:licence ;
    skos:prefLabel "The Eiffel Forum License, version 1 (EFL-1.0)"@en ;
    skos:topConceptOf atold:licence .

<http://publications.europa.eu/resource/authority/licence/EFL_2> a skos:Concept ;
    at:authority-code "EFL_2" ;
    at:deprecated "false" ;
    at:op-code "EFL_2" ;
    at:start.use "2008-01-02" ;
    atold:op-code "EFL_2" ;
    dc:identifier "EFL_2" ;
    skos:altLabel "EFL-2.0"@bg,
        "EFL-2.0"@cs,
        "EFL-2.0"@da,
        "EFL-2.0"@de,
        "EFL-2.0"@el,
        "EFL-2.0"@en,
        "EFL-2.0"@es,
        "EFL-2.0"@et,
        "EFL-2.0"@fi,
        "EFL-2.0"@fr,
        "EFL-2.0"@ga,
        "EFL-2.0"@hr,
        "EFL-2.0"@hu,
        "EFL-2.0"@it,
        "EFL-2.0"@lt,
        "EFL-2.0"@lv,
        "EFL-2.0"@mt,
        "EFL-2.0"@nl,
        "EFL-2.0"@pl,
        "EFL-2.0"@pt,
        "EFL-2.0"@ro,
        "EFL-2.0"@sk,
        "EFL-2.0"@sl,
        "EFL-2.0"@sv ;
    skos:changeNote "The source of the start-use date: https://en.wikipedia.org/wiki/Eiffel_Forum_License"@en ;
    skos:definition "EFL-2.0 is a BSD-style, permissive free software licence approved by the Open Source Initiative."@en ;
    skos:exactMatch <https://opensource.org/licenses/EFL-2.0> ;
    skos:inScheme atold:licence ;
    skos:prefLabel "Eiffel Forum License, version 2"@en ;
    skos:topConceptOf atold:licence .

<http://publications.europa.eu/resource/authority/licence/ENTESSA> a skos:Concept ;
    at:authority-code "ENTESSA" ;
    at:deprecated "false" ;
    at:op-code "ENTESSA" ;
    at:start.use "2003-07-01" ;
    atold:op-code "ENTESSA" ;
    dc:identifier "ENTESSA" ;
    skos:altLabel "Entessa"@bg,
        "Entessa"@cs,
        "Entessa"@da,
        "Entessa"@de,
        "Entessa"@el,
        "Entessa"@en,
        "Entessa"@es,
        "Entessa"@et,
        "Entessa"@fi,
        "Entessa"@fr,
        "Entessa"@ga,
        "Entessa"@hr,
        "Entessa"@hu,
        "Entessa"@it,
        "Entessa"@lt,
        "Entessa"@lv,
        "Entessa"@mt,
        "Entessa"@nl,
        "Entessa"@pl,
        "Entessa"@pt,
        "Entessa"@ro,
        "Entessa"@sk,
        "Entessa"@sl,
        "Entessa"@sv ;
    skos:changeNote "The source of the start-use date: https://enterprise.dejacode.com/licenses/public/entessa-1.0/"@en ;
    skos:definition "Entessa 1.0 is a BSD-style, permissive free software licence approved by the Open Source Initiative. It imposes copyright acknowledgements that are compatible with the EUPL."@en ;
    skos:exactMatch <https://opensource.org/licenses/Entessa> ;
    skos:inScheme atold:licence ;
    skos:prefLabel "Entessa Public License Version 1.0 (Entessa)"@en ;
    skos:topConceptOf atold:licence .

<http://publications.europa.eu/resource/authority/licence/EPL_1_0> a skos:Concept ;
    at:authority-code "EPL_1_0" ;
    at:deprecated "true" ;
    at:end.use "2017-08-23" ;
    at:op-code "EPL_1_0" ;
    at:start.use "2005-06-28" ;
    atold:op-code "EPL_1_0" ;
    dc:identifier "EPL_1_0" ;
    skos:altLabel "EPL-1.0"@bg,
        "EPL-1.0"@cs,
        "EPL-1.0"@da,
        "EPL-1.0"@de,
        "EPL-1.0"@el,
        "EPL-1.0"@en,
        "EPL-1.0"@es,
        "EPL-1.0"@et,
        "EPL-1.0"@fi,
        "EPL-1.0"@fr,
        "EPL-1.0"@ga,
        "EPL-1.0"@hr,
        "EPL-1.0"@hu,
        "EPL-1.0"@it,
        "EPL-1.0"@lt,
        "EPL-1.0"@lv,
        "EPL-1.0"@mt,
        "EPL-1.0"@nl,
        "EPL-1.0"@pl,
        "EPL-1.0"@pt,
        "EPL-1.0"@ro,
        "EPL-1.0"@sk,
        "EPL-1.0"@sl,
        "EPL-1.0"@sv ;
    skos:changeNote "The source of the start-use date: https://spdx.org/licenses/EPL-1.0.html"@en ;
    skos:definition "EPL 1.0 is a copyleft-style, free software licence approved by the Open Source Initiative. Made and mainly used by the Eclipse Foundation, it is similar to GPL but does not submit linking of the covered code to conditions or ”viral” extension of licence coverage to the other linked software. It is superseded by EPL 2.0."@en ;
    skos:exactMatch <https://opensource.org/licenses/EPL-1.0> ;
    skos:inScheme atold:licence ;
    skos:prefLabel "Eclipse Public License 1.0 (EPL-1.0)"@en ;
    skos:topConceptOf atold:licence .

<http://publications.europa.eu/resource/authority/licence/EPL_2_0> a skos:Concept ;
    at:authority-code "EPL_2_0" ;
    at:deprecated "false" ;
    at:op-code "EPL_2_0" ;
    at:start.use "2017-08-24" ;
    atold:op-code "EPL_2_0" ;
    dc:identifier "EPL_2_0" ;
    skos:altLabel "EPL-2.0"@bg,
        "EPL-2.0"@cs,
        "EPL-2.0"@da,
        "EPL-2.0"@de,
        "EPL-2.0"@el,
        "EPL-2.0"@en,
        "EPL-2.0"@es,
        "EPL-2.0"@et,
        "EPL-2.0"@fi,
        "EPL-2.0"@fr,
        "EPL-2.0"@ga,
        "EPL-2.0"@hr,
        "EPL-2.0"@hu,
        "EPL-2.0"@it,
        "EPL-2.0"@lt,
        "EPL-2.0"@lv,
        "EPL-2.0"@mt,
        "EPL-2.0"@nl,
        "EPL-2.0"@pl,
        "EPL-2.0"@pt,
        "EPL-2.0"@ro,
        "EPL-2.0"@sk,
        "EPL-2.0"@sl,
        "EPL-2.0"@sv ;
    skos:changeNote "The source of the start-use date: https://en.wikipedia.org/wiki/Eclipse_Public_License"@en ;
    skos:definition "EPL 2.0 is a copyleft-style, free software licence approved by the Open Source Initiative. Made and mainly used by the Eclipse Foundation, it is similar to GPL but does not submit linking of the covered code to conditions or ”viral” extension of licence coverage to the other linked software."@en ;
    skos:exactMatch <https://opensource.org/licenses/EPL-2.0> ;
    skos:inScheme atold:licence ;
    skos:prefLabel "Eclipse Public License version 2.0"@en ;
    skos:topConceptOf atold:licence .

<http://publications.europa.eu/resource/authority/licence/ETALAB_2_0> a skos:Concept ;
    at:authority-code "ETALAB_2_0" ;
    at:deprecated "false" ;
    at:op-code "ETALAB_2_0" ;
    at:start.use "2011-10-18" ;
    atold:op-code "ETALAB_2_0" ;
    dc:identifier "ETALAB_2_0" ;
    skos:altLabel "Etalab-2.0"@bg,
        "Etalab-2.0"@cs,
        "Etalab-2.0"@da,
        "Etalab-2.0"@de,
        "Etalab-2.0"@el,
        "Etalab-2.0"@en,
        "Etalab-2.0"@es,
        "Etalab-2.0"@et,
        "Etalab-2.0"@fi,
        "Etalab-2.0"@fr,
        "Etalab-2.0"@ga,
        "Etalab-2.0"@hr,
        "Etalab-2.0"@hu,
        "Etalab-2.0"@it,
        "Etalab-2.0"@lt,
        "Etalab-2.0"@lv,
        "Etalab-2.0"@mt,
        "Etalab-2.0"@nl,
        "Etalab-2.0"@pl,
        "Etalab-2.0"@pt,
        "Etalab-2.0"@ro,
        "Etalab-2.0"@sk,
        "Etalab-2.0"@sl,
        "Etalab-2.0"@sv ;
    skos:definition "The Licence Ouverte / Open Licence is a French open licence published by Etalab for open data from the State of France. The licence was designed to be compatible with Creative Commons Licences, Open Government Licence and the Open Data Commons Attribution License."@en,
        "La Licence ouverte / Open Licence, aussi appelée Licence Ouverte Etalab, est une licence libre française créée par la mission Etalab afin d’encadrer l’ouverture des données de l’État français. Cette licence a été voulue comme une licence compatible avec les licences Open Government Licence du Royaume-Uni, Open Data Commons Attribution de l’Open Knowledge Foundation et Creative Commons Attribution 2.0 de Creative Commons."@fr ;
    skos:exactMatch <https://www.etalab.gouv.fr/licence-ouverte-open-licence/> ;
    skos:inScheme atold:licence ;
    skos:prefLabel "Etalab Open Licence V 2.0"@en,
        "Licence Ouverte Etalab V 2.0 "@fr ;
    skos:topConceptOf atold:licence .

<http://publications.europa.eu/resource/authority/licence/EUPL_1_0> a skos:Concept ;
    at:authority-code "EUPL_1_0" ;
    at:deprecated "false" ;
    at:op-code "EUPL_1_0" ;
    at:start.use "2007-01-09" ;
    atold:op-code "EUPL_1_0" ;
    dc:identifier "EUPL_1_0" ;
    skos:altLabel "EUPL v.1.0"@bg,
        "EUPL v.1.0"@cs,
        "EUPL v.1.0"@da,
        "EUPL v.1.0"@de,
        "EUPL v.1.0"@el,
        "EUPL v.1.0"@en,
        "EUPL v.1.0"@es,
        "EUPL v.1.0"@et,
        "EUPL v.1.0"@fi,
        "EUPL v.1.0"@fr,
        "EUPL v.1.0"@ga,
        "EUPL v.1.0"@hr,
        "EUPL v.1.0"@hu,
        "EUPL v.1.0"@it,
        "EUPL v.1.0"@lt,
        "EUPL v.1.0"@lv,
        "EUPL v.1.0"@mt,
        "EUPL v.1.0"@nl,
        "EUPL v.1.0"@pl,
        "EUPL v.1.0"@pt,
        "EUPL v.1.0"@ro,
        "EUPL v.1.0"@sk,
        "EUPL v.1.0"@sl,
        "EUPL v.1.0"@sv ;
    skos:definition "Created as a tool for publishing any copyrighted work as open source on the initiative of the European Commission, EUPL v.1.0 is the first European Free/Open Source Software (F/OSS) licence. The final version (v.1.0) was officially approved on 9 January 2007 in three linguistic versions. By a second Decision of 9 January 2008, the European Commission validated the EUPL in all the official languages of the European Union."@en ;
    skos:exactMatch <http://ec.europa.eu/idabc/en/document/7330.html> ;
    skos:inScheme atold:licence ;
    skos:prefLabel "Публичен лиценз на Европейския съюз версия v.1.0"@bg,
        "Veřejná Licence Evropské Unie v.1.0"@cs,
        "Europæiske Unions Offentlige Licens v.1.0"@da,
        "Open-Source-Lizenz für die Europäische Union v.1.0"@de,
        "Άδεια δημόσιας χρήσης για την Ευρωπαϊκή Ένωση v.1.0"@el,
        "European Union Public Licence v.1.0"@en,
        "Licencia Pública de la Unión Europea v.1.0"@es,
        "Euroopa Liidu tarkvara vaba kasutuse litsents v.1.0"@et,
        "Euroopan unionin yleinen lisenssi v.1.0"@fi,
        "Licence Publique de l’Union européenne v.1.0"@fr,
        "Javna licencija Europske unije v. 1.0"@hr,
        "Európai Uniós Nyílt Forráskódú Licenc v.1.0"@hu,
        "Licenza Pubblica dell'Unione europea v.1.0"@it,
        "Europos Sąjungos viešoji licencija V.1.0"@lt,
        "Eiropas Savienības sabiedriskā licence V.1.0"@lv,
        "Liċenzja Pubblika ta' l-Unjoni Ewropea V.1.0"@mt,
        "Openbare licentie van de Europese Unie V.1.0"@nl,
        "Licencja publiczna UE wersja 1.0"@pl,
        "Licença Pública da União Europeia V.1.0"@pt,
        "Licenţa publică a Uniunii Europene v.1.0"@ro,
        "Verejná licencia Európskej únie V.1.0"@sk,
        "Javna licenca Evropske unije V.1.0"@sl,
        "Licens till öppen källkod från Europeiska Unionen V.1.0"@sv ;
    skos:topConceptOf atold:licence .

<http://publications.europa.eu/resource/authority/licence/EUPL_1_1> a skos:Concept ;
    at:authority-code "EUPL_1_1" ;
    at:deprecated "false" ;
    at:op-code "EUPL_1_1" ;
    at:start.use "2009-01-09" ;
    atold:op-code "EUPL_1_1" ;
    dc:identifier "EUPL_1_1" ;
    skos:altLabel "EUPL v.1.1"@bg,
        "EUPL v.1.1"@cs,
        "EUPL v.1.1"@da,
        "EUPL v.1.1"@de,
        "EUPL v.1.1"@el,
        "EUPL v.1.1"@en,
        "EUPL v.1.1"@es,
        "EUPL v.1.1"@et,
        "EUPL v.1.1"@fi,
        "EUPL v.1.1"@fr,
        "EUPL v.1.1"@ga,
        "EUPL v.1.1"@hr,
        "EUPL v.1.1"@hu,
        "EUPL v.1.1"@it,
        "EUPL v.1.1"@lt,
        "EUPL v.1.1"@lv,
        "EUPL v.1.1"@mt,
        "EUPL v.1.1"@nl,
        "EUPL v.1.1"@pl,
        "EUPL v.1.1"@pt,
        "EUPL v.1.1"@ro,
        "EUPL v.1.1"@sk,
        "EUPL v.1.1"@sl,
        "EUPL v.1.1"@sv ;
    skos:definition "Created as a tool for publishing any copyrighted work as open source on the initiative of the European Commission, EUPL v.1.1 is the first European Free/Open Source Software (F/OSS) licence. The European Commission published the version 1.1 in all the official languages of the European Union by the Decision of 9 January 2009."@en ;
    skos:exactMatch <https://joinup.ec.europa.eu/collection/eupl/eupl-text-11-12> ;
    skos:inScheme atold:licence ;
    skos:prefLabel "Публичен лиценз на Европейския съюз версия v.1.1"@bg,
        "Veřejná Licence Evropské Unie v.1.1"@cs,
        "Europæiske Unions Offentlige Licens v.1.1"@da,
        "Open-Source-Lizenz für die Europäische Union v.1.1"@de,
        "Άδεια δηµόσιας χρήσης για την Ευρωπαϊκή Ένωση V.1.1"@el,
        "European Union Public Licence v. 1.1"@en,
        "Licencia Pública de la Unión Europea v.1.1"@es,
        "Euroopa Liidu tarkvara vaba kasutuse litsents v.1.1"@et,
        "Euroopan unionin yleinen lisenssi v.1.1"@fi,
        "Licence publique de l'Union européenne v. 1.1"@fr,
        "Javna licencija Europske unije v. 1.1"@hr,
        "Európai Uniós Nyílt Forráskódú Licenc V.1.1"@hu,
        "Licenza Pubblica dell'Unione europea v. 1.1"@it,
        "Europos Sąjungos viešoji licencija V.1.1"@lt,
        "Eiropas Savienības sabiedriskā licence V.1.1"@lv,
        "Liċenzja Pubblika tal-Unjoni Ewropea V.1.1"@mt,
        "Openbare licentie van de Europese Unie V.1.1"@nl,
        "Licencja publiczna Unii Europejskiej v.1.1"@pl,
        "Licença Pública da União Europeia V.1.1"@pt,
        "Licenţa publică a Uniunii Europene V.1.1"@ro,
        "Verejná licencia Európskej únie V.1.1"@sk,
        "Javna licenca Evropske unije V.1.1"@sl,
        "Licens till öppen källkod från Europeiska unionen v.1.1"@sv ;
    skos:topConceptOf atold:licence .

<http://publications.europa.eu/resource/authority/licence/EUPL_1_2> a skos:Concept ;
    at:authority-code "EUPL_1_2" ;
    at:deprecated "false" ;
    at:op-code "EUPL_1_2" ;
    at:start.use "2017-05-19" ;
    atold:op-code "EUPL_1_2" ;
    dc:identifier "EUPL_1_2" ;
    skos:altLabel "EUPL v1.2"@bg,
        "EUPL v1.2"@cs,
        "EUPL v1.2"@da,
        "EUPL v1.2"@de,
        "EUPL v1.2"@el,
        "EUPL v1.2"@en,
        "EUPL v1.2"@es,
        "EUPL v1.2"@et,
        "EUPL v1.2"@fi,
        "EUPL v1.2"@fr,
        "EUPL v1.2"@ga,
        "EUPL v1.2"@hr,
        "EUPL v1.2"@hu,
        "EUPL v1.2"@it,
        "EUPL v1.2"@lt,
        "EUPL v1.2"@lv,
        "EUPL v1.2"@mt,
        "EUPL v1.2"@nl,
        "EUPL v1.2"@pl,
        "EUPL v1.2"@pt,
        "EUPL v1.2"@ro,
        "EUPL v1.2"@sk,
        "EUPL v1.2"@sl,
        "EUPL v1.2"@sv ;
    skos:definition "Created as a tool for publishing any copyrighted work as open source, EUPL v.1.2 is legally consistent with the copyright law of all EU countries and is especially well-suited for public administrations sharing IT solutions. It is also widely used by the private sector. The text of the EUPL version 1.2 was published on 19 May 2017."@en,
        "EUPL v.1.2 a été créée par la Commission en 2007. Elle a pour but de constituer une licence libre valable dans toutes les langues de l’Union, en tenant compte de ses spécificités juridiques et des questions de compatibilité entre licences libres. Il s’agit d’une licence dite «copyleft» dont le but est de garantir la nature «open source» des dérivés des logiciels."@fr ;
    skos:exactMatch <https://joinup.ec.europa.eu/collection/eupl/eupl-text-11-12> ;
    skos:inScheme atold:licence ;
    skos:prefLabel "Публичен лиценз на Европейския съюз версия v.1.2"@bg,
        "Veřejná Licence Evropské Unie v.1.2"@cs,
        "Europæiske Unions Offentlige Licens v.1.2"@da,
        "Open-Source-Lizenz für die Europäische Union v.1.2"@de,
        "Άδεια δημόσιας χρήσης για την Ευρωπαϊκή Ένωση v. 1.2"@el,
        "European Union Public Licence v. 1.2"@en,
        "Licencia Pública de la Unión Europea v.1.2"@es,
        "Euroopa Liidu tarkvara vaba kasutuse litsents v.1.2"@et,
        "Euroopan unionin yleisen lisenssi v. 1.2"@fi,
        "Licence publique de l'Union européenne v. 1.2"@fr,
        "Javna licencija Europske unije v. 1.2"@hr,
        "Európai Uniós Nyilvános Licenc 1.2. verzió"@hu,
        "Licenza Pubblica dell'Unione europea v 1.2"@it,
        "Europos Sąjungos viešoji licencija v. 1.2"@lt,
        "Eiropas Savienības sabiedriskā licence 1.2. redakcija"@lv,
        "Liċenzja Pubblika tal-Unjoni Ewropea v. 1.2"@mt,
        "Openbare licentie van de Europese Unie v. 1.2"@nl,
        "Licencja publiczna Unii Europejskiej wersja 1.2"@pl,
        "Licença Pública da União Europeia v. 1.2"@pt,
        "Licență publică a Uniunii Europene V. 1.2"@ro,
        "Verejná licencia Európskej únie v. 1.2"@sk,
        "Javna licenca Evropske unije v. 1.2"@sl,
        "Licens till öppen källkod från Europeiska unionen v. 1.2"@sv ;
    skos:topConceptOf atold:licence .

<http://publications.europa.eu/resource/authority/licence/EU_DATAGRID> a skos:Concept ;
    at:authority-code "EU_DATAGRID" ;
    at:deprecated "false" ;
    at:op-code "EU_DATAGRID" ;
    at:start.use "2001-06-30" ;
    atold:op-code "EU_DATAGRID" ;
    dc:identifier "EU_DATAGRID" ;
    skos:altLabel "EUDatagrid"@bg,
        "EUDatagrid"@cs,
        "EUDatagrid"@da,
        "EUDatagrid"@de,
        "EUDatagrid"@el,
        "EUDatagrid"@en,
        "EUDatagrid"@es,
        "EUDatagrid"@et,
        "EUDatagrid"@fi,
        "EUDatagrid"@fr,
        "EUDatagrid"@ga,
        "EUDatagrid"@hr,
        "EUDatagrid"@hu,
        "EUDatagrid"@it,
        "EUDatagrid"@lt,
        "EUDatagrid"@lv,
        "EUDatagrid"@mt,
        "EUDatagrid"@nl,
        "EUDatagrid"@pl,
        "EUDatagrid"@pt,
        "EUDatagrid"@ro,
        "EUDatagrid"@sk,
        "EUDatagrid"@sl,
        "EUDatagrid"@sv ;
    skos:changeNote "The source of the start-use date: https://enterprise.dejacode.com/licenses/public/eu-datagrid/"@en ;
    skos:definition "EUDatagrid is a permissive free software licence approved by the Open Source Initiative. It is a classic 3-clause licence. Nothing in this licence restricts redistribution of larger works under the EUPL."@en ;
    skos:exactMatch <https://opensource.org/licenses/EUDatagrid> ;
    skos:inScheme atold:licence ;
    skos:prefLabel "EU DataGrid Software License (EUDatagrid)"@en ;
    skos:topConceptOf atold:licence .

<http://publications.europa.eu/resource/authority/licence/FAIR> a skos:Concept ;
    at:authority-code "FAIR" ;
    at:deprecated "false" ;
    at:op-code "FAIR" ;
    at:start.use "2004-01-31" ;
    atold:op-code "FAIR" ;
    dc:identifier "FAIR" ;
    skos:altLabel "Fair"@bg,
        "Fair"@cs,
        "Fair"@da,
        "Fair"@de,
        "Fair"@el,
        "Fair"@en,
        "Fair"@es,
        "Fair"@et,
        "Fair"@fi,
        "Fair"@fr,
        "Fair"@ga,
        "Fair"@hr,
        "Fair"@hu,
        "Fair"@it,
        "Fair"@lt,
        "Fair"@lv,
        "Fair"@mt,
        "Fair"@nl,
        "Fair"@pl,
        "Fair"@pt,
        "Fair"@ro,
        "Fair"@sk,
        "Fair"@sl,
        "Fair"@sv ;
    skos:changeNote "The source of the start-use date: https://en.wikipedia.org/wiki/Fair_License"@en ;
    skos:definition "Fair is a permissive free software licence approved by the Open Source Initiative. It gives complete freedom to use the given works, as long as this licence is included and a warranty is not placed."@en ;
    skos:exactMatch <https://opensource.org/licenses/Fair> ;
    skos:inScheme atold:licence ;
    skos:prefLabel "Fair License (Fair)"@en ;
    skos:topConceptOf atold:licence .

<http://publications.europa.eu/resource/authority/licence/FRAMEWORX_1_0> a skos:Concept ;
    at:authority-code "FRAMEWORX_1_0" ;
    at:deprecated "false" ;
    at:op-code "FRAMEWORX_1_0" ;
    at:start.use "2003-07-01" ;
    atold:op-code "FRAMEWORX_1_0" ;
    dc:identifier "FRAMEWORX_1_0" ;
    skos:altLabel "Frameworx-1.0"@bg,
        "Frameworx-1.0"@cs,
        "Frameworx-1.0"@da,
        "Frameworx-1.0"@de,
        "Frameworx-1.0"@el,
        "Frameworx-1.0"@en,
        "Frameworx-1.0"@es,
        "Frameworx-1.0"@et,
        "Frameworx-1.0"@fi,
        "Frameworx-1.0"@fr,
        "Frameworx-1.0"@ga,
        "Frameworx-1.0"@hr,
        "Frameworx-1.0"@hu,
        "Frameworx-1.0"@it,
        "Frameworx-1.0"@lt,
        "Frameworx-1.0"@lv,
        "Frameworx-1.0"@mt,
        "Frameworx-1.0"@nl,
        "Frameworx-1.0"@pl,
        "Frameworx-1.0"@pt,
        "Frameworx-1.0"@ro,
        "Frameworx-1.0"@sk,
        "Frameworx-1.0"@sl,
        "Frameworx-1.0"@sv ;
    skos:changeNote "The source of the start-use date: https://enterprise.dejacode.com/licenses/public/frameworx-1.0/?_list_filters=q%3Dframeworx#essentials"@en ;
    skos:definition "Frameworx-1.0 is a copyleft-style, free software licence approved by the Open Source Initiative."@en ;
    skos:exactMatch <https://opensource.org/licenses/Frameworx-1.0> ;
    skos:inScheme atold:licence ;
    skos:prefLabel "Frameworx License 1.0 (Frameworx-1.0)"@en ;
    skos:topConceptOf atold:licence .

<http://publications.europa.eu/resource/authority/licence/GNU_FDL> a skos:Concept ;
    at:authority-code "GNU_FDL" ;
    at:deprecated "true" ;
    at:end.use "2008-11-04" ;
    at:op-code "GNU_FDL" ;
    at:start.use "2008-11-03" ;
    atold:op-code "GNU_FDL" ;
    dc:identifier "GNU_FDL" ;
    skos:altLabel "GFDL"@bg,
        "GFDL"@cs,
        "GFDL"@da,
        "GFDL"@de,
        "GFDL"@el,
        "GFDL"@en,
        "GFDL"@es,
        "GFDL"@et,
        "GFDL"@fi,
        "GFDL"@fr,
        "GFDL"@ga,
        "GFDL"@hr,
        "GFDL"@hu,
        "GFDL"@it,
        "GFDL"@lt,
        "GFDL"@lv,
        "GFDL"@mt,
        "GFDL"@nl,
        "GFDL"@pl,
        "GFDL"@pt,
        "GFDL"@ro,
        "GFDL"@sk,
        "GFDL"@sl,
        "GFDL"@sv ;
    skos:definition "GNU Free Documentation License is a form of copyleft intended for use on a manual, textbook or other document to assure everyone the effective freedom to copy and redistribute it, with or without modifications, either commercially or non-commercially."@en,
        "GNU Free Documentation License est une forme de copyleft destinée aux manuels, aux livres scolaires et autres documents. Son objectif est de garantir à tous la possibilité effective de copier et de redistribuer librement le document avec ou sans modification, et que ce soit ou non dans un but commercial."@fr ;
    skos:exactMatch <http://www.gnu.org/licenses/licenses.html> ;
    skos:inScheme atold:licence ;
    skos:prefLabel "GNU Free Documentation License"@en ;
    skos:topConceptOf atold:licence .

<http://publications.europa.eu/resource/authority/licence/GNU_FDL_1_1> a skos:Concept ;
    at:authority-code "GNU_FDL_1_1" ;
    at:deprecated "true" ;
    at:end.use "2007-06-28" ;
    at:op-code "GNU_FDL_1_1" ;
    at:start.use "2000-03-01" ;
    atold:op-code "GNU_FDL_1_1" ;
    dc:identifier "GNU_FDL_1_1" ;
    skos:altLabel "GNU FDL 1.1"@bg,
        "GNU FDL 1.1"@cs,
        "GNU FDL 1.1"@da,
        "GNU FDL 1.1"@de,
        "GNU FDL 1.1"@el,
        "GNU FDL 1.1"@en,
        "GNU FDL 1.1"@es,
        "GNU FDL 1.1"@et,
        "GNU FDL 1.1"@fi,
        "GNU FDL 1.1"@fr,
        "GNU FDL 1.1"@ga,
        "GNU FDL 1.1"@hr,
        "GNU FDL 1.1"@hu,
        "GNU FDL 1.1"@it,
        "GNU FDL 1.1"@lt,
        "GNU FDL 1.1"@lv,
        "GNU FDL 1.1"@mt,
        "GNU FDL 1.1"@nl,
        "GNU FDL 1.1"@pl,
        "GNU FDL 1.1"@pt,
        "GNU FDL 1.1"@ro,
        "GNU FDL 1.1"@sk,
        "GNU FDL 1.1"@sl,
        "GNU FDL 1.1"@sv ;
    skos:changeNote "The source of the start-use date: https://www.gnu.org/licenses/old-licenses/fdl-1.1"@en ;
    skos:definition "GNU FDL 1.1 is a form of copyleft intended for use on a manual, textbook or other document to assure everyone the effective freedom to copy and redistribute it, with or without modifications, either commercially or non-commercially."@en ;
    skos:exactMatch <https://gnu.org/licenses/old-licenses/fdl-1.1> ;
    skos:inScheme atold:licence ;
    skos:prefLabel "GNU Free Documentation License 1.1"@en ;
    skos:topConceptOf atold:licence .

<http://publications.europa.eu/resource/authority/licence/GNU_FDL_1_2> a skos:Concept ;
    at:authority-code "GNU_FDL_1_2" ;
    at:deprecated "true" ;
    at:end.use "2007-06-28" ;
    at:op-code "GNU_FDL_1_2" ;
    at:start.use "2002-11-01" ;
    atold:op-code "GNU_FDL_1_2" ;
    dc:identifier "GNU_FDL_1_2" ;
    skos:altLabel "GNU FDL 1.2"@bg,
        "GNU FDL 1.2"@cs,
        "GNU FDL 1.2"@da,
        "GNU FDL 1.2"@de,
        "GNU FDL 1.2"@el,
        "GNU FDL 1.2"@en,
        "GNU FDL 1.2"@es,
        "GNU FDL 1.2"@et,
        "GNU FDL 1.2"@fi,
        "GNU FDL 1.2"@fr,
        "GNU FDL 1.2"@ga,
        "GNU FDL 1.2"@hr,
        "GNU FDL 1.2"@hu,
        "GNU FDL 1.2"@it,
        "GNU FDL 1.2"@lt,
        "GNU FDL 1.2"@lv,
        "GNU FDL 1.2"@mt,
        "GNU FDL 1.2"@nl,
        "GNU FDL 1.2"@pl,
        "GNU FDL 1.2"@pt,
        "GNU FDL 1.2"@ro,
        "GNU FDL 1.2"@sk,
        "GNU FDL 1.2"@sl,
        "GNU FDL 1.2"@sv ;
    skos:changeNote "The source of the start-use date: https://www.gnu.org/licenses/old-licenses/fdl-1.2"@en ;
    skos:definition "GNU FDL 1.2 is a form of copyleft intended for use on a manual, textbook or other document to assure everyone the effective freedom to copy and redistribute it, with or without modifications, either commercially or non-commercially."@en ;
    skos:exactMatch <ttps://gnu.org/licenses/old-licenses/fdl-1.2> ;
    skos:inScheme atold:licence ;
    skos:prefLabel "GNU Free Documentation License 1.2"@en ;
    skos:topConceptOf atold:licence .

<http://publications.europa.eu/resource/authority/licence/GNU_FDL_1_3> a skos:Concept ;
    at:authority-code "GNU_FDL_1_3" ;
    at:deprecated "false" ;
    at:op-code "GNU_FDL_1_3" ;
    at:start.use "2008-11-04" ;
    atold:op-code "GNU_FDL_1_3" ;
    dc:identifier "GNU_FDL_1_3" ;
    skos:altLabel "GFDL-1.3"@bg,
        "GNU FDL 1.3"@bg,
        "GFDL-1.3"@cs,
        "GNU FDL 1.3"@cs,
        "GFDL-1.3"@da,
        "GNU FDL 1.3"@da,
        "GFDL-1.3"@de,
        "GNU FDL 1.3"@de,
        "GFDL-1.3"@el,
        "GNU FDL 1.3"@el,
        "GFDL-1.3"@en,
        "GNU FDL 1.3"@en,
        "GFDL-1.3"@es,
        "GNU FDL 1.3"@es,
        "GFDL-1.3"@et,
        "GNU FDL 1.3"@et,
        "GFDL-1.3"@fi,
        "GNU FDL 1.3"@fi,
        "GFDL-1.3"@fr,
        "GNU FDL 1.3"@fr,
        "GFDL-1.3"@ga,
        "GNU FDL 1.3"@ga,
        "GFDL-1.3"@hr,
        "GNU FDL 1.3"@hr,
        "GFDL-1.3"@hu,
        "GNU FDL 1.3"@hu,
        "GFDL-1.3"@it,
        "GNU FDL 1.3"@it,
        "GFDL-1.3"@lt,
        "GNU FDL 1.3"@lt,
        "GFDL-1.3"@lv,
        "GNU FDL 1.3"@lv,
        "GFDL-1.3"@mt,
        "GNU FDL 1.3"@mt,
        "GFDL-1.3"@nl,
        "GNU FDL 1.3"@nl,
        "GFDL-1.3"@pl,
        "GNU FDL 1.3"@pl,
        "GFDL-1.3"@pt,
        "GNU FDL 1.3"@pt,
        "GFDL-1.3"@ro,
        "GNU FDL 1.3"@ro,
        "GFDL-1.3"@sk,
        "GNU FDL 1.3"@sk,
        "GFDL-1.3"@sl,
        "GNU FDL 1.3"@sl,
        "GFDL-1.3"@sv,
        "GNU FDL 1.3"@sv ;
    skos:changeNote "The source of the start-use date: https://www.gnu.org/licenses/fdl-1.3.html"@en ;
    skos:definition "GNU FDL 1.3 is a form of copyleft intended for use on a manual, textbook or other document to assure everyone the effective freedom to copy and redistribute it, with or without modifications, either commercially or non-commercially."@en ;
    skos:exactMatch <http://www.gnu.org/licenses/licenses.html> ;
    skos:inScheme atold:licence ;
    skos:prefLabel "GNU Free Documentation License 1.3"@en ;
    skos:topConceptOf atold:licence .

<http://publications.europa.eu/resource/authority/licence/GPL_2_0> a skos:Concept ;
    at:authority-code "GPL_2_0" ;
    at:deprecated "false" ;
    at:op-code "GPL_2_0" ;
    at:start.use "1991-06-02" ;
    atold:op-code "GPL_2_0" ;
    dc:identifier "GPL_2_0" ;
    skos:altLabel "GPL-2.0"@bg,
        "GPL-2.0"@cs,
        "GPL-2.0"@da,
        "GPL-2.0"@de,
        "GPL-2.0"@el,
        "GPL-2.0"@en,
        "GPL-2.0"@es,
        "GPL-2.0"@et,
        "GPL-2.0"@fi,
        "GPL-2.0"@fr,
        "GPL-2.0"@ga,
        "GPL-2.0"@hr,
        "GPL-2.0"@hu,
        "GPL-2.0"@it,
        "GPL-2.0"@lt,
        "GPL-2.0"@lv,
        "GPL-2.0"@mt,
        "GPL-2.0"@nl,
        "GPL-2.0"@pl,
        "GPL-2.0"@pt,
        "GPL-2.0"@ro,
        "GPL-2.0"@sk,
        "GPL-2.0"@sl,
        "GPL-2.0"@sv ;
    skos:changeNote "The source of the start-use date: https://spdx.org/licenses/GPL-2.0-only.html#licenseText"@en ;
    skos:definition "GPL-2.0 is the ”historical” free software licence. It is supported by the Free Software Foundation. Copy, modification and distribution are authorised, changes/dates must be traced in source files. Any derivative must also be made available under the GPL along with build and install instructions. Lack of compatibility is a known GPL-2.0 issue when a project combines multiple sources and stakeholders."@en ;
    skos:exactMatch <https://opensource.org/licenses/GPL-2.0> ;
    skos:inScheme atold:licence ;
    skos:prefLabel "GNU General Public License version 2"@en,
        "GNU üldine vaba kasutuse litsents versioon 2"@et ;
    skos:topConceptOf atold:licence .

<http://publications.europa.eu/resource/authority/licence/GPL_3_0> a skos:Concept ;
    at:authority-code "GPL_3_0" ;
    at:deprecated "false" ;
    at:op-code "GPL_3_0" ;
    at:start.use "2007-06-29" ;
    atold:op-code "GPL_3_0" ;
    dc:identifier "GPL_3_0" ;
    skos:altLabel "GPL-3.0"@bg,
        "GPL-3.0"@cs,
        "GPL-3.0"@da,
        "GPL-3.0"@de,
        "GPL-3.0"@el,
        "GPL-3.0"@en,
        "GPL-3.0"@es,
        "GPL-3.0"@et,
        "GPL-3.0"@fi,
        "GPL-3.0"@fr,
        "GPL-3.0"@ga,
        "GPL-3.0"@hr,
        "GPL-3.0"@hu,
        "GPL-3.0"@it,
        "GPL-3.0"@lt,
        "GPL-3.0"@lv,
        "GPL-3.0"@mt,
        "GPL-3.0"@nl,
        "GPL-3.0"@pl,
        "GPL-3.0"@pt,
        "GPL-3.0"@ro,
        "GPL-3.0"@sk,
        "GPL-3.0"@sl,
        "GPL-3.0"@sv ;
    skos:changeNote "The source of the start-use date: https://www.tatanka.com/administrative/licenses/fsf_gpl_3.0_license.html"@en ;
    skos:definition "GPL-3.0 is supported by the Free Software Foundation. Under this licence, software can be copied, distributed and modified as long as changes/dates are tracked in source files. Any derivative including (i.e. via compiler) GPL-licenced code must also be made available under the GPL-3.0 along with build and install instructions."@en ;
    skos:exactMatch <https://opensource.org/licenses/GPL-3.0> ;
    skos:inScheme atold:licence ;
    skos:prefLabel "GNU General Public License version 3"@en,
        "GNU üldine vaba kasutuse litsents versioon 3"@et ;
    skos:topConceptOf atold:licence .

<http://publications.europa.eu/resource/authority/licence/HPND> a skos:Concept ;
    at:authority-code "HPND" ;
    at:deprecated "true" ;
    at:end.use "2015-01-01" ;
    at:op-code "HPND" ;
    at:start.use "2002-11-29" ;
    atold:op-code "HPND" ;
    dc:identifier "HPND" ;
    skos:altLabel "HPND"@bg,
        "HPND"@cs,
        "HPND"@da,
        "HPND"@de,
        "HPND"@el,
        "HPND"@en,
        "HPND"@es,
        "HPND"@et,
        "HPND"@fi,
        "HPND"@fr,
        "HPND"@ga,
        "HPND"@hr,
        "HPND"@hu,
        "HPND"@it,
        "HPND"@lt,
        "HPND"@lv,
        "HPND"@mt,
        "HPND"@nl,
        "HPND"@pl,
        "HPND"@pt,
        "HPND"@ro,
        "HPND"@sk,
        "HPND"@sl,
        "HPND"@sv ;
    skos:changeNote "The source of the start-use date: https://en.wikipedia.org/wiki/Historical_Permission_Notice_and_Disclaimer"@en ;
    skos:definition "Deprecated by the author, HPND is a template that provides some protection for the author. The work itself is not restricted by the permissive licence."@en ;
    skos:exactMatch <https://opensource.org/licenses/HPND> ;
    skos:historyNote "The source of the deprecation date: https://www.fsf.org/blogs/licensing/historical-permission-notice-and-disclaimer-added-to-license-list"@en ;
    skos:inScheme atold:licence ;
    skos:prefLabel "Historical Permission Notice and Disclaimer (HPND)"@en ;
    skos:topConceptOf atold:licence .

<http://publications.europa.eu/resource/authority/licence/HROD> a skos:Concept ;
    at:authority-code "HROD" ;
    at:deprecated "false" ;
    at:op-code "HROD" ;
    at:start.use "2017-07-01" ;
    atold:op-code "HROD" ;
    dc:identifier "HROD" ;
    skos:altLabel "HR-OD"@bg,
        "HR-OD"@cs,
        "HR-OD"@da,
        "HR-OD"@de,
        "HR-OD"@el,
        "HR-OD"@en,
        "HR-OD"@es,
        "HR-OD"@et,
        "HR-OD"@fi,
        "HR-OD"@fr,
        "HR-OD"@ga,
        "HR-OD"@hr,
        "HR-OD"@hu,
        "HR-OD"@it,
        "HR-OD"@lt,
        "HR-OD"@lv,
        "HR-OD"@mt,
        "HR-OD"@nl,
        "HR-OD"@pl,
        "HR-OD"@pt,
        "HR-OD"@ro,
        "HR-OD"@sk,
        "HR-OD"@sl,
        "HR-OD"@sv ;
    skos:changeNote "The source of the start-use date: https://www.pristupinfo.hr/objavljena-hrvatska-dozvola-licenca-za-otvorene-podatke/"@en ;
    skos:definition "Published by the Republic of Croatia, HR-OD grants the re-user any re-use of the Information subject to the licence, including a spatially and temporally unrestricted, free-of-charge, non-exclusive and personal right to re-use the Information under this licence."@en ;
    skos:exactMatch <http://data.gov.hr/open-licence-republic-croatia> ;
    skos:inScheme atold:licence ;
    skos:prefLabel "Open Licence – The Republic of Croatia"@en,
        "Objavljena hrvatska dozvola (licenca)"@hr ;
    skos:topConceptOf atold:licence .

<http://publications.europa.eu/resource/authority/licence/IODL_1_0> a skos:Concept ;
    at:authority-code "IODL_1_0" ;
    at:deprecated "false" ;
    at:op-code "IODL_1_0" ;
    at:start.use "2010-10-01" ;
    atold:op-code "IODL_1_0" ;
    dc:identifier "IODL_1_0" ;
    skos:altLabel "IODL 1.0"@bg,
        "IODL 1.0"@cs,
        "IODL 1.0"@da,
        "IODL 1.0"@de,
        "IODL 1.0"@el,
        "IODL 1.0"@en,
        "IODL 1.0"@es,
        "IODL 1.0"@et,
        "IODL 1.0"@fi,
        "IODL 1.0"@fr,
        "IODL 1.0"@ga,
        "IODL 1.0"@hr,
        "IODL 1.0"@hu,
        "IODL 1.0"@it,
        "IODL 1.0"@lt,
        "IODL 1.0"@lv,
        "IODL 1.0"@mt,
        "IODL 1.0"@nl,
        "IODL 1.0"@pl,
        "IODL 1.0"@pt,
        "IODL 1.0"@ro,
        "IODL 1.0"@sk,
        "IODL 1.0"@sl,
        "IODL 1.0"@sv ;
    skos:changeNote "The source of the start-use date: https://it.wikipedia.org/wiki/Italian_Open_Data_License"@en ;
    skos:definition "Published by Italy, IODL 1.0 aims at providing the Italian public sector with a licence facilitating the re-use of public sector information. Even commercial reuse of data is allowed, as long as credit is given to the author and new creations are licenced under the identical terms. All new works based on the original work will carry the same licence, so any derivatives will also allow commercial use."@en ;
    skos:exactMatch <http://www.formez.it/iodl/> ;
    skos:inScheme atold:licence ;
    skos:prefLabel "Italian Open Data License v1.0"@en ;
    skos:topConceptOf atold:licence .

<http://publications.europa.eu/resource/authority/licence/IODL_2_0> a skos:Concept ;
    at:authority-code "IODL_2_0" ;
    at:deprecated "false" ;
    at:op-code "IODL_2_0" ;
    at:start.use "2012-03-02" ;
    atold:op-code "IODL_2_0" ;
    dc:identifier "IODL_2_0" ;
    skos:altLabel "IODL 2.0"@bg,
        "IODL 2.0"@cs,
        "IODL 2.0"@da,
        "IODL 2.0"@de,
        "IODL 2.0"@el,
        "IODL 2.0"@en,
        "IODL 2.0"@es,
        "IODL 2.0"@et,
        "IODL 2.0"@fi,
        "IODL 2.0"@fr,
        "IODL 2.0"@ga,
        "IODL 2.0"@hr,
        "IODL 2.0"@hu,
        "IODL 2.0"@it,
        "IODL 2.0"@lt,
        "IODL 2.0"@lv,
        "IODL 2.0"@mt,
        "IODL 2.0"@nl,
        "IODL 2.0"@pl,
        "IODL 2.0"@pt,
        "IODL 2.0"@ro,
        "IODL 2.0"@sk,
        "IODL 2.0"@sl,
        "IODL 2.0"@sv ;
    skos:changeNote "The source of the start-use date: https://it.wikipedia.org/wiki/Italian_Open_Data_License"@en ;
    skos:definition "Published by Italy, IODL 2.0 aims at providing the Italian public sector with a licence facilitating the re-use of public sector information. It allows distribution and building upon the author’s work, even commercially, as long as credit is given to the author for the original creation."@en ;
    skos:exactMatch <https://www.dati.gov.it/content/italian-open-data-license-v20> ;
    skos:inScheme atold:licence ;
    skos:prefLabel "Italian Open Data License v2.0"@en ;
    skos:topConceptOf atold:licence .

<http://publications.europa.eu/resource/authority/licence/IPA> a skos:Concept ;
    at:authority-code "IPA" ;
    at:deprecated "false" ;
    at:op-code "IPA" ;
    at:start.use "2014-09-30" ;
    atold:op-code "IPA" ;
    dc:identifier "IPA" ;
    skos:altLabel "IPA"@bg,
        "IPA"@cs,
        "IPA"@da,
        "IPA"@de,
        "IPA"@el,
        "IPA"@en,
        "IPA"@es,
        "IPA"@et,
        "IPA"@fi,
        "IPA"@fr,
        "IPA"@ga,
        "IPA"@hr,
        "IPA"@hu,
        "IPA"@it,
        "IPA"@lt,
        "IPA"@lv,
        "IPA"@mt,
        "IPA"@nl,
        "IPA"@pl,
        "IPA"@pt,
        "IPA"@ro,
        "IPA"@sk,
        "IPA"@sl,
        "IPA"@sv ;
    skos:changeNote "The source of the start-use date: https://www.fsf.org/blogs/licensing/ipa-font-license-added-to-license-list"@en ;
    skos:definition "The IPA licence applies only to font programs and allows for a great deal of freedom in distributing them, both commercially and non-commercially. The name of redistributed versions of the original software cannot be changed and must include a copy of the license."@en ;
    skos:exactMatch <https://opensource.org/licenses/IPA> ;
    skos:inScheme atold:licence ;
    skos:prefLabel "IPA Font License (IPA)"@en ;
    skos:topConceptOf atold:licence .

<http://publications.europa.eu/resource/authority/licence/IPL_1_0> a skos:Concept ;
    at:authority-code "IPL_1_0" ;
    at:deprecated "false" ;
    at:op-code "IPL_1_0" ;
    at:start.use "1999-08-31" ;
    atold:op-code "IPL_1_0" ;
    dc:identifier "IPL_1_0" ;
    skos:altLabel "IPL-1.0"@bg,
        "IPL-1.0"@cs,
        "IPL-1.0"@da,
        "IPL-1.0"@de,
        "IPL-1.0"@el,
        "IPL-1.0"@en,
        "IPL-1.0"@es,
        "IPL-1.0"@et,
        "IPL-1.0"@fi,
        "IPL-1.0"@fr,
        "IPL-1.0"@ga,
        "IPL-1.0"@hr,
        "IPL-1.0"@hu,
        "IPL-1.0"@it,
        "IPL-1.0"@lt,
        "IPL-1.0"@lv,
        "IPL-1.0"@mt,
        "IPL-1.0"@nl,
        "IPL-1.0"@pl,
        "IPL-1.0"@pt,
        "IPL-1.0"@ro,
        "IPL-1.0"@sk,
        "IPL-1.0"@sl,
        "IPL-1.0"@sv ;
    skos:changeNote "The source of the start-use date: https://en.wikipedia.org/wiki/IBM_Public_License"@en ;
    skos:definition "The IPL-1.0 is the open-source licence IBM uses for some of its software. Supposed to facilitate commercial use of said software, is very clear on the specifics of liability. It also grants explicit patent rights."@en ;
    skos:exactMatch <https://opensource.org/licenses/IPL-1.0> ;
    skos:inScheme atold:licence ;
    skos:prefLabel "IBM Public License Version 1.0 (IPL-1.0)"@en ;
    skos:topConceptOf atold:licence .

<http://publications.europa.eu/resource/authority/licence/ISA_OML> a skos:Concept ;
    at:authority-code "ISA_OML" ;
    at:deprecated "true" ;
    at:end.use "2012-04-19" ;
    at:op-code "ISA_OML" ;
    at:start.use "2011-01-01" ;
    atold:op-code "ISA_OML" ;
    dc:identifier "ISA_OML" ;
    skos:altLabel "ISA OMdL 1.1"@bg,
        "ISA OMdL 1.1"@cs,
        "ISA OMdL 1.1"@da,
        "ISA OMdL 1.1"@de,
        "ISA OMdL 1.1"@el,
        "ISA OMdL 1.1"@en,
        "ISA Open Metadata Licence 1.0"@en,
        "ISA OMdL 1.1"@es,
        "ISA OMdL 1.1"@et,
        "ISA OMdL 1.1"@fi,
        "ISA OMdL 1.1"@fr,
        "ISA OMdL 1.1"@ga,
        "ISA OMdL 1.1"@hr,
        "ISA OMdL 1.1"@hu,
        "ISA OMdL 1.1"@it,
        "ISA OMdL 1.1"@lt,
        "ISA OMdL 1.1"@lv,
        "ISA OMdL 1.1"@mt,
        "ISA OMdL 1.1"@nl,
        "ISA OMdL 1.1"@pl,
        "ISA OMdL 1.1"@pt,
        "ISA OMdL 1.1"@ro,
        "ISA OMdL 1.1"@sk,
        "ISA OMdL 1.1"@sl,
        "ISA OMdL 1.1"@sv ;
    skos:definition "The ISA Open metadata licence 1.1 is a permissive open licence created by the European Commission to support the publication of technical and semantic specifications. Users are allowed to distribute, copy, adapt or modify the licenced work for any commercial and non-commercial purpose with only a limited set of conditions."@en ;
    skos:exactMatch <https://joinup.ec.europa.eu/licence/isa-open-metadata-licence-v11> ;
    skos:inScheme atold:licence ;
    skos:prefLabel "ISA Open Metadata Licence 1.1"@en ;
    skos:topConceptOf atold:licence .

<http://publications.europa.eu/resource/authority/licence/ISA_OML_1_1> a skos:Concept ;
    at:authority-code "ISA_OML_1_1" ;
    at:deprecated "false" ;
    at:op-code "ISA_OML_1_1" ;
    at:start.use "2012-04-18" ;
    atold:op-code "ISA_OML_1_1" ;
    dc:identifier "ISA_OML_1_1" ;
    skos:altLabel "ISA OMdL 1.1"@bg,
        "ISA OMdL 1.1"@cs,
        "ISA OMdL 1.1"@da,
        "ISA OMdL 1.1"@de,
        "ISA OMdL 1.1"@el,
        "ISA OMdL 1.1"@en,
        "ISA OMdL 1.1"@es,
        "ISA OMdL 1.1"@et,
        "ISA OMdL 1.1"@fi,
        "ISA OMdL 1.1"@fr,
        "ISA OMdL 1.1"@ga,
        "ISA OMdL 1.1"@hr,
        "ISA OMdL 1.1"@hu,
        "ISA OMdL 1.1"@it,
        "ISA OMdL 1.1"@lt,
        "ISA OMdL 1.1"@lv,
        "ISA OMdL 1.1"@mt,
        "ISA OMdL 1.1"@nl,
        "ISA OMdL 1.1"@pl,
        "ISA OMdL 1.1"@pt,
        "ISA OMdL 1.1"@ro,
        "ISA OMdL 1.1"@sk,
        "ISA OMdL 1.1"@sl,
        "ISA OMdL 1.1"@sv ;
    skos:definition "The ISA Open metadata licence 1.1 is a permissive open licence created by the European Commission to support the publication of technical and semantic specifications. Users are allowed to distribute, copy, adapt or modify the licenced work for any commercial and non-commercial purpose with only a limited set of conditions."@en ;
    skos:exactMatch <https://joinup.ec.europa.eu/licence/isa-open-metadata-licence-v11> ;
    skos:inScheme atold:licence ;
    skos:prefLabel "ISA Open Metadata Licence 1.1"@en ;
    skos:topConceptOf atold:licence .

<http://publications.europa.eu/resource/authority/licence/ISC> a skos:Concept ;
    at:authority-code "ISC" ;
    at:deprecated "false" ;
    at:op-code "ISC" ;
    at:start.use "1995-06-30" ;
    atold:op-code "ISC" ;
    dc:identifier "ISC" ;
    skos:altLabel "ISC"@bg,
        "ISC"@cs,
        "ISC"@da,
        "ISC"@de,
        "ISC"@el,
        "ISC"@en,
        "ISC"@es,
        "ISC"@et,
        "ISC"@fi,
        "ISC"@fr,
        "ISC"@ga,
        "ISC"@hr,
        "ISC"@hu,
        "ISC"@it,
        "ISC"@lt,
        "ISC"@lv,
        "ISC"@mt,
        "ISC"@nl,
        "ISC"@pl,
        "ISC"@pt,
        "ISC"@ro,
        "ISC"@sk,
        "ISC"@sl,
        "ISC"@sv ;
    skos:changeNote "The source of the start-use date: https://enterprise.dejacode.com/licenses/public/isc/?_list_filters=q%3Disc; https://en.wikipedia.org/wiki/ISC_license"@en ;
    skos:definition "ISC is a short and permissive software permissive licence (like MIT and BSD). Main obligation is to include the original copyright notice. For reducing licence proliferation, it is advised to use the MIT licence instead."@en ;
    skos:exactMatch <https://opensource.org/licenses/ISC> ;
    skos:inScheme atold:licence ;
    skos:prefLabel "ISC License (ISC)"@en ;
    skos:topConceptOf atold:licence .

<http://publications.europa.eu/resource/authority/licence/LGPL_2_1> a skos:Concept ;
    at:authority-code "LGPL_2_1" ;
    at:deprecated "false" ;
    at:op-code "LGPL_2_1" ;
    at:start.use "1999-02-15" ;
    atold:op-code "LGPL_2_1" ;
    dc:identifier "LGPL_2_1" ;
    skos:altLabel "LGPL-2.1"@bg,
        "LGPL-2.1"@cs,
        "LGPL-2.1"@da,
        "LGPL-2.1"@de,
        "LGPL-2.1"@el,
        "LGPL-2.1"@en,
        "LGPL-2.1"@es,
        "LGPL-2.1"@et,
        "LGPL-2.1"@fi,
        "LGPL-2.1"@fr,
        "LGPL-2.1"@ga,
        "LGPL-2.1"@hr,
        "LGPL-2.1"@hu,
        "LGPL-2.1"@it,
        "LGPL-2.1"@lt,
        "LGPL-2.1"@lv,
        "LGPL-2.1"@mt,
        "LGPL-2.1"@nl,
        "LGPL-2.1"@pl,
        "LGPL-2.1"@pt,
        "LGPL-2.1"@ro,
        "LGPL-2.1"@sk,
        "LGPL-2.1"@sl,
        "LGPL-2.1"@sv ;
    skos:changeNote "The source of the start-use date: https://opensource.org/licenses/LGPL-2.1"@en ;
    skos:definition "LGPL 2.1 is supported by the Free Software Foundation for libraries. Works made by using the covered software could be distributed under any licence. Distribution of derivatives (code modifications) must be done under LGPL. Reverse engineering must be allowed."@en ;
    skos:exactMatch <https://opensource.org/licenses/LGPL-2.1> ;
    skos:inScheme atold:licence ;
    skos:prefLabel "GNU Lesser General Public License version 2.1"@en ;
    skos:topConceptOf atold:licence .

<http://publications.europa.eu/resource/authority/licence/LGPL_3_0> a skos:Concept ;
    at:authority-code "LGPL_3_0" ;
    at:deprecated "false" ;
    at:op-code "LGPL_3_0" ;
    at:start.use "2007-06-29" ;
    atold:op-code "LGPL_3_0" ;
    dc:identifier "LGPL_3_0" ;
    skos:altLabel "LGPL-3.0"@bg,
        "LGPL-3.0"@cs,
        "LGPL-3.0"@da,
        "LGPL-3.0"@de,
        "LGPL-3.0"@el,
        "LGPL-3.0"@en,
        "LGPL-3.0"@es,
        "LGPL-3.0"@et,
        "LGPL-3.0"@fi,
        "LGPL-3.0"@fr,
        "LGPL-3.0"@ga,
        "LGPL-3.0"@hr,
        "LGPL-3.0"@hu,
        "LGPL-3.0"@it,
        "LGPL-3.0"@lt,
        "LGPL-3.0"@lv,
        "LGPL-3.0"@mt,
        "LGPL-3.0"@nl,
        "LGPL-3.0"@pl,
        "LGPL-3.0"@pt,
        "LGPL-3.0"@ro,
        "LGPL-3.0"@sk,
        "LGPL-3.0"@sl,
        "LGPL-3.0"@sv ;
    skos:changeNote "The source of the start-use date: https://opensource.org/licenses/LGPL-3.0"@en ;
    skos:definition "LGPL-3.0 was produced by the Free Software Foundation for libraries. Works made by using the covered software could be distributed under any licence. Distribution of derivatives (code modifications) must be done under LGPL. Reverse engineering must be allowed."@en ;
    skos:exactMatch <https://opensource.org/licenses/LGPL-3.0> ;
    skos:inScheme atold:licence ;
    skos:prefLabel "GNU Lesser General Public License version 3"@en ;
    skos:topConceptOf atold:licence .

<http://publications.europa.eu/resource/authority/licence/LILIQ_P_1_1> a skos:Concept ;
    at:authority-code "LILIQ_P_1_1" ;
    at:deprecated "false" ;
    at:op-code "LILIQ_P_1_1" ;
    at:start.use "2016-01-31" ;
    atold:op-code "LILIQ_P_1_1" ;
    dc:identifier "LILIQ_P_1_1" ;
    skos:altLabel "LiLiQ-P-1.1"@bg,
        "LiLiQ-P-1.1"@cs,
        "LiLiQ-P-1.1"@da,
        "LiLiQ-P-1.1"@de,
        "LiLiQ-P-1.1"@el,
        "LiLiQ-P-1.1"@en,
        "LiLiQ-P-1.1"@es,
        "LiLiQ-P-1.1"@et,
        "LiLiQ-P-1.1"@fi,
        "LiLiQ-P-1.1"@fr,
        "LiLiQ-P-1.1"@ga,
        "LiLiQ-P-1.1"@hr,
        "LiLiQ-P-1.1"@hu,
        "LiLiQ-P-1.1"@it,
        "LiLiQ-P-1.1"@lt,
        "LiLiQ-P-1.1"@lv,
        "LiLiQ-P-1.1"@mt,
        "LiLiQ-P-1.1"@nl,
        "LiLiQ-P-1.1"@pl,
        "LiLiQ-P-1.1"@pt,
        "LiLiQ-P-1.1"@ro,
        "LiLiQ-P-1.1"@sk,
        "LiLiQ-P-1.1"@sl,
        "LiLiQ-P-1.1"@sv ;
    skos:changeNote "The source of the start-use date: https://forge.gouv.qc.ca/licence/"@en ;
    skos:definition "Approved by the Open Source Initiative, LiLiQ-P-1.1 is a permissive licence produced by the State of Quebec (Canada)."@en ;
    skos:exactMatch <https://opensource.org/licenses/LiLiQ-P-1.1> ;
    skos:inScheme atold:licence ;
    skos:prefLabel "Québec Free and Open-Source Licence – Permissive (LiLiQ-P) version 1.1"@en,
        "Licence Libre du Québec – Permissive (LiLiQ-P) version 1.1"@fr ;
    skos:topConceptOf atold:licence .

<http://publications.europa.eu/resource/authority/licence/LILIQ_RPLUS_1_1> a skos:Concept ;
    at:authority-code "LILIQ_RPLUS_1_1" ;
    at:deprecated "false" ;
    at:op-code "LILIQ_RPLUS_1_1" ;
    at:start.use "2016-01-31" ;
    atold:op-code "LILIQ_RPLUS_1_1" ;
    dc:identifier "LILIQ_RPLUS_1_1" ;
    skos:altLabel "LiLiQ-Rplus-1.1"@bg,
        "LiLiQ-Rplus-1.1"@cs,
        "LiLiQ-Rplus-1.1"@da,
        "LiLiQ-Rplus-1.1"@de,
        "LiLiQ-Rplus-1.1"@el,
        "LiLiQ-Rplus-1.1"@en,
        "LiLiQ-Rplus-1.1"@es,
        "LiLiQ-Rplus-1.1"@et,
        "LiLiQ-Rplus-1.1"@fi,
        "LiLiQ-Rplus-1.1"@fr,
        "LiLiQ-Rplus-1.1"@ga,
        "LiLiQ-Rplus-1.1"@hr,
        "LiLiQ-Rplus-1.1"@hu,
        "LiLiQ-Rplus-1.1"@it,
        "LiLiQ-Rplus-1.1"@lt,
        "LiLiQ-Rplus-1.1"@lv,
        "LiLiQ-Rplus-1.1"@mt,
        "LiLiQ-Rplus-1.1"@nl,
        "LiLiQ-Rplus-1.1"@pl,
        "LiLiQ-Rplus-1.1"@pt,
        "LiLiQ-Rplus-1.1"@ro,
        "LiLiQ-Rplus-1.1"@sk,
        "LiLiQ-Rplus-1.1"@sl,
        "LiLiQ-Rplus-1.1"@sv ;
    skos:changeNote "The source of the start-use date: https://forge.gouv.qc.ca/licence/"@en ;
    skos:definition "LiLiQ-Rplus-1.1 is a reciprocate (copyleft) licence produced by the State of Quebec (Canada). Other reciprocal licences GPL-2.0-or-later and the EUPL are expressly listed as compatible, meaning that the covered code can be reused in other projects covered by these licences. It is approved by the Open Source Initiative."@en ;
    skos:exactMatch <https://opensource.org/licenses/LiLiQ-Rplus-1.1> ;
    skos:inScheme atold:licence ;
    skos:prefLabel "Québec Free and Open-Source Licence – Strong Reciprocity (LiLiQ-R+) version 1.1"@en,
        "Licence Libre du Québec – Réciprocité forte (LiLiQ-R+) version 1.1"@fr ;
    skos:topConceptOf atold:licence .

<http://publications.europa.eu/resource/authority/licence/LILIQ_R_1_1> a skos:Concept ;
    at:authority-code "LILIQ_R_1_1" ;
    at:deprecated "false" ;
    at:op-code "LILIQ_R_1_1" ;
    at:start.use "2016-01-31" ;
    atold:op-code "LILIQ_R_1_1" ;
    dc:identifier "LILIQ_R_1_1" ;
    skos:altLabel "LiLiQ-R-1.1"@bg,
        "LiLiQ-R-1.1"@cs,
        "LiLiQ-R-1.1"@da,
        "LiLiQ-R-1.1"@de,
        "LiLiQ-R-1.1"@el,
        "LiLiQ-R-1.1"@en,
        "LiLiQ-R-1.1"@es,
        "LiLiQ-R-1.1"@et,
        "LiLiQ-R-1.1"@fi,
        "LiLiQ-R-1.1"@fr,
        "LiLiQ-R-1.1"@ga,
        "LiLiQ-R-1.1"@hr,
        "LiLiQ-R-1.1"@hu,
        "LiLiQ-R-1.1"@it,
        "LiLiQ-R-1.1"@lt,
        "LiLiQ-R-1.1"@lv,
        "LiLiQ-R-1.1"@mt,
        "LiLiQ-R-1.1"@nl,
        "LiLiQ-R-1.1"@pl,
        "LiLiQ-R-1.1"@pt,
        "LiLiQ-R-1.1"@ro,
        "LiLiQ-R-1.1"@sk,
        "LiLiQ-R-1.1"@sl,
        "LiLiQ-R-1.1"@sv ;
    skos:changeNote "The source of the start-use date: https://forge.gouv.qc.ca/licence/"@en ;
    skos:definition "LiLiQ-R 1.1 is a moderately reciprocate licence produced by the State of Quebec (Canada). A list of liences with similar level of reciprocity is declared compatible, including GPL, EUPL, MPL, LGPL etc., meaning that the covered code can be reused in other projects covered by these licences. It is approved by the Open Source Initiative."@en ;
    skos:exactMatch <https://opensource.org/licenses/LiLiQ-R-1.1> ;
    skos:inScheme atold:licence ;
    skos:prefLabel "Québec Free and Open-Source Licence – Reciprocity (LiLiQ-R) version 1.1"@en,
        "Licence Libre du Québec – Réciprocité (LiLiQ-R) version 1.1"@fr ;
    skos:topConceptOf atold:licence .

<http://publications.europa.eu/resource/authority/licence/LPL_1_0> a skos:Concept ;
    at:authority-code "LPL_1_0" ;
    at:deprecated "true" ;
    at:end.use "2003-06-30" ;
    at:op-code "LPL_1_0" ;
    at:start.use "2003-01-01" ;
    atold:op-code "LPL_1_0" ;
    dc:identifier "LPL_1_0" ;
    skos:altLabel "LPL-1.0"@bg,
        "LPL-1.0"@cs,
        "LPL-1.0"@da,
        "LPL-1.0"@de,
        "LPL-1.0"@el,
        "LPL-1.0"@en,
        "LPL-1.0"@es,
        "LPL-1.0"@et,
        "LPL-1.0"@fi,
        "LPL-1.0"@fr,
        "LPL-1.0"@ga,
        "LPL-1.0"@hr,
        "LPL-1.0"@hu,
        "LPL-1.0"@it,
        "LPL-1.0"@lt,
        "LPL-1.0"@lv,
        "LPL-1.0"@mt,
        "LPL-1.0"@nl,
        "LPL-1.0"@pl,
        "LPL-1.0"@pt,
        "LPL-1.0"@ro,
        "LPL-1.0"@sk,
        "LPL-1.0"@sl,
        "LPL-1.0"@sv ;
    skos:changeNote "The source of the start-use date: https://enterprise.dejacode.com/licenses/public/lucent-pl-1.0/?_list_filters=q%3Dlucent"@en ;
    skos:definition "LPL-1.0 is a copyleft-style, free software licence approved by the Open Source Initiative. It is superseded by LPL-1.02."@en ;
    skos:exactMatch <https://opensource.org/licenses/LPL-1.0> ;
    skos:inScheme atold:licence ;
    skos:prefLabel "Lucent Public License, Plan 9, version 1.0 (LPL-1.0)"@en ;
    skos:topConceptOf atold:licence .

<http://publications.europa.eu/resource/authority/licence/LPL_1_02> a skos:Concept ;
    at:authority-code "LPL_1_02" ;
    at:deprecated "false" ;
    at:op-code "LPL_1_02" ;
    at:start.use "2003-07-01" ;
    atold:op-code "LPL_1_02" ;
    dc:identifier "LPL_1_02" ;
    skos:altLabel "LPL-1.02"@bg,
        "LPL-1.02"@cs,
        "LPL-1.02"@da,
        "LPL-1.02"@de,
        "LPL-1.02"@el,
        "LPL-1.02"@en,
        "LPL-1.02"@es,
        "LPL-1.02"@et,
        "LPL-1.02"@fi,
        "LPL-1.02"@fr,
        "LPL-1.02"@ga,
        "LPL-1.02"@hr,
        "LPL-1.02"@hu,
        "LPL-1.02"@it,
        "LPL-1.02"@lt,
        "LPL-1.02"@lv,
        "LPL-1.02"@mt,
        "LPL-1.02"@nl,
        "LPL-1.02"@pl,
        "LPL-1.02"@pt,
        "LPL-1.02"@ro,
        "LPL-1.02"@sk,
        "LPL-1.02"@sl,
        "LPL-1.02"@sv ;
    skos:changeNote "The source of the start-use date: https://enterprise.dejacode.com/licenses/public/lucent-pl-1.02/?_list_filters=q%3Dlucent"@en ;
    skos:definition "LPL-1.02 is a copyleft-style, free software licence approved by the Open Source Initiative. Similar to the Common Public License, this licence makes liability rules very clear."@en ;
    skos:exactMatch <https://opensource.org/licenses/LPL-1.02> ;
    skos:inScheme atold:licence ;
    skos:prefLabel "Lucent Public License Version 1.02 (LPL-1.02)"@en ;
    skos:topConceptOf atold:licence .

<http://publications.europa.eu/resource/authority/licence/LPPL_1_3C> a skos:Concept ;
    at:authority-code "LPPL_1_3C" ;
    at:deprecated "false" ;
    at:op-code "LPPL_1_3C" ;
    at:start.use "2008-05-04" ;
    atold:op-code "LPPL_1_3C" ;
    dc:identifier "LPPL_1_3C" ;
    skos:altLabel "LPPL-1.3c"@bg,
        "LPPL-1.3c"@cs,
        "LPPL-1.3c"@da,
        "LPPL-1.3c"@de,
        "LPPL-1.3c"@el,
        "LPPL-1.3c"@en,
        "LPPL-1.3c"@es,
        "LPPL-1.3c"@et,
        "LPPL-1.3c"@fi,
        "LPPL-1.3c"@fr,
        "LPPL-1.3c"@ga,
        "LPPL-1.3c"@hr,
        "LPPL-1.3c"@hu,
        "LPPL-1.3c"@it,
        "LPPL-1.3c"@lt,
        "LPPL-1.3c"@lv,
        "LPPL-1.3c"@mt,
        "LPPL-1.3c"@nl,
        "LPPL-1.3c"@pl,
        "LPPL-1.3c"@pt,
        "LPPL-1.3c"@ro,
        "LPPL-1.3c"@sk,
        "LPPL-1.3c"@sl,
        "LPPL-1.3c"@sv ;
    skos:changeNote "The source of the start-use date: https://en.wikipedia.org/wiki/LaTeX_Project_Public_License"@en ;
    skos:definition "LPPL-1.3c is a very specific, non-copyleft licence. It organises rights of the ”maintainer” of a work V/S other distributors who have to comply with documentation requirements and to communicate the original code (or report where it can be available)."@en ;
    skos:exactMatch <https://opensource.org/licenses/LPPL-1.3c> ;
    skos:inScheme atold:licence ;
    skos:prefLabel "LaTeX Project Public License v1.3c (LPPL-1.3c)"@en ;
    skos:topConceptOf atold:licence .

<http://publications.europa.eu/resource/authority/licence/MIROS> a skos:Concept ;
    at:authority-code "MIROS" ;
    at:deprecated "false" ;
    at:op-code "MIROS" ;
    at:start.use "2006-12-11" ;
    atold:op-code "MIROS" ;
    dc:identifier "MIROS" ;
    skos:altLabel "MirOS"@bg,
        "MirOS"@cs,
        "MirOS"@da,
        "MirOS"@de,
        "MirOS"@el,
        "MirOS"@en,
        "MirOS"@es,
        "MirOS"@et,
        "MirOS"@fi,
        "MirOS"@fr,
        "MirOS"@ga,
        "MirOS"@hr,
        "MirOS"@hu,
        "MirOS"@it,
        "MirOS"@lt,
        "MirOS"@lv,
        "MirOS"@mt,
        "MirOS"@nl,
        "MirOS"@pl,
        "MirOS"@pt,
        "MirOS"@ro,
        "MirOS"@sk,
        "MirOS"@sl,
        "MirOS"@sv ;
    skos:changeNote "The source of the start-use date: https://en.wikipedia.org/wiki/MirOS_Licence"@en ;
    skos:definition "MirOS is a BSD-style, permissive free software licence approved by the Open Source Initiative."@en ;
    skos:exactMatch <https://opensource.org/licenses/MS-RL> ;
    skos:inScheme atold:licence ;
    skos:prefLabel "MirOS License (MirOS)"@en ;
    skos:topConceptOf atold:licence .

<http://publications.europa.eu/resource/authority/licence/MIT> a skos:Concept ;
    at:authority-code "MIT" ;
    at:deprecated "false" ;
    at:op-code "MIT" ;
    at:start.use "1988-08-14" ;
    atold:op-code "MIT" ;
    dc:identifier "MIT" ;
    skos:altLabel "MIT"@bg,
        "MIT"@cs,
        "MIT"@da,
        "MIT"@de,
        "MIT"@el,
        "MIT"@en,
        "MIT"@es,
        "MIT"@et,
        "MIT"@fi,
        "MIT"@fr,
        "MIT"@ga,
        "MIT"@hr,
        "MIT"@hu,
        "MIT"@it,
        "MIT"@lt,
        "MIT"@lv,
        "MIT"@mt,
        "MIT"@nl,
        "MIT"@pl,
        "MIT"@pt,
        "MIT"@ro,
        "MIT"@sk,
        "MIT"@sl,
        "MIT"@sv ;
    skos:changeNote "The source of the start-use date: https://opensource.com/article/19/4/history-mit-license; https://webcache.googleusercontent.com/search?q=cache:GAPzrOqxGoMJ:https://libexpat.github.io/doc/news/+&cd=3&hl=en&ct=clnk&gl=lu"@en ;
    skos:definition "Approved by the Open Source Initiative, MIT is the most recommended permissive licence: short and very popular. Everything is allowed as long as the original copyright and licence notice is included in any copy of the software/source."@en ;
    skos:exactMatch <https://opensource.org/licenses/MIT> ;
    skos:inScheme atold:licence ;
    skos:prefLabel "The MIT License"@en,
        "MIT litsents"@et ;
    skos:topConceptOf atold:licence .

<http://publications.europa.eu/resource/authority/licence/MOTOSOTO> a skos:Concept ;
    at:authority-code "MOTOSOTO" ;
    at:deprecated "false" ;
    at:op-code "MOTOSOTO" ;
    at:start.use "1995-01-01" ;
    atold:op-code "MOTOSOTO" ;
    dc:identifier "MOTOSOTO" ;
    skos:altLabel "Motosoto"@bg,
        "Motosoto"@cs,
        "Motosoto"@da,
        "Motosoto"@de,
        "Motosoto"@el,
        "Motosoto"@en,
        "Motosoto"@es,
        "Motosoto"@et,
        "Motosoto"@fi,
        "Motosoto"@fr,
        "Motosoto"@ga,
        "Motosoto"@hr,
        "Motosoto"@hu,
        "Motosoto"@it,
        "Motosoto"@lt,
        "Motosoto"@lv,
        "Motosoto"@mt,
        "Motosoto"@nl,
        "Motosoto"@pl,
        "Motosoto"@pt,
        "Motosoto"@ro,
        "Motosoto"@sk,
        "Motosoto"@sl,
        "Motosoto"@sv ;
    skos:changeNote "The source of the start-use date: http://www.worldlii.org/int/other/PubRL/1995/8.html"@en ;
    skos:definition "Motosoto is a copyleft-style, free software licence approved by the Open Source Initiative."@en ;
    skos:exactMatch <https://opensource.org/licenses/Motosoto> ;
    skos:inScheme atold:licence ;
    skos:prefLabel "Motosoto Open Source License – Version 0.9.1 (Motosoto)"@en ;
    skos:topConceptOf atold:licence .

<http://publications.europa.eu/resource/authority/licence/MPL_1_0> a skos:Concept ;
    at:authority-code "MPL_1_0" ;
    at:deprecated "true" ;
    at:end.use "2012-01-02" ;
    at:op-code "MPL_1_0" ;
    at:start.use "1998-01-01" ;
    atold:op-code "MPL_1_0" ;
    dc:identifier "MPL_1_0" ;
    skos:altLabel "MPL-1.0"@bg,
        "MPL-1.0"@cs,
        "MPL-1.0"@da,
        "MPL-1.0"@de,
        "MPL-1.0"@el,
        "MPL-1.0"@en,
        "MPL-1.0"@es,
        "MPL-1.0"@et,
        "MPL-1.0"@fi,
        "MPL-1.0"@fr,
        "MPL-1.0"@ga,
        "MPL-1.0"@hr,
        "MPL-1.0"@hu,
        "MPL-1.0"@it,
        "MPL-1.0"@lt,
        "MPL-1.0"@lv,
        "MPL-1.0"@mt,
        "MPL-1.0"@nl,
        "MPL-1.0"@pl,
        "MPL-1.0"@pt,
        "MPL-1.0"@ro,
        "MPL-1.0"@sk,
        "MPL-1.0"@sl,
        "MPL-1.0"@sv ;
    skos:changeNote "The source of the start-use date: https://en.wikipedia.org/wiki/Mozilla_Public_License"@en ;
    skos:definition "MPL-1.0 is a weak copyleft licence, characterised as a middle ground between permissive free software licences and the GNU General Public License that seeks to balance the concerns of proprietary and open source developers. As such, it allows re-licencing. It is approved by the Open Source Initiative. It has been superseded by v2.0."@en ;
    skos:exactMatch <https://opensource.org/licenses/MPL-1.0> ;
    skos:inScheme atold:licence ;
    skos:prefLabel "The Mozilla Public License (MPL), version 1.0 (MPL-1.0)"@en ;
    skos:topConceptOf atold:licence .

<http://publications.europa.eu/resource/authority/licence/MPL_1_1> a skos:Concept ;
    at:authority-code "MPL_1_1" ;
    at:deprecated "true" ;
    at:end.use "2012-01-02" ;
    at:op-code "MPL_1_1" ;
    at:start.use "1999-01-01" ;
    atold:op-code "MPL_1_1" ;
    dc:identifier "MPL_1_1" ;
    skos:altLabel "MPL-1.1"@bg,
        "MPL-1.1"@cs,
        "MPL-1.1"@da,
        "MPL-1.1"@de,
        "MPL-1.1"@el,
        "MPL-1.1"@en,
        "MPL-1.1"@es,
        "MPL-1.1"@et,
        "MPL-1.1"@fi,
        "MPL-1.1"@fr,
        "MPL-1.1"@ga,
        "MPL-1.1"@hr,
        "MPL-1.1"@hu,
        "MPL-1.1"@it,
        "MPL-1.1"@lt,
        "MPL-1.1"@lv,
        "MPL-1.1"@mt,
        "MPL-1.1"@nl,
        "MPL-1.1"@pl,
        "MPL-1.1"@pt,
        "MPL-1.1"@ro,
        "MPL-1.1"@sk,
        "MPL-1.1"@sl,
        "MPL-1.1"@sv ;
    skos:changeNote "The source of the start-use date: https://en.wikisource.org/wiki/Mozilla_Public_License"@en ;
    skos:definition "MPL-1.1 is a weak copyleft licence, characterised as a middle ground between permissive free software licences and the GNU General Public License that seeks to balance the concerns of proprietary and open source developers. As such, it allows re-licencing. It is approved by the Open Source Initiative. It has been superseded by v2.0."@en ;
    skos:exactMatch <https://opensource.org/licenses/MPL-1.1> ;
    skos:inScheme atold:licence ;
    skos:prefLabel "Mozilla Public License (MPL), version 1.1 (MPL-1.1)"@en ;
    skos:topConceptOf atold:licence .

<http://publications.europa.eu/resource/authority/licence/MPL_2_0> a skos:Concept ;
    at:authority-code "MPL_2_0" ;
    at:deprecated "false" ;
    at:op-code "MPL_2_0" ;
    at:start.use "2012-01-03" ;
    atold:op-code "MPL_2_0" ;
    dc:identifier "MPL_2_0" ;
    skos:altLabel "MPL-2.0"@bg,
        "MPL-2.0"@cs,
        "MPL-2.0"@da,
        "MPL-2.0"@de,
        "MPL-2.0"@el,
        "MPL-2.0"@en,
        "MPL-2.0"@es,
        "MPL-2.0"@et,
        "MPL-2.0"@fi,
        "MPL-2.0"@fr,
        "MPL-2.0"@ga,
        "MPL-2.0"@hr,
        "MPL-2.0"@hu,
        "MPL-2.0"@it,
        "MPL-2.0"@lt,
        "MPL-2.0"@lv,
        "MPL-2.0"@mt,
        "MPL-2.0"@nl,
        "MPL-2.0"@pl,
        "MPL-2.0"@pt,
        "MPL-2.0"@ro,
        "MPL-2.0"@sk,
        "MPL-2.0"@sl,
        "MPL-2.0"@sv ;
    skos:changeNote "The source of the start-use date: https://en.wikipedia.org/wiki/Mozilla_Public_License#cite_note-17"@en ;
    skos:definition "MPL-2.0 is a weak copyleft licence, characterised as a middle ground between permissive free software licences and the GNU General Public License that seeks to balance the concerns of proprietary and open source developers. As such, it allows re-licencing. It is approved by the Open Source Initiative."@en ;
    skos:exactMatch <https://opensource.org/licenses/MPL-2.0> ;
    skos:inScheme atold:licence ;
    skos:prefLabel "Mozilla Public License (MPL), version 2.0 (MPL-2.0)"@en ;
    skos:topConceptOf atold:licence .

<http://publications.europa.eu/resource/authority/licence/MS_PL> a skos:Concept ;
    at:authority-code "MS_PL" ;
    at:deprecated "false" ;
    at:op-code "MS_PL" ;
    at:start.use "2007-10-12" ;
    atold:op-code "MS_PL" ;
    dc:identifier "MS_PL" ;
    skos:altLabel "MS-PL"@bg,
        "MS-PL"@cs,
        "MS-PL"@da,
        "MS-PL"@de,
        "MS-PL"@el,
        "MS-PL"@en,
        "MS-PL"@es,
        "MS-PL"@et,
        "MS-PL"@fi,
        "MS-PL"@fr,
        "MS-PL"@ga,
        "MS-PL"@hr,
        "MS-PL"@hu,
        "MS-PL"@it,
        "MS-PL"@lt,
        "MS-PL"@lv,
        "MS-PL"@mt,
        "MS-PL"@nl,
        "MS-PL"@pl,
        "MS-PL"@pt,
        "MS-PL"@ro,
        "MS-PL"@sk,
        "MS-PL"@sl,
        "MS-PL"@sv ;
    skos:changeNote "The source of the start-use date: https://en.wikipedia.org/wiki/Shared_Source_Initiative#Microsoft_Public_License_(Ms-PL)"@en ;
    skos:definition "MS-PL is a BSD-style, permissive free software licence approved by the Open Source Initiative."@en ;
    skos:exactMatch <https://opensource.org/licenses/MS-PL> ;
    skos:inScheme atold:licence ;
    skos:prefLabel "Microsoft Public License (MS-PL)"@en ;
    skos:topConceptOf atold:licence .

<http://publications.europa.eu/resource/authority/licence/MS_RL> a skos:Concept ;
    at:authority-code "MS_RL" ;
    at:deprecated "false" ;
    at:op-code "MS_RL" ;
    at:start.use "2007-08-10" ;
    atold:op-code "MS_RL" ;
    dc:identifier "MS_RL" ;
    skos:altLabel "MS-RL"@bg,
        "MS-RL"@cs,
        "MS-RL"@da,
        "MS-RL"@de,
        "MS-RL"@el,
        "MS-RL"@en,
        "MS-RL"@es,
        "MS-RL"@et,
        "MS-RL"@fi,
        "MS-RL"@fr,
        "MS-RL"@ga,
        "MS-RL"@hr,
        "MS-RL"@hu,
        "MS-RL"@it,
        "MS-RL"@lt,
        "MS-RL"@lv,
        "MS-RL"@mt,
        "MS-RL"@nl,
        "MS-RL"@pl,
        "MS-RL"@pt,
        "MS-RL"@ro,
        "MS-RL"@sk,
        "MS-RL"@sl,
        "MS-RL"@sv ;
    skos:changeNote "The source of the start-use date: https://de.wikipedia.org/wiki/Microsoft_Reciprocal_License"@en ;
    skos:definition "MS-RL is a copyleft-style, free software licence approved by the Open Source Initiative."@en ;
    skos:exactMatch <https://opensource.org/licenses/MS-RL> ;
    skos:inScheme atold:licence ;
    skos:prefLabel "Microsoft Reciprocal License (MS-RL)"@en ;
    skos:topConceptOf atold:licence .

<http://publications.europa.eu/resource/authority/licence/MULTICS> a skos:Concept ;
    at:authority-code "MULTICS" ;
    at:deprecated "false" ;
    at:op-code "MULTICS" ;
    at:start.use "2006-07-01" ;
    atold:op-code "MULTICS" ;
    dc:identifier "MULTICS" ;
    skos:altLabel "Multics"@bg,
        "Multics"@cs,
        "Multics"@da,
        "Multics"@de,
        "Multics"@el,
        "Multics"@en,
        "Multics"@es,
        "Multics"@et,
        "Multics"@fi,
        "Multics"@fr,
        "Multics"@ga,
        "Multics"@hr,
        "Multics"@hu,
        "Multics"@it,
        "Multics"@lt,
        "Multics"@lv,
        "Multics"@mt,
        "Multics"@nl,
        "Multics"@pl,
        "Multics"@pt,
        "Multics"@ro,
        "Multics"@sk,
        "Multics"@sl,
        "Multics"@sv ;
    skos:changeNote "The source of the start-use date: https://enterprise.dejacode.com/licenses/public/multics/?_list_filters=q%3Dmultics"@en ;
    skos:definition "Multics is a permissive free software licence approved by the Open Source Initiative. The legal text of this licence is only a paragraph long and both protects the authors' trademarks and requires users to include this licence."@en ;
    skos:exactMatch <https://opensource.org/licenses/Multics> ;
    skos:inScheme atold:licence ;
    skos:prefLabel "Multics License (Multics)"@en ;
    skos:topConceptOf atold:licence .

<http://publications.europa.eu/resource/authority/licence/NASA_1_3> a skos:Concept ;
    at:authority-code "NASA_1_3" ;
    at:deprecated "false" ;
    at:op-code "NASA_1_3" ;
    at:start.use "2012-01-01" ;
    atold:op-code "NASA_1_3" ;
    dc:identifier "NASA_1_3" ;
    skos:altLabel "NASA-1.3"@bg,
        "NASA-1.3"@cs,
        "NASA-1.3"@da,
        "NASA-1.3"@de,
        "NASA-1.3"@el,
        "NASA-1.3"@en,
        "NASA-1.3"@es,
        "NASA-1.3"@et,
        "NASA-1.3"@fi,
        "NASA-1.3"@fr,
        "NASA-1.3"@ga,
        "NASA-1.3"@hr,
        "NASA-1.3"@hu,
        "NASA-1.3"@it,
        "NASA-1.3"@lt,
        "NASA-1.3"@lv,
        "NASA-1.3"@mt,
        "NASA-1.3"@nl,
        "NASA-1.3"@pl,
        "NASA-1.3"@pt,
        "NASA-1.3"@ro,
        "NASA-1.3"@sk,
        "NASA-1.3"@sl,
        "NASA-1.3"@sv ;
    skos:changeNote "The source of the start-use date: https://en.wikipedia.org/wiki/NASA_Open_Source_Agreement; http://openvsp.org/learn.shtml"@en ;
    skos:definition "Approved by the Open Source Initiative, NASA-1.3 is a licence used by NASA containing an obligation to register with the government when receiving the software and to tell a specified agency how the modifications are used."@en ;
    skos:exactMatch <https://opensource.org/licenses/NASA-1.3> ;
    skos:inScheme atold:licence ;
    skos:prefLabel "NASA Open Source Agreement v1.3 (NASA-1.3)"@en ;
    skos:topConceptOf atold:licence .

<http://publications.europa.eu/resource/authority/licence/NAUMEN> a skos:Concept ;
    at:authority-code "NAUMEN" ;
    at:deprecated "false" ;
    at:op-code "NAUMEN" ;
    at:start.use "2001-12-01" ;
    atold:op-code "NAUMEN" ;
    dc:identifier "NAUMEN" ;
    skos:altLabel "Naumen"@bg,
        "Naumen"@cs,
        "Naumen"@da,
        "Naumen"@de,
        "Naumen"@el,
        "Naumen"@en,
        "Naumen"@es,
        "Naumen"@et,
        "Naumen"@fi,
        "Naumen"@fr,
        "Naumen"@ga,
        "Naumen"@hr,
        "Naumen"@hu,
        "Naumen"@it,
        "Naumen"@lt,
        "Naumen"@lv,
        "Naumen"@mt,
        "Naumen"@nl,
        "Naumen"@pl,
        "Naumen"@pt,
        "Naumen"@ro,
        "Naumen"@sk,
        "Naumen"@sl,
        "Naumen"@sv ;
    skos:changeNote "The source of the start-use date: https://ru.wikipedia.org/wiki/Naumen; http://licenseit.ru/wiki/index.php/Naumen_Public_License"@en ;
    skos:definition "Approved by the Open Source Initiative, Naumen is a fairly restrictive free software licence, but provides good protection for the author of the software."@en ;
    skos:exactMatch <https://opensource.org/licenses/Naumen> ;
    skos:inScheme atold:licence ;
    skos:prefLabel "NAUMEN Public License (Naumen)"@en ;
    skos:topConceptOf atold:licence .

<http://publications.europa.eu/resource/authority/licence/NCSA> a skos:Concept ;
    at:authority-code "NCSA" ;
    at:deprecated "false" ;
    at:op-code "NCSA" ;
    at:start.use "2002-03-28" ;
    atold:op-code "NCSA" ;
    dc:identifier "NCSA" ;
    skos:altLabel "NCSA"@bg,
        "NCSA"@cs,
        "NCSA"@da,
        "NCSA"@de,
        "NCSA"@el,
        "NCSA"@en,
        "NCSA"@es,
        "NCSA"@et,
        "NCSA"@fi,
        "NCSA"@fr,
        "NCSA"@ga,
        "NCSA"@hr,
        "NCSA"@hu,
        "NCSA"@it,
        "NCSA"@lt,
        "NCSA"@lv,
        "NCSA"@mt,
        "NCSA"@nl,
        "NCSA"@pl,
        "NCSA"@pt,
        "NCSA"@ro,
        "NCSA"@sk,
        "NCSA"@sl,
        "NCSA"@sv ;
    skos:changeNote "The source of the start-use date: https://en.wikipedia.org/wiki/University_of_Illinois/NCSA_Open_Source_License"@en ;
    skos:definition "NCSA Open Source License is a BSD-style, permissive free software licence approved by the Open Source Initiative."@en ;
    skos:exactMatch <https://opensource.org/licenses/NCSA> ;
    skos:inScheme atold:licence ;
    skos:prefLabel "The University of Illinois/NCSA Open Source License (NCSA)"@en ;
    skos:topConceptOf atold:licence .

<http://publications.europa.eu/resource/authority/licence/NGPL> a skos:Concept ;
    at:authority-code "NGPL" ;
    at:deprecated "false" ;
    at:op-code "NGPL" ;
    at:start.use "1989-07-31" ;
    atold:op-code "NGPL" ;
    dc:identifier "NGPL" ;
    skos:altLabel "NGPL"@bg,
        "NGPL"@cs,
        "NGPL"@da,
        "NGPL"@de,
        "NGPL"@el,
        "NGPL"@en,
        "NGPL"@es,
        "NGPL"@et,
        "NGPL"@fi,
        "NGPL"@fr,
        "NGPL"@ga,
        "NGPL"@hr,
        "NGPL"@hu,
        "NGPL"@it,
        "NGPL"@lt,
        "NGPL"@lv,
        "NGPL"@mt,
        "NGPL"@nl,
        "NGPL"@pl,
        "NGPL"@pt,
        "NGPL"@ro,
        "NGPL"@sk,
        "NGPL"@sl,
        "NGPL"@sv ;
    skos:changeNote "The source of the start-use date: https://en.wikipedia.org/wiki/NetHack"@en ;
    skos:definition "Approved by the Open Source Initiative, NGPL is a very old licence used for the game NetHack. It allows users to freely share their modifications, in exchange for several restrictions and little protection for the authors."@en ;
    skos:exactMatch <https://opensource.org/licenses/NGPL> ;
    skos:inScheme atold:licence ;
    skos:prefLabel "The Nethack General Public License (NGPL)"@en ;
    skos:topConceptOf atold:licence .

<http://publications.europa.eu/resource/authority/licence/NLOD_1_0> a skos:Concept ;
    at:authority-code "NLOD_1_0" ;
    at:deprecated "false" ;
    at:op-code "NLOD_1_0" ;
    at:start.use "2012-01-01" ;
    atold:op-code "NLOD_1_0" ;
    dc:identifier "NLOD_1_0" ;
    skos:altLabel "NLOD 1.0"@bg,
        "NLOD 1.0"@cs,
        "NLOD 1.0"@da,
        "NLOD 1.0"@de,
        "NLOD 1.0"@el,
        "NLOD 1.0"@en,
        "NLOD 1.0"@es,
        "NLOD 1.0"@et,
        "NLOD 1.0"@fi,
        "NLOD 1.0"@fr,
        "NLOD 1.0"@ga,
        "NLOD 1.0"@hr,
        "NLOD 1.0"@hu,
        "NLOD 1.0"@it,
        "NLOD 1.0"@lt,
        "NLOD 1.0"@lv,
        "NLOD 1.0"@mt,
        "NLOD 1.0"@nl,
        "NLOD 1.0"@pl,
        "NLOD 1.0"@pt,
        "NLOD 1.0"@ro,
        "NLOD 1.0"@sk,
        "NLOD 1.0"@sl,
        "NLOD 1.0"@sv ;
    skos:changeNote "The source of the start-use date: https://github.com/difi/veileder-opnedata/blob/master/build/html/en/_sources/Hvordan-aapne-opp-data/index.txt"@en ;
    skos:definition "Published by Norway, NLOD 1.0 grants the user the right to copy, use and distribute information, provided the user acknowledges the contributors and complies with the terms and conditions stipulated in this licence."@en ;
    skos:exactMatch <http://data.norge.no/nlod/en/1.0> ;
    skos:inScheme atold:licence ;
    skos:prefLabel "Norwegian Licence for Open Government Data 1.0"@en ;
    skos:topConceptOf atold:licence .

<http://publications.europa.eu/resource/authority/licence/NLOD_2_0> a skos:Concept ;
    at:authority-code "NLOD_2_0" ;
    at:deprecated "false" ;
    at:op-code "NLOD_2_0" ;
    at:start.use "2016-09-01" ;
    atold:op-code "NLOD_2_0" ;
    dc:identifier "NLOD_2_0" ;
    skos:altLabel "NLOD 2.0"@bg,
        "NLOD 2.0"@cs,
        "NLOD 2.0"@da,
        "NLOD 2.0"@de,
        "NLOD 2.0"@el,
        "NLOD 2.0"@en,
        "NLOD 2.0"@es,
        "NLOD 2.0"@et,
        "NLOD 2.0"@fi,
        "NLOD 2.0"@fr,
        "NLOD 2.0"@ga,
        "NLOD 2.0"@hr,
        "NLOD 2.0"@hu,
        "NLOD 2.0"@it,
        "NLOD 2.0"@lt,
        "NLOD 2.0"@lv,
        "NLOD 2.0"@mt,
        "NLOD 2.0"@nl,
        "NLOD 2.0"@pl,
        "NLOD 2.0"@pt,
        "NLOD 2.0"@ro,
        "NLOD 2.0"@sk,
        "NLOD 2.0"@sl,
        "NLOD 2.0"@sv ;
    skos:definition "Published by Norway, NLOD 2.0 grants the user the right to copy, use and distribute information, provided the user acknowledges the contributors and complies with the terms and conditions stipulated in this licence."@en ;
    skos:exactMatch <https://data.norge.no/nlod/en/2.0/> ;
    skos:inScheme atold:licence ;
    skos:prefLabel "Norwegian Licence for Open Government Data (NLOD) 2.0"@en ;
    skos:topConceptOf atold:licence .

<http://publications.europa.eu/resource/authority/licence/NOKIA> a skos:Concept ;
    at:authority-code "NOKIA" ;
    at:deprecated "false" ;
    at:op-code "NOKIA" ;
    at:start.use "2006-01-01" ;
    atold:op-code "NOKIA" ;
    dc:identifier "NOKIA" ;
    skos:altLabel "NOKIA"@bg,
        "NOKIA"@cs,
        "NOKIA"@da,
        "NOKIA"@de,
        "NOKIA"@el,
        "NOKIA"@en,
        "NOKIA"@es,
        "NOKIA"@et,
        "NOKIA"@fi,
        "NOKIA"@fr,
        "NOKIA"@ga,
        "NOKIA"@hr,
        "NOKIA"@hu,
        "NOKIA"@it,
        "NOKIA"@lt,
        "NOKIA"@lv,
        "NOKIA"@mt,
        "NOKIA"@nl,
        "NOKIA"@pl,
        "NOKIA"@pt,
        "NOKIA"@ro,
        "NOKIA"@sk,
        "NOKIA"@sl,
        "NOKIA"@sv ;
    skos:changeNote "The source of the start-use date: http://www.kansai-u.ac.jp/riss/rcss/conf/confdocs/3rdRCSS_ueda.pdf; https://opensource.org/minutes20060208"@en ;
    skos:definition "Approved by the Open Source Initiative, NOKIA is a slightly altered variant on the Mozilla Public License specified for Nokia. It requires including a notice in each source file. Disputes must be settled through a Finnish arbitration process."@en ;
    skos:exactMatch <https://opensource.org/licenses/NOKIA> ;
    skos:inScheme atold:licence ;
    skos:prefLabel "Nokia Open Source License Version 1.0a (NOKIA)"@en ;
    skos:topConceptOf atold:licence .

<http://publications.europa.eu/resource/authority/licence/NPOSL_3_0> a skos:Concept ;
    at:authority-code "NPOSL_3_0" ;
    at:deprecated "false" ;
    at:op-code "NPOSL_3_0" ;
    at:start.use "2007-09-20" ;
    atold:op-code "NPOSL_3_0" ;
    dc:identifier "NPOSL_3_0" ;
    skos:altLabel "NPOSL-3.0"@bg,
        "NPOSL-3.0"@cs,
        "NPOSL-3.0"@da,
        "NPOSL-3.0"@de,
        "NPOSL-3.0"@el,
        "NPOSL-3.0"@en,
        "NPOSL-3.0"@es,
        "NPOSL-3.0"@et,
        "NPOSL-3.0"@fi,
        "NPOSL-3.0"@fr,
        "NPOSL-3.0"@ga,
        "NPOSL-3.0"@hr,
        "NPOSL-3.0"@hu,
        "NPOSL-3.0"@it,
        "NPOSL-3.0"@lt,
        "NPOSL-3.0"@lv,
        "NPOSL-3.0"@mt,
        "NPOSL-3.0"@nl,
        "NPOSL-3.0"@pl,
        "NPOSL-3.0"@pt,
        "NPOSL-3.0"@ro,
        "NPOSL-3.0"@sk,
        "NPOSL-3.0"@sl,
        "NPOSL-3.0"@sv ;
    skos:changeNote "The source of the start-use date: https://lists.debian.org/debian-legal/2008/04/msg00055.html; https://trustee.ietf.org/licenses.html"@en ;
    skos:definition "A variant of the Open Software License 3.0, NPOSL-3.0 requires that the organisation using it is a non-profit and that no revenue is generated from sale of the software, support or services. It is approved by the Open Source Initiative."@en ;
    skos:exactMatch <https://opensource.org/licenses/NPOSL-3.0> ;
    skos:inScheme atold:licence ;
    skos:prefLabel "The Non-Profit Open Software License version 3.0 (NPOSL-3.0)"@en ;
    skos:topConceptOf atold:licence .

<http://publications.europa.eu/resource/authority/licence/NTP> a skos:Concept ;
    at:authority-code "NTP" ;
    at:deprecated "false" ;
    at:op-code "NTP" ;
    at:start.use "2008-08-01" ;
    atold:op-code "NTP" ;
    dc:identifier "NTP" ;
    skos:altLabel "NTP"@bg,
        "NTP"@cs,
        "NTP"@da,
        "NTP"@de,
        "NTP"@el,
        "NTP"@en,
        "NTP"@es,
        "NTP"@et,
        "NTP"@fi,
        "NTP"@fr,
        "NTP"@ga,
        "NTP"@hr,
        "NTP"@hu,
        "NTP"@it,
        "NTP"@lt,
        "NTP"@lv,
        "NTP"@mt,
        "NTP"@nl,
        "NTP"@pl,
        "NTP"@pt,
        "NTP"@ro,
        "NTP"@sk,
        "NTP"@sl,
        "NTP"@sv ;
    skos:changeNote "The source of the start-use date: http://lists.opensource.org/pipermail/license-review_lists.opensource.org/2008-March/000099.html; https://opensource.org/node/1015"@en ;
    skos:definition "Approved by the Open Source Initiative, NTP is a simple licence, written as a template, that provides protection for the author while giving users full rights to the software."@en ;
    skos:exactMatch <https://opensource.org/licenses/NTP> ;
    skos:inScheme atold:licence ;
    skos:prefLabel "NTP License (NTP)"@en ;
    skos:topConceptOf atold:licence .

<http://publications.europa.eu/resource/authority/licence/OCLC_2_0> a skos:Concept ;
    at:authority-code "OCLC_2_0" ;
    at:deprecated "false" ;
    at:op-code "OCLC_2_0" ;
    at:start.use "2002-05-31" ;
    atold:op-code "OCLC_2_0" ;
    dc:identifier "OCLC_2_0" ;
    skos:altLabel "OCLC-2.0"@bg,
        "OCLC-2.0"@cs,
        "OCLC-2.0"@da,
        "OCLC-2.0"@de,
        "OCLC-2.0"@el,
        "OCLC-2.0"@en,
        "OCLC-2.0"@es,
        "OCLC-2.0"@et,
        "OCLC-2.0"@fi,
        "OCLC-2.0"@fr,
        "OCLC-2.0"@ga,
        "OCLC-2.0"@hr,
        "OCLC-2.0"@hu,
        "OCLC-2.0"@it,
        "OCLC-2.0"@lt,
        "OCLC-2.0"@lv,
        "OCLC-2.0"@mt,
        "OCLC-2.0"@nl,
        "OCLC-2.0"@pl,
        "OCLC-2.0"@pt,
        "OCLC-2.0"@ro,
        "OCLC-2.0"@sk,
        "OCLC-2.0"@sl,
        "OCLC-2.0"@sv ;
    skos:changeNote "The source of the start-use date: https://opensource.org/licenses/OCLC-2.0"@en ;
    skos:definition "While OCLC Research now uses the Apache 2.0 licence, OCLC-2.0 is a relatively strong copyleft licence with fairly lenient restrictions and built-in protection for the author. It is approved by the Open Source Initiative."@en ;
    skos:exactMatch <https://opensource.org/licenses/OCLC-2.0> ;
    skos:inScheme atold:licence ;
    skos:prefLabel "The OCLC Research Public License 2.0 License (OCLC-2.0)"@en ;
    skos:topConceptOf atold:licence .

<http://publications.europa.eu/resource/authority/licence/ODC_BL> a skos:Concept ;
    at:authority-code "ODC_BL" ;
    at:deprecated "false" ;
    at:op-code "ODC_BL" ;
    at:start.use "2009-01-01" ;
    atold:op-code "ODC_BL" ;
    dc:identifier "ODC_BL" ;
    skos:altLabel "ODbL"@bg,
        "ODbL"@cs,
        "ODbL"@da,
        "ODbL"@de,
        "ODbL"@el,
        "ODbL"@en,
        "ODbL"@es,
        "ODbL"@et,
        "ODbL"@fi,
        "ODbL"@fr,
        "ODbL"@ga,
        "ODbL"@hr,
        "ODbL"@hu,
        "ODbL"@it,
        "ODbL"@lt,
        "ODbL"@lv,
        "ODbL"@mt,
        "ODbL"@nl,
        "ODbL"@pl,
        "ODbL"@pt,
        "ODbL"@ro,
        "ODbL"@sk,
        "ODbL"@sl,
        "ODbL"@sv ;
    skos:definition "ODbL is a licence agreement intended to allow users to freely share, modify, and use the database concerned while maintaining this same freedom for others. Some jurisdictions, mainly in the European Union, have specific rights that cover databases, and so this licence addresses these rights, too. This licence is also an agreement in contract for users of this database to act in certain ways in return for accessing the database concerned."@en,
        "ODbL est un contrat de licence ayant pour objet d’autoriser les utilisateurs à partager, modifier et utiliser librement la base de données initiale tout en maintenant ces mêmes libertés pour les autres. De nombreuses bases de données étant protégées par des droits d’auteur, les présentes règles ont pour objet de céder ces droits. Certains États, principalement au sein de l’Union européenne, prévoient des droits spécifiques régissant les bases de données, de ce fait ces droits sont également concernés par cette licence. Cette licence est aussi un contrat en ce que les utilisateurs de la base de données initiale s’engagent à respecter certaines obligations en contrepartie de l’autorisation d’accéder à ladite base de données initiale."@fr ;
    skos:exactMatch <http://opendatacommons.org/licenses/odbl/1.0/> ;
    skos:inScheme atold:licence ;
    skos:prefLabel "Open Data Commons Open Database License v1.0"@en ;
    skos:topConceptOf atold:licence .

<http://publications.europa.eu/resource/authority/licence/ODC_BY> a skos:Concept ;
    at:authority-code "ODC_BY" ;
    at:deprecated "false" ;
    at:op-code "ODC_BY" ;
    at:start.use "2010-10-24" ;
    atold:op-code "ODC_BY" ;
    dc:identifier "ODC_BY" ;
    skos:altLabel "ODC-By-1.0"@bg,
        "ODC-By-1.0"@cs,
        "ODC-By-1.0"@da,
        "ODC-By-1.0"@de,
        "ODC-By-1.0"@el,
        "ODC-By-1.0"@en,
        "ODC-By-1.0"@es,
        "ODC-By-1.0"@et,
        "ODC-By-1.0"@fi,
        "ODC-By-1.0"@fr,
        "ODC-By-1.0"@ga,
        "ODC-By-1.0"@hr,
        "ODC-By-1.0"@hu,
        "ODC-By-1.0"@it,
        "ODC-By-1.0"@lt,
        "ODC-By-1.0"@lv,
        "ODC-By-1.0"@mt,
        "ODC-By-1.0"@nl,
        "ODC-By-1.0"@pl,
        "ODC-By-1.0"@pt,
        "ODC-By-1.0"@ro,
        "ODC-By-1.0"@sk,
        "ODC-By-1.0"@sl,
        "ODC-By-1.0"@sv ;
    skos:definition "ODC-By-1.0 is a licence agreement intended to allow users to freely share, modify, and use the database concerned subject only to the attribution requirements set out in Section 4 (notices, no sublicensing). Databases can contain a wide variety of types of content, and so this licence only governs the rights over the database, and not the contents of the database individually."@en ;
    skos:exactMatch <http://opendatacommons.org/licenses/by/1.0/> ;
    skos:inScheme atold:licence ;
    skos:prefLabel "Open Data Commons Attribution License v1.0"@en ;
    skos:topConceptOf atold:licence .

<http://publications.europa.eu/resource/authority/licence/ODC_PDDL> a skos:Concept ;
    at:authority-code "ODC_PDDL" ;
    at:deprecated "false" ;
    at:op-code "ODC_PDDL" ;
    at:start.use "2008-03-01" ;
    atold:op-code "ODC_PDDL" ;
    dc:identifier "ODC_PDDL" ;
    skos:altLabel "PDDL"@bg,
        "PDDL"@cs,
        "PDDL"@da,
        "PDDL"@de,
        "PDDL"@el,
        "PDDL"@en,
        "PDDL"@es,
        "PDDL"@et,
        "PDDL"@fi,
        "PDDL"@fr,
        "PDDL"@ga,
        "PDDL"@hr,
        "PDDL"@hu,
        "PDDL"@it,
        "PDDL"@lt,
        "PDDL"@lv,
        "PDDL"@mt,
        "PDDL"@nl,
        "PDDL"@pl,
        "PDDL"@pt,
        "PDDL"@ro,
        "PDDL"@sk,
        "PDDL"@sl,
        "PDDL"@sv ;
    skos:changeNote "https://www.geeklawblog.com/2010/10/creative-commons-releases-public-domain.html"@en ;
    skos:definition "ODC PDDL is a document intended to allow the user to freely share, modify, and use this work for any purpose and without any restrictions. It is intended for use on databases or their contents (“data”), either together or individually."@en ;
    skos:exactMatch <http://opendatacommons.org/licenses/pddl/1.0/> ;
    skos:inScheme atold:licence ;
    skos:prefLabel "Open Data Commons Public Domain Dedication and License 1.0"@en ;
    skos:topConceptOf atold:licence .

<http://publications.europa.eu/resource/authority/licence/OFL_1_1> a skos:Concept ;
    at:authority-code "OFL_1_1" ;
    at:deprecated "false" ;
    at:op-code "OFL_1_1" ;
    at:start.use "2007-02-26" ;
    atold:op-code "OFL_1_1" ;
    dc:identifier "OFL_1_1" ;
    skos:altLabel "OFL-1.1"@bg,
        "OFL-1.1"@cs,
        "OFL-1.1"@da,
        "OFL-1.1"@de,
        "OFL-1.1"@el,
        "OFL-1.1"@en,
        "OFL-1.1"@es,
        "OFL-1.1"@et,
        "OFL-1.1"@fi,
        "OFL-1.1"@fr,
        "OFL-1.1"@ga,
        "OFL-1.1"@hr,
        "OFL-1.1"@hu,
        "OFL-1.1"@it,
        "OFL-1.1"@lt,
        "OFL-1.1"@lv,
        "OFL-1.1"@mt,
        "OFL-1.1"@nl,
        "OFL-1.1"@pl,
        "OFL-1.1"@pt,
        "OFL-1.1"@ro,
        "OFL-1.1"@sk,
        "OFL-1.1"@sl,
        "OFL-1.1"@sv ;
    skos:changeNote "The source of the start-use date: https://scripts.sil.org/cms/scripts/page.php?site_id=nrsi&id=OFL"@en ;
    skos:definition "The SIL Open Font License 1.1 is one of the major open font licences, which allows embedding of the font in commercially sold products. It is a free and open source licence approved by the Open Source Initiative."@en ;
    skos:exactMatch <https://opensource.org/licenses/OFL-1.1> ;
    skos:inScheme atold:licence ;
    skos:prefLabel "SIL Open Font License (OFL-1.1)"@en ;
    skos:topConceptOf atold:licence .

<http://publications.europa.eu/resource/authority/licence/OGL_1_0> a skos:Concept ;
    at:authority-code "OGL_1_0" ;
    at:deprecated "false" ;
    at:op-code "OGL_1_0" ;
    at:start.use "2010-09-01" ;
    atold:op-code "OGL_1_0" ;
    dc:identifier "OGL_1_0" ;
    skos:altLabel "OGL 1.0"@bg,
        "OGL 1.0"@cs,
        "OGL 1.0"@da,
        "OGL 1.0"@de,
        "OGL 1.0"@el,
        "OGL 1.0"@en,
        "OGL 1.0"@es,
        "OGL 1.0"@et,
        "OGL 1.0"@fi,
        "OGL 1.0"@fr,
        "OGL 1.0"@ga,
        "OGL 1.0"@hr,
        "OGL 1.0"@hu,
        "OGL 1.0"@it,
        "OGL 1.0"@lt,
        "OGL 1.0"@lv,
        "OGL 1.0"@mt,
        "OGL 1.0"@nl,
        "OGL 1.0"@pl,
        "OGL 1.0"@pt,
        "OGL 1.0"@ro,
        "OGL 1.0"@sk,
        "OGL 1.0"@sl,
        "OGL 1.0"@sv ;
    skos:changeNote "The source of the start-use date: https://en.wikipedia.org/wiki/Open_Government_Licence"@en ;
    skos:definition "Developed and maintained by the National Archives, OGL-1.0 is a copyright licence for Crown Copyright works published by the UK government consisting of a simple set of terms and conditions facilitating the re-use of a wide range of public sector information free of charge. The OGL terms are compatible with the latest versions of the Creative Commons Attribution Licence and the Open Data Commons Attribution Licence. The OGL is a perpetual licence so any past and continuing use of information authorised under v1.0 or v2.0 may continue."@en ;
    skos:exactMatch <http://www.nationalarchives.gov.uk/doc/open-government-licence/version/1/> ;
    skos:inScheme atold:licence ;
    skos:prefLabel "Open Government Licence 1.0"@en ;
    skos:topConceptOf atold:licence .

<http://publications.europa.eu/resource/authority/licence/OGL_2_0> a skos:Concept ;
    at:authority-code "OGL_2_0" ;
    at:deprecated "false" ;
    at:op-code "OGL_2_0" ;
    at:start.use "2013-06-28" ;
    atold:op-code "OGL_2_0" ;
    dc:identifier "OGL_2_0" ;
    skos:altLabel "OGL 2.0"@bg,
        "OGL 2.0"@cs,
        "OGL 2.0"@da,
        "OGL 2.0"@de,
        "OGL 2.0"@el,
        "OGL 2.0"@en,
        "OGL 2.0"@es,
        "OGL 2.0"@et,
        "OGL 2.0"@fi,
        "OGL 2.0"@fr,
        "OGL 2.0"@ga,
        "OGL 2.0"@hr,
        "OGL 2.0"@hu,
        "OGL 2.0"@it,
        "OGL 2.0"@lt,
        "OGL 2.0"@lv,
        "OGL 2.0"@mt,
        "OGL 2.0"@nl,
        "OGL 2.0"@pl,
        "OGL 2.0"@pt,
        "OGL 2.0"@ro,
        "OGL 2.0"@sk,
        "OGL 2.0"@sl,
        "OGL 2.0"@sv ;
    skos:changeNote "The source of the start-use date: https://en.wikipedia.org/wiki/Open_Government_Licence"@en ;
    skos:definition "Developed and maintained by the National Archives, OGL-2.0 is a copyright licence for Crown Copyright works published by the UK government consisting of a simple set of terms and conditions facilitating the re-use of a wide range of public sector information free of charge. The OGL terms are compatible with the latest versions of the Creative Commons Attribution Licence and the Open Data Commons Attribution Licence. The OGL is a perpetual licence so any past and continuing use of information authorised under v1.0 or v2.0 may continue."@en ;
    skos:exactMatch <http://www.nationalarchives.gov.uk/doc/open-government-licence/version/2/> ;
    skos:inScheme atold:licence ;
    skos:prefLabel "Open Government Licence 2.0"@en ;
    skos:topConceptOf atold:licence .

<http://publications.europa.eu/resource/authority/licence/OGL_3_0> a skos:Concept ;
    at:authority-code "OGL_3_0" ;
    at:deprecated "false" ;
    at:op-code "OGL_3_0" ;
    at:start.use "2014-10-31" ;
    atold:op-code "OGL_3_0" ;
    dc:identifier "OGL_3_0" ;
    skos:altLabel "OGL 3.0"@bg,
        "OGL 3.0"@cs,
        "OGL 3.0"@da,
        "OGL 3.0"@de,
        "OGL 3.0"@el,
        "OGL 3.0"@en,
        "OGL 3.0"@es,
        "OGL 3.0"@et,
        "OGL 3.0"@fi,
        "OGL 3.0"@fr,
        "OGL 3.0"@ga,
        "OGL 3.0"@hr,
        "OGL 3.0"@hu,
        "OGL 3.0"@it,
        "OGL 3.0"@lt,
        "OGL 3.0"@lv,
        "OGL 3.0"@mt,
        "OGL 3.0"@nl,
        "OGL 3.0"@pl,
        "OGL 3.0"@pt,
        "OGL 3.0"@ro,
        "OGL 3.0"@sk,
        "OGL 3.0"@sl,
        "OGL 3.0"@sv ;
    skos:changeNote "The source of the start-use date: https://en.wikipedia.org/wiki/Open_Government_Licence"@en ;
    skos:definition "Developed and maintained by the National Archives, OGL-3.0 is a copyright licence for Crown Copyright works published by the UK government consisting of a simple set of terms and conditions facilitating the re-use of a wide range of public sector information free of charge. The OGL terms are compatible with the latest versions of the Creative Commons Attribution Licence and the Open Data Commons Attribution Licence. The OGL is a perpetual licence so any past and continuing use of information authorised under v1.0 or v2.0 may continue."@en ;
    skos:exactMatch <http://www.nationalarchives.gov.uk/doc/open-government-licence/version/3/> ;
    skos:inScheme atold:licence ;
    skos:prefLabel "Open Government Licence 3.0"@en ;
    skos:topConceptOf atold:licence .

<http://publications.europa.eu/resource/authority/licence/OGL_NC> a skos:Concept ;
    at:authority-code "OGL_NC" ;
    at:deprecated "false" ;
    at:op-code "OGL_NC" ;
    at:start.use "2013-06-28" ;
    atold:op-code "OGL_NC" ;
    dc:identifier "OGL_NC" ;
    skos:altLabel "OGL-NC"@bg,
        "OGL-NC"@cs,
        "OGL-NC"@da,
        "OGL-NC"@de,
        "OGL-NC"@el,
        "OGL-NC"@en,
        "OGL-NC"@es,
        "OGL-NC"@et,
        "OGL-NC"@fi,
        "OGL-NC"@fr,
        "OGL-NC"@ga,
        "OGL-NC"@hr,
        "OGL-NC"@hu,
        "OGL-NC"@it,
        "OGL-NC"@lt,
        "OGL-NC"@lv,
        "OGL-NC"@mt,
        "OGL-NC"@nl,
        "OGL-NC"@pl,
        "OGL-NC"@pt,
        "OGL-NC"@ro,
        "OGL-NC"@sk,
        "OGL-NC"@sl,
        "OGL-NC"@sv ;
    skos:changeNote "The source of the start-use date: https://en.wikipedia.org/wiki/Open_Government_Licence"@en ;
    skos:definition "Developed and maintained by the National Archives, the Non-Commercial Government Licence (OGL-NC) may be used by public sector bodies that have a Delegation of Authority to licence Crown copyright material non-commercially. It may also be used by public sector bodies holding non-Crown copyright information in accordance with the PSI Regulations 2015."@en ;
    skos:exactMatch <http://www.nationalarchives.gov.uk/doc/non-commercial-government-licence/non-commercial-government-licence.htm> ;
    skos:inScheme atold:licence ;
    skos:prefLabel "Non-Commercial Government Licence"@en ;
    skos:topConceptOf atold:licence .

<http://publications.europa.eu/resource/authority/licence/OGL_ROU_1_0> a skos:Concept ;
    at:authority-code "OGL_ROU_1_0" ;
    at:deprecated "false" ;
    at:op-code "OGL_ROU_1_0" ;
    at:start.use "2010-09-01" ;
    atold:op-code "OGL_ROU_1_0" ;
    dc:identifier "OGL_ROU_1_0" ;
    skos:altLabel "OGL-ROU 1.0"@bg,
        "OGL-ROU 1.0"@cs,
        "OGL-ROU 1.0"@da,
        "OGL-ROU 1.0"@de,
        "OGL-ROU 1.0"@el,
        "OGL-ROU 1.0"@en,
        "OGL-ROU 1.0"@es,
        "OGL-ROU 1.0"@et,
        "OGL-ROU 1.0"@fi,
        "OGL-ROU 1.0"@fr,
        "OGL-ROU 1.0"@ga,
        "OGL-ROU 1.0"@hr,
        "OGL-ROU 1.0"@hu,
        "OGL-ROU 1.0"@it,
        "OGL-ROU 1.0"@lt,
        "OGL-ROU 1.0"@lv,
        "OGL-ROU 1.0"@mt,
        "OGL-ROU 1.0"@nl,
        "OGL-ROU 1.0"@pl,
        "OGL-ROU 1.0"@pt,
        "OGL-ROU 1.0"@ro,
        "OGL-ROU 1.0"@sk,
        "OGL-ROU 1.0"@sl,
        "OGL-ROU 1.0"@sv ;
    skos:changeNote "The source of the start-use date: https://en.wikipedia.org/wiki/Open_Government_Licence"@en ;
    skos:definition "Having a working value in Romanian, the Non-Commercial Government Licence 1.0 (OGL-ROU 1.0) consists of a simple set of terms and conditions facilitating the re-use of a wide range of public sector information free of charge. The OGL terms are compatible with the latest versions of the Creative Commons Attribution Licence and the Open Data Commons Attribution Licence."@en ;
    skos:exactMatch <http://data.gov.ro/base/images/logoinst/OGL-ROU-1.0.pdf> ;
    skos:inScheme atold:licence ;
    skos:prefLabel "Non-Commercial Government Licence 1.0"@en ;
    skos:topConceptOf atold:licence .

<http://publications.europa.eu/resource/authority/licence/OGTSL> a skos:Concept ;
    at:authority-code "OGTSL" ;
    at:deprecated "false" ;
    at:op-code "OGTSL" ;
    at:start.use "2007-04-01" ;
    atold:op-code "OGTSL" ;
    dc:identifier "OGTSL" ;
    skos:altLabel "OGTSL"@bg,
        "OGTSL"@cs,
        "OGTSL"@da,
        "OGTSL"@de,
        "OGTSL"@el,
        "OGTSL"@en,
        "OGTSL"@es,
        "OGTSL"@et,
        "OGTSL"@fi,
        "OGTSL"@fr,
        "OGTSL"@ga,
        "OGTSL"@hr,
        "OGTSL"@hu,
        "OGTSL"@it,
        "OGTSL"@lt,
        "OGTSL"@lv,
        "OGTSL"@mt,
        "OGTSL"@nl,
        "OGTSL"@pl,
        "OGTSL"@pt,
        "OGTSL"@ro,
        "OGTSL"@sk,
        "OGTSL"@sl,
        "OGTSL"@sv ;
    skos:changeNote "The source of the start-use date: https://appaji.livejournal.com/53826.html"@en ;
    skos:definition "OGTSL was meant to facilitate software testing, without placing severe restrictions on use of the software except in terms of including original versions of the software. It is approved by the Open Source Initiative."@en ;
    skos:exactMatch <https://opensource.org/licenses/OGTSL> ;
    skos:inScheme atold:licence ;
    skos:prefLabel "The Open Group Test Suite License (OGTSL)"@en ;
    skos:topConceptOf atold:licence .

<http://publications.europa.eu/resource/authority/licence/OPL_2_1> a skos:Concept ;
    at:authority-code "OPL_2_1" ;
    at:deprecated "false" ;
    at:op-code "OPL_2_1" ;
    at:start.use "2015-08-31" ;
    atold:op-code "OPL_2_1" ;
    dc:identifier "OPL_2_1" ;
    skos:altLabel "OPL-2.1"@bg,
        "OPL-2.1"@cs,
        "OPL-2.1"@da,
        "OPL-2.1"@de,
        "OPL-2.1"@el,
        "OPL-2.1"@en,
        "OPL-2.1"@es,
        "OPL-2.1"@et,
        "OPL-2.1"@fi,
        "OPL-2.1"@fr,
        "OPL-2.1"@ga,
        "OPL-2.1"@hr,
        "OPL-2.1"@hu,
        "OPL-2.1"@it,
        "OPL-2.1"@lt,
        "OPL-2.1"@lv,
        "OPL-2.1"@mt,
        "OPL-2.1"@nl,
        "OPL-2.1"@pl,
        "OPL-2.1"@pt,
        "OPL-2.1"@ro,
        "OPL-2.1"@sk,
        "OPL-2.1"@sl,
        "OPL-2.1"@sv ;
    skos:changeNote "The source of the start-use date: https://libraries.io/search?licenses=OSET-PL-2.1&order=desc&page=4&sort=latest_release_published_at"@en ;
    skos:definition "OSET Public License 2.1 is a copyleft-style, free software licence approved by the Open Source Initiative."@en ;
    skos:exactMatch <https://opensource.org/licenses/OPL-2.1> ;
    skos:inScheme atold:licence ;
    skos:prefLabel "OSET Public License version 2.1"@en ;
    skos:topConceptOf atold:licence .

<http://publications.europa.eu/resource/authority/licence/OP_DATPRO> a skos:Concept ;
    at:authority-code "OP_DATPRO" ;
    at:deprecated "false" ;
    at:op-code "OP_DATPRO" ;
    at:start.use "1952-07-23" ;
    atold:op-code "OP_DATPRO" ;
    dc:identifier "OP_DATPRO" ;
    skos:inScheme atold:licence ;
    skos:prefLabel "Неокончателни данни"@bg,
        "Předběžné údaje"@cs,
        "Midlertidige data"@da,
        "Vorläufige Daten"@de,
        "Προσωρινά δεδομένα"@el,
        "Provisional data"@en,
        "Datos provisionales"@es,
        "Esialgsed andmed"@et,
        "Alustavat tiedot"@fi,
        "Données provisoires"@fr,
        "Sonraí sealadacha"@ga,
        "Privremeni podaci"@hr,
        "Ideiglenes adatok"@hu,
        "Dati provvisori"@it,
        "Laikinieji duomenys"@lt,
        "Provizoriski dati"@lv,
        "Dejta provviżorja"@mt,
        "Voorlopige gegevens"@nl,
        "Dane tymczasowe"@pl,
        "Dados provisórios"@pt,
        "Date provizorii"@ro,
        "Predbežné údaje"@sk,
        "Začasni podatki"@sl,
        "Tillfälliga uppgifter"@sv ;
    skos:topConceptOf atold:licence .

<http://publications.europa.eu/resource/authority/licence/OSL_1_0> a skos:Concept ;
    at:authority-code "OSL_1_0" ;
    at:deprecated "true" ;
    at:end.use "2005-11-30" ;
    at:op-code "OSL_1_0" ;
    at:start.use "2002-08-31" ;
    atold:op-code "OSL_1_0" ;
    dc:identifier "OSL_1_0" ;
    skos:altLabel "OSL-1.0"@bg,
        "OSL-1.0"@cs,
        "OSL-1.0"@da,
        "OSL-1.0"@de,
        "OSL-1.0"@el,
        "OSL-1.0"@en,
        "OSL-1.0"@es,
        "OSL-1.0"@et,
        "OSL-1.0"@fi,
        "OSL-1.0"@fr,
        "OSL-1.0"@ga,
        "OSL-1.0"@hr,
        "OSL-1.0"@hu,
        "OSL-1.0"@it,
        "OSL-1.0"@lt,
        "OSL-1.0"@lv,
        "OSL-1.0"@mt,
        "OSL-1.0"@nl,
        "OSL-1.0"@pl,
        "OSL-1.0"@pt,
        "OSL-1.0"@ro,
        "OSL-1.0"@sk,
        "OSL-1.0"@sl,
        "OSL-1.0"@sv ;
    skos:changeNote "The source of the start-use date: https://old.computerra.ru/2002/466/200189/"@en ;
    skos:definition "Open Software License 1.0 is a copyleft-style, free software licence approved by the Open Source Initiative."@en ;
    skos:exactMatch <https://opensource.org/licenses/OSL-1.0> ;
    skos:inScheme atold:licence ;
    skos:prefLabel "Open Software License, version 1.0 (OSL-1.0)"@en ;
    skos:topConceptOf atold:licence .

<http://publications.europa.eu/resource/authority/licence/OSL_2_1> a skos:Concept ;
    at:authority-code "OSL_2_1" ;
    at:deprecated "true" ;
    at:end.use "2005-11-30" ;
    at:op-code "OSL_2_1" ;
    at:start.use "2003-10-31" ;
    atold:op-code "OSL_2_1" ;
    dc:identifier "OSL_2_1" ;
    skos:altLabel "OSL-2.1"@bg,
        "OSL-2.1"@cs,
        "OSL-2.1"@da,
        "OSL-2.1"@de,
        "OSL-2.1"@el,
        "OSL-2.1"@en,
        "OSL-2.1"@es,
        "OSL-2.1"@et,
        "OSL-2.1"@fi,
        "OSL-2.1"@fr,
        "OSL-2.1"@ga,
        "OSL-2.1"@hr,
        "OSL-2.1"@hu,
        "OSL-2.1"@it,
        "OSL-2.1"@lt,
        "OSL-2.1"@lv,
        "OSL-2.1"@mt,
        "OSL-2.1"@nl,
        "OSL-2.1"@pl,
        "OSL-2.1"@pt,
        "OSL-2.1"@ro,
        "OSL-2.1"@sk,
        "OSL-2.1"@sl,
        "OSL-2.1"@sv ;
    skos:changeNote "The source of the start-use date: https://lists.debian.org/debian-legal/2003/11/msg00181.html"@en ;
    skos:definition "Open Software License 2.1 is a copyleft-style, free software licence approved by the Open Source Initiative."@en ;
    skos:exactMatch <https://opensource.org/licenses/OSL-2.1> ;
    skos:inScheme atold:licence ;
    skos:prefLabel "The Open Software License, version 2.1 (OSL-2.1)"@en ;
    skos:topConceptOf atold:licence .

<http://publications.europa.eu/resource/authority/licence/OSL_3_0> a skos:Concept ;
    at:authority-code "OSL_3_0" ;
    at:deprecated "false" ;
    at:op-code "OSL_3_0" ;
    at:start.use "2005-12-01" ;
    atold:op-code "OSL_3_0" ;
    dc:identifier "OSL_3_0" ;
    skos:altLabel "OSL-3.0"@bg,
        "OSL-3.0"@cs,
        "OSL-3.0"@da,
        "OSL-3.0"@de,
        "OSL-3.0"@el,
        "OSL-3.0"@en,
        "OSL-3.0"@es,
        "OSL-3.0"@et,
        "OSL-3.0"@fi,
        "OSL-3.0"@fr,
        "OSL-3.0"@ga,
        "OSL-3.0"@hr,
        "OSL-3.0"@hu,
        "OSL-3.0"@it,
        "OSL-3.0"@lt,
        "OSL-3.0"@lv,
        "OSL-3.0"@mt,
        "OSL-3.0"@nl,
        "OSL-3.0"@pl,
        "OSL-3.0"@pt,
        "OSL-3.0"@ro,
        "OSL-3.0"@sk,
        "OSL-3.0"@sl,
        "OSL-3.0"@sv ;
    skos:changeNote "The source of the start-use date: http://rosenlaw.com/OSL3.0-explained.htm; https://lwn.net/Articles/147660/"@en ;
    skos:definition "Open Software License 3.0 is a copyleft-style, free software licence approved by the Open Source Initiative. Similar to the AGPL, the OSL requires the user to disclose the source code when communicating software."@en ;
    skos:exactMatch <https://opensource.org/licenses/OSL-3.0> ;
    skos:inScheme atold:licence ;
    skos:prefLabel "Open Software License, version 3.0 (OSL-3.0)"@en ;
    skos:topConceptOf atold:licence .

<http://publications.europa.eu/resource/authority/licence/PHP_3_0> a skos:Concept ;
    at:authority-code "PHP_3_0" ;
    at:deprecated "false" ;
    at:op-code "PHP_3_0" ;
    at:start.use "2002-07-21" ;
    atold:op-code "PHP_3_0" ;
    dc:identifier "PHP_3_0" ;
    skos:altLabel "PHP-3.0"@bg,
        "PHP-3.0"@cs,
        "PHP-3.0"@da,
        "PHP-3.0"@de,
        "PHP-3.0"@el,
        "PHP-3.0"@en,
        "PHP-3.0"@es,
        "PHP-3.0"@et,
        "PHP-3.0"@fi,
        "PHP-3.0"@fr,
        "PHP-3.0"@ga,
        "PHP-3.0"@hr,
        "PHP-3.0"@hu,
        "PHP-3.0"@it,
        "PHP-3.0"@lt,
        "PHP-3.0"@lv,
        "PHP-3.0"@mt,
        "PHP-3.0"@nl,
        "PHP-3.0"@pl,
        "PHP-3.0"@pt,
        "PHP-3.0"@ro,
        "PHP-3.0"@sk,
        "PHP-3.0"@sl,
        "PHP-3.0"@sv ;
    skos:changeNote "The source of the start-use date: http://lists.opensource.org/pipermail/license-review_lists.opensource.org/2020-March/004716.html"@en ;
    skos:definition "The PHP License 3.0 is a permissive free software licence approved by the Open Source Initiative. It has minimal, clear requirements, and explicitly bars the use of the PHP name to endorse the software."@en ;
    skos:exactMatch <https://opensource.org/licenses/PHP-3.0> ;
    skos:inScheme atold:licence ;
    skos:prefLabel "The PHP License 3.0 (PHP-3.0)"@en ;
    skos:topConceptOf atold:licence .

<http://publications.europa.eu/resource/authority/licence/POSTGRE_SQL> a skos:Concept ;
    at:authority-code "POSTGRE_SQL" ;
    at:deprecated "false" ;
    at:op-code "POSTGRE_SQL" ;
    at:start.use "1996-07-08" ;
    atold:op-code "POSTGRE_SQL" ;
    dc:identifier "POSTGRE_SQL" ;
    skos:altLabel "PostgreSQL"@bg,
        "PostgreSQL"@cs,
        "PostgreSQL"@da,
        "PostgreSQL"@de,
        "PostgreSQL"@el,
        "PostgreSQL"@en,
        "PostgreSQL"@es,
        "PostgreSQL"@et,
        "PostgreSQL"@fi,
        "PostgreSQL"@fr,
        "PostgreSQL"@ga,
        "PostgreSQL"@hr,
        "PostgreSQL"@hu,
        "PostgreSQL"@it,
        "PostgreSQL"@lt,
        "PostgreSQL"@lv,
        "PostgreSQL"@mt,
        "PostgreSQL"@nl,
        "PostgreSQL"@pl,
        "PostgreSQL"@pt,
        "PostgreSQL"@ro,
        "PostgreSQL"@sk,
        "PostgreSQL"@sl,
        "PostgreSQL"@sv ;
    skos:changeNote "The source of the start-use date: https://en.wikipedia.org/wiki/PostgreSQL"@en ;
    skos:definition "PostgreSQL is a BSD-style permissive free software licence approved by the Open Source Initiative."@en ;
    skos:exactMatch <https://opensource.org/licenses/PostgreSQL> ;
    skos:inScheme atold:licence ;
    skos:prefLabel "The PostgreSQL Licence (PostgreSQL)"@en ;
    skos:topConceptOf atold:licence .

<http://publications.europa.eu/resource/authority/licence/PSEUL> a skos:Concept ;
    at:authority-code "PSEUL" ;
    at:deprecated "false" ;
    at:op-code "PSEUL" ;
    at:start.use "2013-08-01" ;
    atold:op-code "PSEUL" ;
    dc:identifier "PSEUL" ;
    skos:altLabel "PSEUL"@bg,
        "PSEUL"@cs,
        "PSEUL"@da,
        "PSEUL"@de,
        "PSEUL"@el,
        "PSEUL"@en,
        "PSEUL"@es,
        "PSEUL"@et,
        "PSEUL"@fi,
        "PSEUL"@fr,
        "PSEUL"@ga,
        "PSEUL"@hr,
        "PSEUL"@hu,
        "PSEUL"@it,
        "PSEUL"@lt,
        "PSEUL"@lv,
        "PSEUL"@mt,
        "PSEUL"@nl,
        "PSEUL"@pl,
        "PSEUL"@pt,
        "PSEUL"@ro,
        "PSEUL"@sk,
        "PSEUL"@sl,
        "PSEUL"@sv ;
    skos:changeNote "The source of the start-use date: https://data.blog.gov.uk/2013/08/23/new-psma-end-user-licences-for-inspire/"@en ;
    skos:definition "The INSPIRE End User Licence (PSEUL) aims to enable the sharing of environmental spatial information amongst public sector organisations. Licenced data under PSEUL is limited to data created (derived) by the user using Ordnance Survey (OS) licenced data."@en ;
    skos:exactMatch <https://www.ordnancesurvey.co.uk/documents/licensing/inspire-end-user-licence.pdf> ;
    skos:inScheme atold:licence ;
    skos:prefLabel "INSPIRE End User Licence"@en ;
    skos:topConceptOf atold:licence .

<http://publications.europa.eu/resource/authority/licence/PYTHON_2_0> a skos:Concept ;
    at:authority-code "PYTHON_2_0" ;
    at:deprecated "false" ;
    at:op-code "PYTHON_2_0" ;
    at:start.use "2000-09-01" ;
    atold:op-code "PYTHON_2_0" ;
    dc:identifier "PYTHON_2_0" ;
    skos:altLabel "Python-2.0"@bg,
        "Python-2.0"@cs,
        "Python-2.0"@da,
        "Python-2.0"@de,
        "Python-2.0"@el,
        "Python-2.0"@en,
        "Python-2.0"@es,
        "Python-2.0"@et,
        "Python-2.0"@fi,
        "Python-2.0"@fr,
        "Python-2.0"@ga,
        "Python-2.0"@hr,
        "Python-2.0"@hu,
        "Python-2.0"@it,
        "Python-2.0"@lt,
        "Python-2.0"@lv,
        "Python-2.0"@mt,
        "Python-2.0"@nl,
        "Python-2.0"@pl,
        "Python-2.0"@pt,
        "Python-2.0"@ro,
        "Python-2.0"@sk,
        "Python-2.0"@sl,
        "Python-2.0"@sv ;
    skos:changeNote "The source of the start-use date: https://www.slideshare.net/kanchilug/python-quick-guide1; https://en.wikipedia.org/wiki/Python_License"@en ;
    skos:definition "Python 2.0 is a permissive free software licence approved by the Open Source Initiative."@en ;
    skos:exactMatch <https://opensource.org/licenses/Python-2.0> ;
    skos:inScheme atold:licence ;
    skos:prefLabel "Python License (Python-2.0)"@en ;
    skos:topConceptOf atold:licence .

<http://publications.europa.eu/resource/authority/licence/QPL_1_0> a skos:Concept ;
    at:authority-code "QPL_1_0" ;
    at:deprecated "false" ;
    at:op-code "QPL_1_0" ;
    at:start.use "1999-03-04" ;
    atold:op-code "QPL_1_0" ;
    dc:identifier "QPL_1_0" ;
    skos:altLabel "QPL-1.0"@bg,
        "QPL-1.0"@cs,
        "QPL-1.0"@da,
        "QPL-1.0"@de,
        "QPL-1.0"@el,
        "QPL-1.0"@en,
        "QPL-1.0"@es,
        "QPL-1.0"@et,
        "QPL-1.0"@fi,
        "QPL-1.0"@fr,
        "QPL-1.0"@ga,
        "QPL-1.0"@hr,
        "QPL-1.0"@hu,
        "QPL-1.0"@it,
        "QPL-1.0"@lt,
        "QPL-1.0"@lv,
        "QPL-1.0"@mt,
        "QPL-1.0"@nl,
        "QPL-1.0"@pl,
        "QPL-1.0"@pt,
        "QPL-1.0"@ro,
        "QPL-1.0"@sk,
        "QPL-1.0"@sl,
        "QPL-1.0"@sv ;
    skos:changeNote "The source of the start-use date: http://blog.hermit4.info/2013/01/qt-news-title.html"@en ;
    skos:definition "The Q Public License Version 1.0 is a copyleft-style, free software licence approved by the Open Source Initiative. It was designed by the Norwegian firm Trolltech to govern the distribution of its software, the Qt Toolkit."@en ;
    skos:exactMatch <https://opensource.org/licenses/QPL-1.0> ;
    skos:inScheme atold:licence ;
    skos:prefLabel "The Q Public License Version (QPL-1.0)"@en ;
    skos:topConceptOf atold:licence .

<http://publications.europa.eu/resource/authority/licence/RPL_1_1> a skos:Concept ;
    at:authority-code "RPL_1_1" ;
    at:deprecated "true" ;
    at:end.use "2007-07-14" ;
    at:op-code "RPL_1_1" ;
    at:start.use "2002-11-01" ;
    atold:op-code "RPL_1_1" ;
    dc:identifier "RPL_1_1" ;
    skos:altLabel "RPL-1.1"@bg,
        "RPL-1.1"@cs,
        "RPL-1.1"@da,
        "RPL-1.1"@de,
        "RPL-1.1"@el,
        "RPL-1.1"@en,
        "RPL-1.1"@es,
        "RPL-1.1"@et,
        "RPL-1.1"@fi,
        "RPL-1.1"@fr,
        "RPL-1.1"@ga,
        "RPL-1.1"@hr,
        "RPL-1.1"@hu,
        "RPL-1.1"@it,
        "RPL-1.1"@lt,
        "RPL-1.1"@lv,
        "RPL-1.1"@mt,
        "RPL-1.1"@nl,
        "RPL-1.1"@pl,
        "RPL-1.1"@pt,
        "RPL-1.1"@ro,
        "RPL-1.1"@sk,
        "RPL-1.1"@sl,
        "RPL-1.1"@sv ;
    skos:changeNote "The source of the start-use date: https://cc.com.au/files/acquisition_of_open-source_software_-_text.pdf"@en ;
    skos:definition "The Reciprocal Public License, version 1.1 is a copyleft-style, free software licence approved by the Open Source Initiative. It contains rules on redistribution."@en ;
    skos:exactMatch <https://opensource.org/licenses/RPL-1.1> ;
    skos:inScheme atold:licence ;
    skos:prefLabel "Reciprocal Public License, version 1.1"@en ;
    skos:topConceptOf atold:licence .

<http://publications.europa.eu/resource/authority/licence/RPL_1_5> a skos:Concept ;
    at:authority-code "RPL_1_5" ;
    at:deprecated "false" ;
    at:op-code "RPL_1_5" ;
    at:start.use "2007-07-15" ;
    atold:op-code "RPL_1_5" ;
    dc:identifier "RPL_1_5" ;
    skos:altLabel "RPL-1.5"@bg,
        "RPL-1.5"@cs,
        "RPL-1.5"@da,
        "RPL-1.5"@de,
        "RPL-1.5"@el,
        "RPL-1.5"@en,
        "RPL-1.5"@es,
        "RPL-1.5"@et,
        "RPL-1.5"@fi,
        "RPL-1.5"@fr,
        "RPL-1.5"@ga,
        "RPL-1.5"@hr,
        "RPL-1.5"@hu,
        "RPL-1.5"@it,
        "RPL-1.5"@lt,
        "RPL-1.5"@lv,
        "RPL-1.5"@mt,
        "RPL-1.5"@nl,
        "RPL-1.5"@pl,
        "RPL-1.5"@pt,
        "RPL-1.5"@ro,
        "RPL-1.5"@sk,
        "RPL-1.5"@sl,
        "RPL-1.5"@sv ;
    skos:changeNote "The source of the start-use date: https://spdx.org/licenses/RPL-1.5.html"@en ;
    skos:definition "The Reciprocal Public License 1.5 is a copyleft-style, free software licence approved by the Open Source Initiative with detailed liability protection and numerous requirements, created to close a loophole in the GPL which let users sell modified software without ”fairly” distributing it."@en ;
    skos:exactMatch <https://opensource.org/licenses/RPL-1.5> ;
    skos:inScheme atold:licence ;
    skos:prefLabel "Reciprocal Public License 1.5 (RPL-1.5)"@en ;
    skos:topConceptOf atold:licence .

<http://publications.europa.eu/resource/authority/licence/RPSL_1_0> a skos:Concept ;
    at:authority-code "RPSL_1_0" ;
    at:deprecated "false" ;
    at:op-code "RPSL_1_0" ;
    at:start.use "2002-10-28" ;
    atold:op-code "RPSL_1_0" ;
    dc:identifier "RPSL_1_0" ;
    skos:altLabel "RPSL-1.0"@bg,
        "RPSL-1.0"@cs,
        "RPSL-1.0"@da,
        "RPSL-1.0"@de,
        "RPSL-1.0"@el,
        "RPSL-1.0"@en,
        "RPSL-1.0"@es,
        "RPSL-1.0"@et,
        "RPSL-1.0"@fi,
        "RPSL-1.0"@fr,
        "RPSL-1.0"@ga,
        "RPSL-1.0"@hr,
        "RPSL-1.0"@hu,
        "RPSL-1.0"@it,
        "RPSL-1.0"@lt,
        "RPSL-1.0"@lv,
        "RPSL-1.0"@mt,
        "RPSL-1.0"@nl,
        "RPSL-1.0"@pl,
        "RPSL-1.0"@pt,
        "RPSL-1.0"@ro,
        "RPSL-1.0"@sk,
        "RPSL-1.0"@sl,
        "RPSL-1.0"@sv ;
    skos:changeNote "The source of the start-use date: https://spdx.org/licenses/RPSL-1.0.html"@en ;
    skos:definition "Published by RealNetworks, RPSL-1.0 is a copyleft-style, free software licence approved by the Open Source Initiative."@en ;
    skos:exactMatch <https://opensource.org/licenses/RPSL-1.0> ;
    skos:inScheme atold:licence ;
    skos:prefLabel "RealNetworks Public Source License Version 1.0 (RPSL-1.0)"@en ;
    skos:topConceptOf atold:licence .

<http://publications.europa.eu/resource/authority/licence/RSCPL> a skos:Concept ;
    at:authority-code "RSCPL" ;
    at:deprecated "false" ;
    at:op-code "RSCPL" ;
    at:start.use "1995-12-01" ;
    atold:op-code "RSCPL" ;
    dc:identifier "RSCPL" ;
    skos:altLabel "RSCPL"@bg,
        "RSCPL"@cs,
        "RSCPL"@da,
        "RSCPL"@de,
        "RSCPL"@el,
        "RSCPL"@en,
        "RSCPL"@es,
        "RSCPL"@et,
        "RSCPL"@fi,
        "RSCPL"@fr,
        "RSCPL"@ga,
        "RSCPL"@hr,
        "RSCPL"@hu,
        "RSCPL"@it,
        "RSCPL"@lt,
        "RSCPL"@lv,
        "RSCPL"@mt,
        "RSCPL"@nl,
        "RSCPL"@pl,
        "RSCPL"@pt,
        "RSCPL"@ro,
        "RSCPL"@sk,
        "RSCPL"@sl,
        "RSCPL"@sv ;
    skos:changeNote "The source of the start-use date: http://ploug22.free.fr/doc/oss-market-structure-urope.pdf; https://spdx.org/licenses/RSCPL.html"@en ;
    skos:definition "The Ricoh Source Code Public License (RSCPL) is a copyleft-style, free software licence approved by the Open Source Initiative with much built-in protection for the author."@en ;
    skos:exactMatch <https://opensource.org/licenses/RSCPL> ;
    skos:inScheme atold:licence ;
    skos:prefLabel "The Ricoh Source Code Public License (RSCPL)"@en ;
    skos:topConceptOf atold:licence .

<http://publications.europa.eu/resource/authority/licence/SIMPL_2_0> a skos:Concept ;
    at:authority-code "SIMPL_2_0" ;
    at:deprecated "false" ;
    at:op-code "SIMPL_2_0" ;
    at:start.use "2007-11-01" ;
    atold:op-code "SIMPL_2_0" ;
    dc:identifier "SIMPL_2_0" ;
    skos:altLabel "SimPL-2.0"@bg,
        "SimPL-2.0"@cs,
        "SimPL-2.0"@da,
        "SimPL-2.0"@de,
        "SimPL-2.0"@el,
        "SimPL-2.0"@en,
        "SimPL-2.0"@es,
        "SimPL-2.0"@et,
        "SimPL-2.0"@fi,
        "SimPL-2.0"@fr,
        "SimPL-2.0"@ga,
        "SimPL-2.0"@hr,
        "SimPL-2.0"@hu,
        "SimPL-2.0"@it,
        "SimPL-2.0"@lt,
        "SimPL-2.0"@lv,
        "SimPL-2.0"@mt,
        "SimPL-2.0"@nl,
        "SimPL-2.0"@pl,
        "SimPL-2.0"@pt,
        "SimPL-2.0"@ro,
        "SimPL-2.0"@sk,
        "SimPL-2.0"@sl,
        "SimPL-2.0"@sv ;
    skos:changeNote "The source of the start-use date: https://opensource.org/node/228"@en ;
    skos:definition "Simple Public License 2.0 is a copyleft-style, free software licence approved by the Open Source Initiative."@en ;
    skos:exactMatch <https://opensource.org/licenses/SimPL-2.0> ;
    skos:inScheme atold:licence ;
    skos:prefLabel "Simple Public License (SimPL-2.0)"@en ;
    skos:topConceptOf atold:licence .

<http://publications.europa.eu/resource/authority/licence/SLEEPYCAT> a skos:Concept ;
    at:authority-code "SLEEPYCAT" ;
    at:deprecated "false" ;
    at:op-code "SLEEPYCAT" ;
    at:start.use "1990-01-01" ;
    atold:op-code "SLEEPYCAT" ;
    dc:identifier "SLEEPYCAT" ;
    skos:altLabel "Sleepycat"@bg,
        "Sleepycat"@cs,
        "Sleepycat"@da,
        "Sleepycat"@de,
        "Sleepycat"@el,
        "Sleepycat"@en,
        "Sleepycat"@es,
        "Sleepycat"@et,
        "Sleepycat"@fi,
        "Sleepycat"@fr,
        "Sleepycat"@ga,
        "Sleepycat"@hr,
        "Sleepycat"@hu,
        "Sleepycat"@it,
        "Sleepycat"@lt,
        "Sleepycat"@lv,
        "Sleepycat"@mt,
        "Sleepycat"@nl,
        "Sleepycat"@pl,
        "Sleepycat"@pt,
        "Sleepycat"@ro,
        "Sleepycat"@sk,
        "Sleepycat"@sl,
        "Sleepycat"@sv ;
    skos:changeNote "The source of the start-use date: https://en.wikipedia.org/wiki/Talk%3ASleepycat_License"@en ;
    skos:definition "The Sleepycat License is a BSD plus-style, permissive free software licence approved by the Open Source Initiative."@en ;
    skos:exactMatch <https://opensource.org/licenses/Sleepycat> ;
    skos:inScheme atold:licence ;
    skos:prefLabel "The Sleepycat License (Sleepycat)"@en ;
    skos:topConceptOf atold:licence .

<http://publications.europa.eu/resource/authority/licence/SPL_1_0> a skos:Concept ;
    at:authority-code "SPL_1_0" ;
    at:deprecated "false" ;
    at:op-code "SPL_1_0" ;
    at:start.use "1995-01-01" ;
    atold:op-code "SPL_1_0" ;
    dc:identifier "SPL_1_0" ;
    skos:altLabel "SPL-1.0"@bg,
        "SPL-1.0"@cs,
        "SPL-1.0"@da,
        "SPL-1.0"@de,
        "SPL-1.0"@el,
        "SPL-1.0"@en,
        "SPL-1.0"@es,
        "SPL-1.0"@et,
        "SPL-1.0"@fi,
        "SPL-1.0"@fr,
        "SPL-1.0"@ga,
        "SPL-1.0"@hr,
        "SPL-1.0"@hu,
        "SPL-1.0"@it,
        "SPL-1.0"@lt,
        "SPL-1.0"@lv,
        "SPL-1.0"@mt,
        "SPL-1.0"@nl,
        "SPL-1.0"@pl,
        "SPL-1.0"@pt,
        "SPL-1.0"@ro,
        "SPL-1.0"@sk,
        "SPL-1.0"@sl,
        "SPL-1.0"@sv ;
    skos:changeNote "The source of the start-use date: https://enterprise.dejacode.com/licenses/public/spl-1.0/?_list_filters=q%3DSun%2BPublic%2BLicense"@en ;
    skos:definition "Sun Public License 1.0 is a copyleft-style, free software licence approved by the Open Source Initiative."@en ;
    skos:exactMatch <https://opensource.org/licenses/SPL-1.0> ;
    skos:inScheme atold:licence ;
    skos:prefLabel "Sun Public License Version 1.0 (SPL-1.0)"@en ;
    skos:topConceptOf atold:licence .

<http://publications.europa.eu/resource/authority/licence/UCL_1_0> a skos:Concept ;
    at:authority-code "UCL_1_0" ;
    at:deprecated "false" ;
    at:op-code "UCL_1_0" ;
    at:start.use "2017-02-01" ;
    atold:op-code "UCL_1_0" ;
    dc:identifier "UCL_1_0" ;
    skos:altLabel "UCL-1.0"@bg,
        "UCL-1.0"@cs,
        "UCL-1.0"@da,
        "UCL-1.0"@de,
        "UCL-1.0"@el,
        "UCL-1.0"@en,
        "UCL-1.0"@es,
        "UCL-1.0"@et,
        "UCL-1.0"@fi,
        "UCL-1.0"@fr,
        "UCL-1.0"@ga,
        "UCL-1.0"@hr,
        "UCL-1.0"@hu,
        "UCL-1.0"@it,
        "UCL-1.0"@lt,
        "UCL-1.0"@lv,
        "UCL-1.0"@mt,
        "UCL-1.0"@nl,
        "UCL-1.0"@pl,
        "UCL-1.0"@pt,
        "UCL-1.0"@ro,
        "UCL-1.0"@sk,
        "UCL-1.0"@sl,
        "UCL-1.0"@sv ;
    skos:changeNote "The source of the start-use date: http://lists.opensource.org/pipermail/license-review_lists.opensource.org/2017-February/002983.html"@en ;
    skos:definition "Upstream Compatibility License v1.0 is a copyleft-style, free software licence approved by the Open Source Initiative."@en ;
    skos:exactMatch <https://opensource.org/licenses/UCL-1.0> ;
    skos:inScheme atold:licence ;
    skos:prefLabel "Upstream Compatibility License v1.0"@en ;
    skos:topConceptOf atold:licence .

<http://publications.europa.eu/resource/authority/licence/UPL_1_0> a skos:Concept ;
    at:authority-code "UPL_1_0" ;
    at:deprecated "false" ;
    at:op-code "UPL_1_0" ;
    at:start.use "2015-02-01" ;
    atold:op-code "UPL_1_0" ;
    dc:identifier "UPL_1_0" ;
    skos:altLabel "UPL"@bg,
        "UPL"@cs,
        "UPL"@da,
        "UPL"@de,
        "UPL"@el,
        "UPL"@en,
        "UPL"@es,
        "UPL"@et,
        "UPL"@fi,
        "UPL"@fr,
        "UPL"@ga,
        "UPL"@hr,
        "UPL"@hu,
        "UPL"@it,
        "UPL"@lt,
        "UPL"@lv,
        "UPL"@mt,
        "UPL"@nl,
        "UPL"@pl,
        "UPL"@pt,
        "UPL"@ro,
        "UPL"@sk,
        "UPL"@sl,
        "UPL"@sv ;
    skos:changeNote "The source of the start-use date: https://oss.oracle.com/licenses/upl/"@en ;
    skos:definition "The Universal Permissive License 1.0 is an attribution+patent-style, permissive free software licence issued by Oracle and approved by the Open Source Initiative."@en ;
    skos:exactMatch <https://opensource.org/licenses/UPL> ;
    skos:inScheme atold:licence ;
    skos:prefLabel "The Universal Permissive License (UPL), Version 1.0"@en ;
    skos:topConceptOf atold:licence .

<http://publications.europa.eu/resource/authority/licence/VSL_1_0> a skos:Concept ;
    at:authority-code "VSL_1_0" ;
    at:deprecated "false" ;
    at:op-code "VSL_1_0" ;
    at:start.use "2000-01-01" ;
    atold:op-code "VSL_1_0" ;
    dc:identifier "VSL_1_0" ;
    skos:altLabel "VSL-1.0"@bg,
        "VSL-1.0"@cs,
        "VSL-1.0"@da,
        "VSL-1.0"@de,
        "VSL-1.0"@el,
        "VSL-1.0"@en,
        "VSL-1.0"@es,
        "VSL-1.0"@et,
        "VSL-1.0"@fi,
        "VSL-1.0"@fr,
        "VSL-1.0"@ga,
        "VSL-1.0"@hr,
        "VSL-1.0"@hu,
        "VSL-1.0"@it,
        "VSL-1.0"@lt,
        "VSL-1.0"@lv,
        "VSL-1.0"@mt,
        "VSL-1.0"@nl,
        "VSL-1.0"@pl,
        "VSL-1.0"@pt,
        "VSL-1.0"@ro,
        "VSL-1.0"@sk,
        "VSL-1.0"@sl,
        "VSL-1.0"@sv ;
    skos:changeNote "The source of the start-use date: https://spdx.org/licenses/VSL-1.0.html#licenseText"@en ;
    skos:definition "The Vovida Software License v. 1.0 is a BSD plus-style, permissive free software licence approved by the Open Source Initiative."@en ;
    skos:exactMatch <https://opensource.org/licenses/VSL-1.0> ;
    skos:inScheme atold:licence ;
    skos:prefLabel "The Vovida Software License v. 1.0 (VSL-1.0)"@en ;
    skos:topConceptOf atold:licence .

<http://publications.europa.eu/resource/authority/licence/W3C> a skos:Concept ;
    at:authority-code "W3C" ;
    at:deprecated "false" ;
    at:op-code "W3C" ;
    at:start.use "2002-12-31" ;
    atold:op-code "W3C" ;
    dc:identifier "W3C" ;
    skos:altLabel "W3C"@bg,
        "W3C"@cs,
        "W3C"@da,
        "W3C"@de,
        "W3C"@el,
        "W3C"@en,
        "W3C"@es,
        "W3C"@et,
        "W3C"@fi,
        "W3C"@fr,
        "W3C"@ga,
        "W3C"@hr,
        "W3C"@hu,
        "W3C"@it,
        "W3C"@lt,
        "W3C"@lv,
        "W3C"@mt,
        "W3C"@nl,
        "W3C"@pl,
        "W3C"@pt,
        "W3C"@ro,
        "W3C"@sk,
        "W3C"@sl,
        "W3C"@sv ;
    skos:changeNote "The source of the start-use date: https://en.wikipedia.org/wiki/W3C_Software_Notice_and_License"@en ;
    skos:definition "The W3C Software Notice and License is a permissive free software licence used by software released by the World Wide Web Consortium. It is a permissive licence, compatible with the GNU General Public License and approved by the Open Source Initiative."@en ;
    skos:exactMatch <https://opensource.org/licenses/W3C> ;
    skos:inScheme atold:licence ;
    skos:prefLabel "The W3C Software Notice and License (W3C)"@en ;
    skos:topConceptOf atold:licence .

<http://publications.europa.eu/resource/authority/licence/WATCOM_1_0> a skos:Concept ;
    at:authority-code "WATCOM_1_0" ;
    at:deprecated "false" ;
    at:op-code "WATCOM_1_0" ;
    at:start.use "2002-05-19" ;
    atold:op-code "WATCOM_1_0" ;
    dc:identifier "WATCOM_1_0" ;
    skos:altLabel "Watcom-1.0"@bg,
        "Watcom-1.0"@cs,
        "Watcom-1.0"@da,
        "Watcom-1.0"@de,
        "Watcom-1.0"@el,
        "Watcom-1.0"@en,
        "Watcom-1.0"@es,
        "Watcom-1.0"@et,
        "Watcom-1.0"@fi,
        "Watcom-1.0"@fr,
        "Watcom-1.0"@ga,
        "Watcom-1.0"@hr,
        "Watcom-1.0"@hu,
        "Watcom-1.0"@it,
        "Watcom-1.0"@lt,
        "Watcom-1.0"@lv,
        "Watcom-1.0"@mt,
        "Watcom-1.0"@nl,
        "Watcom-1.0"@pl,
        "Watcom-1.0"@pt,
        "Watcom-1.0"@ro,
        "Watcom-1.0"@sk,
        "Watcom-1.0"@sl,
        "Watcom-1.0"@sv ;
    skos:changeNote "The source of the start-use date: http://howlingmad.gmxhome.de/watcom_new_en.html"@en ;
    skos:definition "Watcom-1.0 is a proprietary+patent-style, strong copyleft software licence approved by the Open Source Initiative."@en ;
    skos:exactMatch <https://opensource.org/licenses/Watcom-1.0> ;
    skos:inScheme atold:licence ;
    skos:prefLabel "The Sybase Open Source Licence (Watcom-1.0)"@en ;
    skos:topConceptOf atold:licence .

<http://publications.europa.eu/resource/authority/licence/WXWINDOWS> a skos:Concept ;
    at:authority-code "WXWINDOWS" ;
    at:deprecated "true" ;
    at:end.use "2007-06-28" ;
    at:op-code "WXWINDOWS" ;
    at:start.use "1998-07-01" ;
    atold:op-code "WXWINDOWS" ;
    dc:identifier "WXWINDOWS" ;
    skos:altLabel "wxWindows"@bg,
        "wxWindows"@cs,
        "wxWindows"@da,
        "wxWindows"@de,
        "wxWindows"@el,
        "wxWindows"@en,
        "wxWindows"@es,
        "wxWindows"@et,
        "wxWindows"@fi,
        "wxWindows"@fr,
        "wxWindows"@ga,
        "wxWindows"@hr,
        "wxWindows"@hu,
        "wxWindows"@it,
        "wxWindows"@lt,
        "wxWindows"@lv,
        "wxWindows"@mt,
        "wxWindows"@nl,
        "wxWindows"@pl,
        "wxWindows"@pt,
        "wxWindows"@ro,
        "wxWindows"@sk,
        "wxWindows"@sl,
        "wxWindows"@sv ;
    skos:changeNote "The source of the start-use date: https://opensource.org/licenses/WXwindows"@en ;
    skos:definition "Approved by the Open Source Initiative, wxWindows is a copyleft-style, free software licence created for wxWidgets."@en ;
    skos:exactMatch <https://opensource.org/licenses/WXwindows> ;
    skos:inScheme atold:licence ;
    skos:prefLabel "The wxWindows Library Licence (wxWindows)"@en ;
    skos:topConceptOf atold:licence .

<http://publications.europa.eu/resource/authority/licence/XNET> a skos:Concept ;
    at:authority-code "XNET" ;
    at:deprecated "true" ;
    at:end.use "2020-01-01" ;
    at:op-code "XNET" ;
    at:start.use "2000-07-01" ;
    atold:op-code "XNET" ;
    dc:identifier "XNET" ;
    skos:altLabel "Xnet"@bg,
        "Xnet"@cs,
        "Xnet"@da,
        "Xnet"@de,
        "Xnet"@el,
        "Xnet"@en,
        "Xnet"@es,
        "Xnet"@et,
        "Xnet"@fi,
        "Xnet"@fr,
        "Xnet"@ga,
        "Xnet"@hr,
        "Xnet"@hu,
        "Xnet"@it,
        "Xnet"@lt,
        "Xnet"@lv,
        "Xnet"@mt,
        "Xnet"@nl,
        "Xnet"@pl,
        "Xnet"@pt,
        "Xnet"@ro,
        "Xnet"@sk,
        "Xnet"@sl,
        "Xnet"@sv ;
    skos:changeNote "The source of the start-use date: https://opensource.org/licenses/Xnet"@en ;
    skos:definition "Xnet is a MIT-style, permissive free software licence approved by the Open Source Initiative."@en ;
    skos:exactMatch <https://opensource.org/licenses/Xnet> ;
    skos:inScheme atold:licence ;
    skos:prefLabel "The X.Net, Inc. License (Xnet)"@en ;
    skos:topConceptOf atold:licence .

<http://publications.europa.eu/resource/authority/licence/ZLIB> a skos:Concept ;
    at:authority-code "ZLIB" ;
    at:deprecated "false" ;
    at:op-code "ZLIB" ;
    at:start.use "1995-05-01" ;
    atold:op-code "ZLIB" ;
    dc:identifier "ZLIB" ;
    skos:altLabel "Zlib"@bg,
        "Zlib"@cs,
        "Zlib"@da,
        "Zlib"@de,
        "Zlib"@el,
        "Zlib"@en,
        "Zlib"@es,
        "Zlib"@et,
        "Zlib"@fi,
        "Zlib"@fr,
        "Zlib"@ga,
        "Zlib"@hr,
        "Zlib"@hu,
        "Zlib"@it,
        "Zlib"@lt,
        "Zlib"@lv,
        "Zlib"@mt,
        "Zlib"@nl,
        "Zlib"@pl,
        "Zlib"@pt,
        "Zlib"@ro,
        "Zlib"@sk,
        "Zlib"@sl,
        "Zlib"@sv ;
    skos:changeNote "The source of the start-use date: https://en.wikipedia.org/wiki/Zlib"@en ;
    skos:definition "Zlib is designed to be a free, general-purpose, legally unencumbered – not covered by any patents – lossless data-compression library for use on virtually any computer hardware and operating system. It is approved by the Open Source Initiative."@en ;
    skos:exactMatch <https://opensource.org/licenses/Zlib> ;
    skos:inScheme atold:licence ;
    skos:prefLabel "The zlib/libpng License (Zlib)"@en ;
    skos:topConceptOf atold:licence .

<http://publications.europa.eu/resource/authority/licence/ZPL_2_0> a skos:Concept ;
    at:authority-code "ZPL_2_0" ;
    at:deprecated "false" ;
    at:op-code "ZPL_2_0" ;
    at:start.use "2002-02-01" ;
    atold:op-code "ZPL_2_0" ;
    dc:identifier "ZPL_2_0" ;
    skos:altLabel "ZPL-2.0"@bg,
        "ZPL-2.0"@cs,
        "ZPL-2.0"@da,
        "ZPL-2.0"@de,
        "ZPL-2.0"@el,
        "ZPL-2.0"@en,
        "ZPL-2.0"@es,
        "ZPL-2.0"@et,
        "ZPL-2.0"@fi,
        "ZPL-2.0"@fr,
        "ZPL-2.0"@ga,
        "ZPL-2.0"@hr,
        "ZPL-2.0"@hu,
        "ZPL-2.0"@it,
        "ZPL-2.0"@lt,
        "ZPL-2.0"@lv,
        "ZPL-2.0"@mt,
        "ZPL-2.0"@nl,
        "ZPL-2.0"@pl,
        "ZPL-2.0"@pt,
        "ZPL-2.0"@ro,
        "ZPL-2.0"@sk,
        "ZPL-2.0"@sl,
        "ZPL-2.0"@sv ;
    skos:changeNote "The source of the start-use date: Open Source Software: From Open Science to New Marketing Model, p. 116"@en ;
    skos:definition "The Zope Public License Version 2.0 is a free software licence approved by the Open Source Initiative, used primarily for the Zope application server software. It is similar to the well-known BSD license, however the ZPL also adds clauses prohibiting trademark use and requiring documentation of all changes."@en ;
    skos:exactMatch <https://opensource.org/licenses/ZPL-2.0> ;
    skos:inScheme atold:licence ;
    skos:prefLabel "The Zope Public License Version 2.0 (ZPL-2.0)"@en ;
    skos:topConceptOf atold:licence .

atold:licence a skos:ConceptScheme ;
    rdfs:label "Licence"@en ;
    at:prefLabel "Licence"@en ;
    at:table.id "licence" ;
    at:table.version.number "20220928-0" ;
    owl:versionInfo "20220928-0" ;
    skos:prefLabel "Licence"@en .

