<?xml version="1.0" encoding="UTF-8"?>
<rdf:RDF xmlns:rdf="http://www.w3.org/1999/02/22-rdf-syntax-ns#"
         xmlns:at="http://publications.europa.eu/ontology/authority/"
         xmlns:rdfs="http://www.w3.org/2000/01/rdf-schema#"
         xmlns:owl="http://www.w3.org/2002/07/owl#"
         xmlns:skos="http://www.w3.org/2004/02/skos/core#"
         xmlns:atold="http://publications.europa.eu/resource/authority/"
         xmlns:dc="http://purl.org/dc/elements/1.1/"
         xml:base="http://publications.europa.eu/resource/authority/public-event-type">
   <skos:ConceptScheme rdf:about="http://publications.europa.eu/resource/authority/public-event-type"
                       at:table.id="public-event-type"
                       at:table.version.number="20220615-0">
      <at:prefLabel xml:lang="en">Public event type</at:prefLabel>
      <rdfs:label xml:lang="en">Public event type</rdfs:label>
      <owl:versionInfo>20220615-0</owl:versionInfo>
      <skos:prefLabel xml:lang="en">Public event type</skos:prefLabel>
   </skos:ConceptScheme>
   <skos:Concept rdf:about="http://publications.europa.eu/resource/authority/public-event-type/CAMP_LAUNCH"
                 at:deprecated="false">
      <skos:prefLabel xml:lang="bg">Стартиране на кампании</skos:prefLabel>
      <skos:prefLabel xml:lang="cs">Zahájení kampaně</skos:prefLabel>
      <skos:prefLabel xml:lang="da">Kampagnestart</skos:prefLabel>
      <skos:prefLabel xml:lang="de">Kampagnendebüts</skos:prefLabel>
      <skos:prefLabel xml:lang="el">Έναρξη εκστρατειών</skos:prefLabel>
      <skos:prefLabel xml:lang="en">Campaign launches</skos:prefLabel>
      <skos:prefLabel xml:lang="es">Lanzamiento de la campaña</skos:prefLabel>
      <skos:prefLabel xml:lang="et">Kampaania avaüritused</skos:prefLabel>
      <skos:prefLabel xml:lang="fi">Kampanja-avajaiset</skos:prefLabel>
      <skos:prefLabel xml:lang="fr">Lancements de campagnes</skos:prefLabel>
      <skos:prefLabel xml:lang="ga">Seoltaí feachtas</skos:prefLabel>
      <skos:prefLabel xml:lang="hr">Pokretanje kampanje</skos:prefLabel>
      <skos:prefLabel xml:lang="hu">Kampányindító rendezvények</skos:prefLabel>
      <skos:prefLabel xml:lang="it">Lancio di una campagna</skos:prefLabel>
      <skos:prefLabel xml:lang="lt">Kampanijos pradžios renginiai</skos:prefLabel>
      <skos:prefLabel xml:lang="lv">Kampaņas uzsākšana</skos:prefLabel>
      <skos:prefLabel xml:lang="mt">Tnedija ta’ kampanja</skos:prefLabel>
      <skos:prefLabel xml:lang="nl">Campagnestartevenementen</skos:prefLabel>
      <skos:prefLabel xml:lang="pl">Inauguracje kampanii</skos:prefLabel>
      <skos:prefLabel xml:lang="pt">Lançamento da campanha</skos:prefLabel>
      <skos:prefLabel xml:lang="ro">Lansarea unei campanii</skos:prefLabel>
      <skos:prefLabel xml:lang="sk">Kampaň sa začína</skos:prefLabel>
      <skos:prefLabel xml:lang="sl">Začetek kampanje</skos:prefLabel>
      <skos:prefLabel xml:lang="sv">Kampanjlanseringar</skos:prefLabel>
      <at:authority-code>CAMP_LAUNCH</at:authority-code>
      <at:op-code>CAMP_LAUNCH</at:op-code>
      <at:start.use>2020-11-01</at:start.use>
      <atold:op-code>CAMP_LAUNCH</atold:op-code>
      <dc:identifier>CAMP_LAUNCH</dc:identifier>
      <skos:definition xml:lang="en">Campaign launches include events with the objective of highlighting the launch of public awareness campaigns, policies and other types of initiatives.</skos:definition>
      <skos:inScheme rdf:resource="http://publications.europa.eu/resource/authority/public-event-type"/>
      <skos:topConceptOf rdf:resource="http://publications.europa.eu/resource/authority/public-event-type"/>
   </skos:Concept>
   <skos:Concept rdf:about="http://publications.europa.eu/resource/authority/public-event-type/COMPETITION_AWARD_CEREMONY"
                 at:deprecated="false">
      <skos:prefLabel xml:lang="bg">Конкурси и церемонии по награждаване</skos:prefLabel>
      <skos:prefLabel xml:lang="cs">Soutěže a slavnostní udílení cen</skos:prefLabel>
      <skos:prefLabel xml:lang="da">Konkurrencer og prisuddelinger</skos:prefLabel>
      <skos:prefLabel xml:lang="de">Wettbewerbe und Preisverleihungen</skos:prefLabel>
      <skos:prefLabel xml:lang="el">Διαγωνισμοί και τελετές απονομής βραβείων</skos:prefLabel>
      <skos:prefLabel xml:lang="en">Competitions and award ceremonies</skos:prefLabel>
      <skos:prefLabel xml:lang="es">Concursos y ceremonias de entrega de premios</skos:prefLabel>
      <skos:prefLabel xml:lang="et">Konkursid ja auhinnatseremooniad</skos:prefLabel>
      <skos:prefLabel xml:lang="fi">Kilpailut ja palkintoseremoniat</skos:prefLabel>
      <skos:prefLabel xml:lang="fr">Concours et cérémonies de remise de prix</skos:prefLabel>
      <skos:prefLabel xml:lang="ga">Comórtais agus searmanais bhronnta</skos:prefLabel>
      <skos:prefLabel xml:lang="hr">Natjecanja i svečanosti dodjele nagrada</skos:prefLabel>
      <skos:prefLabel xml:lang="hu">Versenyek és díjátadó ünnepségek</skos:prefLabel>
      <skos:prefLabel xml:lang="it">Concorsi e cerimonie di premiazione</skos:prefLabel>
      <skos:prefLabel xml:lang="lt">Konkursai ir apdovanojimų iškilmės</skos:prefLabel>
      <skos:prefLabel xml:lang="lv">Konkursi un apbalvošanas ceremonijas</skos:prefLabel>
      <skos:prefLabel xml:lang="mt">Kompetizzjonijiet u ċerimonji ta’ premjazzjoni</skos:prefLabel>
      <skos:prefLabel xml:lang="nl">Wedstrijden en prijsuitreikingen</skos:prefLabel>
      <skos:prefLabel xml:lang="pl">Konkursy i ceremonie wręczenia nagród</skos:prefLabel>
      <skos:prefLabel xml:lang="pt">Concursos e cerimónias de entrega de prémios</skos:prefLabel>
      <skos:prefLabel xml:lang="ro">Concursuri și ceremonii de decernare a premiilor</skos:prefLabel>
      <skos:prefLabel xml:lang="sk">Súťaže a slávnostné odovzdávanie cien</skos:prefLabel>
      <skos:prefLabel xml:lang="sl">Natečaji in podelitve nagrad</skos:prefLabel>
      <skos:prefLabel xml:lang="sv">Tävlingar och prisutdelningar</skos:prefLabel>
      <at:authority-code>COMPETITION_AWARD_CEREMONY</at:authority-code>
      <at:op-code>COMPETITION_AWARD_CEREMONY</at:op-code>
      <at:start.use>1958-01-01</at:start.use>
      <atold:op-code>COMPETITION_AWARD_CEREMONY</atold:op-code>
      <dc:identifier>COMPETITION_AWARD_CEREMONY</dc:identifier>
      <skos:definition xml:lang="en">Competitions and award ceremonies include public events such as award ceremonies, competitions and contests.</skos:definition>
      <skos:inScheme rdf:resource="http://publications.europa.eu/resource/authority/public-event-type"/>
      <skos:topConceptOf rdf:resource="http://publications.europa.eu/resource/authority/public-event-type"/>
   </skos:Concept>
   <skos:Concept rdf:about="http://publications.europa.eu/resource/authority/public-event-type/CONFERENCE_SUMMIT"
                 at:deprecated="false">
      <skos:prefLabel xml:lang="bg">Конференции и срещи на високо равнище</skos:prefLabel>
      <skos:prefLabel xml:lang="cs">Konference a summity</skos:prefLabel>
      <skos:prefLabel xml:lang="da">Konferencer og topmøder</skos:prefLabel>
      <skos:prefLabel xml:lang="de">Konferenzen und Gipfeltreffen</skos:prefLabel>
      <skos:prefLabel xml:lang="el">Διασκέψεις και σύνοδοι κορυφής</skos:prefLabel>
      <skos:prefLabel xml:lang="en">Conferences and summits</skos:prefLabel>
      <skos:prefLabel xml:lang="es">Conferencias y cumbres</skos:prefLabel>
      <skos:prefLabel xml:lang="et">Konverentsid ja tippkohtumised</skos:prefLabel>
      <skos:prefLabel xml:lang="fi">Konferenssit ja huippukokoukset</skos:prefLabel>
      <skos:prefLabel xml:lang="fr">Conférences et sommets</skos:prefLabel>
      <skos:prefLabel xml:lang="ga">Comhdhálacha agus cruinnithe mullaigh</skos:prefLabel>
      <skos:prefLabel xml:lang="hr">Konferencije i sastanci na vrhu</skos:prefLabel>
      <skos:prefLabel xml:lang="hu">Konferenciák és csúcstalálkozók</skos:prefLabel>
      <skos:prefLabel xml:lang="it">Conferenze e vertici</skos:prefLabel>
      <skos:prefLabel xml:lang="lt">Konferencijos ir aukščiausiojo lygio susitikimai</skos:prefLabel>
      <skos:prefLabel xml:lang="lv">Konferences un samiti</skos:prefLabel>
      <skos:prefLabel xml:lang="mt">Konferenzi u summits</skos:prefLabel>
      <skos:prefLabel xml:lang="nl">Conferenties en topontmoetingen</skos:prefLabel>
      <skos:prefLabel xml:lang="pl">Konferencje i szczyty</skos:prefLabel>
      <skos:prefLabel xml:lang="pt">Conferências e cimeiras</skos:prefLabel>
      <skos:prefLabel xml:lang="ro">Conferințe și reuniuni la nivel înalt</skos:prefLabel>
      <skos:prefLabel xml:lang="sk">Konferencie a samity</skos:prefLabel>
      <skos:prefLabel xml:lang="sl">Konference in srečanja na vrhu</skos:prefLabel>
      <skos:prefLabel xml:lang="sv">Konferenser och toppmöten</skos:prefLabel>
      <at:authority-code>CONFERENCE_SUMMIT</at:authority-code>
      <at:op-code>CONFERENCE_SUMMIT</at:op-code>
      <at:start.use>1958-01-01</at:start.use>
      <atold:op-code>CONFERENCE_SUMMIT</atold:op-code>
      <dc:identifier>CONFERENCE_SUMMIT</dc:identifier>
      <skos:definition xml:lang="en">Conferences and summits include public events such as conferences, summits, congresses and colloquiums.</skos:definition>
      <skos:inScheme rdf:resource="http://publications.europa.eu/resource/authority/public-event-type"/>
      <skos:topConceptOf rdf:resource="http://publications.europa.eu/resource/authority/public-event-type"/>
   </skos:Concept>
   <skos:Concept rdf:about="http://publications.europa.eu/resource/authority/public-event-type/EXHIBITION"
                 at:deprecated="false">
      <skos:prefLabel xml:lang="bg">Изложения</skos:prefLabel>
      <skos:prefLabel xml:lang="cs">Akce</skos:prefLabel>
      <skos:prefLabel xml:lang="da">Udstillinger</skos:prefLabel>
      <skos:prefLabel xml:lang="de">Ausstellungen</skos:prefLabel>
      <skos:prefLabel xml:lang="el">Εκθέσεις</skos:prefLabel>
      <skos:prefLabel xml:lang="en">Exhibitions</skos:prefLabel>
      <skos:prefLabel xml:lang="es">Exposiciones</skos:prefLabel>
      <skos:prefLabel xml:lang="et">Näitused</skos:prefLabel>
      <skos:prefLabel xml:lang="fi">Näyttelyt</skos:prefLabel>
      <skos:prefLabel xml:lang="fr">Expositions</skos:prefLabel>
      <skos:prefLabel xml:lang="ga">Taispeántais</skos:prefLabel>
      <skos:prefLabel xml:lang="hr">Izložbe</skos:prefLabel>
      <skos:prefLabel xml:lang="hu">Kiállítások</skos:prefLabel>
      <skos:prefLabel xml:lang="it">Esposizioni</skos:prefLabel>
      <skos:prefLabel xml:lang="lt">Parodos</skos:prefLabel>
      <skos:prefLabel xml:lang="lv">Izstādes</skos:prefLabel>
      <skos:prefLabel xml:lang="mt">Wirjiet</skos:prefLabel>
      <skos:prefLabel xml:lang="nl">Tentoonstellingen</skos:prefLabel>
      <skos:prefLabel xml:lang="pl">Wystawy</skos:prefLabel>
      <skos:prefLabel xml:lang="pt">Exposições</skos:prefLabel>
      <skos:prefLabel xml:lang="ro">Expoziții</skos:prefLabel>
      <skos:prefLabel xml:lang="sk">Výstavy</skos:prefLabel>
      <skos:prefLabel xml:lang="sl">Razstave</skos:prefLabel>
      <skos:prefLabel xml:lang="sv">Utställningar</skos:prefLabel>
      <at:authority-code>EXHIBITION</at:authority-code>
      <at:op-code>EXHIBITION</at:op-code>
      <at:start.use>1958-01-01</at:start.use>
      <atold:op-code>EXHIBITION</atold:op-code>
      <dc:identifier>EXHIBITION</dc:identifier>
      <skos:definition xml:lang="en">Exhibitions include public events such as expos, industry exhibitions, cultural events and fairs.</skos:definition>
      <skos:inScheme rdf:resource="http://publications.europa.eu/resource/authority/public-event-type"/>
      <skos:topConceptOf rdf:resource="http://publications.europa.eu/resource/authority/public-event-type"/>
   </skos:Concept>
   <skos:Concept rdf:about="http://publications.europa.eu/resource/authority/public-event-type/EXPERT_MEETING"
                 at:deprecated="false">
      <skos:prefLabel xml:lang="bg">Експертни заседания</skos:prefLabel>
      <skos:prefLabel xml:lang="cs">Zasedání odborníků</skos:prefLabel>
      <skos:prefLabel xml:lang="da">Ekspertmøder</skos:prefLabel>
      <skos:prefLabel xml:lang="de">Expertentreffen</skos:prefLabel>
      <skos:prefLabel xml:lang="el">Συνεδριάσεις εμπειρογνωμόνων</skos:prefLabel>
      <skos:prefLabel xml:lang="en">Expert meetings</skos:prefLabel>
      <skos:prefLabel xml:lang="es">Reuniones de expertos</skos:prefLabel>
      <skos:prefLabel xml:lang="et">Ekspertide koosolekud</skos:prefLabel>
      <skos:prefLabel xml:lang="fi">Asiantuntijakokoukset</skos:prefLabel>
      <skos:prefLabel xml:lang="fr">Réunions d'experts </skos:prefLabel>
      <skos:prefLabel xml:lang="ga">Cruinnithe saineolaithe</skos:prefLabel>
      <skos:prefLabel xml:lang="hr">Sastanci stručnjaka</skos:prefLabel>
      <skos:prefLabel xml:lang="hu">Szakértői értekezletek</skos:prefLabel>
      <skos:prefLabel xml:lang="it">Riunioni di esperti</skos:prefLabel>
      <skos:prefLabel xml:lang="lt">Ekspertų posėdžiai</skos:prefLabel>
      <skos:prefLabel xml:lang="lv">Ekspertu sanāksmes</skos:prefLabel>
      <skos:prefLabel xml:lang="mt">Laqgħat ta’ esperti</skos:prefLabel>
      <skos:prefLabel xml:lang="nl">Vergaderingen van deskundigen</skos:prefLabel>
      <skos:prefLabel xml:lang="pl">Spotkania ekspertów</skos:prefLabel>
      <skos:prefLabel xml:lang="pt">Reuniuni ale experților</skos:prefLabel>
      <skos:prefLabel xml:lang="pt">Reuniões de peritos</skos:prefLabel>
      <skos:prefLabel xml:lang="sk">Zasadnutia expertov</skos:prefLabel>
      <skos:prefLabel xml:lang="sl">Sestanki strokovnjakov</skos:prefLabel>
      <skos:prefLabel xml:lang="sv">Expertmöten</skos:prefLabel>
      <at:authority-code>EXPERT_MEETING</at:authority-code>
      <at:op-code>EXPERT_MEETING</at:op-code>
      <at:start.use>2022-02-21</at:start.use>
      <atold:op-code>EXPERT_MEETING</atold:op-code>
      <dc:identifier>EXPERT_MEETING</dc:identifier>
      <skos:definition xml:lang="bg">Заседания на независими експертни групи, чиито резултати са по-скоро от технически, научен, регулаторен и процедурен, отколкото от политически характер.</skos:definition>
      <skos:definition xml:lang="cs">Nezávislá grémia odborníků, jejichž výsledky jsou spíše technické, vědecké, regulační nebo procedurální povahy než politické.</skos:definition>
      <skos:definition xml:lang="da">Møder i uafhængige ekspertpaneler hvis resultater er tekniske, videnskabelige, lovgivningsmæssige eller proceduremæssige, snarere end politiske.</skos:definition>
      <skos:definition xml:lang="de">Zusammenkünfte unabhängiger Sachverständigengremien, deren Ergebnisse eher technischer, wissenschaftlicher, rechtlicher oder verfahrenstechnischer als politischer Art sind.</skos:definition>
      <skos:definition xml:lang="el">Συνεδριάσεις ανεξάρτητων ομάδων εμπειρογνωμόνων, τα αποτελέσματα των οποίων έχουν τεχνικό, επιστημονικό, κανονιστικό ή διαδικαστικό χαρακτήρα, αντί για πολιτικό.</skos:definition>
      <skos:definition xml:lang="en">Meetings of independent expert panels whose outcomes are technical, scientific, regulatory or procedural, rather than political.</skos:definition>
      <skos:definition xml:lang="es">Reuniones de grupos de expertos independientes cuyos resultados son técnicos, científicos, reglamentarios o de procedimiento, y no políticos. </skos:definition>
      <skos:definition xml:lang="et">Sõltumatute eksperdirühmade koosolekud, mille tulemused on pigem tehnilised, teaduslikud, regulatiivsed või menetluslikud kui poliitilised. </skos:definition>
      <skos:definition xml:lang="fi">Riippumattomien asiantuntijapaneelien kokoukset, joiden tulokset ovat pikemminkin teknisiä, tieteellisiä, sääntelyyn tai menettelyihin liittyviä kuin poliittisia.</skos:definition>
      <skos:definition xml:lang="fr">Réunions de groupes d’experts indépendants dont les résultats sont de nature technique, scientifique, réglementaire ou procédurale plutôt que politique. </skos:definition>
      <skos:definition xml:lang="ga">Cruinnithe de phainéil saineolaithe neamhspleácha a bhfuil a dtorthaí teicniúil, eolaíoch, rialaitheach nó nós imeachta, seachas polaitiúil.</skos:definition>
      <skos:definition xml:lang="hr">Sastanci neovisnih stručnih skupina čiji su ishodi tehnički, znanstveni, regulatorni ili postupovni, a ne politički. </skos:definition>
      <skos:definition xml:lang="hu">Független szakértői testületek ülései, amelyek eredményei inkább technikai, tudományos, szabályozási vagy eljárási jellegűek, mintsem politikaiak.</skos:definition>
      <skos:definition xml:lang="it">Riunioni di gruppi di esperti indipendenti i cui risultati sono di natura tecnica, scientifica, regolamentare o procedurale, piuttosto che politica.</skos:definition>
      <skos:definition xml:lang="lt">Nepriklausomų ekspertų grupių posėdžiai, kurių išvados yra ne politinės, o techninės, mokslinės, reguliacinės ar procedūrinės. </skos:definition>
      <skos:definition xml:lang="lv">Neatkarīgu ekspertu grupu sanāksmes, kuru rezultāti ir tehniski, zinātniski, regulatīvi vai procesuāli, nevis politiski. </skos:definition>
      <skos:definition xml:lang="mt">Laqgħat ta’ gruppi ta’ esperti indipendenti li l-eżiti tagħhom huma tekniċi, xjentifiċi, regolatorji jew proċedurali, aktar milli politiċi.</skos:definition>
      <skos:definition xml:lang="nl">Vergaderingen van onafhankelijke panels van deskundigen waarvan de uitkomst niet zozeer politiek, maar eerder technisch, wetenschappelijk, regelgevend of procedureel is. </skos:definition>
      <skos:definition xml:lang="pl">Spotkania paneli niezależnych ekspertów, których wyniki są raczej techniczne, naukowe, regulacyjne lub proceduralne niż polityczne. </skos:definition>
      <skos:definition xml:lang="pt">Reuniões de grupos de peritos independentes cujos resultados são de natureza técnica, científica, regulamentar ou processual e não tanto política.</skos:definition>
      <skos:definition xml:lang="ro">Reuniuni ale grupurilor de experți independenți, ale căror rezultate sunt de natură tehnică, științifică, normativă sau procedurală, mai degrabă decât politică. </skos:definition>
      <skos:definition xml:lang="sk">Zasadnutia nezávislých expertných panelov, ktorých výstupy sú technické, vedecké, regulačné alebo procedurálne, nie politické.</skos:definition>
      <skos:definition xml:lang="sl">Sestanki neodvisnih strokovnih odborov, katerih rezultati so tehnični, znanstveni, regulativni ali postopkovni, ne politični. </skos:definition>
      <skos:definition xml:lang="sv">Möten med oberoende expertpaneler för att diskutera tekniska, vetenskapliga, regleringsmässiga eller förfarandemässiga frågor snarare än politiska.</skos:definition>
      <skos:inScheme rdf:resource="http://publications.europa.eu/resource/authority/public-event-type"/>
      <skos:topConceptOf rdf:resource="http://publications.europa.eu/resource/authority/public-event-type"/>
   </skos:Concept>
   <skos:Concept rdf:about="http://publications.europa.eu/resource/authority/public-event-type/INFO_DAY"
                 at:deprecated="false">
      <skos:prefLabel xml:lang="bg">Информационни дни</skos:prefLabel>
      <skos:prefLabel xml:lang="cs">Informační dny</skos:prefLabel>
      <skos:prefLabel xml:lang="da">Infodage</skos:prefLabel>
      <skos:prefLabel xml:lang="de">Info-Tage</skos:prefLabel>
      <skos:prefLabel xml:lang="el">Ημερίδες ενημέρωσης</skos:prefLabel>
      <skos:prefLabel xml:lang="en">Info days</skos:prefLabel>
      <skos:prefLabel xml:lang="es">Jornadas informativas</skos:prefLabel>
      <skos:prefLabel xml:lang="et">Teabepäevad</skos:prefLabel>
      <skos:prefLabel xml:lang="fi">Infopäivät</skos:prefLabel>
      <skos:prefLabel xml:lang="fr">Journées d’information</skos:prefLabel>
      <skos:prefLabel xml:lang="ga">Laethanta eolais</skos:prefLabel>
      <skos:prefLabel xml:lang="hr">Dani informiranja</skos:prefLabel>
      <skos:prefLabel xml:lang="hu">Tájékoztató napok</skos:prefLabel>
      <skos:prefLabel xml:lang="it">Giornate d'informazione</skos:prefLabel>
      <skos:prefLabel xml:lang="lt">Informacinės dienos</skos:prefLabel>
      <skos:prefLabel xml:lang="lv">Infodienas</skos:prefLabel>
      <skos:prefLabel xml:lang="mt">Jiem ta’ informazzjoni</skos:prefLabel>
      <skos:prefLabel xml:lang="nl">Infodagen</skos:prefLabel>
      <skos:prefLabel xml:lang="pl">Dni informacyjne</skos:prefLabel>
      <skos:prefLabel xml:lang="pt">Jornadas de informação</skos:prefLabel>
      <skos:prefLabel xml:lang="ro">Zile de informare</skos:prefLabel>
      <skos:prefLabel xml:lang="sk">Informačné dni</skos:prefLabel>
      <skos:prefLabel xml:lang="sl">Informativni dnevi</skos:prefLabel>
      <skos:prefLabel xml:lang="sv">Informationsdagar</skos:prefLabel>
      <at:authority-code>INFO_DAY</at:authority-code>
      <at:op-code>INFO_DAY</at:op-code>
      <at:start.use>1958-01-01</at:start.use>
      <atold:op-code>INFO_DAY</atold:op-code>
      <dc:identifier>INFO_DAY</dc:identifier>
      <skos:definition xml:lang="en">Info days include public events such as open days, information days, information meetings and networking events.</skos:definition>
      <skos:inScheme rdf:resource="http://publications.europa.eu/resource/authority/public-event-type"/>
      <skos:topConceptOf rdf:resource="http://publications.europa.eu/resource/authority/public-event-type"/>
   </skos:Concept>
   <skos:Concept rdf:about="http://publications.europa.eu/resource/authority/public-event-type/PARTNER_MEETING"
                 at:deprecated="false">
      <skos:prefLabel xml:lang="bg">Срещи с партньори</skos:prefLabel>
      <skos:prefLabel xml:lang="cs">Setkání partnerských subjektů</skos:prefLabel>
      <skos:prefLabel xml:lang="da">Partnermøder</skos:prefLabel>
      <skos:prefLabel xml:lang="de">Veranstaltungen mit Partnern</skos:prefLabel>
      <skos:prefLabel xml:lang="el">Συναντήσεις εταίρων</skos:prefLabel>
      <skos:prefLabel xml:lang="en">Partner meetings</skos:prefLabel>
      <skos:prefLabel xml:lang="es">Reuniones de socios</skos:prefLabel>
      <skos:prefLabel xml:lang="et">Kohtumised partneritega</skos:prefLabel>
      <skos:prefLabel xml:lang="fi">Kumppanikokoukset</skos:prefLabel>
      <skos:prefLabel xml:lang="fr">Réunions de partenaires</skos:prefLabel>
      <skos:prefLabel xml:lang="ga">Cruinnithe comhpháirtíochta</skos:prefLabel>
      <skos:prefLabel xml:lang="hr">Partnerski sastanci</skos:prefLabel>
      <skos:prefLabel xml:lang="hu">Partneri találkozók</skos:prefLabel>
      <skos:prefLabel xml:lang="it">Riunioni dei partner</skos:prefLabel>
      <skos:prefLabel xml:lang="lt">Partnerių susitikimai</skos:prefLabel>
      <skos:prefLabel xml:lang="lv">Partneru sanāksmes</skos:prefLabel>
      <skos:prefLabel xml:lang="mt">Laqgħat tal-imsieħba</skos:prefLabel>
      <skos:prefLabel xml:lang="nl">Vergaderingen met partners</skos:prefLabel>
      <skos:prefLabel xml:lang="pl">Spotkania partnerskie</skos:prefLabel>
      <skos:prefLabel xml:lang="pt">Reuniões de parceiros</skos:prefLabel>
      <skos:prefLabel xml:lang="ro">Reuniuni ale partenerilor</skos:prefLabel>
      <skos:prefLabel xml:lang="sk">Stretnutia partnerských subjektov</skos:prefLabel>
      <skos:prefLabel xml:lang="sl">Partnerski sestanki</skos:prefLabel>
      <skos:prefLabel xml:lang="sv">Möten med samarbetspartner</skos:prefLabel>
      <at:authority-code>PARTNER_MEETING</at:authority-code>
      <at:op-code>PARTNER_MEETING</at:op-code>
      <at:start.use>1958-01-01</at:start.use>
      <atold:op-code>PARTNER_MEETING</atold:op-code>
      <dc:identifier>PARTNER_MEETING</dc:identifier>
      <skos:definition xml:lang="en">Partner meetings include public events such as stakeholder meetings.</skos:definition>
      <skos:inScheme rdf:resource="http://publications.europa.eu/resource/authority/public-event-type"/>
      <skos:topConceptOf rdf:resource="http://publications.europa.eu/resource/authority/public-event-type"/>
   </skos:Concept>
   <skos:Concept rdf:about="http://publications.europa.eu/resource/authority/public-event-type/POLITICAL_MEETING"
                 at:deprecated="false">
      <skos:prefLabel xml:lang="bg">Политически срещи</skos:prefLabel>
      <skos:prefLabel xml:lang="cs">Politická setkání</skos:prefLabel>
      <skos:prefLabel xml:lang="da">Politiske møder</skos:prefLabel>
      <skos:prefLabel xml:lang="de">Politische Veranstaltungen</skos:prefLabel>
      <skos:prefLabel xml:lang="el">Πολιτικές εκδηλώσεις</skos:prefLabel>
      <skos:prefLabel xml:lang="en">Political meetings</skos:prefLabel>
      <skos:prefLabel xml:lang="es">Reuniones políticas</skos:prefLabel>
      <skos:prefLabel xml:lang="et">Poliitilised kohtumised</skos:prefLabel>
      <skos:prefLabel xml:lang="fi">Poliittiset kokoukset</skos:prefLabel>
      <skos:prefLabel xml:lang="fr">Réunions politiques</skos:prefLabel>
      <skos:prefLabel xml:lang="ga">Cruinnithe polaitiúla</skos:prefLabel>
      <skos:prefLabel xml:lang="hr">Politički sastanci</skos:prefLabel>
      <skos:prefLabel xml:lang="hu">Politikai ülések</skos:prefLabel>
      <skos:prefLabel xml:lang="it">Riunioni politiche</skos:prefLabel>
      <skos:prefLabel xml:lang="lt">Politiniai susitikimai</skos:prefLabel>
      <skos:prefLabel xml:lang="lv">Politiskas sanāksmes</skos:prefLabel>
      <skos:prefLabel xml:lang="mt">Laqgħat politiċi</skos:prefLabel>
      <skos:prefLabel xml:lang="nl">Politieke vergaderingen</skos:prefLabel>
      <skos:prefLabel xml:lang="pl">Spotkania polityczne</skos:prefLabel>
      <skos:prefLabel xml:lang="pt">Reuniões políticas</skos:prefLabel>
      <skos:prefLabel xml:lang="ro">Reuniuni politice</skos:prefLabel>
      <skos:prefLabel xml:lang="sk">Politické stretnutia</skos:prefLabel>
      <skos:prefLabel xml:lang="sl">Politični sestanki</skos:prefLabel>
      <skos:prefLabel xml:lang="sv">Politiska möten</skos:prefLabel>
      <at:authority-code>POLITICAL_MEETING</at:authority-code>
      <at:op-code>POLITICAL_MEETING</at:op-code>
      <at:start.use>1958-01-01</at:start.use>
      <atold:op-code>POLITICAL_MEETING</atold:op-code>
      <dc:identifier>POLITICAL_MEETING</dc:identifier>
      <skos:definition xml:lang="en">Political meetings include political events involving the public.</skos:definition>
      <skos:inScheme rdf:resource="http://publications.europa.eu/resource/authority/public-event-type"/>
      <skos:topConceptOf rdf:resource="http://publications.europa.eu/resource/authority/public-event-type"/>
   </skos:Concept>
   <skos:Concept rdf:about="http://publications.europa.eu/resource/authority/public-event-type/PUBLIC_DEBATE"
                 at:deprecated="false">
      <skos:prefLabel xml:lang="bg">Публични дебати</skos:prefLabel>
      <skos:prefLabel xml:lang="cs">Veřejné diskuse</skos:prefLabel>
      <skos:prefLabel xml:lang="da">Offentlige debatter</skos:prefLabel>
      <skos:prefLabel xml:lang="de">Öffentliche Veranstaltungen</skos:prefLabel>
      <skos:prefLabel xml:lang="el">Δημόσιες συζητήσεις</skos:prefLabel>
      <skos:prefLabel xml:lang="en">Public debates</skos:prefLabel>
      <skos:prefLabel xml:lang="es">Debates públicos</skos:prefLabel>
      <skos:prefLabel xml:lang="et">Avalikud arutelud</skos:prefLabel>
      <skos:prefLabel xml:lang="fi">Julkiset keskustelutilaisuudet</skos:prefLabel>
      <skos:prefLabel xml:lang="fr">Débats publics</skos:prefLabel>
      <skos:prefLabel xml:lang="ga">Díospóireachtaí poiblí</skos:prefLabel>
      <skos:prefLabel xml:lang="hr">Javne debate</skos:prefLabel>
      <skos:prefLabel xml:lang="hu">Nyilvános viták</skos:prefLabel>
      <skos:prefLabel xml:lang="it">Dibattiti pubblici</skos:prefLabel>
      <skos:prefLabel xml:lang="lt">Vieši debatai</skos:prefLabel>
      <skos:prefLabel xml:lang="lv">Atklātas debates</skos:prefLabel>
      <skos:prefLabel xml:lang="mt">Dibattiti pubbliċi</skos:prefLabel>
      <skos:prefLabel xml:lang="nl">Openbare debatten</skos:prefLabel>
      <skos:prefLabel xml:lang="pl">Debaty publiczne</skos:prefLabel>
      <skos:prefLabel xml:lang="pt">Debates públicos</skos:prefLabel>
      <skos:prefLabel xml:lang="ro">Dezbateri publice</skos:prefLabel>
      <skos:prefLabel xml:lang="sk">Verejné diskusie</skos:prefLabel>
      <skos:prefLabel xml:lang="sl">Javne razprave</skos:prefLabel>
      <skos:prefLabel xml:lang="sv">Offentliga debatter</skos:prefLabel>
      <at:authority-code>PUBLIC_DEBATE</at:authority-code>
      <at:op-code>PUBLIC_DEBATE</at:op-code>
      <at:start.use>1958-01-01</at:start.use>
      <atold:op-code>PUBLIC_DEBATE</atold:op-code>
      <dc:identifier>PUBLIC_DEBATE</dc:identifier>
      <skos:definition xml:lang="en">Public debates include public events such as public debates, dialogues, forums and public meetings.</skos:definition>
      <skos:inScheme rdf:resource="http://publications.europa.eu/resource/authority/public-event-type"/>
      <skos:topConceptOf rdf:resource="http://publications.europa.eu/resource/authority/public-event-type"/>
   </skos:Concept>
   <skos:Concept rdf:about="http://publications.europa.eu/resource/authority/public-event-type/TRAINING_WORKSHOP"
                 at:deprecated="false">
      <skos:prefLabel xml:lang="bg">Обучения и семинари</skos:prefLabel>
      <skos:prefLabel xml:lang="cs">Odborná příprava a semináře</skos:prefLabel>
      <skos:prefLabel xml:lang="da">Kurser og workshopper</skos:prefLabel>
      <skos:prefLabel xml:lang="de">Schulungen und Workshops</skos:prefLabel>
      <skos:prefLabel xml:lang="el">Εκπαιδευτικά σεμινάρια και εργαστήρια</skos:prefLabel>
      <skos:prefLabel xml:lang="en">Training and workshops</skos:prefLabel>
      <skos:prefLabel xml:lang="es">Formación y talleres</skos:prefLabel>
      <skos:prefLabel xml:lang="et">Koolitused ja seminarid</skos:prefLabel>
      <skos:prefLabel xml:lang="fi">Koulutus ja työpajat</skos:prefLabel>
      <skos:prefLabel xml:lang="fr">Formations et ateliers</skos:prefLabel>
      <skos:prefLabel xml:lang="ga">Oiliúint agus ceardlanna</skos:prefLabel>
      <skos:prefLabel xml:lang="hr">Tečajevi i radionice</skos:prefLabel>
      <skos:prefLabel xml:lang="hu">Képzések és műhelytalálkozók</skos:prefLabel>
      <skos:prefLabel xml:lang="it">Formazione e seminari</skos:prefLabel>
      <skos:prefLabel xml:lang="lt">Mokymas ir praktiniai seminarai</skos:prefLabel>
      <skos:prefLabel xml:lang="lv">Mācības un semināri</skos:prefLabel>
      <skos:prefLabel xml:lang="mt">Taħriġ u workshops</skos:prefLabel>
      <skos:prefLabel xml:lang="nl">Opleidingen en workshops</skos:prefLabel>
      <skos:prefLabel xml:lang="pl">Szkolenia i warsztaty</skos:prefLabel>
      <skos:prefLabel xml:lang="pt">Formação e seminários</skos:prefLabel>
      <skos:prefLabel xml:lang="ro">Cursuri de formare și seminare de lucru</skos:prefLabel>
      <skos:prefLabel xml:lang="sk">Odborná príprava a semináre</skos:prefLabel>
      <skos:prefLabel xml:lang="sl">Usposabljanja in delavnice</skos:prefLabel>
      <skos:prefLabel xml:lang="sv">Kurser och seminarier</skos:prefLabel>
      <at:authority-code>TRAINING_WORKSHOP</at:authority-code>
      <at:op-code>TRAINING_WORKSHOP</at:op-code>
      <at:start.use>1958-01-01</at:start.use>
      <atold:op-code>TRAINING_WORKSHOP</atold:op-code>
      <dc:identifier>TRAINING_WORKSHOP</dc:identifier>
      <skos:definition xml:lang="en">Training and workshops include public events such as training, summer schools, webinars, workshops and seminars.</skos:definition>
      <skos:inScheme rdf:resource="http://publications.europa.eu/resource/authority/public-event-type"/>
      <skos:topConceptOf rdf:resource="http://publications.europa.eu/resource/authority/public-event-type"/>
   </skos:Concept>
</rdf:RDF>
